PREFIX gndr: <https://linked.data.gov.au/def/gender/>
PREFIX dcterms: <http://purl.org/dc/terms/>
PREFIX owl: <http://www.w3.org/2002/07/owl#>
PREFIX prov: <http://www.w3.org/ns/prov#>
PREFIX rdf: <http://www.w3.org/1999/02/22-rdf-syntax-ns#>
PREFIX rdfs: <http://www.w3.org/2000/01/rdf-schema#>
PREFIX skos: <http://www.w3.org/2004/02/skos/core#>
PREFIX xml: <http://www.w3.org/XML/1998/namespace>
PREFIX xsd: <http://www.w3.org/2001/XMLSchema#>

<https://linked.data.gov.au/def/gender> a owl:Ontology ,
		skos:ConceptScheme ;
	dcterms:created "2025-03-14"^^xsd:date ;
	dcterms:creator <https://linked.data.gov.au/org/abs>;
	dcterms:modified "2025-03-14"^^xsd:date ;
	dcterms:publisher <https://linked.data.gov.au/org/abs>;
    dcterms:provenance "Australian Bureau of Statistics - Standard for Sex, Gender, Variations of Sex Characteristics and Sexual Orientation Variables (2020)" ;
	dcterms:references 
		<https://www.abs.gov.au/statistics/standards/standard-sex-gender-variations-sex-characteristics-and-sexual-orientation-variables/latest-release> ;
	skos:definition """Gender is a social and cultural concept. It is about social and cultural differences in identity, expression and experience as a man, woman or non-binary person. Non-binary is an umbrella term describing gender identities that are not exclusively male or female.

	Gender includes the following concepts:

    Gender identity is about who a person feels themself to be
    Gender expression is the way a person expresses their gender. A person's gender expression may also vary depending on the context, for instance expressing different genders at work and home
    Gender experience describes a person's alignment with the sex recorded for them at birth i.e. a cis experience or a trans experience. 
	
	Responses to a gender question may reflect a combination of gender identity, expression and/or experience. In statistical collections, gender may be reported in terms of a person's felt or lived gender, as well as how that person is perceived by others, depending on whether information on gender is based on self-reported data or done by proxy. """@en ;
	skos:scopeNote """The ABS recognises 4 separate and distinct attributes in The Standard for Sex, Gender, Variations of Sex Characteristics and Sexual Orientation Variables, 2020. 
	This product presents statistical standards for four variables:
    - Sex
    - Gender
    - Variations of sex characteristics
    - Sexual orientation. 
	
	This vocabulary exclusively contains gender categories."""@en ;
	skos:hasTopConcept
		gndr:1,
		gndr:2,
		gndr:3,
		gndr:4,
		gndr:5;
	skos:prefLabel "Gender"@en .

gndr:1 a skos:Concept ;
    dcterms:source "https://www.abs.gov.au/statistics/standards/standard-sex-gender-variations-sex-characteristics-and-sexual-orientation-variables/latest-release#gender"^^xsd:anyURI ;
    rdfs:isDefinedBy <https://linked.data.gov.au/def/gender> ;
    skos:inScheme <https://linked.data.gov.au/def/gender> ;
    skos:topConceptOf <https://linked.data.gov.au/def/gender> ;
    skos:definition """Persons who described their gender as man or male."""@en ;
    skos:notation "1" ;
	skos:altLabel "M"@en,
		"Man"@en,
		"Male"@en ;
	skos:prefLabel "Man or male"@en .

gndr:2 a skos:Concept ;
    dcterms:source "https://www.abs.gov.au/statistics/standards/standard-sex-gender-variations-sex-characteristics-and-sexual-orientation-variables/latest-release#gender"^^xsd:anyURI ;
    rdfs:isDefinedBy <https://linked.data.gov.au/def/gender> ;
    skos:inScheme <https://linked.data.gov.au/def/gender> ;
    skos:topConceptOf <https://linked.data.gov.au/def/gender> ;
    skos:definition """Persons who described their gender as man or male."""@en ;
    skos:notation "2" ;
	skos:altLabel "F"@en,
		"Woman"@en,
		"Female"@en ;
	skos:prefLabel "Woman or female"@en .

gndr:3 a skos:Concept ;
	dcterms:source "https://www.abs.gov.au/statistics/standards/standard-sex-gender-variations-sex-characteristics-and-sexual-orientation-variables/latest-release#gender"^^xsd:anyURI ;
	rdfs:isDefinedBy <https://linked.data.gov.au/def/gender> ;
	skos:inScheme <https://linked.data.gov.au/def/gender> ;
	skos:topConceptOf <https://linked.data.gov.au/def/gender> ;
	skos:definition """Persons who described thier gender as non-binary."""@en ;
	skos:notation "3" ;
	skos:altLabel "X"@en,
		"Non-conforming"@en, ;
	skos:prefLabel "Non-binary"@en .

gndr:4 a skos:Concept ;
	dcterms:source "https://www.abs.gov.au/statistics/standards/standard-sex-gender-variations-sex-characteristics-and-sexual-orientation-variables/latest-release#gender"^^xsd:anyURI ;
	rdfs:isDefinedBy <https://linked.data.gov.au/def/gender> ;
	skos:inScheme <https://linked.data.gov.au/def/gender> ;
	skos:topConceptOf <https://linked.data.gov.au/def/gender> ;
	skos:definition """Persons who described their gender as a term other than man/male, woman/female or non-binary."""@en ;
	skos:notation "4" ;
	skos:altLabel "T"@en,
		"Different term"@en ;
	skos:prefLabel "Self-Described"@en .

gndr:5 a skos:Concept ;
	dcterms:source "https://www.abs.gov.au/statistics/standards/standard-sex-gender-variations-sex-characteristics-and-sexual-orientation-variables/latest-release#gender"^^xsd:anyURI ;
	rdfs:isDefinedBy <https://linked.data.gov.au/def/gender> ;
	skos:inScheme <https://linked.data.gov.au/def/gender> ;
	skos:topConceptOf <https://linked.data.gov.au/def/gender> ;
	skos:definition """Persons who preferred not to respond on how they describe their gender."""@en ;
	skos:notation "5" ;
	skos:altLabel "Z"@en ;
	skos:prefLabel "Prefer not to answer"@en .