@prefix aqf: <https://linked.data.gov.au/def/australian-qualifications-framework/> .
@prefix dc: <http://purl.org/dc/elements/1.1/> .
@prefix dcterms: <http://purl.org/dc/terms/> .
@prefix owl: <http://www.w3.org/2002/07/owl#> .
@prefix rdf: <http://www.w3.org/1999/02/22-rdf-syntax-ns#> .
@prefix rdfs: <http://www.w3.org/2000/01/rdf-schema#> .
@prefix sdo: <http://schema.org/> .
@prefix skos: <http://www.w3.org/2004/02/skos/core#> .
@prefix xml: <http://www.w3.org/XML/1998/namespace> .
@prefix xsd: <http://www.w3.org/2001/XMLSchema#> .

<https://linked.data.gov.au/def/australian-qualifications-framework> a owl:Ontology ,
        skos:ConceptScheme ;
    dcterms:created "2023-03-01"^^xsd:date ;
    dcterms:creator <https://linked.data.gov.au/org/engineersaustralia>;
    dcterms:publisher <https://linked.data.gov.au/org/engineersaustralia>;
    dcterms:modified "2023-03-01"^^xsd:date ;
    dcterms:contributor <https://orcid.org/0000-0003-2309-7004> ;
    dcterms:source "https://www.engineersaustralia.org.au"^^xsd:anyURI ;
    dcterms:accessRights <https://linked.data.gov.au/def/data-access-rights/open> ;                                
    skos:definition "Australian Qualifications Framework Issued by the National Staff Development Committee Standards and Curriculum Council of ANTA, the AQF provides a comprehensive, nationally consistent yet flexible Framework for all qualifications in post-compulsory education in Australia. The Framework was introduced Australia wide on 1 January 1995."@en ;
    skos:prefLabel "Australian Qualifications Framework"@en .
    
<https://linked.data.gov.au/org/engineersaustralia>
    a sdo:Organization ;
    sdo:name "Engineers Australia" ;
    sdo:url "https://www.engineersaustralia.org.au"^^xsd:anyURI .

<https://orcid.org/0000-0003-2309-7004> a owl:NamedIndividual,
    sdo:Person ;
    sdo:affiliation [ a sdo:Organization ;
        sdo:name "Engineers Australia" ;
        sdo:url "https://www.engineersaustralia.org.au"^^xsd:anyURI ] ;
    sdo:name "Vance Kelly" ;
    sdo:identifier <https://orcid.org/0000-0003-2309-7004> .

aqf:ssce a skos:Concept ;
    dcterms:source "https://www.aqf.edu.au/"^^xsd:anyURI ;
    rdfs:isDefinedBy <https://linked.data.gov.au/def/australian-qualifications-framework> ;
    skos:definition """The Senior Secondary Certificate of Education qualifies individuals with knowledge, skills and values for diverse pathways to further learning, work and effective participation in civic life.
    Graduates of a Senior Secondary Certificate of Education will have foundational knowledge across a range of learning areas and some specialist discipline or technical knowledge.
    Graduates of a Senior Secondary Certificate of Education will have:
        - literacy, numeracy and communication skills and use information communication technologies skills to present knowledge and ideas to others
        - cognitive skills to access, record and act on information from varied sources appropriate to subject disciplines and to move across subject disciplines to develop new expertise
        - cognitive, technical, communication and creative skills for particular disciplines and to integrate disciplines to solve problems, to underpin flexible and analytical thinking and to work with others.
    Graduates of a Senior Secondary Certificate of Education will demonstrate the application of knowledge and skills:
        - with depth in some areas to tasks or functions in known or changing contexts
        - in particular contexts within civic life, work and lifelong learning as successful learners, confident individuals and team members and active and informed citizens
        - in contexts that include taking individual responsibility with some direction and some accountability for the quality of outcomes.
    The volume of learning of a Senior Secondary Certificate of Education is typically 2 years."""@en ;
    skos:inScheme <https://linked.data.gov.au/def/australian-qualifications-framework> ;
    skos:prefLabel "Senior Secondary Certificate of Education"@en ;
    skos:topConceptOf <https://linked.data.gov.au/def/australian-qualifications-framework> .

aqf:cert-i a skos:Concept ;
    dcterms:source "https://www.aqf.edu.au/"^^xsd:anyURI ;
    rdfs:isDefinedBy <https://linked.data.gov.au/def/australian-qualifications-framework> ;
    skos:definition """The Certificate I qualifies individuals with basic functional knowledge and skills to undertake work, further learning and community involvement.
    Graduates of a Certificate I will have basic fundamental knowledge and understanding in a narrow area of work and learning.
    Graduates of a Certificate I will have:
        - basic skills to participate in everyday life and further learning
        - cognitive and communication skills to receive, pass on and recall information in a narrow range of areas
        - technical skills involving the use of tools appropriate to the activity and use of basic communication technologies.
    Graduates of a Certificate I will demonstrate the application of knowledge and skills:
        - with some autonomy in defined contexts and within established parameters and
        - in contexts that may include preparation for further learning, life activities and/or a variety of initial routine and predictable work-related activities including participation in a team or work group.
    The volume of learning of a Certificate I is typically 0.5-1 year."""@en ;
    skos:inScheme <https://linked.data.gov.au/def/australian-qualifications-framework> ;
    skos:prefLabel "Certificate I"@en ;
    skos:topConceptOf <https://linked.data.gov.au/def/australian-qualifications-framework> .

aqf:cert-ii a skos:Concept ;
    dcterms:source "https://www.aqf.edu.au/"^^xsd:anyURI ;
    rdfs:isDefinedBy <https://linked.data.gov.au/def/australian-qualifications-framework> ;
    skos:definition """The Certificate II qualifies individuals to undertake mainly routine work and as a pathway to further learning.
    Graduates of a Certificate II will have basic factual, technical and procedural knowledge in a defined area of work and learning.
    Graduates of a Certificate II will have:
        - cognitive skills to access, record and act on a defined range of information from a range of sources
        - cognitive and communication skills to apply and communicate known solutions to a limited range of predictable problems
        - technical skills to use a limited range of equipment to complete tasks involving known routines and procedures with a limited range of options.
    Graduates of a Certificate II will demonstrate the application of knowledge and skills:
        - with some accountability for the quality of own outcomes some responsibility for own outputs in work and learning
        - with limited autonomy and judgement in the completion of own defined and routine tasks in known and stable contexts
        - with limited autonomy and judgement to complete routine but variable tasks in collaboration with others in a team environment.
    The volume of learning of a Certificate II is typically 0.5-1 year."""@en ;
    skos:inScheme <https://linked.data.gov.au/def/australian-qualifications-framework> ;
    skos:prefLabel "Certificate II"@en ;
    skos:topConceptOf <https://linked.data.gov.au/def/australian-qualifications-framework> .

aqf:cert-iii a skos:Concept ;
    dcterms:source "https://www.aqf.edu.au/"^^xsd:anyURI ;
    rdfs:isDefinedBy <https://linked.data.gov.au/def/australian-qualifications-framework> ;
    skos:definition """The Certificate III qualifies individuals who apply a broad range of knowledge and skills in varied contexts to undertake skilled work and as a pathway for further learning.
    Graduates of a Certificate III will have factual, technical, procedural and theoretical knowledge in an area of work and learning.
    Graduates of a Certificate III will have:
        - cognitive, technical and communication skills to interpret and act on available information
        - cognitive and communication skills to apply and communicate known solutions to a variety of predictable problems and to deal with unforseen contingencies using known solutions
        - technical and communication skills to provide technical information to a variety of specialist and non-specialist audiences
        - technical skills to undertake routine and some non-routine tasks in a range of skilled operations.
    Graduates of a Certificate III will demonstrate the application of knowledge and skills:
        - with discretion and judgement in the selection of equipment, services or contingency measures
        - to adapt and transfer skills and knowledge within known routines, methods, procedures and time constraints
        - in contexts that include taking responsibility for own outputs in work and learning including participation in teams and taking limited responsibility for the output of others within established parameters.
    The volume of learning of a Certificate III is typically 1-2 years. Up to 4 years may be required to achieve the learning outcomes through a program of indentured training/employment."""@en ;
    skos:inScheme <https://linked.data.gov.au/def/australian-qualifications-framework> ;
    skos:prefLabel "Certificate III"@en ;
    skos:topConceptOf <https://linked.data.gov.au/def/australian-qualifications-framework> .

aqf:cert-iv a skos:Concept ;
    dcterms:source "https://www.aqf.edu.au/"^^xsd:anyURI ;
    rdfs:isDefinedBy <https://linked.data.gov.au/def/australian-qualifications-framework> ;
    skos:definition """The Certificate IV qualifies individuals who apply a broad range of specialised knowledge and skills in varied contexts to undertake skilled work and as a pathway for further learning.
    Graduates of a Certificate IV will have broad factual, technical and theoretical knowledge in a specialised field of work and learning.
    Graduates of a Certificate IV will have:
        - cognitive skills to identify, analyse, compare and act on information from a range of sources
        - cognitive, technical and communication skills to apply and communicate technical solutions of a non-routine or contingency nature to a defined range of predictable and unpredictable problems
        - specialist technical skills to complete routine and non- routine tasks and functions
        - communication skills to guide activities and provide technical advice in the area of work and learning.
    Graduates of a Certificate IV will demonstrate the application of knowledge and skills:
        - to specialised tasks or functions in known or changing contexts
        - with responsibility for own functions and outputs, and may have limited responsibility for organisation of others
        - with limited responsibility for the quantity and quality of the output of others in a team within limited parameters.
    The volume of learning of a Certificate IV is typically 0.5-2 years. There may be variations between short duration specialist qualifications that build on knowledge and skills already acquired and longer duration qualifications that are designed as entry level requirements for work."""@en ;
    skos:inScheme <https://linked.data.gov.au/def/australian-qualifications-framework> ;
    skos:prefLabel "Certificate IV"@en ;
    skos:topConceptOf <https://linked.data.gov.au/def/australian-qualifications-framework> .

aqf:dip a skos:Concept ;
    dcterms:source "https://www.aqf.edu.au/"^^xsd:anyURI ;
    rdfs:isDefinedBy <https://linked.data.gov.au/def/australian-qualifications-framework> ;
    skos:definition """The Diploma qualifies individuals who apply integrated technical and theoretical concepts in a broad range of contexts to undertake advanced skilled or paraprofessional work and as a pathway for further learning.
    Graduates of a Diploma will have technical and theoretical knowledge and concepts, with depth in some areas within a field of work and learning.
    Graduates of a Diploma will have:
        - cognitive and communication skills to identify, analyse, synthesise and act on information from a range of sources
        - cognitive, technical and communication skills to analyse, plan, design and evaluate approaches to unpredictable problems and/or management requirements 
        - specialist technical and creative skills to express ideas and perspectives 
        - communication skills to transfer knowledge and specialised skills to others and demonstrate understanding of knowledge.
    Graduates of a Diploma will demonstrate the application of knowledge and skills:
        - with depth in some areas of specialisation, in known or changing contexts
        - to transfer and apply theoretical concepts and/or technical and/or creative skills in a range of situations
        - with personal responsibility and autonomy in performing complex technical operations with responsibility for own outputs in relation to broad parameters for quantity and quality
        - with initiative and judgement to organise the work of self and others and plan, coordinate and evaluate the work of teams within broad but generally well- defined parameters.
    The volume of learning of a Diploma is typically 1-2 years."""@en ;
    skos:inScheme <https://linked.data.gov.au/def/australian-qualifications-framework> ;
    skos:prefLabel "Diploma"@en ;
    skos:topConceptOf <https://linked.data.gov.au/def/australian-qualifications-framework> .

aqf:ad-dip a skos:Concept ;
    dcterms:source "https://www.aqf.edu.au/"^^xsd:anyURI ;
    rdfs:isDefinedBy <https://linked.data.gov.au/def/australian-qualifications-framework> ;
    skos:definition """The Advanced Diploma qualifies individuals who apply specialised knowledge in a range of contexts to undertake advanced skilled or paraprofessional work and as a pathway for further learning.
    Graduates of an Advanced Diploma will have specialised and integrated technical and theoretical knowledge with depth within one or more fields of work and learning.
    Graduates of an Advanced Diploma will have:
        - cognitive and communication skills to identify, analyse, synthesise and act on information from a range of sources
        - cognitive and communication skills to transfer knowledge and skills to others and to demonstrate understanding of specialised knowledge with depth in some areas
        - cognitive and communication skills to formulate responses to complex problems
        - wide-ranging specialised technical, creative or conceptual skills to express ideas and perspectives.
    Graduates of an Advanced Diploma will demonstrate the application of knowledge and skills:
        - with depth in areas of specialisation, in contexts subject to change
        - with initiative and judgment in planning, design, technical or management functions with some direction
        - to adapt a range of fundamental principles and complex techniques to known and unknown situations
        - across a broad range of technical or management functions with accountability for personal outputs and personal and team outcomes within broad parameters.
    The volume of learning of an Advanced Diploma is typically 1.5-2 years."""@en ;
    skos:inScheme <https://linked.data.gov.au/def/australian-qualifications-framework> ;
    skos:prefLabel "Advanced Diploma"@en ;
    skos:topConceptOf <https://linked.data.gov.au/def/australian-qualifications-framework> .

aqf:associate a skos:Concept ;
    dcterms:source "https://www.aqf.edu.au/"^^xsd:anyURI ;
    rdfs:isDefinedBy <https://linked.data.gov.au/def/australian-qualifications-framework> ;
    skos:definition """The Associate Degree qualifies individuals who apply underpinning technical and theoretical knowledge in a range of contexts to undertake paraprofessional work and as a pathway for further learning.
    Graduates of an Associate Degree will have broad theoretical and technical knowledge with some depth in the underlying principles and concepts in one or more disciplines.
    Graduates of an Associate Degree will have:
        - cognitive skills to identify, analyse and evaluate information and concepts from a range of sources
        - cognitive, technical and creative thinking skills to demonstrate a broad understanding of knowledge and ideas with some depth in a discipline
        - cognitive, communication and analytical skills to interpret and transmit responses to sometimes complex problems
        - communication skills to make a clear and coherent presentation of knowledge and ideas with some intellectual independence.
    Graduates of an Associate Degree will demonstrate the application of knowledge and skills:
        - with initiative and judgement in planning, problem solving and decision making in paraprofessional practice
        - to adapt knowledge and skills in a range of contexts and/or for further studies in one or more disciplines
        - to adapt fundamental principles, concepts and techniques to known and unknown situations
        - with responsibility and accountability for own learning and work and in collaboration with others within broad parameters.
    The volume of learning of an Associate Degree is typically 2 years."""@en ;
    skos:inScheme <https://linked.data.gov.au/def/australian-qualifications-framework> ;
    skos:prefLabel "Associate Degree"@en ;
    skos:topConceptOf <https://linked.data.gov.au/def/australian-qualifications-framework> .

aqf:bachelor a skos:Concept ;
    dcterms:source "https://www.aqf.edu.au/"^^xsd:anyURI ;
    rdfs:isDefinedBy <https://linked.data.gov.au/def/australian-qualifications-framework> ;
    skos:definition """The Bachelor Degree qualifies individuals who apply a broad and coherent body of knowledge in a range of contexts to undertake professional work and as a pathway for further learning.
    Graduates of a Bachelor Degree will have a broad and coherent body of knowledge, with depth in the underlying principles and concepts in one or more disciplines as a basis for independent lifelong learning.
    Graduates of a Bachelor Degree will have:
        - cognitive skills to review critically, analyse, consolidate and synthesise knowledge
        - cognitive and technical skills to demonstrate a broad understanding of knowledge with depth in some areas
        - cognitive and creative skills to exercise critical thinking and judgement in identifying and solving problems with intellectual independence
        - communication skills to present a clear, coherent and independent exposition of knowledge and ideas.
    Graduates of a Bachelor Degree will demonstrate the application of knowledge and skills:
        - with initiative and judgement in planning, problem solving and decision making in professional practice and/or scholarship
        - to adapt knowledge and skills in diverse contexts
        - with responsibility and accountability for own learning and professional practice and in collaboration with others within broad parameters
    The volume of learning of a Bachelor Degree is typically 3-4 years."""@en ;
    skos:inScheme <https://linked.data.gov.au/def/australian-qualifications-framework> ;
    skos:prefLabel "Bachelor Degree"@en ;
    skos:topConceptOf <https://linked.data.gov.au/def/australian-qualifications-framework> .

aqf:bachelor-honours a skos:Concept ;
    dcterms:source "https://www.aqf.edu.au/"^^xsd:anyURI ;
    rdfs:isDefinedBy <https://linked.data.gov.au/def/australian-qualifications-framework> ;
    skos:definition """The Bachelor Honours Degree qualifies individuals who apply a body of knowledge in a specific context to undertake professional work and as a pathway for research and further learning.
    Graduates of a Bachelor Honours Degree will have coherent and advanced knowledge of the underlying principles and concepts in one or more disciplines and knowledge of research principles and methods.
    Graduates of a Bachelor Honours Degree will have:
        - cognitive skills to review, analyse, consolidate and synthesise knowledge to identify and provide solutions to complex problems with intellectual independence
        - cognitive and technical skills to demonstrate a broad understanding of a body of knowledge and theoretical concepts with advanced understanding in some areas
        - cognitive skills to exercise critical thinking and judgement in developing new understanding
        - technical skills to design and use research in a project
        - communication skills to present a clear and coherent exposition of knowledge and ideas to a variety of audiences.
    Graduates of a Bachelor Honours Degree will demonstrate the application of knowledge and skills:
        - with initiative and judgement in professional practice and/or scholarship
        - to adapt knowledge and skills in diverse contexts
        - with responsibility and accountability for own learning and practice and in collaboration with others within broad parameters
        - to plan and execute project work and/or a piece of research and scholarship with some independence 
    The volume of learning of a  Bachelor Honours Degree is typically 1 year following a Bachelor Degree. A Bachelor Honours Degree may also be embedded in a Bachelor Degree, typically as an additional year."""@en ;
    skos:inScheme <https://linked.data.gov.au/def/australian-qualifications-framework> ;
    skos:prefLabel "Bachelor Honours Degree"@en ;
    skos:topConceptOf <https://linked.data.gov.au/def/australian-qualifications-framework> .

aqf:grad-cert a skos:Concept ;
    dcterms:source "https://www.aqf.edu.au/"^^xsd:anyURI ;
    rdfs:isDefinedBy <https://linked.data.gov.au/def/australian-qualifications-framework> ;
    skos:definition """The Graduate Certificate qualifies individuals who apply a body of knowledge in a range of contexts to undertake professional/highly skilled work and as a pathway for further learning.
    Graduates of a Graduate Certificate will have specialised knowledge within a systematic and coherent body of knowledge that may include the acquisition and application of knowledge and skills in a new or existing discipline or professional area.
    Graduates of a Graduate Certificate will have:
        - cognitive skills to review, analyse, consolidate and synthesise knowledge and identify and provide solutions to complex problems
        - cognitive skills to think critically and to generate and evaluate complex ideas
        - specialised technical and creative skills in a field of highly skilled and/or professional practice
        - communication skills to demonstrate an understanding of theoretical concepts
        - communication skills to transfer complex knowledge and ideas to a variety of audiences.
    Graduates of a Graduate Certificate will demonstrate the application of knowledge and skills:
        - to make high level, independent judgements in a range of technical or management functions in varied specialised contexts
        - to initiate, plan, implement and evaluate broad functions within varied specialised technical and/or creative contexts
        - with responsibility and accountability for personal outputs and all aspects of the work or function of others within broad parameters The volume of learning of a.
    Graduate Certificate is typically 0.5-1 year."""@en ;
    skos:inScheme <https://linked.data.gov.au/def/australian-qualifications-framework> ;
    skos:prefLabel "Graduate Certificate"@en ;
    skos:topConceptOf <https://linked.data.gov.au/def/australian-qualifications-framework> .

aqf:grad-dip a skos:Concept ;
    dcterms:source "https://www.aqf.edu.au/"^^xsd:anyURI ;
    rdfs:isDefinedBy <https://linked.data.gov.au/def/australian-qualifications-framework> ;
    skos:definition """The Graduate Diploma qualifies individuals who apply a body of knowledge in a range of contexts to undertake professional/ highly skilled work and as a pathway for further learning.
    Graduates of a Graduate Diploma will have advanced knowledge within a systematic and coherent body of knowledge that may include the acquisition and application of knowledge and skills in a new or existing discipline or professional area.
    Graduates of a Graduate Diploma will have:
        - cognitive skills to review, analyse, consolidate and synthesise knowledge and identify and provide solutions to complex problems
        - cognitive skills to think critically and to generate and evaluate complex ideas
        - specialised technical and creative skills in a field of highly skilled and/or professional practice
        - communication skills to demonstrate an understanding of theoretical concepts 
        - communication skills to transfer complex knowledge and ideas to a variety of audiences.
    Graduates of a Graduate Diploma will demonstrate the application of knowledge and skills:
        - to make high level, independent judgements in a range of technical or management functions in varied specialised contexts
        - to initiate, plan, implement and evaluate broad functions within varied specialised technical and/or creative contexts
        - with responsibility and accountability for personal outputs and all aspects of the work or function of others within broad parameters
    The volume of learning of a Graduate Diploma is typically 1-2 years."""@en ;
    skos:inScheme <https://linked.data.gov.au/def/australian-qualifications-framework> ;
    skos:prefLabel "Graduate Diploma"@en ;
    skos:topConceptOf <https://linked.data.gov.au/def/australian-qualifications-framework> .

aqf:master-research a skos:Concept ;
    dcterms:source "https://www.aqf.edu.au/"^^xsd:anyURI ;
    rdfs:isDefinedBy <https://linked.data.gov.au/def/australian-qualifications-framework> ;
    skos:definition """The Masters Degree (Research) qualifies individuals who apply an advanced body of knowledge in a range of contexts for research and scholarship and as a pathway for further learning.
    Graduates of a Masters Degree (Research) will have:
        - a body of knowledge that includes the understanding of recent developments in one or more disciplines
        - advanced knowledge of research principles and methods applicable to the field of work or learning.
    Graduates of a Masters Degree (Research) will have:
        - cognitive skills to demonstrate mastery of theoretical knowledge and to reflect critically on theory and its application
        - cognitive, technical and creative skills to investigate, analyse and synthesise complex information, problems, concepts and theories and to apply established theories to different bodies of knowledge or practice
        - cognitive, technical and creative skills to generate and evaluate complex ideas and concepts at an abstract level
        - cognitive and technical skills to design, use and evaluate research and research methods
        - communication and technical skills to present a coherent and sustained argument and to disseminate research results to specialist and non-specialist audiences
        - technical and communication skills to design, evaluate, implement, analyse, theorise and disseminate research that makes a contribution to knowledge.
    Graduates of a Masters Degree (Research) will demonstrate the application of knowledge & skills:
        - with creativity and initiative to new situations and/or for further learning
        - with high level personal autonomy and accountability
        - to plan and execute a substantial piece of research
    The volume of learning of a Masters Degree (Research) is typically 1-2 years; in the same discipline 1.5 years following a level 7 qualification or 1 year following a level 8 qualification; in a different discipline 2 years following a level 7 qualification or 1.5 years following a level 8 qualification."""@en ;
    skos:inScheme <https://linked.data.gov.au/def/australian-qualifications-framework> ;
    skos:prefLabel "Masters Degree (Research)"@en ;
    skos:topConceptOf <https://linked.data.gov.au/def/australian-qualifications-framework> .

aqf:master-coursework a skos:Concept ;
    dcterms:source "https://www.aqf.edu.au/"^^xsd:anyURI ;
    rdfs:isDefinedBy <https://linked.data.gov.au/def/australian-qualifications-framework> ;
    skos:definition """The Masters Degree (Coursework) qualifies individuals who apply an advanced body of knowledge in a range of contexts for professional practice or scholarship and as a pathway for further learning.
    Graduates of a Masters Degree (Coursework) will have:
        - a body of knowledge that includes the understanding of recent developments in a discipline and/or area of professional practice
        - knowledge of research principles and methods applicable to a field of work and/or learning.
    Graduates of a Masters Degree (Coursework) will have:
        - cognitive skills to demonstrate mastery of theoretical knowledge and to reflect critically on theory and professional practice or scholarship
        - cognitive, technical and creative skills to investigate, analyse and synthesise complex information, problems, concepts and theories and to apply established theories to different bodies of knowledge or practice
        - cognitive, technical and creative skills to generate and evaluate complex ideas and concepts at an abstract level
        - communication and technical research skills to justify and interpret theoretical propositions, methodologies, conclusions and professional decisions to specialist and non-specialist audiences
        - technical and communication skills to design, evaluate, implement, analyse and theorise about developments that contribute to professional practice or scholarship.
    Graduates of a Masters Degree (Coursework) will demonstrate the application of knowledge & skills:
        - with creativity and initiative to new situations in professional practice and/or for further learning
        - with high level personal autonomy and accountability
        - to plan and execute a substantial research-based project, capstone experience and/or piece of scholarship
    The volume of learning of a Masters Degree (Coursework) is typically 1-2 years; in the same discipline 1.5 years following a level 7 qualification or 1 year following a level 8 qualification; in a different discipline 2 years following a level 7 qualification or 1.5 years following a level 8 qualification."""@en ;
    skos:inScheme <https://linked.data.gov.au/def/australian-qualifications-framework> ;
    skos:prefLabel "Masters Degree (Coursework)"@en ;
    skos:topConceptOf <https://linked.data.gov.au/def/australian-qualifications-framework> .

aqf:master-extended a skos:Concept ;
    dcterms:source "https://www.aqf.edu.au/"^^xsd:anyURI ;
    rdfs:isDefinedBy <https://linked.data.gov.au/def/australian-qualifications-framework> ;
    skos:definition """The Masters Degree (Extended) qualifies individuals who apply an advanced body of knowledge in a range of contexts for professional practice and as a pathway for further learning.
    Graduates of a Masters Degree (Extended) will have:
        - a body of knowledge that includes the extended understanding of recent developments in a discipline and its professional practice
        - knowledge of research principles and methods applicable to the discipline and its professional practice.
    Graduates of a Masters Degree (Extended) will have:
        - cognitive skills to demonstrate mastery of theoretical knowledge and to reflect critically on theory and professional practice
        - cognitive, technical and creative skills to investigate, analyse and synthesise complex information, problems, concepts and theories and to apply established theories to different bodies of knowledge or practice
        - cognitive, technical and creative skills to generate and evaluate complex ideas and concepts at an abstract level
        - communication and technical research skills to justify and interpret theoretical propositions, methodologies, conclusions and professional decisions to specialist and non-specialist audiences
        - technical and communication skills to design, evaluate, implement, analyse and theorise about developments that contribute to professional practice.
    Graduates of a Masters Degree (Extended) will demonstrate the application of knowledge and skills:
        - with creativity and initiative to new situations in professional practice and/or for further learning
        - with high level personal autonomy and accountability
        - to plan and execute a substantial research-based project, capstone experience and/or professionally focused project
    The volume of learning of a Masters Degree (Extended) is typically 3-4 years following completion of a minimum of a 3 year level 7 qualification."""@en ;
    skos:inScheme <https://linked.data.gov.au/def/australian-qualifications-framework> ;
    skos:prefLabel "Masters Degree (Extended)"@en ;
    skos:topConceptOf <https://linked.data.gov.au/def/australian-qualifications-framework> .

aqf:doctoral a skos:Concept ;
    dcterms:source "https://www.aqf.edu.au/"^^xsd:anyURI ;
    rdfs:isDefinedBy <https://linked.data.gov.au/def/australian-qualifications-framework> ;
    skos:definition """"The Doctoral Degree qualifies individuals who apply a substantial body of knowledge to research, investigate and develop new knowledge, in one or more fields of investigation, scholarship or professional practice.
    Graduates of a Doctoral Degree will have:
        - a substantial body of knowledge at the frontier of a field of work or learning, including knowledge that constitutes an original contribution
        - substantial knowledge of research principles and methods applicable to the field of work or learning.
    Graduates of a Doctoral Degree will have:
        - cognitive skills to demonstrate expert understanding of theoretical knowledge and to reflect critically on that theory and practice
        - cognitive skills and use of intellectual independence to think critically, evaluate existing knowledge and ideas, undertake systematic investigation and reflect on theory and practice to generate original knowledge
        - expert technical and creative skills applicable to the field of work or learning
        - communication skills to explain and critique theoretical propositions, methodologies and conclusions
        - communication skills to present cogently a complex investigation of originality or original research for external examination against international standards and to communicate results to peers and the community
        - expert skills to design, implement, analyse, theorise and communicate research that makes a significant and original contribution to knowledge and/or professional practice.
    Graduates of a Doctoral Degree will demonstrate the application of knowledge and skills:
        - with intellectual independence
        - with initiative and creativity in new situations &/or for further learning
        - with full responsibility and accountability for personal outputs
        - to plan and execute original research
        - with the ongoing capacity to generate new knowledge, including in the context of professional practice
    The volume of learning of a Doctoral Degree is typically 3-4 years."""@en ;
    skos:inScheme <https://linked.data.gov.au/def/australian-qualifications-framework> ;
    skos:prefLabel "Doctoral Degree"@en ;
    skos:topConceptOf <https://linked.data.gov.au/def/australian-qualifications-framework> .
