PREFIX ctrl: <https://linked.data.gov.au/def/control-effectiveness/>
PREFIX earl: <https://ref.engineersaustralia.org.au/def/ea-activity-roles/>
PREFIX dcat: <http://www.w3.org/ns/dcat#>
PREFIX dcterms: <http://purl.org/dc/terms/>
PREFIX owl: <http://www.w3.org/2002/07/owl#>
PREFIX prov: <http://www.w3.org/ns/prov#>
PREFIX rdfs: <http://www.w3.org/2000/01/rdf-schema#>
PREFIX sdo: <http://schema.org/>
PREFIX skos: <http://www.w3.org/2004/02/skos/core#>
PREFIX xml: <http://www.w3.org/XML/1998/namespace>
PREFIX xsd: <http://www.w3.org/2001/XMLSchema#>

<https://linked.data.gov.au/org/engineersaustralia> a sdo:Organization ;
    sdo:name "Engineers Australia" ;
    sdo:url "https://www.engineersaustralia.org.au"^^xsd:anyURI .

<https://linked.data.gov.au/def/control-effectiveness> a owl:Ontology ,
        skos:ConceptScheme ;
    dcterms:created "2024-01-10"^^xsd:date ;
    dcterms:creator <https://linked.data.gov.au/org/engineersaustralia>;
    dcterms:publisher <https://linked.data.gov.au/org/engineersaustralia>;
    dcterms:modified "2024-03-01"^^xsd:date ;
    dcterms:contributor <https://orcid.org/0000-0003-2309-7004> ;
    dcterms:references <https://www.iso.org/obp/ui/#iso:std:iso:31000:en>,
        <https://www.finance.gov.au/sites/default/files/2020-12/Information-Sheet-Undertaking-Risk-Management-Process.docx> ;
    dcterms:source "https://www.engineersaustralia.org.au"^^xsd:anyURI ;
    dcterms:accessRights <https://linked.data.gov.au/def/data-access-rights/open> ;
    prov:qualifiedAttribution
        [
            dcat:hadRole earl:data-steward ;
            prov:agent [
                    a prov:Agent ;
                    rdfs:label "Engineers Australia: Test & Quality Assurance Lead"
                ]
        ] ;
    skos:hasTopConcept
        ctrl:good,
        ctrl:satisfactory,
        ctrl:poor,
        ctrl:uncontrolled ;
    skos:definition "The effectiveness to which systems and processes are able to mitigate risk and enable desired outcomes. The level of control over risk that exists within a given set of conditions."@en ;
    skos:altLabel "Control Effectiveness Rating"@en ;
    skos:prefLabel "Control Effectiveness"@en .

ctrl:good a skos:Concept ;
    dcterms:source "https://www.engineersaustralia.org.au"^^xsd:anyURI ;
	rdfs:isDefinedBy <https://linked.data.gov.au/def/control-effectiveness>;
    skos:inScheme <https://linked.data.gov.au/def/control-effectiveness> ;
    skos:topConceptOf <https://linked.data.gov.au/def/control-effectiveness> ;
	skos:definition """- Controls are well designed, address the risk, and are effective and reliable at all times.
    - Require ongoing maintenance and monitoring.
    - Management may, at their discretion, consider further controls to reduce risk."""@en;
    skos:altLabel "Good"@en ;
    skos:prefLabel "1. Good"@en .

ctrl:satisfactory a skos:Concept ;
    dcterms:source "https://www.engineersaustralia.org.au"^^xsd:anyURI ;
	rdfs:isDefinedBy <https://linked.data.gov.au/def/control-effectiveness>;
    skos:inScheme <https://linked.data.gov.au/def/control-effectiveness> ;
    skos:topConceptOf <https://linked.data.gov.au/def/control-effectiveness> ;
	skos:definition """- Most controls are designed correctly and are in place and effective. 
    - Controls address risk at least partially however may require further improvement. 
    - Some work needs to be done to improve operating effectiveness or management has doubts about operational effectiveness and reliability of some controls.
    - Consideration be given to implementing further controls for risks outside of appetite."""@en;
    skos:altLabel "Satisfactory"@en ;
    skos:prefLabel "2. Satisfactory"@en .

ctrl:poor a skos:Concept ;
    dcterms:source "https://www.engineersaustralia.org.au"^^xsd:anyURI ;
	rdfs:isDefinedBy <https://linked.data.gov.au/def/control-effectiveness>;
    skos:inScheme <https://linked.data.gov.au/def/control-effectiveness> ;
    skos:topConceptOf <https://linked.data.gov.au/def/control-effectiveness> ;
	skos:definition """- There are controls, but they do not effectively address the risk or require significant improvement. 
    - Most of the controls do not seem correctly designed, in that they do not operate effectively. 
    - Significant control gaps. 
    - Additional controls must be developed for all risks outside of appetite."""@en;
    skos:altLabel "Poor"@en ;
    skos:prefLabel "3. Poor"@en .

ctrl:uncontrolled a skos:Concept ;
    dcterms:source "https://www.engineersaustralia.org.au"^^xsd:anyURI ;
	rdfs:isDefinedBy <https://linked.data.gov.au/def/control-effectiveness>;
    skos:inScheme <https://linked.data.gov.au/def/control-effectiveness> ;
    skos:topConceptOf <https://linked.data.gov.au/def/control-effectiveness> ;
	skos:definition """- There is virtually no credible control, or controls that exist do not address the risk. 
    - Management has no confidence that any degree of control is being achieved due to poor control design and/or very limited operational effectiveness.
    - Controls must be implemented to address risks outside of appetite."""@en;
    skos:altLabel "Uncontrolled"@en ;
    skos:prefLabel "4. Uncontrolled"@en .