@prefix agnt: <https://ref.engineersaustralia.org.au/def/ea-agents/> .
@prefix cs: <https://ref.engineersaustralia.org.au/def/ea-agents> .
@prefix dcterms: <http://purl.org/dc/terms/> .
@prefix orgtyp: <http://linked.data.gov.au/def/organisation-type/> .
@prefix owl: <http://www.w3.org/2002/07/owl#> .
@prefix rdfs: <http://www.w3.org/2000/01/rdf-schema#> .
@prefix sdo: <http://schema.org/> .
@prefix skos: <http://www.w3.org/2004/02/skos/core#> .
@prefix xsd: <http://www.w3.org/2001/XMLSchema#> .


<https://ref.engineersaustralia.org.au/def/ea-agents> a owl:Ontology,
        skos:ConceptScheme ;
    dcterms:accessRights <https://linked.data.gov.au/def/data-access-rights/open> ;
    dcterms:created "2023-03-01"^^xsd:date ;
    dcterms:creator <https://linked.data.gov.au/org/engineersaustralia> ;
    dcterms:modified "2023-05-09"^^xsd:date ;
    dcterms:publisher <https://linked.data.gov.au/org/engineersaustralia> ;
    dcterms:source "https://linked.data.gov.au/org/engineersaustralia"^^xsd:anyURI ;
    skos:hasTopConcept
        agnt:person,
        agnt:organisation ;
    skos:definition """The types of agents who can interact with Engineers Australia to perform services as customers, staff, advisors, representatives etc. People and Organisations whose actions contribute to the operation of Engineers Australia."""@en ;
    skos:scopeNote """Agents describes the type of agent, whereas roles describes the actions performed by an agent. For example a University or Tertiary institution is a type of organisation but it may play a variety of roles in its interactions with Engineers Australia such as a customer, event host, advisor, vendor, etc."""@en;
    skos:prefLabel "Engineers Australia Agents"@en .

<https://linked.data.gov.au/org/engineersaustralia> a sdo:Organization ;
    sdo:name "Engineers Australia" ;
    sdo:url "https://www.engineersaustralia.org.au"^^xsd:anyURI .

agnt:person a skos:Concept ;
    rdfs:isDefinedBy cs: ;
    dcterms:source "https://linked.data.gov.au/org/engineersaustralia"^^xsd:anyURI ;
    skos:inScheme cs: ;
    skos:topConceptOf cs: ;
    skos:definition """A person is an individual human, acting in a personal or professional capacity. A natural human person."""@en ;
    skos:scopeNote "An individual acting as a business is considered an organisation that consists of one person. Commonly the correct classification for an individual acting in this capacity will be a Sole Trader"@en ;
    skos:altLabel "Individual"@en ;
    skos:prefLabel "Person"@en .

agnt:organisation a skos:Concept ;
    rdfs:isDefinedBy cs: ;
    dcterms:source "https://linked.data.gov.au/org/engineersaustralia"^^xsd:anyURI ;
    skos:inScheme cs: ;
    skos:topConceptOf cs: ;
    skos:definition """An organization is a group of people or other entities that interact to achieve a common goal."""@en ;
    skos:notation "Org" ;
    skos:prefLabel "Organization"@en .

    agnt:internal-group a skos:Concept ;
        rdfs:isDefinedBy cs: ;
        dcterms:source "https://linked.data.gov.au/org/engineersaustralia"^^xsd:anyURI ;
        skos:inScheme cs: ;
        skos:broader agnt:organisation ;
        skos:definition """An internal group is a group of people or other entities within, and intrinsically part of, an organization that work together to achieve a specific goal or set of goals."""@en ;
        skos:prefLabel "Internal Group"@en .

        agnt:business-unit a skos:Concept ;
            rdfs:isDefinedBy cs: ;
            dcterms:source "https://linked.data.gov.au/org/engineersaustralia"^^xsd:anyURI ;
            skos:inScheme cs: ;
            skos:broader agnt:internal-group ;
            skos:definition """A business unit is a department, division, or other functional entity within an organization that is responsible for a specific business function or set of functions."""@en ;
            skos:prefLabel "Business Unit"@en ;
            skos:notation "BU" ;
            skos:altLabel "Functional Unit"@en .

            agnt:division a skos:Concept ;
                rdfs:isDefinedBy cs: ;
                dcterms:source "https://linked.data.gov.au/org/engineersaustralia"^^xsd:anyURI ;
                skos:inScheme cs: ;
                skos:skos:broader agnt:business-unit ;
                skos:definition """A Division is an Engineers Australia Office that serves the EA Members & engineering community in a specific geographical region."""@en ;
                skos:notation "Div" ;
                skos:altLabel "State Division"@en,
                    "EA Office"@en,
                    "Engineers Australia Office"@en ;
                skos:prefLabel "Division"@en .

            agnt:functional-business-unit a skos:Concept ;
                rdfs:isDefinedBy cs: ;
                dcterms:source "https://linked.data.gov.au/org/engineersaustralia"^^xsd:anyURI ;
                skos:inScheme cs: ;
                skos:broader agnt:business-unit ;
                skos:definition """A functional business unit is a business unit that performs a specific function or set of functions within an organization."""@en ;
                skos:prefLabel "Functional Business Unit"@en ;
                skos:notation "FBU" ;
                skos:altLabel "Functional Unit"@en .

        agnt:board a skos:Concept ;
            rdfs:isDefinedBy cs: ;
            dcterms:source "https://linked.data.gov.au/org/engineersaustralia"^^xsd:anyURI ;
            skos:inScheme cs: ;
            skos:broader agnt:internal-group ;
            skos:definition """A group of people that are elected to represent the stakeholders in an organisation."""@en ;
            skos:altLabel "The Board"@en ;
            skos:prefLabel "Board"@en .

            agnt:board-committee a skos:Concept ;
                rdfs:isDefinedBy cs: ;
                dcterms:source "https://linked.data.gov.au/org/engineersaustralia"^^xsd:anyURI ;
                skos:inScheme cs: ;
                skos:broader agnt:learned-society ;
                skos:definition """An advisory body to The Board dedicated to a specific function of the organisation."""@en ;
                skos:prefLabel "Board Committee"@en .            

        agnt:learned-society a skos:Concept ;
            rdfs:isDefinedBy cs: ;
            dcterms:source "https://linked.data.gov.au/org/engineersaustralia"^^xsd:anyURI ;
            skos:inScheme cs: ;
            skos:broader agnt:internal-group ;
            skos:definition """A Learned Society is an association of like minded people who develop the knowledge and set the standards of its members. Learned Societies predominantly relate to a profession such as engineering, law, medicine, commerce etc. The EA Learned Society comprises four major groups: College Boards, National Committees, Technical Societies, and Special Interest Groups."""@en ;
            skos:altLabel "EA Learned Society"@en ;
            skos:prefLabel "Learned Society"@en .

            agnt:engineers-aus-college a skos:Concept ;
                rdfs:isDefinedBy cs: ;
                dcterms:source "https://linked.data.gov.au/org/engineersaustralia"^^xsd:anyURI ;
                skos:inScheme cs: ;
                skos:broader agnt:learned-society ;
                skos:definition """A College provides a discipline based home for members and provides a vehicle through which Engineers Australia advances the science and practice of engineering for the benefit of the Community through building the body of engineering knowledge and supporting the career development of engineering professionals."""@en ;
                skos:prefLabel "Engineers Australia College"@en  .

            agnt:national-committee a skos:Concept ;
                rdfs:isDefinedBy cs: ;
                dcterms:source "https://linked.data.gov.au/org/engineersaustralia"^^xsd:anyURI ;
                skos:inScheme cs: ;
                skos:broader agnt:learned-society ;
                skos:definition """National Committees are consituted by the Engineers Australia Board for issues with a natonal focus. National Committees must include a national focus, a maxium of 6 members, and an appropriate mix of age, gender, location and other aspects of diversity, representation and relevant skills including skills in management; and governance."""@en ;
                skos:prefLabel "National Committee"@en .

            agnt:special-interest-group a skos:Concept ;
                rdfs:isDefinedBy cs: ;
                dcterms:source "https://linked.data.gov.au/org/engineersaustralia"^^xsd:anyURI ;
                skos:inScheme cs: ;
                skos:broader agnt:learned-society ;
                skos:definition """A group or centre established by the Board where a national focus is required to ensure that the needs of a specific membership cohort can be addressed. The role of a Special Interest Group is to: 
                (a)  identify strategies and recommend to the Board actions to address the needs of their identified cohort;
                (b)  work with the Colleges, Technical Societies and the Chief Executive Officer to implement Board approved strategies and policies in relation to their identified cohort into the normal operations of each College, Technical  Society and Division, including undertaking joint activities; 
                (d)  liaise with and provide support to College Boards, Divisions and Technical  Societies regarding the undertaking of activities by these groups to support  their cohort; 
                (e)  communicate with their cohort to identify ongoing needs and to direct  them to areas within Engineers Australia that can assist them; and 
                (f)  arrange for an appropriate range of events or other activities in accordance with their approved plan to address needs that cannot normally be met  through other Engineers Australia channels."""@en ;
                skos:altLabel "Special Interest Centre"@en ;
                skos:prefLabel "Special Interest Group"@en  .

            agnt:technical-society a skos:Concept ;
                rdfs:isDefinedBy cs: ;
                dcterms:source "https://linked.data.gov.au/org/engineersaustralia"^^xsd:anyURI ;
                skos:inScheme cs: ;
                skos:broader agnt:learned-society ;
                skos:definition """An Engineers Australia Technical Society is a group that facilitates networking between professionals in the same area of expertise, hosts discussion forums, and provides access to technical papers and presentations. Technical societies provide professional technical development opportunities that its members may participate in. Membership in a technical society is not contingent on membership to Engineers Australia."""@en ;
                skos:altLabel "Engineers Australia Technical Society"@en ;
                skos:prefLabel "Technical Society"@en .

                agnt:inc-tech-society a skos:Concept ;
                    rdfs:isDefinedBy cs: ;
                    dcterms:source "https://linked.data.gov.au/org/engineersaustralia"^^xsd:anyURI ;
                    skos:inScheme cs: ;
                    skos:broader agnt:technical-society ;
                    skos:definition """Incorporated technical societies are governed by their own constitutions but choose to be aligned with Engineers Australia."""@en ;
                    skos:prefLabel "Incorporated Technical Society"@en .

                agnt:uninc-tech-society a skos:Concept ;
                    rdfs:isDefinedBy cs: ;
                    dcterms:source "https://linked.data.gov.au/org/engineersaustralia"^^xsd:anyURI ;
                    skos:inScheme cs: ;
                    skos:broader agnt:technical-society ;
                    skos:definition """Incorporated technical societies are governed by their own constitutions but choose to be aligned with Engineers Australia."""@en ;
                    skos:prefLabel "Unincorporated Technical Society"@en .

        agnt:overseas-chapter a skos:Concept ;
            rdfs:isDefinedBy cs: ;
            dcterms:source "https://linked.data.gov.au/org/engineersaustralia"^^xsd:anyURI ;
            skos:inScheme cs: ;
            skos:broader agnt:internal-group ;
            skos:definition """Overseas Chapters are representative bodies of a parent organisation consisting of members of the organisation whose principal place of residence is outside the organisation's primary country of operation."""@en ;
            skos:prefLabel "Overseas Chapter"@en .

    agnt:commercial-entity a skos:Concept ;
        rdfs:isDefinedBy cs: ;
        dcterms:source "https://linked.data.gov.au/org/engineersaustralia"^^xsd:anyURI ;
        skos:inScheme cs: ;
        skos:broader agnt:organisation ;
        skos:definition """A commercial entity is an organisation that engages in business activities with the primary goal of making a profit."""@en ;
        skos:prefLabel "Commercial Entity"@en .

        agnt:gov-run-company a skos:Concept ;
            rdfs:isDefinedBy cs: ;
            dcterms:source "https://www.abs.gov.au/ausstats/abs@.nsf/2f762f95845417aeca25706c00834efa/0c54fc71b70654d2ca257bdd00116288!OpenDocument"^^xsd:anyURI ;
            skos:inScheme cs: ;
            skos:broader agnt:commercial-entity ;
            skos:exactMatch orgtyp:government-companies ;
            skos:definition """Government units (as defined in Chapter 2) which are created as bodies corporate through the Corporations Act in Australia or through other legislation (ABS Catalogue 1218.0 SESCA, 2008, Chapter 8)."""@en ;
            skos:altLabel "Government Company"@en ;
            skos:prefLabel "Government-Run Company"@en .

        agnt:private-company a skos:Concept ;
            rdfs:isDefinedBy cs: ;
            dcterms:source "https://linked.data.gov.au/org/engineersaustralia"^^xsd:anyURI ;
            skos:inScheme cs: ;
            skos:broader agnt:commercial-entity ;
            skos:exactMatch orgtyp:proprietary-companies ;
            skos:definition """A private company is a commercial entity that is privately owned and not publicly traded."""@en ;
            skos:prefLabel "Private Company"@en .

        agnt:public-company a skos:Concept ;
            rdfs:isDefinedBy cs: ;
            dcterms:source "https://linked.data.gov.au/org/engineersaustralia"^^xsd:anyURI ;
            skos:inScheme cs: ;
            skos:broader agnt:commercial-entity ;
            skos:exactMatch orgtyp:public-companies ;
            skos:definition """A public company is a commercial entity whose shares can be bought and sold by the general public on a stock exchange."""@en ;
            skos:prefLabel "Public Company"@en .

        agnt:sole-trader a skos:Concept ;
            rdfs:isDefinedBy cs: ;
            dcterms:source "https://linked.data.gov.au/org/engineersaustralia"^^xsd:anyURI ;
            skos:inScheme cs: ;
            skos:broader agnt:commercial-entity ;
            skos:exactMatch orgtyp:sole-proprietorship ;
            skos:definition """A sole trader is an individual who owns and operates a business, and is personally liable for business debts."""@en ;
            skos:prefLabel "Sole Trader"@en .

        agnt:trust a skos:Concept ;
            rdfs:isDefinedBy cs: ;
            dcterms:source "https://linked.data.gov.au/org/engineersaustralia"^^xsd:anyURI ;
            skos:inScheme cs: ;
            skos:broader agnt:organisation ;
            skos:definition """A trust is a legal arrangement where property is held by one party for the benefit of another party."""@en ;
            skos:prefLabel "Trust"@en .

    agnt:government-agency a skos:Concept ;
        rdfs:isDefinedBy cs: ;
        dcterms:source "https://linked.data.gov.au/org/engineersaustralia"^^xsd:anyURI ;
        skos:inScheme cs: ;
        skos:broader agnt:organisation ;
        skos:notation "Gov" ;
        skos:exactMatch orgtyp:other-government-entities ;
        skos:definition """A government agency is a permanent or semi-permanent organization in the machinery of government that is responsible for the oversight and administration of specific functions, such as an intelligence agency, regulatory agency, or tax collection agency."""@en ;
        skos:prefLabel "Government Agency"@en .

        agnt:federal-gov-agency a skos:Concept ;
            rdfs:isDefinedBy cs: ;
            dcterms:source "https://linked.data.gov.au/org/engineersaustralia"^^xsd:anyURI ;
            skos:inScheme cs: ;
            skos:broader agnt:government-agency ;
            skos:definition """A federal government agency is a government agency that is responsible for the oversight and administration of specific functions at the federal level."""@en ;
            skos:prefLabel "Federal Government Agency"@en .

            agnt:defence-force a skos:Concept ;
                rdfs:isDefinedBy cs: ;
                dcterms:source "https://linked.data.gov.au/org/engineersaustralia"^^xsd:anyURI ;
                skos:inScheme cs: ;
                skos:broader agnt:federal-gov-agency ;
                skos:definition """A government funded agency within the Defence Force or Armed Services."""@en ;
                skos:prefLabel "Defence Force Agency"@en .

        agnt:state-gov-agency a skos:Concept ;
            rdfs:isDefinedBy cs: ;
            dcterms:source "https://linked.data.gov.au/org/engineersaustralia"^^xsd:anyURI ;
            skos:inScheme cs: ;
            skos:broader agnt:government-agency ;
            skos:definition """A state government agency is a government agency that is responsible for the oversight and administration of specific functions at the state or territory level."""@en ;
            skos:altLabel "Territory Government Agency"@en ;
            skos:prefLabel "State Government Agency"@en .

        agnt:local-gov-agency a skos:Concept ;
            rdfs:isDefinedBy cs: ;
            dcterms:source "https://linked.data.gov.au/org/engineersaustralia"^^xsd:anyURI ;
            skos:inScheme cs: ;
            skos:broader agnt:government-agency ;
            skos:definition """A local government agency is a government agency that is responsible for the oversight and administration of specific functions at the local level. In Australia this is associated with a Local Government Area (LGA)."""@en ;
            skos:prefLabel "Local Government Agency"@en .

    agnt:tertiary-institution a skos:Concept ;
        rdfs:isDefinedBy cs: ;
        dcterms:source "https://linked.data.gov.au/org/engineersaustralia"^^xsd:anyURI ;
        skos:broader agnt:organisation ;
        skos:inScheme cs: ;
        skos:definition """Tertiary education refers to post-secondary education received at universities and vocational educational institutes."""@en ;
        skos:prefLabel "Tertiary institution"@en .

        agnt:vet-institute a skos:Concept ;
            rdfs:isDefinedBy cs: ;
            dcterms:source "https://www.training.com.au/vet-courses/"^^xsd:anyURI ;
            skos:inScheme cs: ;
            skos:broader agnt:tertiary-institution ;
            skos:definition """A VET institute is an educational institution that provides Vocational Education and Training (VET) courses.
            
            VET courses are offered through both public and private RTOs, generally via TAFE and private training providers. Some VET courses are delivered through Australian Apprenticeships and Traineeships, which enable students to gain structured on-the-job training as a major part of their study. Along with these institutions, VET training and is also accessible through participating schools, as well as external community educational centres."""@en ;
            skos:prefLabel "VET institute"@en .

        agnt:university a skos:Concept ;
            rdfs:isDefinedBy cs: ;
            dcterms:source "https://linked.data.gov.au/org/engineersaustralia"^^xsd:anyURI ;
            skos:inScheme cs: ;
            skos:notation "Uni" ;
            skos:broader agnt:tertiary-institution ;
            skos:definition """A university is an educational institution that provides undergraduate and postgraduate education and research."""@en ;
            skos:prefLabel "University"@en  .