PREFIX award: <https://ref.engineersaustralia.org.au/def/ea-awards/>
PREFIX dcat: <http://www.w3.org/ns/dcat#>
PREFIX dcterms: <http://purl.org/dc/terms/>
PREFIX earl: <https://ref.engineersaustralia.org.au/def/ea-activity-roles/>
PREFIX eaclg: <https://linked.data.gov.au/def/ea-colleges/>
PREFIX ieaoc: <https://linked.data.gov.au/def/iea-occupational-categories/>
PREFIX owl: <http://www.w3.org/2002/07/owl#>
PREFIX prov: <http://www.w3.org/ns/prov#>
PREFIX rdfs: <http://www.w3.org/2000/01/rdf-schema#>
PREFIX sdo: <http://schema.org/>
PREFIX skos: <http://www.w3.org/2004/02/skos/core#>
PREFIX xsd: <http://www.w3.org/2001/XMLSchema#>

<https://linked.data.gov.au/org/engineersaustralia> a sdo:Organization ;
    sdo:name "Engineers Australia" ;
    sdo:url "https://www.engineersaustralia.org.au"^^xsd:anyURI .

<https://ref.engineersaustralia.org.au/def/ea-awards> a owl:Ontology,
        skos:ConceptScheme ;
    dcterms:accessRights <https://linked.data.gov.au/def/data-access-rights/open> ;
    dcterms:created "2023-03-01"^^xsd:date ;
    dcterms:creator <https://linked.data.gov.au/org/engineersaustralia> ;
    dcterms:modified "2023-03-01"^^xsd:date ;
    dcterms:publisher <https://linked.data.gov.au/org/engineersaustralia> ;
    dcterms:source "https://linked.data.gov.au/org/engineersaustralia"^^xsd:anyURI ;
    prov:qualifiedAttribution
        [
            dcat:hadRole earl:data-steward ;
            prov:agent [
                    a prov:Agent ;
                    rdfs:label "Engineers Australia: Awards"
                ]
        ] ;
    skos:definition """An EA Award is an Engineers Australia award for service or achievement to the organisation of Engineers Australia or to the engineering profession."""@en ;
    skos:hasTopConcept
        award:aeea,
        award:division,
        award:recognition,
        award:tertiary ;
    skos:altLabel "EA Award"@en ;
    skos:prefLabel "Engineers Australia Awards"@en .

award:aeea a skos:Concept ;
    rdfs:isDefinedBy <https://ref.engineersaustralia.org.au/def/ea-awards> ;
    dcterms:source "https://www.engineersaustralia.org.au/about-us/excellence-awards-program"^^xsd:anyURI ;
    skos:definition """The Engineers Australia excellence awards program promotes the prestige of the practice of engineering while recognising the outstanding achievements of individual engineering professionals."""@en ;
    skos:altLabel "Australian Engineering Excellence Awards"@en ;
    skos:notation "AEEA" ;
    skos:prefLabel "Engineers Australia Excellence Awards"@en ;
    skos:inScheme <https://ref.engineersaustralia.org.au/def/ea-awards> ;
    skos:topConceptOf <https://ref.engineersaustralia.org.au/def/ea-awards> .


    award:ea-people a skos:Concept ;
        rdfs:isDefinedBy <https://ref.engineersaustralia.org.au/def/ea-awards> ;
        dcterms:source "https://www.engineersaustralia.org.au/about-us/excellence-awards-program"^^xsd:anyURI ;
        skos:definition """People awards acknowledge individual engineers for outstanding innovation and resourcefulness in their work. The engineer of the year awards recognise engineering professionals at all stages of their career. Six awards are available based on the three occupational categories.
        
        Career achievement awards apply to individual engineering professionals at all career levels and across the occupational categories. There are 11 individual awards in this category mostly aligned to each of the engineering colleges.
        
        Also in the people category are the distinguished career awards. This category contains three separate awards which recognise the conspicuous service of individuals who have given longstanding and prominent service to the profession."""@en ;
        skos:prefLabel "Engineers Australia People Awards"@en ;
        skos:inScheme <https://ref.engineersaustralia.org.au/def/ea-awards> ;
        skos:broader award:aeea .

        award:eoy a skos:Concept ;
            rdfs:isDefinedBy <https://ref.engineersaustralia.org.au/def/ea-awards> ;
            dcterms:source "https://www.engineersaustralia.org.au/about-us/excellence-awards-program/engineer-year-awards"^^xsd:anyURI ;
            skos:definition """The engineer of the year awards recognise the outstanding work of engineering professionals at all stages of their career.
            
            These awards acknowledge and reward the outstanding work of individuals and establish an aspirational benchmark for future engineering professionals.
            
            Award recipients will have demonstrated the following in their work:
            - Contribution to the wellbeing of people and communities.
            - Formulation of resourceful, innovative and aesthetically appealing engineering solutions or pioneering use of materials or methods.
            - Contribution to Engineers Australia's purpose and strategic vision.
            - Contribution to and promote the engineering profession.
            - Notable achievements during an engineering career."""@en ;
            skos:altLabel "Engineer of the Year Awards"@en ;
            skos:prefLabel "Engineer of the Year"@en ;
            skos:inScheme <https://ref.engineersaustralia.org.au/def/ea-awards> ;
            skos:broader award:ea-people .

            award:professional-engineer-of-the-year a skos:Concept ;
                rdfs:isDefinedBy <https://ref.engineersaustralia.org.au/def/ea-awards> ;
                dcterms:source "https://aeea.engineersaustralia.org.au/awards/"^^xsd:anyURI ;
                skos:related ieaoc:pro-engineer ;
                skos:definition """The Professional Engineer of the Year award recognises outstanding individual engineering achievements and innovation and resourcefulness of a Professional Engineer."""@en ;
                skos:prefLabel "Professional Engineer of the Year"@en ;
                skos:inScheme <https://ref.engineersaustralia.org.au/def/ea-awards> ;
                skos:broader award:eoy .

            award:engineering-technologist-of-the-year a skos:Concept ;
                rdfs:isDefinedBy <https://ref.engineersaustralia.org.au/def/ea-awards> ;
                dcterms:source "https://aeea.engineersaustralia.org.au/awards/"^^xsd:anyURI ;
                skos:related ieaoc:tech-engineer ;
                skos:definition """The Engineering Technologist of the Year award recognises outstanding individual engineering achievements and innovation and resourcefulness of an Engineering Technologist."""@en ;
                skos:prefLabel "Engineering Technologist of the Year"@en ;
                skos:inScheme <https://ref.engineersaustralia.org.au/def/ea-awards> ;
                skos:broader award:eoy .
                
            award:engineering-associate-of-the-year a skos:Concept ;
                rdfs:isDefinedBy <https://ref.engineersaustralia.org.au/def/ea-awards> ;
                dcterms:source "https://aeea.engineersaustralia.org.au/awards/"^^xsd:anyURI ;
                skos:related ieaoc:assoc-engineer ;
                skos:definition """The Engineering Associate of the Year award recognises outstanding individual engineering achievements and innovation and resourcefulness of an Engineering Associate"""@en ;
                skos:prefLabel "Engineering Associate of the Year"@en ;
                skos:inScheme <https://ref.engineersaustralia.org.au/def/ea-awards> ;
                skos:broader award:eoy .

            award:emerging-professional-engineer-of-the-year a skos:Concept ;
                rdfs:isDefinedBy <https://ref.engineersaustralia.org.au/def/ea-awards> ;
                dcterms:source "https://aeea.engineersaustralia.org.au/awards/"^^xsd:anyURI ;
                skos:related ieaoc:pro-engineer ;
                skos:definition """The Emerging Professional Engineer of the Year award recognises outstanding individual engineering achievements and innovation and resourcefulness of a Professional Engineer under the age of 35."""@en ;
                skos:prefLabel "Emerging Professional Engineer of the Year"@en ;
                skos:inScheme <https://ref.engineersaustralia.org.au/def/ea-awards> ;
                skos:broader award:eoy .

            award:emerging-engineering-technologist-of-the-year a skos:Concept ;
                rdfs:isDefinedBy <https://ref.engineersaustralia.org.au/def/ea-awards> ;
                dcterms:source "https://aeea.engineersaustralia.org.au/awards/"^^xsd:anyURI ;
                skos:related ieaoc:tech-engineer ;
                skos:definition """The Emerging Engineering Technologist of the Year award recognises outstanding individual engineering achievements and innovation and resourcefulness of an Engineering Technologist under the age of 35."""@en ;
                skos:prefLabel "Emerging Engineering Technologist of the Year"@en ;
                skos:inScheme <https://ref.engineersaustralia.org.au/def/ea-awards> ;
                skos:broader award:eoy .

            award:emerging-engineering-associate-of-the-year a skos:Concept ;
                rdfs:isDefinedBy <https://ref.engineersaustralia.org.au/def/ea-awards> ;
                dcterms:source "https://aeea.engineersaustralia.org.au/awards/"^^xsd:anyURI ;
                skos:related ieaoc:assoc-engineer ;
                skos:definition """The Emerging Engineering Associate of the Year award recognises outstanding individual engineering achievements and innovation and resourcefulness of an Engineering Associate under the age of 35."""@en ;
                skos:prefLabel "Emerging Engineering Associate of the Year"@en ;
                skos:inScheme <https://ref.engineersaustralia.org.au/def/ea-awards> ;
                skos:broader award:eoy .

        award:achievement a skos:Concept ;
            rdfs:isDefinedBy <https://ref.engineersaustralia.org.au/def/ea-awards> ;
            dcterms:source "https://www.engineersaustralia.org.au/about-us/excellence-awards-program/achievement-awards"^^xsd:anyURI ;
            skos:definition """Engineers Australias achievement awards recognise the important engineering achievements of individuals at all career stages and across Engineers Australia's colleges and engineering communities."""@en ;
            skos:prefLabel "Achievement Awards"@en ;
            skos:inScheme <https://ref.engineersaustralia.org.au/def/ea-awards> ;
            skos:broader award:ea-people .

            #Biomedical College: David Dewhurst Award
            award:david-dewhurst-award a skos:Concept ;
                rdfs:isDefinedBy <https://ref.engineersaustralia.org.au/def/ea-awards> ;
                dcterms:source "https://www.engineersaustralia.org.au/about-us/excellence-awards-program/achievement-awards"^^xsd:anyURI ;
                skos:definition """The David Dewhurst Award honours one of Australia's first biomedical engineers, Dr David Dewhurst, whose work and legacy contributed to present-day biomedical engineering.
                
                The David Dewhurst Award is presented to a biomedical engineer who has made a significant contribution to the discipline.
                
                Recipients are presented with a framed bronze medal and certificate at an Engineers Australia award event."""@en ;
                skos:related eaclg:biomedical ;
                skos:altLabel "David Dewhurst Medal"@en,
                    "Biomedical College: David Dewhurst Award"@en ;
                skos:prefLabel "David Dewhurst Award"@en ;
                skos:inScheme <https://ref.engineersaustralia.org.au/def/ea-awards> ;
                skos:broader award:achievement .

            #Chemical College: Chemical Engineer Achievement Award
            award:chemical-engineer-achievement-award a skos:Concept ;
                rdfs:isDefinedBy <https://ref.engineersaustralia.org.au/def/ea-awards> ;
                dcterms:source "https://www.engineersaustralia.org.au/about-us/excellence-awards-program/achievement-awards"^^xsd:anyURI ;
                skos:definition """The Chemical Engineer Achievement Award is presented to a prominent Australian or New Zealand chemical engineer who has made an outstanding contribution to chemical engineering by their achievements or service.

                Recipients are presented with a framed certificate at an Engineers Australia award event."""@en ;
                skos:related eaclg:chemical ;
                skos:prefLabel "Chemical Engineer Achievement Award"@en ;
                skos:inScheme <https://ref.engineersaustralia.org.au/def/ea-awards> ;
                skos:broader award:achievement .

            #Civil College: Sir John Holland Civil Engineer of the Year
            award:sir-john-holland-civil-engineer-of-the-year-award a skos:Concept ;
                rdfs:isDefinedBy <https://ref.engineersaustralia.org.au/def/ea-awards> ;
                dcterms:source "https://www.engineersaustralia.org.au/about-us/excellence-awards-program/achievement-awards"^^xsd:anyURI ;
                skos:definition """This award honours Sir John Holland a notable civil engineer and construction magnate who founded the John Holland Construction group. The award is presented to an eminent civil engineer who has made a major contribution to the profession.

                Recipients are presented with a framed certificate and sculpture at an Engineers Australia award event."""@en ;
                skos:related eaclg:civil ;
                skos:prefLabel "Sir John Holland Civil Engineer of the Year"@en ;
                skos:inScheme <https://ref.engineersaustralia.org.au/def/ea-awards> ;
                skos:broader award:achievement .

            #Electrical College: MA Sargent Medal
            award:m-a-sargent-medal a skos:Concept ;
                rdfs:isDefinedBy <https://ref.engineersaustralia.org.au/def/ea-awards> ;
                dcterms:source "https://www.engineersaustralia.org.au/about-us/excellence-awards-program/achievement-awards"^^xsd:anyURI ;
                skos:definition """This award honours Dr Michael Anthony Sargent. Dr Sargent was an outstanding electrical engineer and honorary Fellow of Engineers Australia who served in several prominent Engineers Australia office bearer roles throughout his career.
                
                The MA Sargent Medal is awarded to an electrical engineer who has made a highly significant contribution to electrical engineering.
                
                Recipients are presented with a framed certificate and engraved medal at an Engineers Australia award event."""@en ;
                skos:related eaclg:electrical ;
                skos:prefLabel "M A Sargent Medal"@en ;
                skos:inScheme <https://ref.engineersaustralia.org.au/def/ea-awards> ;
                skos:broader award:achievement .


            #Engineering Heritage Australia: John Monash Medal
            award:john-monash-medal a skos:Concept ;
                rdfs:isDefinedBy <https://ref.engineersaustralia.org.au/def/ea-awards> ;
                dcterms:source "https://www.engineersaustralia.org.au/about-us/excellence-awards-program/achievement-awards"^^xsd:anyURI ;
                skos:definition """This award honours Sir John Monash who was a civil engineer and an important Australian military commander of the first world war. The John Monash Medal is awarded for outstanding contributions to engineering heritage over a considerable period.

                Recipients are awarded an inscribed medal and certificate at an Engineers Australia award event."""@en ;
                skos:prefLabel "John Monash Medal"@en ;
                skos:inScheme <https://ref.engineersaustralia.org.au/def/ea-awards> ;
                skos:broader award:achievement .


            #Environment College: Environmental Engineer Achievement Award
            award:environmental-engineer-achievement-award a skos:Concept ;
                rdfs:isDefinedBy <https://ref.engineersaustralia.org.au/def/ea-awards> ;
                dcterms:source "https://www.engineersaustralia.org.au/about-us/excellence-awards-program/achievement-awards"^^xsd:anyURI ;
                skos:definition """This award acknowledges a prominent environmental engineer who has made an outstanding contribution to engineering by promoting:
                - environmental and sustainability excellence
                - the profession within the community.

                Recipients are presented with a certificate at an Engineers Australia award event."""@en ;
                skos:related eaclg:environmental ;
                skos:prefLabel "Environmental Engineer Achievement Award"@en ;
                skos:inScheme <https://ref.engineersaustralia.org.au/def/ea-awards> ;
                skos:broader award:achievement .

            #ITEE College: IREE Neville Thiele Eminence Award
            award:iree-neville-thiele-eminence-award a skos:Concept ;
                rdfs:isDefinedBy <https://ref.engineersaustralia.org.au/def/ea-awards> ;
                dcterms:source "https://www.engineersaustralia.org.au/about-us/excellence-awards-program/achievement-awards"^^xsd:anyURI ;
                skos:definition """This award honours the Institution of Radio and Electronics Engineers (IREE) an organisation that represented early Australian radio and electronics engineering. It also honours Neville Thiele, a world renown electronic engineer.

                The IREE Neville Thiele Eminence Award is presented annually at an Engineers Australia event. Recipients receive a framed certificate, engraved medal and a cash prize of $10,000."""@en ;
                skos:related eaclg:itee ;
                skos:altLabel "Neville Thiele Eminence Award"@en ;
                skos:prefLabel "IREE Neville Thiele Eminence Award"@en ;
                skos:inScheme <https://ref.engineersaustralia.org.au/def/ea-awards> ;
                skos:broader award:achievement .

            #Mechanical College: AGM Michell Medal
            award:agm-michell-medal a skos:Concept ;
                rdfs:isDefinedBy <https://ref.engineersaustralia.org.au/def/ea-awards> ;
                dcterms:source "https://www.engineersaustralia.org.au/about-us/excellence-awards-program/achievement-awards"^^xsd:anyURI ;
                skos:definition """This award honours Anthony George Maldon Michell, an outstanding Australian mechanical engineer who lived in the late 19th and early 20th centuries.
                
                The AGM Michell Medal was first presented in 1978 and is awarded annually by the Mechanical College Board to someone who has given outstanding service to mechanical engineering.
                
                Successful recipients of the AGM Michell Medal are awarded a bronze medal and accompanying certificate at an Engineers Australia presentation dinner. Winners are also invited to give a presentation on a topic of their choice which will be published in the Australian Journal of Mechanical Engineering."""@en ;
                skos:related eaclg:mechanical ;
                skos:altLabel "A G M Michell Prize"@en ;
                skos:prefLabel "AGM Michell Medal"@en ;
                skos:inScheme <https://ref.engineersaustralia.org.au/def/ea-awards> ;
                skos:broader award:achievement .

            #RISK Society: Risk Engineer Achievement Award
            award:risk-engineer-achievement-award a skos:Concept ;
                rdfs:isDefinedBy <https://ref.engineersaustralia.org.au/def/ea-awards> ;
                dcterms:source "https://www.engineersaustralia.org.au/about-us/excellence-awards-program/achievement-awards"^^xsd:anyURI ;
                skos:definition """This award acknowledges a prominent risk engineer who has made an outstanding contribution to engineering by promoting:
                - excellence in the practice of risk engineering and risk management
                - the profession within the community.

                Leading risk engineers require a comprehensive knowledge of their organisation so they can create solutions that improve business performance. Successful recipients of this award will have demonstrated a business outcome focus and business achievement in their nomination.

                Recipients are presented with a framed certificate at an Engineers Australia award event."""@en ;
                skos:prefLabel "Risk Engineer Achievement Award"@en ;
                skos:inScheme <https://ref.engineersaustralia.org.au/def/ea-awards> ;
                skos:broader award:achievement .

            #Structural College: John Connell Gold Medal
            award:john-connell-gold-medal a skos:Concept ;
                rdfs:isDefinedBy <https://ref.engineersaustralia.org.au/def/ea-awards> ;
                dcterms:source "https://www.engineersaustralia.org.au/about-us/excellence-awards-program/achievement-awards"^^xsd:anyURI ;
                skos:definition """This award honours John Connell who made an outstanding contribution to structural engineering and founded John Connell and Associates in 1958. His company merged with others and eventually became part of Aurecon.

                The John Connell Gold Medal is presented to an individual who has made a significant national and international contribution to the structural engineering profession.
                
                Recipients are presented with a mounted and framed gold medal at an Engineers Australia award event."""@en ;
                skos:related eaclg:structural ;
                skos:prefLabel "John Connell Gold Medal"@en ;
                skos:inScheme <https://ref.engineersaustralia.org.au/def/ea-awards> ;
                skos:broader award:achievement .

            #Transport Australia society: Transport Medal
            award:transport-medal a skos:Concept ;
                rdfs:isDefinedBy <https://ref.engineersaustralia.org.au/def/ea-awards> ;
                dcterms:source "https://www.engineersaustralia.org.au/about-us/excellence-awards-program/achievement-awards"^^xsd:anyURI ;
                skos:definition """The Transport Medal recognises outstanding individual contributions to transport in Australia. The award is open to applicants across public and private sectors including transport operators, consultants, government, academia and researchers.
                
                Applicants don't need to be a member of Engineers Australia and can nominate themselves or be nominated by someone else.

                Recipients are presented with a framed certificate and engraved medal at an Engineers Australia's event."""@en ;
                skos:prefLabel "Transport Medal"@en ;
                skos:inScheme <https://ref.engineersaustralia.org.au/def/ea-awards> ;
                skos:broader award:achievement .
        
        award:distinguished-career a skos:Concept ;
            rdfs:isDefinedBy <https://ref.engineersaustralia.org.au/def/ea-awards> ;
            dcterms:source "https://www.engineersaustralia.org.au/about-us/excellence-awards-program/distinguished-career-awards"^^xsd:anyURI ;
            skos:definition """Engineers Australia's three distinguished career awards recognise and reward the achievements of engineers who have achieved a lifetime of outstanding success."""@en ;
            skos:prefLabel "Distinguished Career Awards"@en ;
            skos:inScheme <https://ref.engineersaustralia.org.au/def/ea-awards> ;
            skos:broader award:ea-people .

            award:pnr-medal a skos:Concept ;
                rdfs:isDefinedBy <https://ref.engineersaustralia.org.au/def/ea-awards> ;
                dcterms:source "https://www.engineersaustralia.org.au/about-us/excellence-awards-program/distinguished-career-awards"^^xsd:anyURI ;
                skos:definition """This award honours Sir Peter Nicol Russell, a Sydney industrialist of the 19th century who made major donations toward engineering in Australia.
                
                It is the most prestigious award conferred by Engineers Australia. It's presented annually to an Honorary Fellow of Engineers Australia and who has made a notable contribution to the science or practice of engineering in Australia.
                
                Recipients epitomise:
                - The highest technical, professional and community service standards of the engineering profession.
                - An outstanding example of leadership and management within the engineering industry.
                - The broad nature and impacts of the engineering profession through their significant contributions.
                
                Winners are presented with a framed certificate and PNR memorial medal at an Engineers Australia award event."""@en ;
                skos:altLabel "Peter Nicol Russel Career Achievement Memorial Medal"@en ;
                skos:prefLabel "PNR Medal"@en ;
                skos:inScheme <https://ref.engineersaustralia.org.au/def/ea-awards> ;
                skos:broader award:distinguished-career .

            award:honorary-fellows a skos:Concept ;
                rdfs:isDefinedBy <https://ref.engineersaustralia.org.au/def/ea-awards> ;
                dcterms:source "https://www.engineersaustralia.org.au/about-us/excellence-awards-program/distinguished-career-awards"^^xsd:anyURI ;
                skos:definition """This award elevates the recipient to the level of Fellow of Engineers Australia, the highest credential available to members.

                The Honorary Fellows Award is conferred by the Board of Engineers Australia on a recipient who has demonstrated:
                - Notable contributions or achievements in the engineering profession or to an allied science.
                - The highest technical, professional and community service standards of engineering
                - Service to the Australian people or in recognition of outstanding achievement.
                
                Recipients are presented with a framed certificate at an Engineers Australia award event."""@en ;
                skos:altLabel "Honorary Fellows"@en,
                    "Honorary Fellow (HonFIEAust)"@en,
                    "Honorary Fellows (HonFIEAust)"@en,
                    "Honorary Fellow Awards"@en ;
                skos:prefLabel "Honorary Fellows Award"@en ;
                skos:inScheme <https://ref.engineersaustralia.org.au/def/ea-awards> ;
                skos:broader award:distinguished-career .

            award:president-prize a skos:Concept ;
                rdfs:isDefinedBy <https://ref.engineersaustralia.org.au/def/ea-awards> ;
                dcterms:source "https://www.engineersaustralia.org.au/about-us/excellence-awards-program/distinguished-career-awards"^^xsd:anyURI ;
                skos:definition """The President Prize award is awarded on an annual basis to an individual or group who has provided distinct service to the profession or the community. The recipient's service must also have contributed towards the strategic goals of Engineers Australia.
                
                Award recipients are chosen by Engineers Australia's National President and presented with a framed certificate at an Engineers Australia award event."""@en ;
                skos:altLabel "President's Prize"@en,
                    "President Prize"@en ;
                skos:prefLabel "The President Prize"@en ;
                skos:inScheme <https://ref.engineersaustralia.org.au/def/ea-awards> ;
                skos:broader award:distinguished-career .

    award:project a skos:Concept ;
        rdfs:isDefinedBy <https://ref.engineersaustralia.org.au/def/ea-awards> ;
        dcterms:source "https://aeea.engineersaustralia.org.au/awards/"^^xsd:anyURI ;
        skos:definition """The project awards recognise Australia's top engineering projects and the teams behind them. It inspires and encourages engineering distinction through teamwork, innovation and technical excellence."""@en ;
        skos:prefLabel "Engineers Australia Project Awards"@en ;
        skos:inScheme <https://ref.engineersaustralia.org.au/def/ea-awards> ;
        skos:broader award:aeea .

        award:division-project-finalist a skos:Concept ;
            rdfs:isDefinedBy <https://ref.engineersaustralia.org.au/def/ea-awards> ;
            dcterms:source "https://aeea.engineersaustralia.org.au/awards/"^^xsd:anyURI ;
            skos:definition """Engineering project teams submit their entries through their local Engineers Australia division. Each division chooses a finalist project team who goes on to compete with other divisional finalists. A national winner is then chosen from the division finalists and is awarded Project of the Year."""@en ;
            skos:altLabel "Project of the Year - Division"@en,
                "Project Award - Division"@en,
                "Division Finalist"@en ;
            skos:prefLabel "Division Project Finalist"@en ;
            skos:inScheme <https://ref.engineersaustralia.org.au/def/ea-awards> ;
            skos:broader award:project .

        award:project-of-the-year a skos:Concept ;
            rdfs:isDefinedBy <https://ref.engineersaustralia.org.au/def/ea-awards> ;
            dcterms:source "https://aeea.engineersaustralia.org.au/awards/"^^xsd:anyURI ;
            skos:definition """Engineers Australia's project awards recognises Australia's top engineering projects and the teams behind them. Engineering project teams submit their entries locally through an Engineers Australia division. Each division chooses a finalist project team who goes on to compete with other divisional finalists. A national winner is then chosen from the division finalists and is awarded Project of the Year."""@en ;
            skos:hiddenLabel "Sir William Hudson Award"@en ;
            skos:prefLabel "Project of the Year"@en ;
            skos:inScheme <https://ref.engineersaustralia.org.au/def/ea-awards> ;
            skos:broader award:project .

award:division a skos:Concept ;
    rdfs:isDefinedBy <https://ref.engineersaustralia.org.au/def/ea-awards> ;
    dcterms:source "https://aeea.engineersaustralia.org.au/awards/"^^xsd:anyURI ;
    skos:definition """Engineering awards given to outstanding work specific to the geographical divisions of Engineers Australia.

    Each award is made annually based on a technical paper but governed by conditions which are broad enough to cover special local requirements. Each award consists of a bronze medal with the winner's name engraved on it and a cash prize set by the Board of Engineers Australia."""@en ;
    skos:prefLabel "Division Awards"@en ;
    skos:inScheme <https://ref.engineersaustralia.org.au/def/ea-awards> ;
    skos:topConceptOf <https://ref.engineersaustralia.org.au/def/ea-awards> .

    award:jennifer-cox-memorial-prize a skos:Concept ;
        rdfs:isDefinedBy <https://ref.engineersaustralia.org.au/def/ea-awards> ;
        dcterms:source "https://aeea.engineersaustralia.org.au/division-awards/"^^xsd:anyURI ;
        skos:definition """The Jennifer Cox Memorial Prize is awarded annually to the student who achieves academic excellence during the second year of an engineering course at the University of Canberra.
        
        It was created in memory of Jennifer Cox, who was studying Communications Engineering at the University of Canberra and would have been the first woman to graduate in Engineering at the University. In her final year she was fatally struck by a motorcycle.
        
        Jennifer was a diligent student and because of her academic record the Faculty of Information Sciences decided unanimously that she should be posthumously awarded the Bachelor of Applied Science Degree in Electronics.
        
        Following the accident, and in recognition of Jennifer's achievements, the Canberra Division of Engineers Australia - on the advice of its Electrical Branch and with the permission of Jennifer's parents - instituted the Jennifer Cox Memorial Prize."""@en ;
        skos:prefLabel "Jennifer Cox Memorial Prize"@en ;
        skos:inScheme <https://ref.engineersaustralia.org.au/def/ea-awards> ;
        skos:broader award:division .

    award:rw-parsons-memorial-prize a skos:Concept ;
        rdfs:isDefinedBy <https://ref.engineersaustralia.org.au/def/ea-awards> ;
        dcterms:source "https://aeea.engineersaustralia.org.au/division-awards/"^^xsd:anyURI ;
        skos:definition """The R W Parsons Memorial Prize is awarded for the best-prepared paper, of approximately 20 minutes duration, on an engineering, or related subject, and delivered to a meeting of the South Australian Division by a graduate (under 30 years of age), or a student member of that division.
        
        If there are more entries than can be heard in one evening, pre-selection is carried out. A significant proportion of the points are awarded for the standard of the presentation.

        The Prize perpetuates the memory of R W Parsons, a former Principal of the South Australian School of Mines (1940-1960) and a former Director of the South Australian Institute of Technology (1960-61). He was also a Councillor of Engineers Australia from 1947-1961 and Chairman of the former Adelaide Division.

        Originally the prize consisted only of cash, but now also includes a medal. It was first awarded in 1962."""@en ;
        skos:prefLabel "R W Parsons Memorial Prize"@en ;
        skos:inScheme <https://ref.engineersaustralia.org.au/def/ea-awards> ;
        skos:broader award:division .

    award:john-mannam-prize a skos:Concept ;
        rdfs:isDefinedBy <https://ref.engineersaustralia.org.au/def/ea-awards> ;
        dcterms:source "https://aeea.engineersaustralia.org.au/division-awards/"^^xsd:anyURI ;
        skos:definition """The John Mannam Prize is an annual award, sponsored by the South Australian Mechanical College Branch, is presented to an outstanding Engineer Practice Report submitted throughout the calendar year from South Australian graduate engineers seeking Chartered Status via professional interviews.
        
        The John Mannam Prize honours the enormous contribution of Dr John Mannam to engineering practice, and in particular his dedication to the education, training and mentoring of mechanical engineers."""@en ;
        skos:altLabel "The John Mannam Prize"@en,
            "The John Mannam Prize (SA)"@en ;
        skos:prefLabel "John Mannam Prize"@en ;
        skos:inScheme <https://ref.engineersaustralia.org.au/def/ea-awards> ;
        skos:broader award:division .

    award:michael-woodhouse-memorial-student-prize a skos:Concept ;
        rdfs:isDefinedBy <https://ref.engineersaustralia.org.au/def/ea-awards> ;
        dcterms:source "https://aeea.engineersaustralia.org.au/division-awards/"^^xsd:anyURI ;
        skos:definition """Sponsored by the Water Panel, Queensland Division, the Michael Woodhouse Memorial Student Prize is awarded to a speaker at the annual Water Panel Students' Night, traditionally held in October. It is based on the quality and content of the speaker's presentation. Final year students from all Queensland tertiary institutions are eligible to take part. The award consists of a certificate and cash prize."""@en ;
        skos:prefLabel "Michael Woodhouse Memorial Student Prize"@en ;
        skos:inScheme <https://ref.engineersaustralia.org.au/def/ea-awards> ;
        skos:broader award:division .

    award:bradfield-award a skos:Concept ;
        rdfs:isDefinedBy <https://ref.engineersaustralia.org.au/def/ea-awards> ;
        dcterms:source "https://aeea.engineersaustralia.org.au/division-awards/"^^xsd:anyURI ;
        skos:definition """The Bradfield Award is chosen from the winners of all categories of the Sydney Division Excellence Awards. The Award recognises an accomplishment of exceptional engineering merit that makes a major contribution to the community."""@en ;
        skos:prefLabel "Bradfield Award"@en ;
        skos:inScheme <https://ref.engineersaustralia.org.au/def/ea-awards> ;
        skos:broader award:division .

    award:eng-student-of-the-year-industrial-training-nsw a skos:Concept ;
        rdfs:isDefinedBy <https://ref.engineersaustralia.org.au/def/ea-awards> ;
        dcterms:source "https://aeea.engineersaustralia.org.au/division-awards/"^^xsd:anyURI ;
        skos:definition """The prestigious Engineering Student of The Year (Industrial Training - NSW)Award recognises the practical experience students gain while studying. It also recognises the employer for providing an outstanding quality-learning environment. There is a winner from each New South Wales university campus (UNSW, USyd, UTS, UWS, Uwoll). Each campus winner becomes eligible for the Sydney Division final, and the winner becomes the NSW Engineering Student of the Year."""@en ;
        skos:prefLabel "Engineering Student of The Year (Industrial Training - NSW)"@en ;
        skos:inScheme <https://ref.engineersaustralia.org.au/def/ea-awards> ;
        skos:broader award:division .

    award:tas-division-award-of-merit a skos:Concept ;
        rdfs:isDefinedBy <https://ref.engineersaustralia.org.au/def/ea-awards> ;
        dcterms:source "https://aeea.engineersaustralia.org.au/division-awards/"^^xsd:anyURI ;
        skos:definition """The Tasmania Division Award Of Merit recognises meritorious contributions to the engineering profession by members of the Tasmania Division.
        
        It is awarded for notable personal contribution to the profession through:
        - Distinguished service to the engineering profession
        - Outstanding contribution to a specific engineering project of a substantial nature
        - Sustained high standard of involvement in and contribution to a specific field of engineering activity."""@en ;
        skos:prefLabel "Tasmania Division Award Of Merit"@en ;
        skos:inScheme <https://ref.engineersaustralia.org.au/def/ea-awards> ;
        skos:broader award:division .

    award:lp-coombes-medal a skos:Concept ;
        rdfs:isDefinedBy <https://ref.engineersaustralia.org.au/def/ea-awards> ;
        dcterms:source "https://aeea.engineersaustralia.org.au/division-awards/"^^xsd:anyURI ;
        skos:definition """The L P Coombes Medal is presented to the speaker who is invited to deliver the L P Coombes Lecture.
        
        The lecture and award are jointly sponsored by the Aviation and Space Branch of the Victoria Division, and the Aeronautical Research Laboratories. The award is made annually and consists of a medal and certificate. The winner is selected by the sponsors.

        The award commemorates Lawrence Percival Coombes, CBE, DFC, BSCEng, FCGI, HonDEng, FIEAust, FRAeS, FAIAA, who was born in Madras, India, in 1899. A World War I aviator and colleague of the late Sir Charles Kingsford Smith, Coombes graduated with 1st Class honours in mechanical engineering from the City and Guilds College, London University, in 1920.
        
        Made a Freeman of the city of London in recognition of his war service, he started a career with the UK Air Ministry. There he achieved acclaim for his use of dynamic models in performance analysis.

        In 1939, he was appointed Chief of the Division of Aeronautics in the then Council for Scientific and Industrial Research (now CSIRO) of Australia, and tasked with establishing the Aeronautical Research Laboratories (ARL).

        He guided ARL through its growth during world War II to be made Chief Superintendent of ARL when it was transferred to the Department of Supply in 1949. He continued as head of ARL on the Australian Aeronautical Research Committee and the Aircraft Advisory Committee until his retirement in 1964."""@en ;
        skos:prefLabel "L P Coombes Medal"@en ;
        skos:inScheme <https://ref.engineersaustralia.org.au/def/ea-awards> ;
        skos:broader award:division .

    award:award-for-achievement-in-eng-enterprise-vic a skos:Concept ;
        rdfs:isDefinedBy <https://ref.engineersaustralia.org.au/def/ea-awards> ;
        dcterms:source "https://aeea.engineersaustralia.org.au/division-awards/"^^xsd:anyURI ;
        skos:definition """An award made by the Victoria Division to a corporate member of Engineers Australia, who has significantly contributed to an enterprise built around the successful commercialisation of an innovative engineering endeavour. A memento is presented in recognition of the award. It was first made in 1986."""@en ;
        skos:prefLabel "Award For Achievement In Engineering Enterprise (Vic)"@en ;
        skos:inScheme <https://ref.engineersaustralia.org.au/def/ea-awards> ;
        skos:broader award:division .

award:recognition a skos:Concept ;
    rdfs:isDefinedBy <https://ref.engineersaustralia.org.au/def/ea-awards> ;
    dcterms:source "https://aeea.engineersaustralia.org.au/recognition-awards/"^^xsd:anyURI ;
    skos:definition """Recognition Awards showcase the achievements of engineers within a specific technical sector and highlight the valuable contributions made to the wider engineering community hosted by EA' s Colleges, Technical Societies, Special Interest Groups and National Committees."""@en ;
    skos:prefLabel "Recognition Awards"@en ;
    skos:inScheme <https://ref.engineersaustralia.org.au/def/ea-awards> ;
    skos:topConceptOf <https://ref.engineersaustralia.org.au/def/ea-awards> .

    award:college a skos:Concept ; 
        rdfs:isDefinedBy <https://ref.engineersaustralia.org.au/def/ea-awards> ;
        dcterms:source "https://aeea.engineersaustralia.org.au/college-awards/"^^xsd:anyURI ; 
        skos:definition """A category of Engineers Australia Recognition Awards, College Awards are engineering awards granted by the Colleges of Engineers Australia in specific engineering disciplines."""@en ;
        skos:prefLabel "College Awards"@en ;
        skos:inScheme <https://ref.engineersaustralia.org.au/def/ea-awards> ;
        skos:broader award:recognition .

        award:david-robinson-award a skos:Concept ;
            rdfs:isDefinedBy <https://ref.engineersaustralia.org.au/def/ea-awards> ;
            dcterms:source "https://www.engineersaustralia.org.au/sites/default/files/awards/ITEE%20College%20Awards%20Flyers-%20David%20Robinson%20flyer.pdf"^^xsd:anyURI ;
            skos:definition """The David Robinson Award is presented in memory of The Institution of Radio and Electronics Engineers (IREE) and is named in honour of the late Dr David Errol Robinson AM, an outstanding Australian electronics engineer, former President of the IREE, and a world renowned expert on ultrasound technology."""@en ;
            skos:related eaclg:itee ;
            skos:prefLabel "David Robinson Award"@en ;
            skos:inScheme <https://ref.engineersaustralia.org.au/def/ea-awards> ;
            skos:broader award:college .
 
        award:john-madsen-medal a skos:Concept ;
            rdfs:isDefinedBy <https://ref.engineersaustralia.org.au/def/ea-awards> ;
            dcterms:source "https://aeea.engineersaustralia.org.au/john-madsen-medal/"^^xsd:anyURI ;
            skos:definition """The John Madsen Medal is awarded for the best paper written by a current member of Engineers Australia, and published in The Australian Journal of Electrical and Electronic Engineering.
            
            The medal perpetuates the memory of Sir John Madsen who was Foundation Professor of Electrical Engineering at the University of Sydney from 1920 to 1949. Sir John Madsen was one of Australia's great electrical engineers and some of his outstanding community service was through his active cooperation with CSIRO. He proposed the founding of a Radio Research Board and was a leader in the development of radar in Australia. He was active in forming the Electrical Research Board and the National Standards Laboratory. He was a Councillor of the Institution from 1930 to 1933 and was awarded the Peter Nicol Russell Memorial Medal in 1944.
            
            In 1976 this medal replaced the Electrical Engineering Prize which was originally founded upon a donation made by the Electrical Association of Australia, one of the Foundation Societies of the Institution. It was first awarded in 1927 and was known as the Electrical Association Premium. The name was changed to the Electrical Engineering Prize in 1954. The award formerly consisted of a certificate and a cash premium."""@en ;
            skos:related eaclg:itee ;
            skos:related eaclg:electrical ;
            skos:prefLabel "John Madsen Medal"@en ;
            skos:inScheme <https://ref.engineersaustralia.org.au/def/ea-awards> ;
            skos:broader award:college .

        award:national-professional-electrical-engineer-of-the-year a skos:Concept ;
            rdfs:isDefinedBy <https://ref.engineersaustralia.org.au/def/ea-awards> ;
            dcterms:source "https://aeea.engineersaustralia.org.au/national-professional-electrical-engineer-of-the-year/"^^xsd:anyURI ;
            skos:definition """The National Professional Electrical Engineer of the Year award is designed to promote excellence and the profession within the community at large, and encourage young people to consider electrical engineering (especially power engineering) as a career.
            
            This award is an annual national award for an outstanding senior electrical engineer member of the College who would be expected to be at (or near) the peak of his or her career, and a good role model for younger members of the profession.
            
            In contrast, the M A Sargent Medal is awarded only when there is a nomination of a candidate who meets the special requirements of that award, normally at the end or near the end of their career, as it is an award recognising overall career achievements.
            
            In summary, the National Professional Electrical Engineer of the Year award is designed to:
            - promote excellence;
            - promote the profession within the community at large; and
            - encourage young people to consider electrical engineering (especially power engineering) as a career.

            The recipient will be a highly respected member of the College and a role model for young members."""@en ;
            skos:related eaclg:electrical ;
            skos:prefLabel "National Professional Electrical Engineer of the Year"@en ;
            skos:inScheme <https://ref.engineersaustralia.org.au/def/ea-awards> ;
            skos:broader award:college .

        award:rw-chapman-medal a skos:Concept ;
            rdfs:isDefinedBy <https://ref.engineersaustralia.org.au/def/ea-awards> ;
            dcterms:source "https://aeea.engineersaustralia.org.au/rw-chapman-medal/"^^xsd:anyURI ;
            skos:definition """The medal was first awarded in 1935 and perpetuates the memory of Sir Robert Chapman, a former Professor of Engineering at the University of Adelaide and a member of the inaugural Council of the Institution. He was Chairman of the former Adelaide Division in 1920 and was President of the Institution in 1922."""@en ;
            skos:related eaclg:structural ;
            skos:prefLabel "RW Chapman Medal"@en ;
            skos:inScheme <https://ref.engineersaustralia.org.au/def/ea-awards> ;
            skos:broader award:college .

        award:sir-george-julius-medal a skos:Concept ;
            rdfs:isDefinedBy <https://ref.engineersaustralia.org.au/def/ea-awards> ;
            dcterms:source "https://aeea.engineersaustralia.org.au/sir-george-julius-medal/"^^xsd:anyURI ;
            skos:definition """In 1976 this medal replaced the Mechanical Engineering Prize, which had been established in 1955. The medal perpetuates the memory of Sir George Julius who practised in Sydney as a consulting engineer in the mechanical/electrical field. One of his best-known achievements was the automatic totalisator before the days of electronics. From 1925-1940 he was Chairman of the Standards Association of Australia, and from 1926 - 1945 he was Chairman of CSIRO."""@en ;
            skos:related eaclg:mechanical ;
            skos:prefLabel "Sir George Julius Medal"@en ;
            skos:inScheme <https://ref.engineersaustralia.org.au/def/ea-awards> ;
            skos:broader award:college .

        award:women-in-biomedical-engineering-scholarship a skos:Concept ;
            rdfs:isDefinedBy <https://ref.engineersaustralia.org.au/def/ea-awards> ;
            dcterms:source "https://aeea.engineersaustralia.org.au/women-in-biomedical-engineering-scholarship/"^^xsd:anyURI ;
            skos:definition """The Women in Biomedical Engineering Scholarship acknowledges and promotes a female Biomedical Engineer who is making an outstanding contribution to her profession and professional community. Nominations are made to the College by the biomedical community.
            
            A panel of members from the Board of the Biomedical College of Engineers Australia will judge the scholarship."""@en ;
            skos:related eaclg:biomedical ;
            skos:prefLabel "Women in Biomedical Engineering Scholarship"@en ;
            skos:inScheme <https://ref.engineersaustralia.org.au/def/ea-awards> ;
            skos:broader award:college .
 
    award:tech-society a skos:Concept ;
        rdfs:isDefinedBy <https://ref.engineersaustralia.org.au/def/ea-awards> ;
        dcterms:source "https://aeea.engineersaustralia.org.au/technical-society-awards/"^^xsd:anyURI ;
         skos:definition """A category of Engineers Australia Recognition Awards, Technical Society Awards are engineering awards granted and administered by the Technical Societies of Engineers Australia.
         
         Engineers Australia has incorporated and unincorporated technical societies.
         - Incorporated technical societies are governed by their own constitutions but choose to be aligned with Engineers Australia.
         - Unincorporated technical societies are governed by a technical society committee that is under the direction of the Engineers Australia Board and is responsible to it."""@en ;
        skos:prefLabel "Technical Society Awards"@en ;
        skos:inScheme <https://ref.engineersaustralia.org.au/def/ea-awards> ;
        skos:broader award:recognition .

        award:aced-national-engineering-education-excellence a skos:Concept ;
            rdfs:isDefinedBy <https://ref.engineersaustralia.org.au/def/ea-awards> ;
            dcterms:source "https://aaee.net.au/aaee-awards/"^^xsd:anyURI ;
            skos:definition """The Australian Council of Engineering Deans National Award for Engineering Education Excellence is awarded for demonstrated excellence in Engineering Education. The award is judged by the Australasian Association for Engineering Education."""@en ;
            skos:prefLabel "Australian Council of Engineering Deans National Award for Engineering Education Excellence"@en ;
            skos:inScheme <https://ref.engineersaustralia.org.au/def/ea-awards> ;
            skos:broader award:tech-society .

        award:aaee-engineering-education-research-design a skos:Concept ;
            rdfs:isDefinedBy <https://ref.engineersaustralia.org.au/def/ea-awards> ;
            dcterms:source "https://aaee.net.au/aaee-awards/"^^xsd:anyURI ;
            skos:definition """The Engineering Education Research Design Award is awarded for rigorous, innovative and transferable research design in the field of Engineering Education. The award is judged by the Australasian Association for Engineering Education."""@en ;
            skos:prefLabel "Engineering Education Research Design Award"@en ;
            skos:inScheme <https://ref.engineersaustralia.org.au/def/ea-awards> ;
            skos:broader award:tech-society .

        award:aaee-engineering-education-engagement a skos:Concept ;
            rdfs:isDefinedBy <https://ref.engineersaustralia.org.au/def/ea-awards> ;
            dcterms:source "https://aaee.net.au/aaee-awards/"^^xsd:anyURI ;
            skos:definition """The Engineering Education Engagement Award is awarded for fostering an excellent standard of successful engagement with stakeholders in Australasian Engineering Education. The award is judged by the Australasian Association for Engineering Education."""@en ;
            skos:prefLabel "Engineering Education Engagement Award"@en ;
            skos:inScheme <https://ref.engineersaustralia.org.au/def/ea-awards> ;
            skos:broader award:tech-society .

    award:special-interest a skos:Concept ;
        rdfs:isDefinedBy <https://ref.engineersaustralia.org.au/def/ea-awards> ;
        dcterms:source "https://aeea.engineersaustralia.org.au/special-interest-awards/"^^xsd:anyURI ;
        skos:definition """A category of Engineers Australia Recognition Awards, Special Interest Awards are engineering awards granted by special interest groups that promote the interests, objectives, and values of Engineers Australia."""@en ;
        skos:prefLabel "Special Interest Group Awards"@en ;
        skos:inScheme <https://ref.engineersaustralia.org.au/def/ea-awards> ;
        skos:broader award:recognition .

        award:gender-diversity-non-profit a skos:Concept ;
            rdfs:isDefinedBy <https://ref.engineersaustralia.org.au/def/ea-awards> ;
            dcterms:source "https://aeea.engineersaustralia.org.au/most-encouraging-student-group-or-non-profit-group-in-gender-diversity/"^^xsd:anyURI ;
            skos:definition """This award promotes national engineering excellence and the contribution women in engineering make to the community. This award seeks to identify, recognise and reward student groups and not-for-profit organisations that strive towards national engineering excellence in encouraging gender diversity."""@en ;
            skos:prefLabel "Most Encouraging Student Group or Non-Profit Group in Gender Diversity"@en ;
            skos:inScheme <https://ref.engineersaustralia.org.au/def/ea-awards> ;
            skos:broader award:special-interest .

    award:national-committee a skos:Concept ; 
        rdfs:isDefinedBy <https://ref.engineersaustralia.org.au/def/ea-awards> ;
        dcterms:source "https://aeea.engineersaustralia.org.au/national-committee-and-panels-awards/"^^xsd:anyURI ;
        skos:definition """A category of Engineers Australia Recognition Awards, National Committee and Panels Awards are engineering awards conferred by the National Committees and Panels of Engineers Australia."""@en ;
        skos:prefLabel "National Committee and Panels Awards"@en ;
        skos:inScheme <https://ref.engineersaustralia.org.au/def/ea-awards> ;
        skos:broader award:recognition .

        award:colin-crisp-award a skos:Concept ; 
            rdfs:isDefinedBy <https://ref.engineersaustralia.org.au/def/ea-awards> ;
            dcterms:source "https://eoas.info/biogs/P006841b.htm"^^xsd:anyURI ;
            skos:definition """The Colin Crisp Award is awarded by Engineering Heritage Australia (EHA), a national committee of Engineers Australia.
            
            The Colin Crisp Award is a project based award given for excellence: in the conservation and recording of items of heritage significance; in recording engineering accomplishment and the development of technology; or in education and raising awareness in engineering heritage.
            
            It is usually presented annually except when, in the opinion of the EHA Board, there is no worthy nomination.
            
            The Colin Crisp Award perpetuates the memory of Colin Crisp, who was a structural engineer well known for his work in the conservation of heritage structures."""@en ;
            skos:prefLabel "Colin Crisp Award"@en ;
            skos:inScheme <https://ref.engineersaustralia.org.au/def/ea-awards> ;
            skos:broader award:national-committee .

        award:dn-foster-award-and-kevin-stark-memorial-award a skos:Concept ; 
            rdfs:isDefinedBy <https://ref.engineersaustralia.org.au/def/ea-awards> ;
            dcterms:source "https://aeea.engineersaustralia.org.au/national-committee-on-coastal-and-ocean-engineering/"^^xsd:anyURI ;
            skos:definition """In recognition of Doug Foster's contribution to Australian coastal engineering, the National Committee on Coastal & Ocean Engineering created the Doug N. Foster Memorial Fellowship Fund in September 2001.
            
            A Professor at University of NSW (UNSW) and an expert in his chosen engineering specialisation of Water, Coastal and Ocean Engineering, Doug was a founding member of the Engineers Australia National Committee on Coastal and Ocean Engineering (NCCOE), which was established in 1971. Doug served on NCCOE until 1985, during which time he was Deputy Chairman from 1979 to 1981 and subsequently Chairman from 1981 to 1983. He was a member of IEAust from 1960 until 1998.
            
            The award is presented to encourage engineering students to pursue career opportunities in coastal and/or ocean engineering. Up to four Awards will be offered to students who are in their final two years of their first engineering degree at the time of the biennal Australasian Coasts & Ports Conference. The award provides the opportunity for students to attend the Australasian Coasts & Ports Conference.
            
            The inaugural presentation of the Award(s) coincided with the Australasian Coasts & Ports Conference in Auckland in September 2003."""@en ;
            skos:prefLabel "D.N. Foster Award and Kevin Stark Memorial Award"@en ;
            skos:inScheme <https://ref.engineersaustralia.org.au/def/ea-awards> ;
            skos:broader award:national-committee .         

        award:jd-lawson-scholarship a skos:Concept ; 
            rdfs:isDefinedBy <https://ref.engineersaustralia.org.au/def/ea-awards> ;
            dcterms:source "https://www.engineersaustralia.org.au/sites/default/files/resource-files/2018-11/JD%20Lawson%20Scholarship%202019.pdf"^^xsd:anyURI ;
            skos:definition """The JD Lawson Scholarship acknowledges and promotes a Professional Engineer who is making an outstanding contribution in hydro-environmental engineering to his/her profession and professional community. It is named after Emeritus Professor Jack Dempster Lawson in recognition of his outstanding contribution to the fields of hydraulic and water resources engineering. After working briefly with the Commonwealth Department of Works and for two years as a Research Hydraulic Engineer with the Snowy Mountains Hydro-electric Authority he joined the University of Melbourne as a Senior Lecturer then Reader in 1954. In 1970 he was appointed Professor of Civil Engineering, a position he held until his retirement in 1989. At the time of his death in 1991 he was the world President of the International Association for HydroEnvironment Engineering and Research (IAHR)."""@en ;
            skos:altLabel "Jack Lawson Scholarship"@en ;
            skos:prefLabel "JD Lawson scholarship"@en ;
            skos:inScheme <https://ref.engineersaustralia.org.au/def/ea-awards> ;
            skos:broader award:national-committee .

        award:ncwe-student-scholarships a skos:Concept ; 
            rdfs:isDefinedBy <https://ref.engineersaustralia.org.au/def/ea-awards> ;
            dcterms:source "https://aeea.engineersaustralia.org.au/national-committee-on-water-engineering-ncwe/"^^xsd:anyURI ;
            skos:definition """The National Committee on Water Engineering (NCWE) Student Scholarships promote engineering excellence and acknowledge the contribution of individuals to the profession of hydrology and water resources engineering and are awarded to students with outstanding performance in the discipline."""@en ;
            skos:prefLabel "NCWE Student Scholarships"@en ;
            skos:inScheme <https://ref.engineersaustralia.org.au/def/ea-awards> ;
            skos:broader award:national-committee .

award:tertiary a skos:Concept ;
    rdfs:isDefinedBy <https://ref.engineersaustralia.org.au/def/ea-awards> ;
    dcterms:source "https://aeea.engineersaustralia.org.au/tertiary-awards/"^^xsd:anyURI ;
    skos:definition """Engineers Australia Teritiary Awards recognise the hard work and achievements of Australia's most dedicated engineering students.

    Every year Engineers Australia seeks to recognise those who will join the engineering profession and contribute to its future through the annual Tertiary Institution Graduate Engineer Awards. Institutions are invited to select graduating students to be awarded an Engineers Australia Institution Graduate Award to recognise the hard work and achievements of Australia's most dedicated engineering students."""@en ;
    skos:prefLabel "Tertiary Awards"@en ;
    skos:inScheme <https://ref.engineersaustralia.org.au/def/ea-awards> ;
    skos:topConceptOf <https://ref.engineersaustralia.org.au/def/ea-awards> .
        
    award:eai-graduate-award a skos:Concept ; 
        rdfs:isDefinedBy <https://ref.engineersaustralia.org.au/def/ea-awards> ;
        dcterms:source "https://aeea.engineersaustralia.org.au/tertiary-awards/"^^xsd:anyURI ;
        skos:definition """An Engineers Australia Institution Graduate Award is awarded to a graduating student engineer from any engineering discipline from each Australian tertiary institution. Each institution is invited to select this award recipient. For institutions with engineering programs at more than one level, an award can be presented at each engineering occupation level (e.g. professional engineering level - BE(Hons) or ME where engineering is a second degree, engineering technologist - BTech, associate engineer - AdvDip or Associate Degree). These awards will be decided by each tertiary institution and presented in conjunction with the local Engineers Australia office."""@en ;
        skos:prefLabel "Engineers Australia Institution Graduate Award"@en ;
        skos:inScheme <https://ref.engineersaustralia.org.au/def/ea-awards> ;
        skos:broader award:tertiary .
