@prefix award: <https://linked.data.gov.au/def/ea-awards/> .
@prefix dcterms: <http://purl.org/dc/terms/> .
@prefix eaclg: <https://linked.data.gov.au/def/ea-colleges/> .
@prefix ieaoc: <https://linked.data.gov.au/def/iea-occupational-categories/> .
@prefix owl: <http://www.w3.org/2002/07/owl#> .
@prefix rdfs: <http://www.w3.org/2000/01/rdf-schema#> .
@prefix sdo: <http://schema.org/> .
@prefix skos: <http://www.w3.org/2004/02/skos/core#> .
@prefix xsd: <http://www.w3.org/2001/XMLSchema#> .

<https://linked.data.gov.au/org/engineersaustralia> a sdo:Organization ;
    sdo:name "Engineers Australia" ;
    sdo:url "https://www.engineersaustralia.org.au"^^xsd:anyURI .

<https://linked.data.gov.au/def/ea-awards> a owl:Ontology,
        skos:ConceptScheme ;
    dcterms:accessRights <https://linked.data.gov.au/def/data-access-rights/open> ;
    dcterms:created "2023-03-01"^^xsd:date ;
    dcterms:creator <https://linked.data.gov.au/org/engineersaustralia> ;
    dcterms:modified "2023-03-01"^^xsd:date ;
    dcterms:publisher <https://linked.data.gov.au/org/engineersaustralia> ;
    dcterms:source "https://linked.data.gov.au/org/engineersaustralia"^^xsd:anyURI ;
    skos:definition """An EA Award is an Engineers Australia managed award for service or achievement to the organisation of Engineers Australia or to the engineering profession."""@en ;
    skos:altLabel "EA Award"@en ;
    skos:prefLabel "Engineers Australia Award"@en .

award:aeea a skos:Concept ;
    rdfs:isDefinedBy <https://linked.data.gov.au/def/ea-awards> ;
    dcterms:source "https://aeea.engineersaustralia.org.au/awards/"^^xsd:anyURI ;
    skos:definition """The Excellence Awards offer a range of national awards, medals and scholarships that highlight contributions to the various areas of engineering, which we support and promote. The Excellence Awards Program seeks to reward outstanding achievement and eminence in the practice of engineering, and standout service to the profession. It plays an important role in promoting engineering excellence and the significant contribution engineering makes to the community. The Australian Engineering Excellence Awards are comprised of awards for projects and for people."""@en ;
    skos:altLabel "Australian Engineering Excellence Awards"@en ;
    skos:notation "AEEA" ;
    skos:prefLabel "Engineers Australia Excellence Awards"@en ;
    skos:inScheme <https://linked.data.gov.au/def/ea-awards> ;
    skos:topConceptOf <https://linked.data.gov.au/def/ea-awards> .


    award:eoy-people a skos:Concept ;
        rdfs:isDefinedBy <https://linked.data.gov.au/def/ea-awards> ;
        dcterms:source "https://aeea.engineersaustralia.org.au/awards/"^^xsd:anyURI ;
        skos:definition """Recognition for outstanding individual engineering achievements and promotes those engineering professionals who show innovation and resourcefulness in their work. Engineers Australia Awards recognise professional achievement, or engineering excellence in its various forms, and promote the profession of engineering. People awards may be conferred at the division level or at the national level.
        Awards Categories:
        - Professional Engineer of the Year
        - Engineering Technologist of the Year
        - Engineering Associate of the Year
        - Young Professional Engineer of the Year
        - Young Engineering Technologist of the Year
        - Young Engineering Associate of the Year"""@en ;
        skos:altLabel "Australian Engineering People Awards"@en,
            "Engineer of the Year Awards"@en ;
        skos:prefLabel "Engineer of the Year"@en ;
        skos:inScheme <https://linked.data.gov.au/def/ea-awards> ;
        skos:broader award:aeea .

        award:professional-engineer-of-the-year a skos:Concept ;
            rdfs:isDefinedBy <https://linked.data.gov.au/def/ea-awards> ;
            dcterms:source "https://aeea.engineersaustralia.org.au/awards/"^^xsd:anyURI ;
            skos:related ieaoc:pro-engineer ;
            skos:definition """The Professional Engineer of the Year award recognises outstanding individual engineering achievements and innovation and resourcefulness of a Professional Engineer."""@en ;
            skos:prefLabel "Professional Engineer of the Year"@en ;
            skos:inScheme <https://linked.data.gov.au/def/ea-awards> ;
            skos:broader award:eoy-people .

        award:engineering-technologist-of-the-year a skos:Concept ;
            rdfs:isDefinedBy <https://linked.data.gov.au/def/ea-awards> ;
            dcterms:source "https://aeea.engineersaustralia.org.au/awards/"^^xsd:anyURI ;
            skos:related ieaoc:tech-engineer ;
            skos:definition """The Engineering Technologist of the Year award recognises outstanding individual engineering achievements and innovation and resourcefulness of an Engineering Technologist."""@en ;
            skos:prefLabel "Engineering Technologist of the Year"@en ;
            skos:inScheme <https://linked.data.gov.au/def/ea-awards> ;
            skos:broader award:eoy-people .
            
        award:engineering-associate-of-the-year a skos:Concept ;
            rdfs:isDefinedBy <https://linked.data.gov.au/def/ea-awards> ;
            dcterms:source "https://aeea.engineersaustralia.org.au/awards/"^^xsd:anyURI ;
            skos:related ieaoc:assoc-engineer ;
            skos:definition """The Engineering Associate of the Year award recognises outstanding individual engineering achievements and innovation and resourcefulness of an Engineering Associate"""@en ;
            skos:prefLabel "Engineering Associate of the Year"@en ;
            skos:inScheme <https://linked.data.gov.au/def/ea-awards> ;
            skos:broader award:eoy-people .

        award:young-professional-engineer-of-the-year a skos:Concept ;
            rdfs:isDefinedBy <https://linked.data.gov.au/def/ea-awards> ;
            dcterms:source "https://aeea.engineersaustralia.org.au/awards/"^^xsd:anyURI ;
            skos:related ieaoc:pro-engineer ;
            skos:definition """The Young Professional Engineer of the Year award recognises outstanding individual engineering achievements and innovation and resourcefulness of a Professional Engineer under the age of 35."""@en ;
            skos:prefLabel "Young Professional Engineer of the Year"@en ;
            skos:inScheme <https://linked.data.gov.au/def/ea-awards> ;
            skos:broader award:eoy-people .

        award:young-engineering-technologist-of-the-year a skos:Concept ;
            rdfs:isDefinedBy <https://linked.data.gov.au/def/ea-awards> ;
            dcterms:source "https://aeea.engineersaustralia.org.au/awards/"^^xsd:anyURI ;
            skos:related ieaoc:tech-engineer ;
            skos:definition """The Young Engineering Technologist of the Year award recognises outstanding individual engineering achievements and innovation and resourcefulness of an Engineering Technologist under the age of 35."""@en ;
            skos:prefLabel "Young Engineering Technologist of the Year"@en ;
            skos:inScheme <https://linked.data.gov.au/def/ea-awards> ;
            skos:broader award:eoy-people .

        award:young-engineering-associate-of-the-year a skos:Concept ;
            rdfs:isDefinedBy <https://linked.data.gov.au/def/ea-awards> ;
            dcterms:source "https://aeea.engineersaustralia.org.au/awards/"^^xsd:anyURI ;
            skos:related ieaoc:assoc-engineer ;
            skos:definition """The Young Engineering Associate of the Year award recognises outstanding individual engineering achievements and innovation and resourcefulness of an Engineering Associate under the age of 35."""@en ;
            skos:prefLabel "Young Engineering Associate of the Year"@en ;
            skos:inScheme <https://linked.data.gov.au/def/ea-awards> ;
            skos:broader award:eoy-people .

    award:project a skos:Concept ;
        rdfs:isDefinedBy <https://linked.data.gov.au/def/ea-awards> ;
        dcterms:source "https://aeea.engineersaustralia.org.au/awards/"^^xsd:anyURI ;
        skos:definition """The Australian Engineering Excellence Project Awards recognise Australia's top engineering projects and the teams behind them. They inspire and encourage engineering distinction through teamwork, innovation, and technical excellence. The national award program first began in 1988 after a decade of celebrating local projects. 
        
        Today, there is a local submission and assessment project awards process. Up to six finalists are selected per location, of which the winner will go on to be a finalist for the Sir William Hudson Award.

        The Sir William Hudson Award is the highest honour that an engineering project can receive from Engineers Australia."""@en ;
        skos:prefLabel "Australian Engineering Excellence Project Awards"@en ;
        skos:inScheme <https://linked.data.gov.au/def/ea-awards> ;
        skos:broader award:aeea .

        award:division-project-award a skos:Concept ;
            rdfs:isDefinedBy <https://linked.data.gov.au/def/ea-awards> ;
            dcterms:source "https://aeea.engineersaustralia.org.au/awards/"^^xsd:anyURI ;
            skos:definition """A Divisonal Project Award recognises outstanding achievement of a project within the geographical region administered by a division. The winners of these awards may be eligible for nomination to the national Sir William Hudson Award for an engineering project."""@en ;
            skos:altLabel "Divisonal Project Award"@en,
                "Project Award - Division"@en ;
            skos:prefLabel "Project of the Year - Division"@en ;
            skos:inScheme <https://linked.data.gov.au/def/ea-awards> ;
            skos:broader award:project .

        award:sir-william-hudson-award a skos:Concept ;
            rdfs:isDefinedBy <https://linked.data.gov.au/def/ea-awards> ;
            dcterms:source "https://aeea.engineersaustralia.org.au/awards/"^^xsd:anyURI ;
            skos:definition """The Sir William Hudson Award is the highest honour that an engineering project can receive from Engineers Australia."""@en ;
            skos:prefLabel "Sir William Hudson Award"@en ;
            skos:inScheme <https://linked.data.gov.au/def/ea-awards> ;
            skos:broader award:project .

    award:president-prize a skos:Concept ;
        rdfs:isDefinedBy <https://linked.data.gov.au/def/ea-awards> ;
        dcterms:source "https://aeea.engineersaustralia.org.au/awards/"^^xsd:anyURI ;
        skos:definition """The President Prize is awarded at the discretion of Engineers Australia's National President each year and recognises conspicuous service to the engineering profession or the community that contributes significantly to Engineers Australia."""@en ;
        skos:altLabel "President's Prize"@en ;
        skos:prefLabel "President Prize"@en ;
        skos:inScheme <https://linked.data.gov.au/def/ea-awards> ;
        skos:broader award:aeea .

    award:peter-nicol-russell-career-achievement-memorial-medal a skos:Concept ;
        rdfs:isDefinedBy <https://linked.data.gov.au/def/ea-awards> ;
        dcterms:source "https://aeea.engineersaustralia.org.au/awards/"^^xsd:anyURI ;
        skos:definition """The Peter Nicol Russell Career Achievement Memorial Medal is the most prestigious award conferred by Engineers Australia upon an individual engineer. It is presented annually to an Honorary Fellow of Engineers Australia who has made a notable contribution to the science and/or practice of engineering in Australia."""@en ;
        skos:altLabel "PNR Medal"@en ;
        skos:prefLabel "Peter Nicol Russel Career Achievement Memorial Medal"@en ;
        skos:inScheme <https://linked.data.gov.au/def/ea-awards> ;
        skos:broader award:aeea .

    award:honorary-fellows a skos:Concept ;
        rdfs:isDefinedBy <https://linked.data.gov.au/def/ea-awards> ;
        dcterms:source "https://aeea.engineersaustralia.org.au/awards/"^^xsd:anyURI ;
        skos:definition """This award elevates the nominee to the highest Engineers Australia membership grade. Eligible recipients are Fellows of The Institution of Engineers Australia or distinguished non-members. They have rendered conspicuous service to the profession of engineering, are eminent in engineering or an allied science, or a distinguished person whom the Board desires to honour, either for having rendered conspicuous service to the Australian people or in recognition of outstanding achievement."""@en ;
        skos:altLabel "Honorary Fellows"@en,
            "Honorary Fellow (HonFIEAust)"@en,
            "Honorary Fellows (HonFIEAust)"@en,
            "Honorary Fellow Awards"@en,
            "Honorary Fellows Award"@en ;
        skos:prefLabel "Honorary Fellow"@en ;
        skos:inScheme <https://linked.data.gov.au/def/ea-awards> ;
        skos:broader award:aeea .

award:division a skos:Concept ;
    rdfs:isDefinedBy <https://linked.data.gov.au/def/ea-awards> ;
    dcterms:source "https://aeea.engineersaustralia.org.au/awards/"^^xsd:anyURI ;
    skos:definition """Engineering awards given to outstanding work specific to the geographical divisions of Engineers Australia.

    Each award is made annually based on a technical paper but governed by conditions which are broad enough to cover special local requirements. Each award consists of a bronze medal with the winner's name engraved on it and a cash prize set by the Board of Engineers Australia."""@en ;
    skos:prefLabel "Division Awards"@en ;
    skos:inScheme <https://linked.data.gov.au/def/ea-awards> ;
    skos:topConceptOf <https://linked.data.gov.au/def/ea-awards> .

    award:jennifer-cox-memorial-prize a skos:Concept ;
        rdfs:isDefinedBy <https://linked.data.gov.au/def/ea-awards> ;
        dcterms:source "https://aeea.engineersaustralia.org.au/division-awards/"^^xsd:anyURI ;
        skos:definition """The Jennifer Cox Memorial Prize is awarded annually to the student who achieves academic excellence during the second year of an engineering course at the University of Canberra.
        
        It was created in memory of Jennifer Cox, who was studying Communications Engineering at the University of Canberra and would have been the first woman to graduate in Engineering at the University. In her final year she was fatally struck by a motorcycle.
        
        Jennifer was a diligent student and because of her academic record the Faculty of Information Sciences decided unanimously that she should be posthumously awarded the Bachelor of Applied Science Degree in Electronics.
        
        Following the accident, and in recognition of Jennifer's achievements, the Canberra Division of Engineers Australia - on the advice of its Electrical Branch and with the permission of Jennifer's parents - instituted the Jennifer Cox Memorial Prize."""@en ;
        skos:prefLabel "Jennifer Cox Memorial Prize"@en ;
        skos:inScheme <https://linked.data.gov.au/def/ea-awards> ;
        skos:broader award:division .

    award:rw-parsons-memorial-prize a skos:Concept ;
        rdfs:isDefinedBy <https://linked.data.gov.au/def/ea-awards> ;
        dcterms:source "https://aeea.engineersaustralia.org.au/division-awards/"^^xsd:anyURI ;
        skos:definition """The R W Parsons Memorial Prize is awarded for the best-prepared paper, of approximately 20 minutes duration, on an engineering, or related subject, and delivered to a meeting of the South Australian Division by a graduate (under 30 years of age), or a student member of that division.
        
        If there are more entries than can be heard in one evening, pre-selection is carried out. A significant proportion of the points are awarded for the standard of the presentation.

        The Prize perpetuates the memory of R W Parsons, a former Principal of the South Australian School of Mines (1940-1960) and a former Director of the South Australian Institute of Technology (1960-61). He was also a Councillor of Engineers Australia from 1947-1961 and Chairman of the former Adelaide Division.

        Originally the prize consisted only of cash, but now also includes a medal. It was first awarded in 1962."""@en ;
        skos:prefLabel "R W Parsons Memorial Prize"@en ;
        skos:inScheme <https://linked.data.gov.au/def/ea-awards> ;
        skos:broader award:division .

    award:john-mannam-prize a skos:Concept ;
        rdfs:isDefinedBy <https://linked.data.gov.au/def/ea-awards> ;
        dcterms:source "https://aeea.engineersaustralia.org.au/division-awards/"^^xsd:anyURI ;
        skos:definition """The John Mannam Prize is an annual award, sponsored by the South Australian Mechanical College Branch, is presented to an outstanding Engineer Practice Report submitted throughout the calendar year from South Australian graduate engineers seeking Chartered Status via professional interviews.
        
        The John Mannam Prize honours the enormous contribution of Dr John Mannam to engineering practice, and in particular his dedication to the education, training and mentoring of mechanical engineers."""@en ;
        skos:altLabel "The John Mannam Prize"@en,
            "The John Mannam Prize (SA)"@en ;
        skos:prefLabel "John Mannam Prize"@en ;
        skos:inScheme <https://linked.data.gov.au/def/ea-awards> ;
        skos:broader award:division .

    award:michael-woodhouse-memorial-student-prize a skos:Concept ;
        rdfs:isDefinedBy <https://linked.data.gov.au/def/ea-awards> ;
        dcterms:source "https://aeea.engineersaustralia.org.au/division-awards/"^^xsd:anyURI ;
        skos:definition """Sponsored by the Water Panel, Queensland Division, the Michael Woodhouse Memorial Student Prize is awarded to a speaker at the annual Water Panel Students' Night, traditionally held in October. It is based on the quality and content of the speaker's presentation. Final year students from all Queensland tertiary institutions are eligible to take part. The award consists of a certificate and cash prize."""@en ;
        skos:prefLabel "Michael Woodhouse Memorial Student Prize"@en ;
        skos:inScheme <https://linked.data.gov.au/def/ea-awards> ;
        skos:broader award:division .

    award:bradfield-award a skos:Concept ;
        rdfs:isDefinedBy <https://linked.data.gov.au/def/ea-awards> ;
        dcterms:source "https://aeea.engineersaustralia.org.au/division-awards/"^^xsd:anyURI ;
        skos:definition """The Bradfield Award is chosen from the winners of all categories of the Sydney Division Excellence Awards. The Award recognises an accomplishment of exceptional engineering merit that makes a major contribution to the community."""@en ;
        skos:prefLabel "Bradfield Award"@en ;
        skos:inScheme <https://linked.data.gov.au/def/ea-awards> ;
        skos:broader award:division .

    award:eng-student-of-the-year-industrial-training-nsw a skos:Concept ;
        rdfs:isDefinedBy <https://linked.data.gov.au/def/ea-awards> ;
        dcterms:source "https://aeea.engineersaustralia.org.au/division-awards/"^^xsd:anyURI ;
        skos:definition """The prestigious Engineering Student of The Year (Industrial Training - NSW)Award recognises the practical experience students gain while studying. It also recognises the employer for providing an outstanding quality-learning environment. There is a winner from each New South Wales university campus (UNSW, USyd, UTS, UWS, Uwoll). Each campus winner becomes eligible for the Sydney Division final, and the winner becomes the NSW Engineering Student of the Year."""@en ;
        skos:prefLabel "Engineering Student of The Year (Industrial Training - NSW)"@en ;
        skos:inScheme <https://linked.data.gov.au/def/ea-awards> ;
        skos:broader award:division .

    award:tas-division-award-of-merit a skos:Concept ;
        rdfs:isDefinedBy <https://linked.data.gov.au/def/ea-awards> ;
        dcterms:source "https://aeea.engineersaustralia.org.au/division-awards/"^^xsd:anyURI ;
        skos:definition """The Tasmania Division Award Of Merit recognises meritorious contributions to the engineering profession by members of the Tasmania Division.
        
        It is awarded for notable personal contribution to the profession through:
        - Distinguished service to the engineering profession
        - Outstanding contribution to a specific engineering project of a substantial nature
        - Sustained high standard of involvement in and contribution to a specific field of engineering activity."""@en ;
        skos:prefLabel "Tasmania Division Award Of Merit"@en ;
        skos:inScheme <https://linked.data.gov.au/def/ea-awards> ;
        skos:broader award:division .

    award:lp-coombes-medal a skos:Concept ;
        rdfs:isDefinedBy <https://linked.data.gov.au/def/ea-awards> ;
        dcterms:source "https://aeea.engineersaustralia.org.au/division-awards/"^^xsd:anyURI ;
        skos:definition """The L P Coombes Medal is presented to the speaker who is invited to deliver the L P Coombes Lecture.
        
        The lecture and award are jointly sponsored by the Aviation and Space Branch of the Victoria Division, and the Aeronautical Research Laboratories. The award is made annually and consists of a medal and certificate. The winner is selected by the sponsors.

        The award commemorates Lawrence Percival Coombes, CBE, DFC, BSCEng, FCGI, HonDEng, FIEAust, FRAeS, FAIAA, who was born in Madras, India, in 1899. A World War I aviator and colleague of the late Sir Charles Kingsford Smith, Coombes graduated with 1st Class honours in mechanical engineering from the City and Guilds College, London University, in 1920.
        
        Made a Freeman of the city of London in recognition of his war service, he started a career with the UK Air Ministry. There he achieved acclaim for his use of dynamic models in performance analysis.

        In 1939, he was appointed Chief of the Division of Aeronautics in the then Council for Scientific and Industrial Research (now CSIRO) of Australia, and tasked with establishing the Aeronautical Research Laboratories (ARL).

        He guided ARL through its growth during world War II to be made Chief Superintendent of ARL when it was transferred to the Department of Supply in 1949. He continued as head of ARL on the Australian Aeronautical Research Committee and the Aircraft Advisory Committee until his retirement in 1964."""@en ;
        skos:prefLabel "L P Coombes Medal"@en ;
        skos:inScheme <https://linked.data.gov.au/def/ea-awards> ;
        skos:broader award:division .

    award:award-for-achievement-in-eng-enterprise-vic a skos:Concept ;
        rdfs:isDefinedBy <https://linked.data.gov.au/def/ea-awards> ;
        dcterms:source "https://aeea.engineersaustralia.org.au/division-awards/"^^xsd:anyURI ;
        skos:definition """An award made by the Victoria Division to a corporate member of Engineers Australia, who has significantly contributed to an enterprise built around the successful commercialisation of an innovative engineering endeavour. A memento is presented in recognition of the award. It was first made in 1986."""@en ;
        skos:prefLabel "Award For Achievement In Engineering Enterprise (Vic)"@en ;
        skos:inScheme <https://linked.data.gov.au/def/ea-awards> ;
        skos:broader award:division .

award:recognition a skos:Concept ;
    rdfs:isDefinedBy <https://linked.data.gov.au/def/ea-awards> ;
    dcterms:source "https://aeea.engineersaustralia.org.au/recognition-awards/"^^xsd:anyURI ;
    skos:definition """Recognition Awards showcase the achievements of engineers within a specific technical sector and highlight the valuable contributions made to the wider engineering community hosted by EA' s Colleges, Technical Societies, Special Interest Groups and National Committees."""@en ;
    skos:prefLabel "Recognition Awards"@en ;
    skos:inScheme <https://linked.data.gov.au/def/ea-awards> ;
    skos:topConceptOf <https://linked.data.gov.au/def/ea-awards> .

    award:college a skos:Concept ; 
        rdfs:isDefinedBy <https://linked.data.gov.au/def/ea-awards> ;
        dcterms:source "https://aeea.engineersaustralia.org.au/college-awards/"^^xsd:anyURI ; 
        skos:definition """A category of Engineers Australia Recognition Awards, College Awards are engineering awards granted by the Colleges of Engineers Australia in specific engineering disciplines."""@en ;
        skos:prefLabel "College Awards"@en ;
        skos:inScheme <https://linked.data.gov.au/def/ea-awards> ;
        skos:broader award:recognition .

        award:agm-michell-medal a skos:Concept ;
            rdfs:isDefinedBy <https://linked.data.gov.au/def/ea-awards> ;
            dcterms:source "https://scholarships.unimelb.edu.au/awards/a-g-m-michell-prize-in-mechanical-engineering/"^^xsd:anyURI ;
            skos:definition """This scholarship is an undergraduate award for best essay, thesis, report or design on a subject relating to mechanical engineering. Awarded by the Engineers Australia Mechanical College."""@en ;
            skos:related eaclg:mechanical ;
            skos:altLabel "A G M Michell Prize"@en ;
            skos:prefLabel "AGM Michell Medal"@en ;
            skos:inScheme <https://linked.data.gov.au/def/ea-awards> ;
            skos:broader award:college .

        award:chemeca-medal a skos:Concept ;
            rdfs:isDefinedBy <https://linked.data.gov.au/def/ea-awards> ;
            dcterms:source "https://www.anzfche.org/awards-of-excellence.php"^^xsd:anyURI ;
            skos:definition """This is the most prestigious award in the chemical engineering profession in New Zealand and Australia. It is awarded to a prominent New Zealand or Australian Chemical Engineer who has made an outstanding contribution, through achievement or service, to the practice of Chemical Engineering in its widest sense and who continues to serve the profession. The recipient of the Award is invited to present a plenary lecture at the annual Chemeca conference."""@en ;
            skos:related eaclg:chemical ;
            skos:prefLabel "Chemeca Medal"@en ;
            skos:inScheme <https://linked.data.gov.au/def/ea-awards> ;
            skos:broader award:college .

        award:david-dewhurst-award a skos:Concept ;
            rdfs:isDefinedBy <https://linked.data.gov.au/def/ea-awards> ;
            dcterms:source "https://en.wikipedia.org/wiki/David_Dewhurst_Medal"^^xsd:anyURI ;
            skos:definition """The David Dewhurst award is a bronze medal bestowed by Engineers Australia and is the most distinguished accolade within their biomedical engineering discipline. It is named in honour of David John Dewhurst (1919 - 1996), an outstanding Australian biophysicist and biomedical engineer who performed pioneering work in the area of the cochlear implant. The award was inaugurated in 1994 as the Eminent Biomedical Engineers Award and its first winner was David Dewhurst. Following his death in 1996 the award's name was changed to the David Dewhurst Award as a permanent memorial."""@en ;
            skos:related eaclg:biomedical ;
            skos:altLabel "David Dewhurst Medal"@en ;
            skos:prefLabel "David Dewhurst Award"@en ;
            skos:inScheme <https://linked.data.gov.au/def/ea-awards> ;
            skos:broader award:college .

        award:david-robinson-award a skos:Concept ;
            rdfs:isDefinedBy <https://linked.data.gov.au/def/ea-awards> ;
            dcterms:source "https://www.engineersaustralia.org.au/sites/default/files/awards/ITEE%20College%20Awards%20Flyers-%20David%20Robinson%20flyer.pdf"^^xsd:anyURI ;
            skos:definition """The David Robinson Award is presented in memory of The Institution of Radio and Electronics Engineers (IREE) and is named in honour of the late Dr David Errol Robinson AM, an outstanding Australian electronics engineer, former President of the IREE, and a world renowned expert on ultrasound technology."""@en ;
            skos:related eaclg:itee ;
            skos:prefLabel "David Robinson Award"@en ;
            skos:inScheme <https://linked.data.gov.au/def/ea-awards> ;
            skos:broader award:college .
 
        award:iree-neville-thiele-eminence-award a skos:Concept ;
            rdfs:isDefinedBy <https://linked.data.gov.au/def/ea-awards> ;
            dcterms:source "https://www.engineersaustralia.org.au/sites/default/files/content-files/2016-12/nt_regulations_19-aug-13.pdf"^^xsd:anyURI ;
            skos:definition """The Neville Thiele Eminence Award is to recognise eminence in information, telecommunications and electronics engineering.

            The Award honours a member of the engineering team who has made significant contributions to the art and practice of engineering in the disciplines covered by the College of Information, Telecommunications and Electronics Engineering of Engineers Australia (ITEE College). The Award also recognises the individual's significant contributions to the community. These contributions and achievements will have been made typically during the preceding five to ten years rather than during a full career. In this way, the Award is open to younger members of the engineering team."""@en ;
            skos:related eaclg:itee ;
            skos:altLabel "The IREE Neville Thiele Eminence Award"@en ;
            skos:prefLabel "The Neville Thiele Eminence Award"@en ;
            skos:inScheme <https://linked.data.gov.au/def/ea-awards> ;
            skos:broader award:college .
 
        award:john-madsen-medal a skos:Concept ;
            rdfs:isDefinedBy <https://linked.data.gov.au/def/ea-awards> ;
            dcterms:source "https://aeea.engineersaustralia.org.au/john-madsen-medal/"^^xsd:anyURI ;
            skos:definition """The John Madsen Medal is awarded for the best paper written by a current member of Engineers Australia, and published in The Australian Journal of Electrical and Electronic Engineering.
            
            The medal perpetuates the memory of Sir John Madsen who was Foundation Professor of Electrical Engineering at the University of Sydney from 1920 to 1949. Sir John Madsen was one of Australia's great electrical engineers and some of his outstanding community service was through his active cooperation with CSIRO. He proposed the founding of a Radio Research Board and was a leader in the development of radar in Australia. He was active in forming the Electrical Research Board and the National Standards Laboratory. He was a Councillor of the Institution from 1930 to 1933 and was awarded the Peter Nicol Russell Memorial Medal in 1944.
            
            In 1976 this medal replaced the Electrical Engineering Prize which was originally founded upon a donation made by the Electrical Association of Australia, one of the Foundation Societies of the Institution. It was first awarded in 1927 and was known as the Electrical Association Premium. The name was changed to the Electrical Engineering Prize in 1954. The award formerly consisted of a certificate and a cash premium."""@en ;
            skos:related eaclg:itee ;
            skos:related eaclg:electrical ;
            skos:prefLabel "John Madsen Medal"@en ;
            skos:inScheme <https://linked.data.gov.au/def/ea-awards> ;
            skos:broader award:college .
 
        award:m-a-sargent-medal a skos:Concept ;
            rdfs:isDefinedBy <https://linked.data.gov.au/def/ea-awards> ;
            dcterms:source "https://aeea.engineersaustralia.org.au/m-a-sargent-medal/"^^xsd:anyURI ;
            skos:definition """This is a prestigious award made jointly by the College of Electrical Engineers and the College of ITEE Engineers. It is named in honour of Dr Michael Anthony (Mike) Sargent, an outstanding Australian electrical engineer. Dr Sargent graduated from the University of Queensland in 1964 and gained a PhD in electrical engineering at the same university in 1967. After holding various engineering appointments in Queensland and North America he joined the South East Queensland Electricity Board in 1978 becoming its Chief Engineer in 1984 and became Manager, Business Systems in 1989.

            Dr Sargent is an Honorary Fellow of Engineers Australia and has served in many positions in Engineers Australia including Chairman of the Electrical and Computing Branch of Queensland Division 1976, Chairman of Queensland Division 1984, member of the then Council 1984 - 1986, Vice President of Engineers Australia 1985 - 1986 and also 1988, Deputy Chairman of the Electrical College Board 1988, Deputy President of Engineers Australia 1989 and President in 1990.."""@en ;
            skos:related eaclg:itee ;
            skos:related eaclg:electrical ;
            skos:prefLabel "M A Sargent Medal"@en ;
            skos:inScheme <https://linked.data.gov.au/def/ea-awards> ;
            skos:broader award:college .

        award:national-professional-electrical-engineer-of-the-year a skos:Concept ;
            rdfs:isDefinedBy <https://linked.data.gov.au/def/ea-awards> ;
            dcterms:source "https://aeea.engineersaustralia.org.au/national-professional-electrical-engineer-of-the-year/"^^xsd:anyURI ;
            skos:definition """The National Professional Electrical Engineer of the Year award is designed to promote excellence and the profession within the community at large, and encourage young people to consider electrical engineering (especially power engineering) as a career.
            
            This award is an annual national award for an outstanding senior electrical engineer member of the College who would be expected to be at (or near) the peak of his or her career, and a good role model for younger members of the profession.
            
            In contrast, the M A Sargent Medal is awarded only when there is a nomination of a candidate who meets the special requirements of that award, normally at the end or near the end of their career, as it is an award recognising overall career achievements.
            
            In summary, the National Professional Electrical Engineer of the Year award is designed to:
            - promote excellence;
            - promote the profession within the community at large; and
            - encourage young people to consider electrical engineering (especially power engineering) as a career.

            The recipient will be a highly respected member of the College and a role model for young members."""@en ;
            skos:related eaclg:electrical ;
            skos:prefLabel "National Professional Electrical Engineer of the Year"@en ;
            skos:inScheme <https://linked.data.gov.au/def/ea-awards> ;
            skos:broader award:college .

        award:professional-environmental-engineer-of-the-year a skos:Concept ;
            rdfs:isDefinedBy <https://linked.data.gov.au/def/ea-awards> ;
            dcterms:source "https://www.engineersaustralia.org.au/news-and-media/2022/07/meet-winners-australias-top-engineering-awards-2021"^^xsd:anyURI ;
            skos:definition """The Professional Environmental Engineer of the Year Award seeks to reward outstanding achievement and eminence in the practice of environmental engineering, and standout service to the profession."""@en ;
            skos:related eaclg:environmental ;
            skos:altLabel "National Professional Environmental Engineer of the Year"@en ;
            skos:prefLabel "Professional Environmental Engineer of the Year"@en ;
            skos:inScheme <https://linked.data.gov.au/def/ea-awards> ;
            skos:broader award:college .

        award:rw-chapman-medal a skos:Concept ;
            rdfs:isDefinedBy <https://linked.data.gov.au/def/ea-awards> ;
            dcterms:source "https://aeea.engineersaustralia.org.au/rw-chapman-medal/"^^xsd:anyURI ;
            skos:definition """The medal was first awarded in 1935 and perpetuates the memory of Sir Robert Chapman, a former Professor of Engineering at the University of Adelaide and a member of the inaugural Council of the Institution. He was Chairman of the former Adelaide Division in 1920 and was President of the Institution in 1922."""@en ;
            skos:related eaclg:structural ;
            skos:prefLabel "RW Chapman Medal"@en ;
            skos:inScheme <https://linked.data.gov.au/def/ea-awards> ;
            skos:broader award:college .

        award:john-connell-gold-medal a skos:Concept ;
            rdfs:isDefinedBy <https://linked.data.gov.au/def/ea-awards> ;
            dcterms:source "https://www.engineersaustralia.org.au/news-and-media/2022/07/victorian-engineer-receives-prestigious-john-connell-gold-medal"^^xsd:anyURI ;
            skos:definition """The John Connell gold medal is given in recognition of significant contribution to the structural engineering profession.

            One of the most influential engineers of his generation, John Connell made an outstanding contribution to the practice of structural engineering in Australia and to exporting Australian engineering skills to Asia in the 1970s and 1980s."""@en ;
            skos:related eaclg:structural ;
            skos:prefLabel "John Connell Gold Medal"@en ;
            skos:inScheme <https://linked.data.gov.au/def/ea-awards> ;
            skos:broader award:college .

        award:sir-george-julius-medal a skos:Concept ;
            rdfs:isDefinedBy <https://linked.data.gov.au/def/ea-awards> ;
            dcterms:source "https://aeea.engineersaustralia.org.au/sir-george-julius-medal/"^^xsd:anyURI ;
            skos:definition """In 1976 this medal replaced the Mechanical Engineering Prize, which had been established in 1955. The medal perpetuates the memory of Sir George Julius who practised in Sydney as a consulting engineer in the mechanical/electrical field. One of his best-known achievements was the automatic totalisator before the days of electronics. From 1925-1940 he was Chairman of the Standards Association of Australia, and from 1926 - 1945 he was Chairman of CSIRO."""@en ;
            skos:related eaclg:mechanical ;
            skos:prefLabel "Sir George Julius Medal"@en ;
            skos:inScheme <https://linked.data.gov.au/def/ea-awards> ;
            skos:broader award:college .

        award:sir-john-holland-civil-engineer-of-the-year-award a skos:Concept ;
            rdfs:isDefinedBy <https://linked.data.gov.au/def/ea-awards> ;
            dcterms:source "https://www.engineersaustralia.org.au/news-and-media/2022/09/sir-john-holland-civil-engineer-year-2022-awarded"^^xsd:anyURI ;
            skos:definition """The Sir John Holland Civil Engineer of the Year, sponsored by John Holland, is the pre-eminent civil engineering award presented annually by Engineers Australia's Civil College.
            
            The award provides a high-profile focus on engineering achievement and serves as both a showcase for civil engineering and a focus for young people interested in pursuing a career in engineering.
            
            This award is presented annually by Engineers Australia to an eminent civil engineer who has made a major contribution to the sector, including the development of new technology, contribution to the use of ecologically sustainable development and service to the engineering profession."""@en ;
            skos:related eaclg:civil ;
            skos:prefLabel "Sir John Holland Civil Engineer of the Year"@en ;
            skos:inScheme <https://linked.data.gov.au/def/ea-awards> ;
            skos:broader award:college .

        award:w-h-warren-medal a skos:Concept ;
            rdfs:isDefinedBy <https://linked.data.gov.au/def/ea-awards> ;
            dcterms:source "https://www.eoas.info/biogs/P006450b.htm"^^xsd:anyURI ;
            skos:definition """The W. H. Warren Medal was established in 1926 by the Institution of Engineers, Australia to perpetuate the memory of the first President of the Institution, the late Professor William Henry Warren, Professor of Engineering at the University of Sydney from 1884 to 1925.
            
            It is usually awarded annually for the best paper presented to the Institution on a civil engineering subject. The award was first presented in 1932."""@en ;
            skos:related eaclg:civil ;
            skos:prefLabel "W H Warren Medal"@en ;
            skos:inScheme <https://linked.data.gov.au/def/ea-awards> ;
            skos:broader award:college .

        award:women-in-biomedical-engineering-scholarship a skos:Concept ;
            rdfs:isDefinedBy <https://linked.data.gov.au/def/ea-awards> ;
            dcterms:source "https://aeea.engineersaustralia.org.au/women-in-biomedical-engineering-scholarship/"^^xsd:anyURI ;
            skos:definition """The Women in Biomedical Engineering Scholarship acknowledges and promotes a female Biomedical Engineer who is making an outstanding contribution to her profession and professional community. Nominations are made to the College by the biomedical community.
            
            A panel of members from the Board of the Biomedical College of Engineers Australia will judge the scholarship."""@en ;
            skos:related eaclg:biomedical ;
            skos:prefLabel "Women in Biomedical Engineering Scholarship"@en ;
            skos:inScheme <https://linked.data.gov.au/def/ea-awards> ;
            skos:broader award:college .

        award:young-biomedical-engineering-scholarship a skos:Concept ;
            rdfs:isDefinedBy <https://linked.data.gov.au/def/ea-awards> ;
            dcterms:source "https://www.engineersaustralia.org.au/engineering-communities/colleges-and-college-national-committees/biomedical-college"^^xsd:anyURI ;
            skos:definition """Young Biomedical Engineering Scholarship acknowledges and promotes a Biomedical Engineer under the age of 35 who is making an outstanding contribution to the profession and professional community. Nominations are made to the College by the biomedical community.
            
            A panel of members from the Board of the Biomedical College of Engineers Australia will judge the scholarship."""@en ;
            skos:related eaclg:biomedical ;
            skos:prefLabel "Young Biomedical Engineering Scholarship"@en ;
            skos:inScheme <https://linked.data.gov.au/def/ea-awards> ;
            skos:broader award:college .

        award:young-electrical-power-engineer-of-the-year-award a skos:Concept ;
            rdfs:isDefinedBy <https://linked.data.gov.au/def/ea-awards> ;
            dcterms:source "https://aeea.engineersaustralia.org.au/young-electrical-power-engineer-of-the-year-award/"^^xsd:anyURI ;
            skos:definition """This national award recognises a professional engineer who has demonstrated significant achievements in electrical power engineering during the preceding six years. Contributions to the community are also valued.
            
            This annual award is an example of an effective partnership between Engineers Australia and industry. Engineers Australia's Electrical College Board and the Electric Energy Society of Australia (EESA) jointly developed the initiative, to encourage young Australians to develop a career in electrical power engineering, and also to reward outstanding achievements."""@en ;
            skos:related eaclg:electrical ;
            skos:prefLabel "Young Electrical Power Engineer of the Year Award"@en ;
            skos:inScheme <https://linked.data.gov.au/def/ea-awards> ;
            skos:broader award:college .

        award:young-environmental-engineer-of-the-year-award a skos:Concept ;
            rdfs:isDefinedBy <https://linked.data.gov.au/def/ea-awards> ;
            dcterms:source "https://www.seng.org.au/awards-competitions/environmental-college-young-professional-engineer-the-year"^^xsd:anyURI ;
            skos:definition """The Young Environmental Engineer of the Year award is presented by the Environmental College of Engineers Australia to acknowledge and reward young environmental engineers who have:
            - Engineering competence
            - Demonstrated leadership skills including leadership of teams
            - Positive/notable outcomes from their engineering work
            - Creativity/innovation
            - Community service to industry, the profession and/or society"""@en ;
            skos:related eaclg:environmental ;
            skos:prefLabel "Young Environmental Engineer of the Year Award"@en ;
            skos:inScheme <https://linked.data.gov.au/def/ea-awards> ;
            skos:broader award:college .

        award:young-mechanical-engineer-of-the-year-award a skos:Concept ;
            rdfs:isDefinedBy <https://linked.data.gov.au/def/ea-awards> ;
            dcterms:source "https://www.seng.org.au/awards-competitions/environmental-college-young-professional-engineer-the-year"^^xsd:anyURI ;
            skos:definition """This national award recognises a professional engineer who has demonstrated significant achievements in mechanical engineering. Contributions to the community are also valued."""@en ;
            skos:related eaclg:mechanical ;
            skos:prefLabel "Young Mechanical Engineer of the Year Award"@en ;
            skos:inScheme <https://linked.data.gov.au/def/ea-awards> ;
            skos:broader award:college .

    award:tech-society a skos:Concept ;
        rdfs:isDefinedBy <https://linked.data.gov.au/def/ea-awards> ;
        dcterms:source "https://aeea.engineersaustralia.org.au/technical-society-awards/"^^xsd:anyURI ;
         skos:definition """A category of Engineers Australia Recognition Awards, Technical Society Awards are engineering awards granted by the Technical Societies of Engineers Australia.
         
         Engineers Australia has incorporated and unincorporated technical societies.
         - Incorporated technical societies are governed by their own constitutions but choose to be aligned with Engineers Australia.
         - Unincorporated technical societies are governed by a technical society committee that is under the direction of the Engineers Australia Board and is responsible to it."""@en ;
        skos:prefLabel "Technical Society Awards"@en ;
        skos:inScheme <https://linked.data.gov.au/def/ea-awards> ;
        skos:broader award:recognition .

        award:aced-national-engineering-education-excellence a skos:Concept ;
            rdfs:isDefinedBy <https://linked.data.gov.au/def/ea-awards> ;
            dcterms:source "https://aaee.net.au/aaee-awards/"^^xsd:anyURI ;
            skos:definition """The Australian Council of Engineering Deans National Award for Engineering Education Excellence is awarded for demonstrated excellence in Engineering Education. The award is judged by the Australasian Association for Engineering Education."""@en ;
            skos:prefLabel "Australian Council of Engineering Deans National Award for Engineering Education Excellence"@en ;
            skos:inScheme <https://linked.data.gov.au/def/ea-awards> ;
            skos:broader award:tech-society .

        award:aaee-engineering-education-research-design a skos:Concept ;
            rdfs:isDefinedBy <https://linked.data.gov.au/def/ea-awards> ;
            dcterms:source "https://aaee.net.au/aaee-awards/"^^xsd:anyURI ;
            skos:definition """The Engineering Education Research Design Award is awarded for rigorous, innovative and transferable research design in the field of Engineering Education. The award is judged by the Australasian Association for Engineering Education."""@en ;
            skos:prefLabel "Engineering Education Research Design Award"@en ;
            skos:inScheme <https://linked.data.gov.au/def/ea-awards> ;
            skos:broader award:tech-society .

        award:aaee-engineering-education-engagement a skos:Concept ;
            rdfs:isDefinedBy <https://linked.data.gov.au/def/ea-awards> ;
            dcterms:source "https://aaee.net.au/aaee-awards/"^^xsd:anyURI ;
            skos:definition """The Engineering Education Engagement Award is awarded for fostering an excellent standard of successful engagement with stakeholders in Australasian Engineering Education. The award is judged by the Australasian Association for Engineering Education."""@en ;
            skos:prefLabel "Engineering Education Engagement Award"@en ;
            skos:inScheme <https://linked.data.gov.au/def/ea-awards> ;
            skos:broader award:tech-society .

        award:transport-medal a skos:Concept ;
            rdfs:isDefinedBy <https://linked.data.gov.au/def/ea-awards> ;
            dcterms:source "https://www.rtsa.com.au/event/transport-australia-society-event-webinar-the-future-of-public-transport-ridership/"^^xsd:anyURI ;
            skos:definition """The Engineers Australia Transport Medal rewards and recognises outstanding individual contributions to transport in Australia and is open to individuals from public and private sectors. The Transport Medal is open to individuals from public and private sectors including transport operators, consultants, government departments and authorities as well as academics and researchers."""@en ;
            skos:prefLabel "Transport Medal"@en ;
            skos:inScheme <https://linked.data.gov.au/def/ea-awards> ;
            skos:broader award:tech-society .

    award:special-interest a skos:Collection ;
        rdfs:isDefinedBy <https://linked.data.gov.au/def/ea-awards> ;
        dcterms:source "https://aeea.engineersaustralia.org.au/special-interest-awards/"^^xsd:anyURI ;
        skos:definition """A category of Engineers Australia Recognition Awards, Special Interest Awards are engineering awards granted by special interest groups that promote the interests, objectives, and values of Engineers Australia."""@en ;
        skos:prefLabel "Special Interest Group Awards"@en ;
        skos:inScheme <https://linked.data.gov.au/def/ea-awards> ;
        skos:broader award:recognition .

        award:gender-diversity-non-profit a skos:Concept ;
            rdfs:isDefinedBy <https://linked.data.gov.au/def/ea-awards> ;
            dcterms:source "https://aeea.engineersaustralia.org.au/most-encouraging-student-group-or-non-profit-group-in-gender-diversity/"^^xsd:anyURI ;
            skos:definition """This award promotes national engineering excellence and the contribution women in engineering make to the community. This award seeks to identify, recognise and reward student groups and not-for-profit organisations that strive towards national engineering excellence in encouraging gender diversity."""@en ;
            skos:prefLabel "Most Encouraging Student Group or Non-Profit Group in Gender Diversity"@en ;
            skos:inScheme <https://linked.data.gov.au/def/ea-awards> ;
            skos:broader award:tech-society .

        award:gender-diversity-company a skos:Concept ;
            rdfs:isDefinedBy <https://linked.data.gov.au/def/ea-awards> ;
            dcterms:source "https://aeea.engineersaustralia.org.au/most-encouraging-student-group-or-non-profit-group-in-gender-diversity/"^^xsd:anyURI ;
            skos:definition """This award promotes national engineering excellence and the contribution women in engineering make to the community. This award seeks to identify, recognise and reward companies that strive towards national engineering excellence in encouraging gender diversity."""@en ;
            skos:prefLabel "Most Outstanding Company in Gender Diversity"@en ;
            skos:inScheme <https://linked.data.gov.au/def/ea-awards> ;
            skos:broader award:tech-society .

    award:national-committee a skos:Concept ; 
        rdfs:isDefinedBy <https://linked.data.gov.au/def/ea-awards> ;
        dcterms:source "https://aeea.engineersaustralia.org.au/national-committee-and-panels-awards/"^^xsd:anyURI ;
        skos:definition """A category of Engineers Australia Recognition Awards, National Committee and Panels Awards are engineering awards conferred by the National Committees and Panels of Engineers Australia."""@en ;
        skos:prefLabel "National Committee and Panels Awards"@en ;
        skos:inScheme <https://linked.data.gov.au/def/ea-awards> ;
        skos:broader award:recognition .

        award:colin-crisp-award a skos:Concept ; 
            rdfs:isDefinedBy <https://linked.data.gov.au/def/ea-awards> ;
            dcterms:source "https://eoas.info/biogs/P006841b.htm"^^xsd:anyURI ;
            skos:definition """The Colin Crisp Award is awarded by Engineering Heritage Australia (EHA), a national committee of Engineers Australia.
            
            The Colin Crisp Award is a project based award given for excellence: in the conservation and recording of items of heritage significance; in recording engineering accomplishment and the development of technology; or in education and raising awareness in engineering heritage.
            
            It is usually presented annually except when, in the opinion of the EHA Board, there is no worthy nomination.
            
            The Colin Crisp Award perpetuates the memory of Colin Crisp, who was a structural engineer well known for his work in the conservation of heritage structures."""@en ;
            skos:prefLabel "Colin Crisp Award"@en ;
            skos:inScheme <https://linked.data.gov.au/def/ea-awards> ;
            skos:broader award:national-committee .

        award:dn-foster-award-and-kevin-stark-memorial-award a skos:Concept ; 
            rdfs:isDefinedBy <https://linked.data.gov.au/def/ea-awards> ;
            dcterms:source "https://aeea.engineersaustralia.org.au/national-committee-on-coastal-and-ocean-engineering/"^^xsd:anyURI ;
            skos:definition """In recognition of Doug Foster's contribution to Australian coastal engineering, the National Committee on Coastal & Ocean Engineering created the Doug N. Foster Memorial Fellowship Fund in September 2001.
            
            A Professor at University of NSW (UNSW) and an expert in his chosen engineering specialisation of Water, Coastal and Ocean Engineering, Doug was a founding member of the Engineers Australia National Committee on Coastal and Ocean Engineering (NCCOE), which was established in 1971. Doug served on NCCOE until 1985, during which time he was Deputy Chairman from 1979 to 1981 and subsequently Chairman from 1981 to 1983. He was a member of IEAust from 1960 until 1998.
            
            The award is presented to encourage engineering students to pursue career opportunities in coastal and/or ocean engineering. Up to four Awards will be offered to students who are in their final two years of their first engineering degree at the time of the biennal Australasian Coasts & Ports Conference. The award provides the opportunity for students to attend the Australasian Coasts & Ports Conference.
            
            The inaugural presentation of the Award(s) coincided with the Australasian Coasts & Ports Conference in Auckland in September 2003."""@en ;
            skos:prefLabel "D.N. Foster Award and Kevin Stark Memorial Award"@en ;
            skos:inScheme <https://linked.data.gov.au/def/ea-awards> ;
            skos:broader award:national-committee .         

        award:john-burton-cumec-trophy a skos:Concept ; 
            rdfs:isDefinedBy <https://linked.data.gov.au/def/ea-awards> ;
            dcterms:source "https://aeea.engineersaustralia.org.au/national-committee-on-water-engineering-ncwe/"^^xsd:anyURI ;
            skos:definition """The National Committee on Water Engineering (NCWE) presents the John Burton Cumec Trophy to the winner of the Hydrological Games at each Hydrology and Water Resources Symposium."""@en ;
            skos:prefLabel "John Burton Cumec Trophy"@en ;
            skos:inScheme <https://linked.data.gov.au/def/ea-awards> ;
            skos:broader award:national-committee .   

        award:gn-alexander-medal a skos:Concept ; 
            rdfs:isDefinedBy <https://linked.data.gov.au/def/ea-awards> ;
            dcterms:source "https://www.engineersaustralia.org.au/sites/default/files/content-files/2016-12/GN_Alexander_Bio-ed.pdf"^^xsd:anyURI ;
            skos:definition """The GN Alexander Medal for Hydrology and Water Resources was created in 1987 by the National Committee on Hydrology & Water Resources (subsequently the National Committee on Water Engineering) of the Institution of Engineers, Australia in recognition of Geoff Alexander's contribution to Australian hydrology.
            
            The award is presented to the authors of the best paper in hydrology and/or water resources published in an Institution publication at each Hydrology and Water Resources Symposium."""@en ;
            skos:prefLabel "GN Alexander Medal"@en ;
            skos:inScheme <https://linked.data.gov.au/def/ea-awards> ;
            skos:broader award:national-committee .

        award:henderson-oration a skos:Concept ; 
            rdfs:isDefinedBy <https://linked.data.gov.au/def/ea-awards> ;
            dcterms:source "https://www.globalwaterinstitute.unsw.edu.au/all-events/13th-hydraulics-in-water-engineering-conference"^^xsd:anyURI ;
            skos:definition """The Henderson Oration is an invitational keynote speech offered by The National Committee on Water Engineering (NCWE) that recognises the contribution of the science of hydraulics to the practice of hydrology and water resources engineering."""@en ;
            skos:prefLabel "Henderson Oration"@en ;
            skos:inScheme <https://linked.data.gov.au/def/ea-awards> ;
            skos:broader award:national-committee .

        award:jd-lawson-scholarship a skos:Concept ; 
            rdfs:isDefinedBy <https://linked.data.gov.au/def/ea-awards> ;
            dcterms:source "https://www.engineersaustralia.org.au/sites/default/files/resource-files/2018-11/JD%20Lawson%20Scholarship%202019.pdf"^^xsd:anyURI ;
            skos:definition """The JD Lawson Scholarship acknowledges and promotes a Professional Engineer who is making an outstanding contribution in hydro-environmental engineering to his/her profession and professional community. It is named after Emeritus Professor Jack Dempster Lawson in recognition of his outstanding contribution to the fields of hydraulic and water resources engineering. After working briefly with the Commonwealth Department of Works and for two years as a Research Hydraulic Engineer with the Snowy Mountains Hydro-electric Authority he joined the University of Melbourne as a Senior Lecturer then Reader in 1954. In 1970 he was appointed Professor of Civil Engineering, a position he held until his retirement in 1989. At the time of his death in 1991 he was the world President of the International Association for HydroEnvironment Engineering and Research (IAHR)."""@en ;
            skos:altLabel "Jack Lawson Scholarship"@En ;
            skos:prefLabel "JD Lawson scholarship"@en ;
            skos:inScheme <https://linked.data.gov.au/def/ea-awards> ;
            skos:broader award:national-committee .

        award:munro-oration a skos:Concept ; 
            rdfs:isDefinedBy <https://linked.data.gov.au/def/ea-awards> ;
            dcterms:source "https://hwrs.com.au/program/speakers"^^xsd:anyURI ;
            skos:definition """The Munro Oration is an invitational keynote speech offered by The National Committee on Water Engineering (NCWE) at the Hydrology and Water Resources Symposium."""@en ;
            skos:prefLabel "Munro Oration"@en ;
            skos:inScheme <https://linked.data.gov.au/def/ea-awards> ;
            skos:broader award:national-committee .

        award:ncwe-hall-of-fame a skos:Concept ; 
            rdfs:isDefinedBy <https://linked.data.gov.au/def/ea-awards> ;
            dcterms:source "https://aeea.engineersaustralia.org.au/national-committee-on-water-engineering-ncwe/"^^xsd:anyURI ;
            skos:definition """The National Committee on Water Engineering (NCWE) Hall of Fame honours outstanding lifetime contribution to the science of hydraulics and to the practice of hydrology and water resources engineering."""@en ;
            skos:prefLabel "NCWE Hall of Fame"@en ;
            skos:inScheme <https://linked.data.gov.au/def/ea-awards> ;
            skos:broader award:national-committee .

        award:ncwe-student-scholarships a skos:Concept ; 
            rdfs:isDefinedBy <https://linked.data.gov.au/def/ea-awards> ;
            dcterms:source "https://aeea.engineersaustralia.org.au/national-committee-on-water-engineering-ncwe/"^^xsd:anyURI ;
            skos:definition """The National Committee on Water Engineering (NCWE) Student Scholarships promote engineering excellence and acknowledge the contribution of individuals to the profession of hydrology and water resources engineering and are awarded to students with outstanding performance in the discipline."""@en ;
            skos:prefLabel "NCWE Student Scholarships"@en ;
            skos:inScheme <https://linked.data.gov.au/def/ea-awards> ;
            skos:broader award:national-committee .

award:tertiary a skos:Concept ;
    rdfs:isDefinedBy <https://linked.data.gov.au/def/ea-awards> ;
    dcterms:source "https://aeea.engineersaustralia.org.au/tertiary-awards/"^^xsd:anyURI ;
    skos:definition """Engineers Australia Teritiary Awards recognise the hard work and achievements of Australia's most dedicated engineering students.

    Every year Engineers Australia seeks to recognise those who will join the engineering profession and contribute to its future through the annual Tertiary Institution Graduate Engineer Awards. Institutions are invited to select graduating students to be awarded an Engineers Australia Institution Graduate Award to recognise the hard work and achievements of Australia's most dedicated engineering students."""@en ;
    skos:prefLabel "Tertiary Awards"@en ;
    skos:inScheme <https://linked.data.gov.au/def/ea-awards> ;
    skos:topConceptOf <https://linked.data.gov.au/def/ea-awards> .
        
    award:ncwe-student-scholarships a skos:Concept ; 
        rdfs:isDefinedBy <https://linked.data.gov.au/def/ea-awards> ;
        dcterms:source "https://aeea.engineersaustralia.org.au/tertiary-awards/"^^xsd:anyURI ;
        skos:definition """An Engineers Australia Institution Graduate Award is awarded to a graduating student engineer from any engineering discipline from each Australian tertiary institution. Each institution is invited to select this award recipient. For institutions with engineering programs at more than one level, an award can be presented at each engineering occupation level (e.g. professional engineering level - BE(Hons) or ME where engineering is a second degree, engineering technologist - BTech, associate engineer - AdvDip or Associate Degree). These awards will be decided by each tertiary institution and presented in conjunction with the local Engineers Australia office."""@en ;
        skos:prefLabel "Engineers Australia Institution Graduate Award"@en ;
        skos:inScheme <https://linked.data.gov.au/def/ea-awards> ;
        skos:broader award:tertiary .

#COLLECTIONS

#awards:current-awards