@prefix eaec: <https://linked.data.gov.au/def/ea-engineering-credentials/> .
@prefix dc: <http://purl.org/dc/elements/1.1/> .
@prefix dcterms: <http://purl.org/dc/terms/> .
@prefix owl: <http://www.w3.org/2002/07/owl#> .
@prefix rdf: <http://www.w3.org/1999/02/22-rdf-syntax-ns#> .
@prefix rdfs: <http://www.w3.org/2000/01/rdf-schema#> .
@prefix sdo: <http://schema.org/> .
@prefix skos: <http://www.w3.org/2004/02/skos/core#> .
@prefix xml: <http://www.w3.org/XML/1998/namespace> .
@prefix xsd: <http://www.w3.org/2001/XMLSchema#> .

<https://linked.data.gov.au/def/ea-engineering-credentials> a owl:Ontology ,
        skos:ConceptScheme ;
    dcterms:created "2022-11-09"^^xsd:date ;
    dcterms:creator <https://linked.data.gov.au/org/engineersaustralia>;
    dcterms:publisher <https://linked.data.gov.au/org/engineersaustralia>;
    dcterms:modified "2023-05-26"^^xsd:date ;
    dcterms:contributor <https://orcid.org/0000-0003-2309-7004> ;
    dcterms:source "https://www.engineersaustralia.org.au"^^xsd:anyURI ;
    dcterms:accessRights <https://linked.data.gov.au/def/data-access-rights/open> ;
    skos:definition """The formally administered lists and registers of credentials describing the experience of professional Engineers. Registers also describe the details of General Areas of Practice and Specific Areas of Practice, that are entered onto the EA National Engineering Register (NER) held by an engineer."""@en ;
    skos:altLabel "Credentials"@en ;
    skos:prefLabel "Engineers Australia Credentials and Registration"@en .

eaec:aiet a skos:Concept ;
    rdfs:isDefinedBy <https://linked.data.gov.au/def/ea-engineering-credentials> ;
    dcterms:source "https://www.ieagreements.org/agreements/apec/registered-apec-engineers/"^^xsd:anyURI ;
    skos:definition "Engineers Australia is a participant in the International Engineering Technicians (AIET) agreement. This reciprocal arrangement enables overseas engineering professionals who have a substantially equivalent role to the Australian engineering associate to register and vice versa."@en ;
    skos:prefLabel "International Engineering Technicians"@en ;
    skos:notation "AIET" ;
    skos:inScheme <https://linked.data.gov.au/def/ea-engineering-credentials> ;
    skos:topConceptOf <https://linked.data.gov.au/def/ea-engineering-credentials> .

eaec:apec a skos:Concept ;
    rdfs:isDefinedBy <https://linked.data.gov.au/def/ea-engineering-credentials> ;
    dcterms:source "https://www.ieagreements.org/agreements/apec/registered-apec-engineers/"^^xsd:anyURI ;
    skos:definition "The IEA provides lists to APEC Registered Engineers in their jurisdictions. These lists hold information on APEC Engineers who have achieved the required common standards of professional competence in their home economies."@en ;
    skos:prefLabel "Asia-Pacific Economic Cooperation"@en ;
    skos:notation "APEC" ;
    skos:inScheme <https://linked.data.gov.au/def/ea-engineering-credentials> ;
    skos:topConceptOf <https://linked.data.gov.au/def/ea-engineering-credentials> .

eaec:chartered a skos:Concept ;
    rdfs:isDefinedBy <https://linked.data.gov.au/def/ea-engineering-credentials> ;
    dcterms:source "https://www.engineersaustralia.org.au/credentials/chartered"^^xsd:anyURI ;
    skos:definition "The Chartered credential is the highest available technical credential for an engineering professional. It is nationally and internationally recognised as a measure of excellence and signifies a certain level of skill, talent and experience."@en ;
    skos:prefLabel "Chartered"@en ;
    skos:notation "C" ;
    skos:inScheme <https://linked.data.gov.au/def/ea-engineering-credentials> ;
    skos:topConceptOf <https://linked.data.gov.au/def/ea-engineering-credentials> .

eaec:chartered-ret a skos:Concept ;
    rdfs:isDefinedBy <https://linked.data.gov.au/def/ea-engineering-credentials> ;
    dcterms:source "https://www.engineersaustralia.org.au/credentials/chartered"^^xsd:anyURI ;
    skos:definition "A chartered engineer who has retired from the profession."@en ;
    skos:prefLabel "Chartered (Retired)"@en ;
    skos:notation "(Ret)" ;
    skos:inScheme <https://linked.data.gov.au/def/ea-engineering-credentials> ;
    skos:broader eaec:chartered .

eaec:destra a skos:Concept ;
    rdfs:isDefinedBy <https://linked.data.gov.au/def/ea-engineering-credentials> ;
    dcterms:source "https://www.engineersaustralia.org.au/news-and-media/2022/07/why-new-defence-partnership-signals-growing-need-professional-standards"^^xsd:anyURI ;
    skos:definition """Under the Defence Engineer and Senior Technician Agreement (DESTRA) all technical Flight Sergeants and Warrant Officers, and all engineers above Squadron Leader rank, will have their leadership, management and technical skills accredited against a global benchmark.
    
    Defence meets - and in some cases exceeds - the level required for certification and registration."@en ;
    skos:prefLabel "Defence Engineer and Senior Technician Agreement"""@en ;
    skos:notation "DESTRA" ;
    skos:inScheme <https://linked.data.gov.au/def/ea-engineering-credentials> ;
    skos:topConceptOf <https://linked.data.gov.au/def/ea-engineering-credentials> .

eaec:eng-exec a skos:Concept ;
    rdfs:isDefinedBy <https://linked.data.gov.au/def/ea-engineering-credentials> ;
    dcterms:source "https://www.engineersaustralia.org.au/credentials/engexec"^^xsd:anyURI ;
    skos:definition "The Engineering Executive, or EngExec is a credential that recognises pre-eminent individuals in executive positions who have shown exceptional leadership and talent. After an outstanding career which has culminated in a senior leadership position, the receipt of EngExec is the next step in your career."@en ;
    skos:prefLabel "Engineering Executive"@en ;
    skos:notation "EngExec" ;
    skos:inScheme <https://linked.data.gov.au/def/ea-engineering-credentials> ;
    skos:topConceptOf <https://linked.data.gov.au/def/ea-engineering-credentials> .

eaec:ipea a skos:Concept ;
    rdfs:isDefinedBy <https://linked.data.gov.au/def/ea-engineering-credentials> ;
    dcterms:source "https://www.ieagreements.org/agreements/ipea/"^^xsd:anyURI ;
    skos:definition "The international professional engineers agreement recognises the substantial equivalency of standards establishing the competency of professional engineers for independent practice."@en ;
    skos:prefLabel "International Professional Engineers Agreement"@en ;
    skos:notation "IPEA" ;
    skos:inScheme <https://linked.data.gov.au/def/ea-engineering-credentials> ;
    skos:topConceptOf <https://linked.data.gov.au/def/ea-engineering-credentials> .

eaec:ieta a skos:Concept ;
    rdfs:isDefinedBy <https://linked.data.gov.au/def/ea-engineering-credentials> ;
    dcterms:source "https://www.engineersaustralia.org.au/credentials/registration/international-registers#accordion-1626"^^xsd:anyURI ;
    skos:definition "The Register of International Engineering Technologists (IETA) is a reciprocal arrangement. It enables overseas engineering professionals who have a substantially equivalent role to the Australian engineering technologist to register and vice versa."@en ;
    skos:prefLabel "International Engineering Technologists"@en ;
    skos:notation "IETA" ;
    skos:inScheme <https://linked.data.gov.au/def/ea-engineering-credentials> ;
    skos:topConceptOf <https://linked.data.gov.au/def/ea-engineering-credentials> .

eaec:ner a skos:Concept ;
    rdfs:isDefinedBy <https://linked.data.gov.au/def/ea-engineering-credentials> ;
    dcterms:source "http://linked.data.gov.au/org/engineersaustralia"^^xsd:anyURI ;
    skos:definition "A comprehensive directory of Australian engineers who have met the high standards of professionalism expected within the industry. Engineers Australia created the NER to provide engineering professionals and employers with a tool that connects talent to opportunities.
        
    The National Engineering Register supersedes the National Professional Engineering Register, National National Engineering Technologists Register, and the National Engineering Associates Register."@en ;
    skos:prefLabel "National Engineering Register"@en ;
    skos:notation "NER" ;
    skos:inScheme <https://linked.data.gov.au/def/ea-engineering-credentials> ;
    skos:topConceptOf <https://linked.data.gov.au/def/ea-engineering-credentials> .

eaec:rpeq a skos:Concept ;
    rdfs:isDefinedBy <https://linked.data.gov.au/def/ea-engineering-credentials> ;
    dcterms:source "https://bpeq.qld.gov.au/thinkrpeq/"^^xsd:anyURI ;
    skos:definition "Any engineer wanting to undertake professional engineering services in or for Queensland is legally required to register as a RPEQ."@en ;
    skos:prefLabel "Registered Professional Engineer of Queensland"@en ;
    skos:notation "RPEQ" ;
    skos:inScheme <https://linked.data.gov.au/def/ea-engineering-credentials> ;
    skos:topConceptOf <https://linked.data.gov.au/def/ea-engineering-credentials> .

<https://linked.data.gov.au/org/engineersaustralia>
    a sdo:Organization ;
    sdo:name "Engineers Australia" ;
    sdo:url "https://www.engineersaustralia.org.au"^^xsd:anyURI ;
.

<https://orcid.org/0000-0003-2309-7004> a owl:NamedIndividual,
        sdo:Person ;
    sdo:affiliation [ a sdo:Organization ;
            sdo:name "Engineers Australia" ;
            sdo:url "https://www.engineersaustralia.org.au"^^xsd:anyURI ] ;
    sdo:name "Vance Kelly" ;
    sdo:identifier <https://orcid.org/0000-0003-2309-7004> .