@prefix eaec: <https://ref.engineersaustralia.org.au/def/ea-engineering-credentials/> .
@prefix dc: <http://purl.org/dc/elements/1.1/> .
@prefix dcterms: <http://purl.org/dc/terms/> .
@prefix owl: <http://www.w3.org/2002/07/owl#> .
@prefix rdf: <http://www.w3.org/1999/02/22-rdf-syntax-ns#> .
@prefix rdfs: <http://www.w3.org/2000/01/rdf-schema#> .
@prefix sdo: <http://schema.org/> .
@prefix skos: <http://www.w3.org/2004/02/skos/core#> .
@prefix xml: <http://www.w3.org/XML/1998/namespace> .
@prefix xsd: <http://www.w3.org/2001/XMLSchema#> .

<https://ref.engineersaustralia.org.au/def/ea-engineering-credentials> a owl:Ontology ,
        skos:ConceptScheme ;
    dcterms:created "2022-11-09"^^xsd:date ;
    dcterms:creator <https://linked.data.gov.au/org/engineersaustralia>;
    dcterms:publisher <https://linked.data.gov.au/org/engineersaustralia>;
    dcterms:modified "2023-05-26"^^xsd:date ;
    dcterms:contributor <https://orcid.org/0000-0003-2309-7004> ;
    dcterms:source "https://www.engineersaustralia.org.au"^^xsd:anyURI ;
    dcterms:accessRights <https://linked.data.gov.au/def/data-access-rights/open> ;
    skos:definition """The formally administered lists and registers of credentials describing the experience of professional Engineers. Registers also describe the details of General Areas of Practice and Specific Areas of Practice, that are entered onto the EA National Engineering Register (NER) held by an engineer."""@en ;
    skos:altLabel "Credentials"@en ;
    skos:prefLabel "Engineers Australia Credentials and Registration"@en .

eaec:chartered a skos:Concept ;
    rdfs:isDefinedBy <https://ref.engineersaustralia.org.au/def/ea-engineering-credentials> ;
    dcterms:source "https://www.engineersaustralia.org.au/credentials/chartered"^^xsd:anyURI ;
    skos:definition "The Chartered credential is the highest available technical credential for an engineering professional. It is nationally and internationally recognised as a measure of excellence and signifies a certain level of skill, talent and experience."@en ;
    skos:prefLabel "Chartered"@en ;
    skos:notation "C" ;
    skos:inScheme <https://ref.engineersaustralia.org.au/def/ea-engineering-credentials> ;
    skos:topConceptOf <https://ref.engineersaustralia.org.au/def/ea-engineering-credentials> .

eaec:chartered-ret a skos:Concept ;
    rdfs:isDefinedBy <https://ref.engineersaustralia.org.au/def/ea-engineering-credentials> ;
    dcterms:source "https://www.engineersaustralia.org.au/credentials/chartered"^^xsd:anyURI ;
    skos:definition "A chartered engineer who has retired from the profession."@en ;
    skos:prefLabel "Chartered (Retired)"@en ;
    skos:notation "(Ret)" ;
    skos:inScheme <https://ref.engineersaustralia.org.au/def/ea-engineering-credentials> ;
    skos:broader eaec:chartered .

eaec:eng-exec a skos:Concept ;
    rdfs:isDefinedBy <https://ref.engineersaustralia.org.au/def/ea-engineering-credentials> ;
    dcterms:source "https://www.engineersaustralia.org.au/credentials/engexec"^^xsd:anyURI ;
    skos:definition "The Engineering Executive, or EngExec is a credential that recognises pre-eminent individuals in executive positions who have shown exceptional leadership and talent. After an outstanding career which has culminated in a senior leadership position, the receipt of EngExec is the next step in your career."@en ;
    skos:prefLabel "Engineering Executive"@en ;
    skos:notation "EngExec" ;
    skos:inScheme <https://ref.engineersaustralia.org.au/def/ea-engineering-credentials> ;
    skos:topConceptOf <https://ref.engineersaustralia.org.au/def/ea-engineering-credentials> .

eaec:ner a skos:Concept ;
    rdfs:isDefinedBy <https://ref.engineersaustralia.org.au/def/ea-engineering-credentials> ;
    dcterms:source "http://linked.data.gov.au/org/engineersaustralia"^^xsd:anyURI ;
    skos:definition "A comprehensive directory of Australian engineers who have met the high standards of professionalism expected within the industry. Engineers Australia created the NER to provide engineering professionals and employers with a tool that connects talent to opportunities.
        
    The National Engineering Register supersedes the National Professional Engineering Register, National National Engineering Technologists Register, and the National Engineering Associates Register."@en ;
    skos:prefLabel "National Engineering Register"@en ;
    skos:notation "NER" ;
    skos:inScheme <https://ref.engineersaustralia.org.au/def/ea-engineering-credentials> ;
    skos:topConceptOf <https://ref.engineersaustralia.org.au/def/ea-engineering-credentials> .

eaec:rpeq a skos:Concept ;
    rdfs:isDefinedBy <https://ref.engineersaustralia.org.au/def/ea-engineering-credentials> ;
    dcterms:source "https://bpeq.qld.gov.au/thinkrpeq/"^^xsd:anyURI ;
    skos:definition "Any engineer wanting to undertake professional engineering services in or for Queensland is legally required to register as a RPEQ."@en ;
    skos:prefLabel "Registered Professional Engineer of Queensland"@en ;
    skos:notation "RPEQ" ;
    skos:inScheme <https://ref.engineersaustralia.org.au/def/ea-engineering-credentials> ;
    skos:topConceptOf <https://ref.engineersaustralia.org.au/def/ea-engineering-credentials> .

<https://linked.data.gov.au/org/engineersaustralia>
    a sdo:Organization ;
    sdo:name "Engineers Australia" ;
    sdo:url "https://www.engineersaustralia.org.au"^^xsd:anyURI ;
.

<https://orcid.org/0000-0003-2309-7004> a owl:NamedIndividual,
        sdo:Person ;
    sdo:affiliation [ a sdo:Organization ;
            sdo:name "Engineers Australia" ;
            sdo:url "https://www.engineersaustralia.org.au"^^xsd:anyURI ] ;
    sdo:name "Vance Kelly" ;
    sdo:identifier <https://orcid.org/0000-0003-2309-7004> .