PREFIX eaec: <https://ref.engineersaustralia.org.au/def/ea-engineering-credentials/>
PREFIX eaox: <https://ref.engineersaustralia.org.au/def/properties#>
PREFIX aop: <https://ref.engineersaustralia.org.au/def/areasofpractice/>
PREFIX dc: <http://purl.org/dc/elements/1.1/>
PREFIX dcterms: <http://purl.org/dc/terms/>
PREFIX owl: <http://www.w3.org/2002/07/owl#>
PREFIX rdf: <http://www.w3.org/1999/02/22-rdf-syntax-ns#>
PREFIX rdfs: <http://www.w3.org/2000/01/rdf-schema#>
PREFIX sdo: <http://schema.org/>
PREFIX skos: <http://www.w3.org/2004/02/skos/core#>
PREFIX xml: <http://www.w3.org/XML/1998/namespace>
PREFIX xsd: <http://www.w3.org/2001/XMLSchema#>

<https://ref.engineersaustralia.org.au/def/ea-engineering-credentials> a owl:Ontology ,
        skos:ConceptScheme ;
    dcterms:created "2022-11-09"^^xsd:date ;
    dcterms:creator <https://linked.data.gov.au/org/engineersaustralia>;
    dcterms:publisher <https://linked.data.gov.au/org/engineersaustralia>;
    dcterms:modified "2023-05-26"^^xsd:date ;
    dcterms:source "https://www.engineersaustralia.org.au"^^xsd:anyURI ;
    dcterms:accessRights <https://linked.data.gov.au/def/data-access-rights/open> ;
    prov:qualifiedAttribution
        [
            dcat:hadRole earl:data-steward ;
            prov:agent [
                    a prov:Agent ;
                    rdfs:label "Engineers Australia: Head of Registration"
                ]
        ] ;
    skos:hasTopConcept
        eaec:aiet,
        eaec:apec,
        eaec:chartered,
        eaec:eng-exec,
        eaec:ieta,
        eaec:ipea,
        eaec:ner,
        eaec:pers,
        eaec:rpeq,
        eaec:tas-cbos,
        eaec:nsw-dbp,
        eaec:nt-bpb,
        eaec:vic-per,
        eaec:wa-ber,
        eaec:ea-college,
        eaec:sea-freight-container,
        eaec:strata-inspector,
        eaec:vertical-transport ;
    skos:definition """The formally administered registers and records of credentials describing the experience and associations of professional Engineers. Registers may describe the details of General Areas of Practice and Specific Areas of Practice, that are entered onto the EA National Engineering Register (NER) held by an engineer. The administered lists also include the formal agreements betweeen Engineers Australia and other organisations for member sponsorship and the recognition of equivalent credientials, competency, or standards."""@en ;
    skos:note """The skos notations in this vocabulary are specifically used as the post-nominals associated with the credentials and registrations. Where a post-nominal is not associated with the concept, no notation should be described"""@en ;
    skos:altLabel "Credentials"@en,
        "Registrations"@en,
        "Eligibility Assessments"@en ;
    skos:prefLabel "Engineers Australia Credentials and Registration"@en .

<https://linked.data.gov.au/org/engineersaustralia>
    a sdo:Organization ;
    sdo:name "Engineers Australia" ;
    sdo:url "https://www.engineersaustralia.org.au"^^xsd:anyURI ;
.

# International Registrations

eaec:apec a skos:Concept ;
    dcterms:source "https://www.ieagreements.org/agreements/apec/registered-apec-engineers/"^^xsd:anyURI ;
    rdfs:isDefinedBy <https://ref.engineersaustralia.org.au/def/ea-engineering-credentials> ;
    eaox:validCollection aop:areas-of-practice-international ;
    eaox:orderOfDisplay "11"^^xsd:integer ;
    skos:inScheme <https://ref.engineersaustralia.org.au/def/ea-engineering-credentials> ;
    skos:topConceptOf <https://ref.engineersaustralia.org.au/def/ea-engineering-credentials> ;
    skos:definition "The Asia-Pacific Economic Cooperation (APEC) is a regional economic forum established in 1989 to leverage the growing interdependence of the Asia-Pacific. APEC's 21 members aim to create greater prosperity for the people of the region by promoting balanced, inclusive, sustainable, innovative and secure growth and by accelerating regional economic integration.
    
    The IEA provides lists to APEC Registered Engineers in their jurisdictions. These lists hold information on APEC Engineers who have achieved the required common standards of professional competence in their home economies.
    
    A user registered on the APEC register, can use the post-nominal APECEngineer."@en ;
    skos:notation "APEC Engineer" ;
    skos:altLabel "APEC Agreement"@en,
        "APEC Engineers"@en,
        "APEC Engineer Register"@en ;
    skos:prefLabel "Asia-Pacific Economic Cooperation"@en .

eaec:ipea a skos:Concept ;
    dcterms:source "https://www.ieagreements.org/agreements/ipea/"^^xsd:anyURI ;
    rdfs:isDefinedBy <https://ref.engineersaustralia.org.au/def/ea-engineering-credentials> ;
    eaox:validCollection aop:areas-of-practice-international ;
    eaox:orderOfDisplay "12"^^xsd:integer ;
    skos:inScheme <https://ref.engineersaustralia.org.au/def/ea-engineering-credentials> ;
    skos:topConceptOf <https://ref.engineersaustralia.org.au/def/ea-engineering-credentials>;
    skos:definition "the International Professional Engineers Agreement (IPEA),  is a multi-national agreement between engineering organisations in the member jurisdictions which creates the framework for the establishment of an international standard of competence for professional engineering, and then empowers each member organization to establish a section of the International Professional Engineers Register. The IPEA recognises the substantial equivalency of standards establishing the competency of professional engineers for independent practice.
    
    A user registered on the IPEA register, can use the post-nominal IntPE(Aus)."@en ;
    skos:notation "IntPE(Aus)" ;
    skos:hiddenLabel "Engineers Mobility Forum"@en ;
    skos:altLabel "IPEA"@en ;
    skos:prefLabel "International Professional Engineers Agreement"@en  .

eaec:ieta a skos:Concept ;
    dcterms:source "https://www.theiet.org/career/professional-registration/international-professional-registration/international-engineering-technologist"^^xsd:anyURI ;
    rdfs:isDefinedBy <https://ref.engineersaustralia.org.au/def/ea-engineering-credentials> ;
    eaox:validCollection aop:areas-of-practice-international ;
    eaox:orderOfDisplay "13"^^xsd:integer ;
    skos:inScheme <https://ref.engineersaustralia.org.au/def/ea-engineering-credentials> ;
    skos:topConceptOf <https://ref.engineersaustralia.org.au/def/ea-engineering-credentials> ;
    skos:definition "The Register of International Engineering Technologists (IETA) is a reciprocal arrangement. It enables overseas engineering professionals who have a substantially equivalent role to the Australian engineering technologist to register and vice versa."@en ;
    skos:notation "IntET(Aus)" ;
    skos:altLabel "IETA"@en,
        "Register of International Engineering Technologists"@en ;
    skos:prefLabel "International Engineering Technologists"@en .

eaec:aiet a skos:Concept ;
    dcterms:source "https://www.theiet.org/career/professional-registration/international-professional-registration/international-engineering-technician"^^xsd:anyURI ;
    rdfs:isDefinedBy <https://ref.engineersaustralia.org.au/def/ea-engineering-credentials> ;
    eaox:validCollection aop:areas-of-practice-international ;
    eaox:orderOfDisplay "14"^^xsd:integer ;
    skos:inScheme <https://ref.engineersaustralia.org.au/def/ea-engineering-credentials> ;
    skos:topConceptOf <https://ref.engineersaustralia.org.au/def/ea-engineering-credentials> ;
    skos:definition "Engineers Australia is a participant in the International Engineering Technicians (AIET) agreement. This reciprocal arrangement enables overseas engineering professionals who have a substantially equivalent role to the Australian engineering associate to register and vice versa."@en ;
    skos:notation "IntETn(Aus)" ;
    skos:altLabel "AIET"@en,
        "Register of International Engineering Technicians"@en ;
    skos:prefLabel "International Engineering Technicians"@en .

#State Registrations (order of display alphabetical)

eaec:pers a skos:Concept ;
    dcterms:source "https://www.planning.act.gov.au/professionals/regulation-and-responsibilities/professional-engineers-registration-scheme"^^xsd:anyURI ;
    rdfs:isDefinedBy <https://ref.engineersaustralia.org.au/def/ea-engineering-credentials> ;
    eaox:validCollection aop:areas-of-practice-act ;
    eaox:orderOfDisplay "2"^^xsd:integer ;
    skos:inScheme <https://ref.engineersaustralia.org.au/def/ea-engineering-credentials> ;
    skos:topConceptOf <https://ref.engineersaustralia.org.au/def/ea-engineering-credentials> ;
    skos:definition """The ACT's Professional Engineers Registration Scheme commenced on 6 March 2025.
    
    This means, engineers must now be registered if offering professional engineering services in any of the following areas of engineering:
    - Civil,
    - Structural,
    - Electrical,
    - Mechanical, and
    - Fire Safety."""@en ;
    skos:altLabel "Professional engineers registration scheme"@en ;
    skos:prefLabel "ACT Professional engineers registration scheme"@en .

eaec:nsw-dbp a skos:Concept ;
    dcterms:source "https://www.nsw.gov.au/business-and-economy/licences-and-credentials/building-and-trade-licences-and-registrations/register/professional-engineers"^^xsd:anyURI ;
    rdfs:isDefinedBy <https://ref.engineersaustralia.org.au/def/ea-engineering-credentials> ;
    eaox:validCollection aop:areas-of-practice-nsw ;
    eaox:orderOfDisplay "3"^^xsd:integer ;
    skos:inScheme <https://ref.engineersaustralia.org.au/def/ea-engineering-credentials> ;
    skos:topConceptOf <https://ref.engineersaustralia.org.au/def/ea-engineering-credentials> ;
    skos:definition """Professional engineers must meet eligibility requirements to register to work on regulated buildings under the NSW Design and Building Practitioners (DBP) scheme."""@en ;
    skos:altLabel "Design and Building Practitioners"@en ;
    skos:prefLabel "NSW Design and Building Practitioners"@en .

eaec:nt-bpb a skos:Concept ;
    dcterms:source "https://bpb.nt.gov.au/"^^xsd:anyURI ;
    rdfs:isDefinedBy <https://ref.engineersaustralia.org.au/def/ea-engineering-credentials> ;
    eaox:validCollection aop:areas-of-practice-nt ;
    eaox:orderOfDisplay "4"^^xsd:integer ;
    skos:inScheme <https://ref.engineersaustralia.org.au/def/ea-engineering-credentials> ;
    skos:topConceptOf <https://ref.engineersaustralia.org.au/def/ea-engineering-credentials> ;
    skos:definition """Building Practitioners in the Northern Territory are required to hold appropriate registration to work in the building industry.

    To build trust and capability in the industry and help monitor and regulate practitioners' competence and compliance, the Building Practitioners Board is established by the Building Act 1993."""@en ;
    skos:altLabel "Building Practitioners Board"@en ;
    skos:prefLabel "NT Building Practitioners Board"@en .

eaec:rpeq a skos:Concept ;
    dcterms:source "https://bpeq.qld.gov.au/for-engineers/become-a-rpeq"^^xsd:anyURI ;
    rdfs:isDefinedBy <https://ref.engineersaustralia.org.au/def/ea-engineering-credentials> ;
    eaox:validCollection aop:areas-of-practice-qld ;
    eaox:orderOfDisplay "5"^^xsd:integer ;
    skos:inScheme <https://ref.engineersaustralia.org.au/def/ea-engineering-credentials> ;
    skos:topConceptOf <https://ref.engineersaustralia.org.au/def/ea-engineering-credentials> ;
    skos:definition """Registration as a registered professional engineer of Queensland (RPEQ) demonstrates an engineer's qualification, competency and experience and ongoing commitment to development and learning.

    Engineers carry out highly complex work and it is appropriate - just like many other professions - that they meet and uphold high standards of professional practice. The PE Act requires that anyone carrying out a professional engineering service in Queensland or for Queensland (e.g. a design project carried out interstate or overseas for a Queensland based project) must meet these standards and then be registered as a RPEQ. This ensures that only qualified, competent and experienced professionals design, build, maintain and develop the products, infrastructure and services we use every day."""@en ;
    skos:notation "RPEQ" ;
    skos:prefLabel "Registered Professional Engineer of Queensland"@en .

eaec:tas-cbos a skos:Concept ;
    dcterms:source "https://www.cbos.tas.gov.au/topics/licensing-and-registration/licensed-occupations/building-provider-licences/engineer"^^xsd:anyURI ;
    rdfs:isDefinedBy <https://ref.engineersaustralia.org.au/def/ea-engineering-credentials> ;
    eaox:validCollection aop:areas-of-practice-tas ;
    eaox:orderOfDisplay "6"^^xsd:integer ;
    skos:inScheme <https://ref.engineersaustralia.org.au/def/ea-engineering-credentials> ;
    skos:topConceptOf <https://ref.engineersaustralia.org.au/def/ea-engineering-credentials> ;
    skos:definition """For an engineer to be licensed in Tasmania they must have a degree for the relevant engineer sub-class and satisfy the relevant experience requirement, or be listed on the National Engineers Register or be recognised by Engineers Australia as a Chartered Professional Engineer.
    All building service providers must act only within the area of their competence, as detailed in the Occupational Licensing (Building Services Work) Determination.

    There are three sub-classes of licensed engineers.
    1. Engineer fire safety: This class is unrestricted in the field of fire safety engineering and includes deemed-to-satisfy and performance solutions. Fire safety engineering is the application of engineering principles, rules and expert judgement based on a scientific appreciation of fire and its effects, and of the reaction and behaviour of people in the event of fire.
    2. Engineer building services: This class is unrestricted in the field of building services and includes deemed-to-satisfy and performance solutions. Building services may include mechanical building services, hydraulic building services, electrical building services, fire safety systems, building acoustics and energy management in buildings.
    3. Engineer civil: This class is unrestricted in the field of civil engineering and includes deemed-to-satisfy and performance solutions. Civil engineering may include civil, structural, geotechnical and environmental engineering."""@en ;
    skos:altLabel "Engineer Licence"@en ;
    skos:prefLabel "Tasmania Engineer Licence"@en .

eaec:vic-per a skos:Concept ;
    dcterms:source "https://www.consumer.vic.gov.au/licensing-and-registration/professional-engineers/who-needs-to-be-registered"^^xsd:anyURI ;
    rdfs:isDefinedBy <https://ref.engineersaustralia.org.au/def/ea-engineering-credentials> ;
    eaox:validCollection aop:areas-of-practice-vic ;
    eaox:orderOfDisplay "7"^^xsd:integer ;
    skos:inScheme <https://ref.engineersaustralia.org.au/def/ea-engineering-credentials> ;
    skos:topConceptOf <https://ref.engineersaustralia.org.au/def/ea-engineering-credentials> ;
    skos:definition """You must be registered as a Professional Engineer to provide:
    - professional engineering services
    - those services in a prescribed area of engineering, and
    - those services in or for Victoria.

    
    A professional engineering service is an engineering service that requires, or is based on, the application of engineering principles and data to:
    - a design relating to engineering, or
    - a construction, production, operation or maintenance activity relating to engineering.

    Professional engineering services are a specialist subset of engineering services. They are distinguished from other engineering services by a high degree of engineering judgement, knowledge and skill. Many, but not all, engineering services are professional engineering services.
    The five prescribed areas of engineering under the Act are:
        - fire safety engineering,
        - civil engineering,
        - structural engineering,
        - electrical engineering,
        - mechanical engineering."""@en ;
    skos:notation "RPEng" ;
    skos:altLabel "Professional Engineer in Victoria"@en,
        "Professional Engineer Registration - Victoria"@en ;
    skos:prefLabel "Victoria Professional Engineer Registration"@en .

eaec:wa-ber a skos:concept
    dcterms:source "https://www.wa.gov.au/government/multi-step-guides/building-engineering-registration"^^xsd:anyURI ;
    rdfs:isDefinedBy <https://ref.engineersaustralia.org.au/def/ea-engineering-credentials> ;
    eaox:validCollection aop:areas-of-practice-wa ;
    eaox:orderOfDisplay "8"^^xsd:integer ;
    skos:inScheme <https://ref.engineersaustralia.org.au/def/ea-engineering-credentials> ;
    skos:topConceptOf <https://ref.engineersaustralia.org.au/def/ea-engineering-credentials> ;
    skos:definition """The building engineer's registration scheme (the Registration Scheme) commenced 1 July 2024 and will be implemented in two phases over three years.
    
    The scheme is prescribed under the Building Services (Registration) Act 2011 (WA) (the Act). Under the scheme, engineers must be registered to undertake design, construction or production work in prescribed areas of engineering for a building or incidental structure under the Building Act 2011 and the National Construction Code."""@en ;
    skos:prefLabel "Western Australia Building Engineers Registration"@en .

# EA Engineering Credentials and Registrations

eaec:chartered a skos:Concept ;
    dcterms:source "https://www.engineersaustralia.org.au/credentials/chartered"^^xsd:anyURI ;
    dcterms:references <https://www.engineersaustralia.org.au/credentials/chartered>,
        <https://www.engineersaustralia.org.au/sites/default/files/resource-files/2020-02/EA%20General%20Regulations%205%20Dec%202019.pdf> ;
    rdfs:isDefinedBy <https://ref.engineersaustralia.org.au/def/ea-engineering-credentials> ;
    eaox:validCollection aop:areas-of-practice-chartered ;
    eaox:orderOfDisplay "1"^^xsd:integer ;
    skos:inScheme <https://ref.engineersaustralia.org.au/def/ea-engineering-credentials> ;
    skos:related <https://ref.engineersaustralia.org.au/def/aus-eng-comp-std/stage-2> ;
    skos:topConceptOf <https://ref.engineersaustralia.org.au/def/ea-engineering-credentials>;
    skos:definition """The Chartered credential is the highest available technical credential for an engineering professional. It is nationally and internationally recognised as a measure of excellence and signifies a high level of skill, talent and experience. To be eligible for the Chartered title an individual must be a financial member, meet stage 2 competency requirements, and meet Continuing Professional Development (CPD requirements)."""@en ;
    skos:notation "C" ;
    skos:prefLabel "Chartered"@en .

    eaec:chartered-ret a skos:Concept ;
        dcterms:source "https://www.engineersaustralia.org.au/credentials/chartered"^^xsd:anyURI ;
        rdfs:isDefinedBy <https://ref.engineersaustralia.org.au/def/ea-engineering-credentials> ;
        eaox:orderOfDisplay "1"^^xsd:integer ;
        skos:inScheme <https://ref.engineersaustralia.org.au/def/ea-engineering-credentials> ;
        skos:related <https://ref.engineersaustralia.org.au/def/aus-eng-comp-std/stage-2> ;
        skos:broader eaec:chartered ;
        skos:definition """A chartered engineer who has retired from the profession."""@en ;
        skos:notation "C(Ret)" ;
        skos:prefLabel "Chartered (Retired)"@en .

eaec:eng-exec a skos:Concept ;
    dcterms:source "https://www.engineersaustralia.org.au/credentials/engexec"^^xsd:anyURI ;
    rdfs:isDefinedBy <https://ref.engineersaustralia.org.au/def/ea-engineering-credentials> ;
    eaox:orderOfDisplay "9"^^xsd:integer ;
    skos:related <https://ref.engineersaustralia.org.au/def/aus-eng-comp-std/stage-3> ;
    skos:inScheme <https://ref.engineersaustralia.org.au/def/ea-engineering-credentials> ;
    skos:topConceptOf <https://ref.engineersaustralia.org.au/def/ea-engineering-credentials> ;
    skos:definition """The Engineering Executive, or EngExec is a credential that recognises pre-eminent individuals in executive positions who have shown exceptional leadership and talent. After an outstanding career which has culminated in a senior leadership position, the receipt of EngExec is the next step in your career."""@en ;
    skos:notation "EngExec" ;
    skos:prefLabel "Engineering Executive"@en .

eaec:ner a skos:Concept ;
    dcterms:source "https://www.engineersaustralia.org.au/credentials/registration/national-engineering-register"^^xsd:anyURI ;
    rdfs:isDefinedBy <https://ref.engineersaustralia.org.au/def/ea-engineering-credentials> ;
    eaox:validCollection aop:areas-of-practice-ner ;
    eaox:orderOfDisplay "10"^^xsd:integer ;
    skos:inScheme <https://ref.engineersaustralia.org.au/def/ea-engineering-credentials> ;
    skos:topConceptOf <https://ref.engineersaustralia.org.au/def/ea-engineering-credentials> ;
    skos:definition """Engineers Australia introduced the National Engineering Register (NER) in 2015. This comprehensive directory is a way to recognise engineers who meet the high standards of skill, qualification and professionalism expected in the industry.
    
    It provides a national framework of registration for professional engineers, engineering technologists and engineering associates across the private and public sectors.
    
    As a publicly-searchable database, the NER gives individuals and businesses access to a qualified pool of engineers, endorsed by Australia's engineering peak body.
        
    The National Engineering Register supersedes the National Professional Engineering Register, National National Engineering Technologists Register, and the National Engineering Associates Register."""@en ;
    skos:notation "NER" ;
    skos:prefLabel "National Engineering Register"@en .

# Enrollments and Associations

eaec:ea-college a skos:Concept ;
    dcterms:source "https://www.engineersaustralia.org.au/engineering-communities/colleges-and-college-national-committees"^^xsd:anyURI ;
    rdfs:isDefinedBy <https://ref.engineersaustralia.org.au/def/ea-engineering-credentials> ;
    skos:inScheme <https://ref.engineersaustralia.org.au/def/ea-engineering-credentials> ;
    skos:topConceptOf <https://ref.engineersaustralia.org.au/def/ea-engineering-credentials> ;
    skos:definition """Each member of Engineers Australia, regardless of grade, must be associated with one or more of the 9 Engineers Australia Colleges as per the EA Bye-Laws. Colleges are 'assigned' by EA staff at the point of membership confirmation. Colleges provide a high-level grouping of our membership."""@en ;
    skos:notation "NER" ;
    skos:prefLabel "Engineers Australia College Registration"@en .

# Specialisations

eaec:sea-freight-container a skos:Concept ;
    dcterms:source "https://www.agriculture.gov.au/biosecurity-trade/import/industry-advice/2019/146-2019"^^xsd:anyURI ;
    rdfs:isDefinedBy <https://ref.engineersaustralia.org.au/def/ea-engineering-credentials> ;
    skos:inScheme <https://ref.engineersaustralia.org.au/def/ea-engineering-credentials> ;
    skos:topConceptOf <https://ref.engineersaustralia.org.au/def/ea-engineering-credentials>;
    skos:definition """A register of engineers and structural inspectors who undertake certification and inspection of sea container inspection stands. The Department of Agriculture, Fisheries and Forestry has appointed Engineers Australia to assess the qualifications and experience of engineers practicing in this capacity.
    
    To be eligible for assessment, an individual must be:
    - registered on the National Engineering Register as a professional engineer.
    - registered on a state register if practising in a state or territory that requires it.
    - have valid state certification if required.
    - able to demonstrate a minimum of five years of experience in the specialisation. 
    - be an independent worker, not employed by the site or premises authorities."""@en ;
    skos:altLabel "Sea Freight Container Inspection Stand Engineer"@en ;
    skos:prefLabel "Sea Freight Container Inspection Stand Register"@en .

eaec:strata-inspector a skos:Concept ;
    dcterms:source "https://www.engineersaustralia.org.au/credentials/specialisations#accordion-87356"^^xsd:anyURI ;
    rdfs:isDefinedBy <https://ref.engineersaustralia.org.au/def/ea-engineering-credentials> ;
    skos:inScheme <https://ref.engineersaustralia.org.au/def/ea-engineering-credentials> ;
    skos:topConceptOf <https://ref.engineersaustralia.org.au/def/ea-engineering-credentials>;
    skos:definition """Strata Inspectors have the authority to inspect new apartment builds in New South Wales. Under the Strata building bond & inspections scheme (SBBIS), developers of new apartment buildings 4 storeys or higher must pay a building bond to NSW Fair Trading equal to 2% of the total price paid or payable of all contracts for the building.
    
    To be eligible for assessment as a strata inspector, an individual needs to be a member of Engineers Australia working as a professional engineer, engineering technologist or engineering associate.
    
    Affiliate members may apply, but a required to complete a competency assessment."""@en ;
    skos:notation "SBBIS" ;
    skos:altLabel "Strata Inspector Register"@en,
        "Strata Inspector Panel"@en ;
    skos:prefLabel "Strata Inspector"@en .

eaec:vertical-transport a skos:Concept ;
    dcterms:source "https://www.engineersaustralia.org.au/credentials/specialisations#accordion-87366"^^xsd:anyURI ;
    rdfs:isDefinedBy <https://ref.engineersaustralia.org.au/def/ea-engineering-credentials> ;
    skos:inScheme <https://ref.engineersaustralia.org.au/def/ea-engineering-credentials> ;
    skos:topConceptOf <https://ref.engineersaustralia.org.au/def/ea-engineering-credentials>;
    skos:definition """A New South Wales register of qualified and competent engineers in the practice of vertical transport (lift) design."""@en ;
    skos:notation " DP(VT)" ;
    skos:altLabel "Organisation Sponsorship Agreement"@en ;
    skos:prefLabel "Design Practitioner Vertical Transport Engineer"@en .

#COLLECTIONS

eaec:ea-credentials a skos:Collection ;
    dcterms:source "https://www.engineersaustralia.org.au/credentials"^^xsd:anyURI ;
	skos:prefLabel "Engineers Australia Credentials"@en ;
	skos:definition """Credentials and registers administered, assessed, and granted by Engineers Australia."""@en ;
    skos:member
        eaec:chartered,
        eaec:chartered-ret,
        eaec:eng-exec,
        eaec:ner .

eaec:eng-specialisations a skos:Collection ;
    dcterms:source "https://www.engineersaustralia.org.au/credentials/specialisations"^^xsd:anyURI ;
	skos:altLabel "Specialisations"@en ;
    skos:prefLabel "Engineering Specialisations"@en ;
	skos:definition """Specialisations are niche, distinct areas of engineering practice which originate from an area of practice or area of engineering.
    
    Specialist roles can exist in any of the occupational categories and are usually nominated by business or government stakeholders in response to a vocational need."""@en ;
    skos:member
        eaec:sea-freight-container,
        eaec:strata-inspector ,
        eaec:vertical-transport.

eaec:state-registrations a skos:Collection ;
    dcterms:source "https://www.engineersaustralia.org.au/credentials/registration/state-registration"^^xsd:anyURI ;
	skos:altLabel "State Registers"@en ;
    skos:prefLabel "State Registrations"@en ;
	skos:definition """Specialisations are niche, distinct areas of engineering practice which originate from an area of practice or area of engineering.
    
    Specialist roles can exist in any of the occupational categories and are usually nominated by business or government stakeholders in response to a vocational need."""@en ;
    skos:member
        eaec:nsw-dbp,
        eaec:nt-bpb,
        eaec:pers,
        eaec:rpeq,
        eaec:tas-cbos,
        eaec:wa-ber,
        eaec:vic-per .

eaec:bie a skos:Collection ;
    dcterms:source "https://www.engineersaustralia.org.au/credentials/registration/state-registration/assessment-state-registration"^^xsd:anyURI ;
	skos:altLabel "BIE"@en,
        "Building Industry assessment"@en ;
    skos:prefLabel "Building Industy Endorsement"@en ;
	skos:definition """Endorsements and assessments required by some states and territories to provide professional engineering services to the building industry."""@en ;
    skos:member
        eaec:pers,
        eaec:tas-cbos,
        eaec:wa-ber,
        eaec:vic-per .