PREFIX eaj: <https://ref.engineersaustralia.org.au/def/ea-jargon/>
PREFIX eatm: <https://ref.engineersaustralia.org.au/def/ea-teams/>
PREFIX earegb: <https://ref.engineersaustralia.org.au/def/ea-regulated-bodies/>
PREFIX prty: <https://ref.engineersaustralia.org.au/def/ea-party/>
PREFIX docs: <https://ref.engineersaustralia.org.au/def/ea-documents/>
PREFIX earl: <https://ref.engineersaustralia.org.au/def/ea-activity-roles/>
PREFIX earp: <https://ref.engineersaustralia.org.au/def/ea-party-roles/>
PREFIX ieaoc: <https://linked.data.gov.au/def/iea-occupational-categories/>
PREFIX itev: <https://ref.engineersaustralia.org.au/def/ict-event/>
PREFIX dcat: <http://www.w3.org/ns/dcat#>
PREFIX dcterms: <http://purl.org/dc/terms/>
PREFIX owl: <http://www.w3.org/2002/07/owl#>
PREFIX prov: <http://www.w3.org/ns/prov#>
PREFIX rdfs: <http://www.w3.org/2000/01/rdf-schema#>
PREFIX sdo: <http://schema.org/>
PREFIX skos: <http://www.w3.org/2004/02/skos/core#>
PREFIX xsd: <http://www.w3.org/2001/XMLSchema#>

<https://ref.engineersaustralia.org.au/def/ea-jargon> a owl:Ontology,
        skos:ConceptScheme ;
    dcterms:accessRights <https://linked.data.gov.au/def/data-access-rights/restricted> ;
    dcterms:contributor <https://orcid.org/0000-0003-2309-7004> ;
    dcterms:created "2023-01-31"^^xsd:date ;
    dcterms:creator <https://linked.data.gov.au/org/engineersaustralia> ;
    dcterms:modified "2024-06-013"^^xsd:date ;
    dcterms:publisher <https://linked.data.gov.au/org/engineersaustralia> ;
    dcterms:source "https://linked.data.gov.au/org/engineersaustralia"^^xsd:anyURI ;
    prov:qualifiedAttribution
        [
            dcat:hadRole earl:data-steward ;
            prov:agent [
                    a prov:Agent ;
                    rdfs:label "Engineers Australia: Data and Analytics"
                ]
        ] ;
    skos:hasTopConcept
        prty:board,
        prty:committee,
        prty:project-control-board,
        prty:technical-society,
        docs:skilled-visa,
        eaj:accords,
        eaj:accreditation,
        eaj:active-directory,
        eaj:agent,
        eaj:agile,
        eaj:analytical-model,
        eaj:anzsco,
        eaj:areas-of-practice,
        eaj:audit,
        eaj:aus-privacy-act,
        eaj:aus-privacy-principles,
        eaj:bcm,
        eaj:bcp,
        eaj:benchmarking,
        eaj:bi-platform,
        eaj:business-process,
        eaj:business-process-reengineering,
        eaj:change-management,
        eaj:chartered,
        eaj:competency-standard,
        eaj:content-management-system,
        eaj:code-of-ethics,
        eaj:consequence,
        eaj:continuing-professional-development,
        eaj:continuous-monitoring,
        eaj:control,
        eaj:control-owner,
        eaj:country-education-profiles,
        eaj:credentials,
        eaj:crm,
        eaj:data,
        eaj:data-catalogue,
        eaj:data-dictionary,
        eaj:data-lifecycle,
        eaj:data-model,
        eaj:data-multiple-storage,
        eaj:data-profiling,
        eaj:data-store,
        eaj:data-warehouse,
        eaj:database,
        eaj:defensibly-destroyed,
        eaj:digital-transformation,
        eaj:digital-experience,
        eaj:digital-governance-groups,
        eaj:disciplinary-and-appeals,
        eaj:div-rules,
        eaj:documents,
        eaj:doc-management-system,
        eaj:duty-separation,
        eaj:ea-assessment,
        eaj:ea-by-laws,
        eaj:ea-event,
        eaj:ea-membership-regulations,
        eaj:ea-activity-roles,
        eaj:ea-party-roles,
        eaj:ea-royal-charter,
        eaj:ewc,
        eaj:ict-change,
        eaj:ict-change-freeze,
        eaj:ict-change-priority,
        eaj:ict-event,
        eaj:ict-problem,
        eaj:identity-management,
        eaj:identity-management-app,
        eaj:information,
        eaj:issue,
        eaj:knowledgebase,
        eaj:learning-management-system,
        eaj:least-privilege,
        eaj:master-data-management,
        eaj:membership-grade,
        eaj:membership-change,
        eaj:mfa,
        eaj:occupational-categories,
        eaj:offering,
        eaj:ner,
        eaj:pcas,
        eaj:persistent-identifier,
        eaj:personal-information,
        eaj:personally-identifiable-information,
        eaj:post-nominals,
        eaj:product-feature,
        eaj:professional-development-program,
        eaj:prosci,
        eaj:qualifications,
        eaj:quality-assurance,
        eaj:quality-control,
        eaj:raci,
        eaj:recognition-of-prior-learning,
        eaj:records,
        eaj:ref-data-management-system,
        eaj:review,
        eaj:risk,
        eaj:risk-analysis,
        eaj:risk-appetite,
        eaj:risk-criteria,
        eaj:risk-owner,
        eaj:risk-source,
        eaj:risk-sponsor,
        eaj:risk-exposure,
        eaj:risk-tolerance,
        eaj:risk-treatment,
        eaj:risk-maturity,
        eaj:risk-evaluation,
        eaj:risk-assessment,
        eaj:strategic-context,
        eaj:source-of-truth,
        eaj:sponsorship,
        eaj:sso,
        eaj:study-bridging,
        eaj:system-architecture,
        eaj:event,
        eaj:likelihood,
        eaj:monitoring,
        eaj:shared-risks,
        eaj:stakeholder,
        eaj:threats-opportunities,
        eaj:trades-recognition-australia,
        eaj:unsolicited-customer-data,
        eaj:validation,
        eaj:verification,
        earegb:professional-conduct-committee,
        earl:actor,
        earp:applicant,
        earp:customer ;
    skos:definition """The business language and terminology used throughout Engineers Australia in common communication.
    
    This vocabulary contains general language with minimal heirarchy applied and an unconfined concept scheme. It is presented in this format for consistent and consolidated representation with controlled reference data."""@en ;
    skos:editorialNote """This vocabulary formalises the definitions of shared terminology for the sake of clarity and reference. It may use skos:related and rdfs:seeAlso declarations to refer to related vocabularies. This vocabulary is to present a human-readable format and should not be used as a reference data resource. Therefore some rdf rules may not be strictly followed, such as allowing non-unique notations and having locally relevant hierachy that does not apply to the complete vocabulary.
    
    In some cases, skos:broader may be used to represent related concepts in display platforms, where relationships such as dcterms:isPartOf is a more accurate descriptor."""@en;
    skos:prefLabel "Engineers Australia Business Glossary"@en .

<https://linked.data.gov.au/org/engineersaustralia> a sdo:Organization ;
    sdo:name "Engineers Australia" ;
    sdo:url "https://www.engineersaustralia.org.au"^^xsd:anyURI .

<https://orcid.org/0000-0003-2309-7004> a sdo:Person,
        owl:NamedIndividual ;
    sdo:affiliation [ a sdo:Organization ;
            sdo:name "Engineers Australia" ;
            sdo:url "https://www.engineersaustralia.org.au"^^xsd:anyURI ] ;
    sdo:identifier <https://orcid.org/0000-0003-2309-7004> ;
    sdo:name "Vance Kelly" .

earegb:professional-conduct-committee a skos:Concept ;
    rdfs:seeAlso <https://ref.engineersaustralia.org.au/def/ea-regulated-bodies/professional-conduct-committee> ;
    rdfs:isDefinedBy <https://ref.engineersaustralia.org.au/def/ea-regulated-bodies/professional-conduct-committee> ;
    skos:inScheme <https://ref.engineersaustralia.org.au/def/ea-jargon> ;
    skos:topConceptOf <https://ref.engineersaustralia.org.au/def/ea-jargon> .

eaj:accords a skos:Concept ;
    dcterms:source "https://www.ieagreements.org/assets/Uploads/Documents/IEA-Extended-Glossary.pdf"^^xsd:anyURI ;
    rdfs:isDefinedBy <https://ref.engineersaustralia.org.au/def/ea-jargon> ;
    skos:inScheme <https://ref.engineersaustralia.org.au/def/ea-jargon> ;
    skos:topConceptOf <https://ref.engineersaustralia.org.au/def/ea-jargon> ;
    skos:definition """Is an agreement that provides benchmarking of educational standards and mutual recognition benefits to individuals who hold qualifications accredited by signatories."""@en ;
    skos:altLabel "Eductional Accords"@en,
        "Accords (Educational)"@en ;
    skos:prefLabel "Accords"@en .

    eaj:engineering-accords a skos:Concept ;
        dcterms:source "https://www.ieagreements.org/"^^xsd:anyURI ;
        rdfs:isDefinedBy <https://ref.engineersaustralia.org.au/def/ea-jargon> ;
        rdfs:seeAlso <https://linked.data.gov.au/def/iea-occupational-categories> ;
        skos:related <https://linked.data.gov.au/def/iea-occupational-categories> ;
        skos:inScheme <https://ref.engineersaustralia.org.au/def/ea-jargon> ;
        skos:broader eaj:accords ;
        skos:definition """The engineering accords are multi-lateral agreements between bodies responsible for accreditation or recognition of tertiary-level engineering qualifications within their jurisdictions who have chosen to work collectively to assist the mobility of engineers, technologists and associates. These accords define the criteria for the corresponding engineering occupational categories.
        
        The accords relate directly to occupational categories: The Dublin Accords (Engineering Associates), Sydney Accords (Engineering Technologists), Washington Accords (Professional Engineers)."""@en ;
        skos:prefLabel "International Engineering Accords"@en .

eaj:accreditation a skos:Concept ;
    dcterms:source "https://www.ieagreements.org/assets/Uploads/Documents/IEA-Extended-Glossary.pdf"^^xsd:anyURI ;
    rdfs:isDefinedBy <https://ref.engineersaustralia.org.au/def/ea-jargon> ;
    skos:inScheme <https://ref.engineersaustralia.org.au/def/ea-jargon> ;
    skos:topConceptOf <https://ref.engineersaustralia.org.au/def/ea-jargon> ;
    skos:definition """Accreditation is recognition given to a programme as meeting applicable criteria as a result of an evaluation process. 
    
    Engineers Australia, through its Australian Engineering Accreditation Centre, operates an accreditation system for engineering education programs offered by tertiary institutions. The process involves the review and accreditation of all Australian University level professional engineering and technologist courses. It is managed by the Education and Assessment Directorate at National Office. Engineers Australia is a founding signatory to the Washington Accord (1989) and the Sydney Accord (2001)."""@en ;
    skos:altLabel "Accreditation"@en ;
    skos:prefLabel "Accreditation of Engineering Programs"@en .

eaj:active-directory a skos:Concept ;
    dcterms:source "https://learn.microsoft.com/en-us/windows-server/identity/ad-ds/get-started/virtual-dc/active-directory-domain-services-overview"^^xsd:anyURI ;
    rdfs:isDefinedBy <https://ref.engineersaustralia.org.au/def/ea-jargon> ;
    skos:inScheme <https://ref.engineersaustralia.org.au/def/ea-jargon> ;
    skos:topConceptOf <https://ref.engineersaustralia.org.au/def/ea-jargon> ;
    skos:definition """Active Directory is a directory service that stores information about objects on the network and makes this information easy for administrators and users to find and use. Active Directory uses a structured data store as the basis for a logical, hierarchical organization of directory information. For example, Active Directory stores information about user accounts, such as names, passwords, phone numbers, and so on, and enables other authorized users on the same network to access this information."""@en ;
    skos:notation "AD" ;
    skos:prefLabel "Active Directory"@en .

earl:actor a skos:Concept ;
    skos:inScheme <https://ref.engineersaustralia.org.au/def/ea-jargon> ;
    skos:topConceptOf <https://ref.engineersaustralia.org.au/def/ea-jargon> .

eaj:agent a skos:Concept ;
    dcterms:source "https://linked.data.gov.au/org/engineersaustralia"^^xsd:anyURI ;
    rdfs:isDefinedBy <https://ref.engineersaustralia.org.au/def/ea-party> ;
    skos:inScheme <https://ref.engineersaustralia.org.au/def/ea-jargon> ;
    skos:topConceptOf <https://ref.engineersaustralia.org.au/def/ea-jargon> ;
    skos:definition """The types of agents who can interact with Engineers Australia to perform services as customers, staff, advisors, representatives etc. People and Organisations whose actions contribute to the operation of Engineers Australia."""@en ;
    skos:altLabel "Agents"@en,
        "Parties"@en,
        "Actors"@en,
        "Entity"@en,
        "Being"@en ;
    skos:prefLabel "Engineers Australia Agents"@en .

eaj:agile a skos:Concept ;
    dcterms:source "hhttps://www.atlassian.com/agile"^^xsd:anyURI ;
    rdfs:isDefinedBy <https://ref.engineersaustralia.org.au/def/ea-jargon> ;
    rdfs:seeAlso <https://www.agilealliance.org/agile101/agile-glossary/> ;
    skos:inScheme <https://ref.engineersaustralia.org.au/def/ea-jargon> ;
    skos:topConceptOf <https://ref.engineersaustralia.org.au/def/ea-jargon> ;
    skos:definition """The Agile methodology is a project management approach that involves breaking the project into phases and emphasizes continuous collaboration and improvement. Teams follow a cycle of planning, executing, and evaluating."""@en ;
    skos:altLabel "Agile Methodology"@en ;
    skos:prefLabel "Agile"@en .

eaj:anzsco a skos:Concept ;
    dcterms:source "https://www.abs.gov.au/statistics/classifications/anzsco-australian-and-new-zealand-standard-classification-occupations/latest-release#data-downloads"^^xsd:anyURI ;
    rdfs:isDefinedBy <https://ref.engineersaustralia.org.au/def/ea-jargon> ;
    skos:related <https://linked.data.gov.au/def/anzsco> ;
    skos:inScheme <https://ref.engineersaustralia.org.au/def/ea-jargon> ;
    skos:topConceptOf <https://ref.engineersaustralia.org.au/def/ea-jargon> ;
    skos:definition "The Australian and New Zealand Standard Classification of Occupations (ANZSCO) was jointly developed by the ABS, Stats NZ and the then Australian Government Department of Education, Employment and Workplace Relations. It provides a basis for the standardised collection, analysis and dissemination of occupation data for Australia and New Zealand."@en ;
    skos:altLabel "ANZSCO"@en ;
    skos:prefLabel "Australian and New Zealand Standard Classification of Occupations"@en .

    eaj:anzsco-main a skos:Concept ;
        dcterms:source "https://www.abs.gov.au/statistics/classifications/anzsco-australian-and-new-zealand-standard-classification-occupations/2022/classification-structure"^^xsd:anyURI ;
        rdfs:isDefinedBy <https://ref.engineersaustralia.org.au/def/ea-jargon> ;
        skos:related <https://linked.data.gov.au/def/anzsco/anzsco-aus-coder> ;
        skos:inScheme <https://ref.engineersaustralia.org.au/def/ea-jargon> ;
        skos:broader eaj:anzsco ;
        skos:definition "The Main Code from the Australian & New Zealand Standard Classification of Occupations, denoted with a six-digit code (notation), used in the ANZSCO Australian Coder."@en ;
        skos:altLabel "Australian and New Zealand Standard Classification of Occupations Main"@en ;
        skos:prefLabel "ANZSCO Main"@en .

    eaj:anzsco-specialistions a skos:Concept ;
        dcterms:source "https://www.abs.gov.au/statistics/classifications/anzsco-australian-and-new-zealand-standard-classification-occupations/2022/classification-structure"^^xsd:anyURI ;
        rdfs:isDefinedBy <https://ref.engineersaustralia.org.au/def/ea-jargon> ;
        skos:related <https://linked.data.gov.au/def/anzsco/anzsco-specialisations> ;
        skos:inScheme <https://ref.engineersaustralia.org.au/def/ea-jargon> ;
        skos:broader eaj:anzsco ;
        skos:definition "An ANZSCO Specialisation is a further level of occupational breakdown for a specific ANZSCO Main classification. The Specialisation titles are any commonly used titles which refer to a subset of jobs belonging to the occupation designated in the principal/parent title. These jobs involve the performance of specialised tasks rather than the broader range of tasks usually performed in the occupation."@en ;
        skos:altLabel "Australian and New Zealand Standard Classification of Occupations Specialisation"@en ;
        skos:prefLabel "ANZSCO Specialisation"@en .

earp:applicant a skos:Concept ;
    skos:inScheme <https://ref.engineersaustralia.org.au/def/ea-jargon> ;
    skos:topConceptOf <https://ref.engineersaustralia.org.au/def/ea-jargon> .

eaj:areas-of-practice a skos:Concept ;
    dcterms:source "https://ref.engineersaustralia.org.au/def/areasofpractice"^^xsd:anyURI ;
    rdfs:isDefinedBy <https://ref.engineersaustralia.org.au/def/areasofpractice> ;
    skos:related <https://ref.engineersaustralia.org.au/def/areasofpractice> ;
    skos:inScheme <https://ref.engineersaustralia.org.au/def/ea-jargon> ;
    skos:topConceptOf <https://ref.engineersaustralia.org.au/def/ea-jargon> ;
    skos:related <https://ref.engineersaustralia.org.au/def/areasofpractice/areas-of-practice-chartered>,
        <https://ref.engineersaustralia.org.au/def/areasofpractice/areas-of-practice-ner> ;
    skos:definition """Areas of Practice are the types of engineering undertaken by an individual or organisation, e.g. Civil, Chemical, Mechanical, Structural. Depending on the use case these may be referred to as Areas of Business, Areas of Engineering, or Areas of Practice and consist of variable subsets of the greater categorisation of Engineering types."""@en ;
    skos:notation "AOP" ;
    skos:altLabel "Areas of Business"@en,
        "Areas of Engineering"@en,
        "Branch of Engineering"@en ;
    skos:prefLabel "Areas of Practice"@en .

eaj:audit a skos:Concept ;
    dcterms:source "https://track.g2.com/resources/compliance-audits"^^xsd:anyURI ;
    rdfs:isDefinedBy <https://ref.engineersaustralia.org.au/def/ea-jargon> ;
    skos:inScheme <https://ref.engineersaustralia.org.au/def/ea-jargon> ;
    skos:topConceptOf <https://ref.engineersaustralia.org.au/def/ea-jargon> ;
    skos:definition """A formal review process that evaluates whether an organization is adhering to laws, regulations, policies, and industry standards relevant to its operations. It's conducted either by internal audit teams or by external auditors and ensures that the organization is operating in a legal and ethical manner. A means to provide assurance to the sponsor or board of a project that governance is effective and that the project is being managed as intended. 
    
    At Engineers Australia this may be applied to Chartered Status, Registration (National Engineering Register), Continuous Professional Development (CPD) or Complaints scenarios. Registered engineers and members with Chartered status may be audited for their compliance with the specific requirements that they practise in their area at least one full time year in every three, and that they maintain records of their continuing professional development activities. Compliance with these criteria is audited periodically. An audit notice requires respondents to submit a statement of experience and a CPD record sheet, which are reviewed by auditors. The audit program ensures members continue to have an adequate knowledge of both the theory and practice of engineering throughout their careers and so increases the confidence of the community in the employment of engineers."""@en ;
    skos:altLabel "Auditing Compliance"@en,
        "Compliance Audit"@en ;
    skos:prefLabel "Audit"@en .

    eaj:cpd-audit a skos:Concept ;
        dcterms:source "https://www.engineersaustralia.org.au/sites/default/files/resource-files/2020-02/EA%20General%20Regulations%205%20Dec%202019.pdf"^^xsd:anyURI ;
        rdfs:isDefinedBy <https://ref.engineersaustralia.org.au/def/ea-jargon> ;
        skos:inScheme <https://ref.engineersaustralia.org.au/def/ea-jargon> ;
        skos:broader eaj:audit ;
        skos:definition """An audit conducted under the CPD Policy and Procedure."""@en ;
        skos:prefLabel "CPD Audit"@en .

eaj:aus-privacy-act a skos:Concept ;
    dcterms:source "https://www.oaic.gov.au/privacy/the-privacy-act"^^xsd:anyURI ;
    rdfs:isDefinedBy <https://ref.engineersaustralia.org.au/def/ea-jargon> ;
    rdfs:seeAlso <https://www.oaic.gov.au/privacy/the-privacy-act> ;
    skos:inScheme <https://ref.engineersaustralia.org.au/def/ea-jargon> ;
    skos:topConceptOf <https://ref.engineersaustralia.org.au/def/ea-jargon> ;
    skos:related eaj:aus-privacy-principles ;
    skos:definition """The Privacy Act 1988 (Privacy Act) was introduced to promote and protect the privacy of individuals and to regulate how Australian Government agencies and organisations with an annual turnover of more than $3 million, and some other organisations, handle personal information.
    
    The Privacy Act includes 13 Australian Privacy Principles (APPs), which apply to some private sector organisations, as well as most Australian Government agencies. These are collectively referred to as 'APP entities'. The Privacy Act also regulates the privacy component of the consumer credit reporting system, tax file numbers, and health and medical research."""@en ;
    skos:notation "APA" ;
    skos:altLabel "The Privacy Act"@en,
        "Privacy Act"@en,
        "Privacy Act 1988"@en ;
    skos:prefLabel "Australian Privacy Act"@en .

eaj:aus-privacy-principles a skos:Concept ;
    dcterms:source "https://www.oaic.gov.au/privacy/australian-privacy-principles"^^xsd:anyURI ;
    rdfs:isDefinedBy <https://ref.engineersaustralia.org.au/def/ea-jargon> ;
    rdfs:seeAlso <https://www.oaic.gov.au/privacy/australian-privacy-principles> ;
    skos:inScheme <https://ref.engineersaustralia.org.au/def/ea-jargon> ;
    skos:topConceptOf <https://ref.engineersaustralia.org.au/def/ea-jargon> ;
    skos:related eaj:aus-privacy-act ;
    skos:definition """The Australian Privacy Principles (or APPs) are the cornerstone of the privacy protection framework in the Privacy Act 1988 (Privacy Act). They apply to any organisation or agency the Privacy Act covers.

    There are 13 Australian Privacy Principles and they govern standards, rights and obligations around:
    - the collection, use and disclosure of personal information
    - an organisation or agency's governance and accountability
    - integrity and correction of personal information
    - the rights of individuals to access their personal information
    The Australian Privacy Principles are principles-based law. This gives an organisation or agency flexibility to tailor their personal information handling practices to their business models and the diverse needs of individuals. They are also technology neutral, which allows them to adapt to changing technologies.
    
    A breach of an Australian Privacy Principle is an 'interference with the privacy of an individual' and can lead to regulatory action and penalties."""@en ;
    skos:notation "APP" ;
    skos:altLabel "APPs"@en ;
    skos:prefLabel "Australian Privacy Principles"@en .

eaj:awareness a skos:Concept ;
    dcterms:source "https://www.ieagreements.org/assets/Uploads/Documents/IEA-Extended-Glossary.pdf"^^xsd:anyURI ;
    rdfs:isDefinedBy <https://ref.engineersaustralia.org.au/def/ea-jargon> ;
    skos:inScheme <https://ref.engineersaustralia.org.au/def/ea-jargon> ;
    skos:topConceptOf <https://ref.engineersaustralia.org.au/def/ea-jargon> ;
    skos:definition """In general, knowledge being conscious; cognizant, informed alert; specifically in engineering context; being alert to identify conditions or situations that require action."""@en ;
    skos:prefLabel "Awareness"@en .

eaj:bcm a skos:Concept ;
    dcterms:source "https://en.wikipedia.org/wiki/Business_capability_model"^^xsd:anyURI ;
    rdfs:isDefinedBy <https://ref.engineersaustralia.org.au/def/ea-jargon> ;
    skos:inScheme <https://ref.engineersaustralia.org.au/def/ea-jargon> ;
    skos:topConceptOf <https://ref.engineersaustralia.org.au/def/ea-jargon> ;
    skos:definition """A business capability model or business capability map (BCM) provides structured graphical representations of all organisational business capabilities, their relationships and hierarchy. They describe what an organsation can do. They are largely independent of specific organisational structures, reporting relationships, and cultural aspects of individual business leaders, current initiatives and projects."""@en ;
    skos:notation "BCM" ;
    skos:altLabel "Business Capability Map"@en,
        "Business Capability Model"@en ;
    skos:prefLabel "Business Capability Matrix"@en .

eaj:bcp a skos:Concept ;
    dcterms:source "https://www.techtarget.com/searchdisasterrecovery/definition/business-continuity-action-plan"^^xsd:anyURI ;
    rdfs:isDefinedBy <https://ref.engineersaustralia.org.au/def/ea-jargon> ;
    skos:inScheme <https://ref.engineersaustralia.org.au/def/ea-jargon> ;
    skos:topConceptOf <https://ref.engineersaustralia.org.au/def/ea-jargon> ;
    skos:definition """A Business Continuity Plan is a document that explains the actions you should take before, during and after unexpected events and situations."""@en ;
    skos:notation "BCP" ;
    skos:altLabel "Business Continuity Action Plan"@en,
        "Business Continuity Planning"@en ;
    skos:prefLabel "Business Continuity Plan"@en .

eaj:benchmarking a skos:Concept ;
    dcterms:source "https://www.apqc.org/blog/what-are-four-types-benchmarking"^^xsd:anyURI ;
    rdfs:isDefinedBy <https://ref.engineersaustralia.org.au/def/ea-jargon> ;
    skos:inScheme <https://ref.engineersaustralia.org.au/def/ea-jargon> ;
    skos:topConceptOf <https://ref.engineersaustralia.org.au/def/ea-jargon> ;
    skos:definition """Benchmarking is the process of measuring key business metrics and practices and comparing them within business areas or against a competitor, industry peers and partners, or other companies around the world. Benchmarking may provides an understanding of how and where an organisation needs to change in order to improve performance, or how an organisation can align with partner organisations with shared standards and mutal recognition agreements."""@en ;
    skos:prefLabel "Benchmarking"@en .

eaj:bi-platform a skos:Concept ;
    dcterms:source "https://azure.microsoft.com/en-us/overview/what-are-business-intelligence-tools/"^^xsd:anyURI ;
    rdfs:isDefinedBy <https://ref.engineersaustralia.org.au/def/ea-jargon> ;
    skos:inScheme <https://ref.engineersaustralia.org.au/def/ea-jargon> ;
    skos:topConceptOf <https://ref.engineersaustralia.org.au/def/ea-jargon> ;
    skos:definition """Business intelligence (BI) tools are types of application software that collect and process large amounts of unstructured data from internal and external systems, including books, journals, documents, health records, images, files, email, video, and other business sources.
    
    Business inteliigence tools commonly derive data via a data warehouse that consolidate data through a set of data views or semantic layers to transform raw data into prepared consumable information without the need to materialise duplicated tables and data.
    
    Popular BI Tools include Microsoft Power BI, Tableau, Oracle Business Intelligence, IBM Cognos Analytics."""@en ;
    skos:altLabel "BI Tool"@en ;
    skos:prefLabel "Business Intelligence Tool"@en .

eaj:business-capability a skos:Concept ;
    dcterms:source "https://www.opengroup.org/togaf-standard-version-92-overview"^^xsd:anyURI ;
    rdfs:isDefinedBy <https://ref.engineersaustralia.org.au/def/ea-jargon> ;
    skos:inScheme <https://ref.engineersaustralia.org.au/def/ea-jargon> ;
    skos:topConceptOf <https://ref.engineersaustralia.org.au/def/ea-jargon> ;
    skos:scopeNote "Capabilties describe what a business does, or can do. Processes describe how capabilities are achieved. Tasks describe the individual activities that consitute a process."@en ;
    skos:definition """A business capability is a particular ability that a business may possess or exchange to achieve a specific purpose."""@en ;
    skos:prefLabel "Business Capability"@en . 

eaj:business-process a skos:Concept ;
    dcterms:source "https://www.bpmn.org/"^^xsd:anyURI ;
    rdfs:isDefinedBy <https://ref.engineersaustralia.org.au/def/ea-jargon> ;
    skos:inScheme <https://ref.engineersaustralia.org.au/def/ea-jargon> ;
    skos:topConceptOf <https://ref.engineersaustralia.org.au/def/ea-jargon> ;
    skos:scopeNote "Capabilties describe what a business does, or can do. Processes describe how capabilities are achieved. Tasks describe the individual activities that consitute a process."@en ;
    skos:definition """A business process, is a series of related tasks that result in a desired output; it is an established set of repeatable activities. A Process describes a sequence or flow of Activities in an organization with the objective of carrying out work."""@en ;
    skos:prefLabel "Business Process"@en . 

eaj:business-process-reengineering a skos:Concept ;
    dcterms:source "https://www.ibm.com/think/topics/business-process-reengineering"^^xsd:anyURI ;
    rdfs:isDefinedBy <https://ref.engineersaustralia.org.au/def/ea-jargon> ;
    rdfs:seeAlso eaj:business-process ;
    skos:inScheme <https://ref.engineersaustralia.org.au/def/ea-jargon> ;
    skos:topConceptOf <https://ref.engineersaustralia.org.au/def/ea-jargon> ;
    skos:definition """Business process reengineering (BPR) is the radical redesign of business processes to achieve dramatic improvements in performance, efficiency, and effectiveness."""@en ;
    skos:altLabel "BPR"@en,
        "Business Process Reengineering"@en ;
    skos:prefLabel "Business Process Re-engineering"@en . 

eaj:business-task a skos:Concept ;
    dcterms:source "https://www.bpmn.org/"^^xsd:anyURI ;
    rdfs:isDefinedBy <https://ref.engineersaustralia.org.au/def/ea-jargon> ;
    skos:inScheme <https://ref.engineersaustralia.org.au/def/ea-jargon> ;
    skos:topConceptOf <https://ref.engineersaustralia.org.au/def/ea-jargon> ;
    skos:scopeNote "Capabilties describe what a business does, or can do. Processes describe how capabilities are achieved. Tasks describe the individual activities that consitute a process."@en ;
    skos:definition """A task is a single discrete activity in a process. Tasks are atomic activities within a flow. A Task is used when the work in the Process cannot be broken down to a finer level of detail. Generally, an end-user and/or applications are used to perform the Task when it is executed."""@en ;
    skos:altLabel "Task"@en ;
    skos:prefLabel "Business Task"@en . 

eaj:career-engineer a skos:Concept ;
    dcterms:source "https://linked.data.gov.au/org/engineersaustralia"^^xsd:anyURI ;
    rdfs:isDefinedBy <https://ref.engineersaustralia.org.au/def/ea-jargon> ;
    skos:inScheme <https://ref.engineersaustralia.org.au/def/ea-jargon> ;
    skos:topConceptOf <https://ref.engineersaustralia.org.au/def/ea-jargon> ;
    skos:definition """An individual that has been a contact of Engineers Australia through Stage 1 Competency, Stage 2/Chartered Assessments, MSA. Career engineers are not necessarily members. The formal record including the relevant occupational category is known as the Career Engineer history."""@en ;
    skos:prefLabel "Career Engineer"@en . 

eaj:change-management a skos:Concept ;
    dcterms:source "https://www.apm.org.uk/resources/what-is-project-management/what-is-change-management/"^^xsd:anyURI ;
    dcterms:references 
        <https://www.apm.org.uk/resources/what-is-project-management/what-is-change-management/>,
        <https://www.iso.org/obp/ui/fr/#iso:std:iso:9000:ed-4:v1:en>,
        <https://www.ieagreements.org/assets/Uploads/Documents/IEA-Extended-Glossary.pdf> ;
    rdfs:isDefinedBy <https://ref.engineersaustralia.org.au/def/ea-jargon> ;
    skos:inScheme <https://ref.engineersaustralia.org.au/def/ea-jargon> ;
    skos:topConceptOf <https://ref.engineersaustralia.org.au/def/ea-jargon> ;
    skos:definition """The overarching structured approach taken to move from a current state to a desirable future in collaboration with stakeholders by individuals, teams, technologies and organizations.
    
    This includes preparing and supporting employees, establishing the necessary steps for change, risks and impact assessments, and monitoring pre-change and post-change activities to ensure successful implementation."""@en ;
    skos:scopeNote """In the context of	ICT, Change Management is a set of processes and procedures within the ITIL framework that provides a systematic approach for managing changes to IT systems, services, and infrastructure."""@en ;
    skos:notation "CM" ;
    skos:altLabel "Organisational Change Management"@en ;
    skos:prefLabel "Change Management"@en . 

eaj:chartered a skos:Concept ;
    dcterms:source "https://dictionary.cambridge.org/dictionary/english/chartered"^^xsd:anyURI ;
	rdfs:isDefinedBy <https://ref.engineersaustralia.org.au/def/ea-jargon>;
    rdfs:seeAlso <https://ref.engineersaustralia.org.au/def/ea-engineering-credentials/chartered> ;
    skos:inScheme <https://ref.engineersaustralia.org.au/def/ea-jargon> ;
    skos:topConceptOf <https://ref.engineersaustralia.org.au/def/ea-jargon> ;
	skos:definition """Chartered refers to people who do particular jobs having successfully finished the necessary training and exams. Chartered titles are commonly confered by an authorising professional organisation."""@en;
    skos:scopeNote "Within a professional organisation, Chartered commonly refers specifically to the Chartered title conferred to members of the profession to which its assessments apply."@en ;
    skos:prefLabel "Chartered"@en .

eaj:content-management-system a skos:Concept ;
    dcterms:source "https://www.techtarget.com/searchcontentmanagement/definition/content-management-system-CMS"^^xsd:anyURI ;
    rdfs:isDefinedBy <https://ref.engineersaustralia.org.au/def/ea-jargon> ;
    skos:inScheme <https://ref.engineersaustralia.org.au/def/ea-jargon> ;
    skos:topConceptOf <https://ref.engineersaustralia.org.au/def/ea-jargon> ;
    skos:altLabel "Content Management System (CMS)"@en,
        "CMS"@en ;
    skos:definition """A content management system (CMS) is a software application that enables users to create, edit, collaborate on, publish and store digital content."""@en ;
    skos:notation "CMS" ;
    skos:prefLabel "Content Management System"@en .

eaj:code-of-ethics a skos:Concept ;
    dcterms:source "https://www.engineersaustralia.org.au/publications/code-ethics"^^xsd:anyURI ;
    rdfs:isDefinedBy <https://ref.engineersaustralia.org.au/def/ea-jargon> ;
    rdfs:seeAlso <https://www.engineersaustralia.org.au/publications/code-ethics> ;
    skos:inScheme <https://ref.engineersaustralia.org.au/def/ea-jargon> ;
    skos:topConceptOf <https://ref.engineersaustralia.org.au/def/ea-jargon> ;
    skos:definition """The Code of Ethics and Guidelines on Professional Conduct defines the values and principles that shape the decisions made, and provides a framework for members of Engineers Australia to use when exercising their judgment, in engineering practice and as members of Engineers Australia. The Cardinal Principles of the Code of Ethics are:
    - to respect the inherent dignity of the individual
    - to act on the basis of a well informed conscience, and
    - to act in the interest of the community.
    These principles are encapsulated within and established by the Tenets of the Code of Ethics."""@en ;
    skos:altLabel "The Code of Ethics and Guidelines on Professional Conduct"@en ;
    skos:prefLabel "Code of Ethics"@en .

    eaj:demonstrate-integrity a skos:Concept ;
        dcterms:source "https://www.engineersaustralia.org.au/sites/default/files/2022-08/code-ethics-guidelines-professional-conduct-2022.pdf"^^xsd:anyURI ;
        rdfs:isDefinedBy <https://ref.engineersaustralia.org.au/def/ea-jargon> ;
        skos:inScheme <https://ref.engineersaustralia.org.au/def/ea-jargon> ;
        skos:broader eaj:code-of-ethics ;
        skos:definition """Demonstrate Interity means:
        1.1 Act on the basis of a well-informed conscience. 
            a. be discerning and do what you think is right, 
            b. act impartially and objectively, 
            c. act appropriately, and in a professional manner, when you perceive something to be wrong, 
            d. give due weight to all legal, contractual and employment obligations, 
            e. act within your area of expertise ; 
        1.2 Be honest and trustworthy. 
            a. accept, as well as give, honest and fair criticism, 
            b. be prepared to explain your work and reasoning, 
            c. give proper credit to those to whom proper credit is due, 
            d. in managing perceived conflicts of interest, ensure that those conflicts are disclosed to relevant parties, 
            e. respect confidentiality obligations, express or implied, 
            f. do not engage in fraudulent, corrupt, or criminal conduct ; 
        1.3 Respect the dignity of all persons. 
            a. treat others with courtesy and without discrimination or harassment, 
            b. apply knowledge and skills without bias in respect of race, religion, gender, age, sexual orientation, marital or family status, national origin, or mental or physical abilities."""@en ;
        skos:altLabel "Integrity"@en ;
        skos:prefLabel "Demonstrate Integrity"@en .
    
    eaj:practise-competently a skos:Concept ;
        dcterms:source "https://www.engineersaustralia.org.au/sites/default/files/2022-08/code-ethics-guidelines-professional-conduct-2022.pdf"^^xsd:anyURI ;
        rdfs:seeAlso <https://ref.engineersaustralia.org.au/def/ea-engineering-competency/stage-2-1-2> ;
        rdfs:isDefinedBy <https://ref.engineersaustralia.org.au/def/ea-jargon> ;
        skos:inScheme <https://ref.engineersaustralia.org.au/def/ea-jargon> ;
        skos:broader eaj:code-of-ethics ;
        skos:definition """Practise Competently means:
        2.1 Maintain and develop knowledge and skills.
            a. continue to develop relevant knowledge and expertise, 
            b. act in a careful and diligent manner, 
            c. seek peer review, 
            d. support the ongoing development of others, 
            e. maintain continuing professional development ; 
        2.2 Represent areas of competence objectively. 
            a. practise within areas of competence,
            b. neither falsify nor misrepresent qualifications, grades of membership, experience or prior responsibilities ; 
        2.3 Act on the basis of adequate knowledge. 
            a. practise in accordance with legal and statutory requirements, and with the standards of the day accepted within the Engineers Australia community, 
            b. inform employers or clients if a task requires qualifications and experience outside your areas of competence."""@en ;
        skos:altLabel "Competent"@en ;
        skos:prefLabel "Practise Competently"@en .

    eaj:exercise-leadership a skos:Concept ;
        dcterms:source "https://www.engineersaustralia.org.au/sites/default/files/2022-08/code-ethics-guidelines-professional-conduct-2022.pdf"^^xsd:anyURI ;
        rdfs:seeAlso <https://ref.engineersaustralia.org.au/def/ea-engineering-competency/stage-3-1> ;
        rdfs:isDefinedBy <https://ref.engineersaustralia.org.au/def/ea-jargon> ;
        skos:inScheme <https://ref.engineersaustralia.org.au/def/ea-jargon> ;
        skos:broader eaj:code-of-ethics ;
        skos:definition """Exercise Leadership means:
        3.1 Uphold the reputation and trustworthiness of the practice of engineering. 
            a. advocate and support the extension of ethical practice, 
            b. engage responsibly in public debate and deliberation ; 
        3.2 Support and encourage diversity. 
            a. select, and provide opportunities for, all engineering practitioners and other team members on the basis of merit, 
            b. promote diversity in engineering ; 
        3.3 Make reasonable efforts to communicate honestly and effectively to all stakeholders, taking into account the reliance of others on engineering expertise. 
            a. provide clear and timely communications on issues such as engineering services, costs, outcomes and risks."""@en ;
        skos:altLabel "Leadership"@en ;
        skos:prefLabel "Exercise Leadership"@en .

    eaj:promote-sustainability a skos:Concept ;
        dcterms:source "https://www.engineersaustralia.org.au/sites/default/files/2022-08/code-ethics-guidelines-professional-conduct-2022.pdf"^^xsd:anyURI ;
        rdfs:isDefinedBy <https://ref.engineersaustralia.org.au/def/ea-jargon> ;
        skos:inScheme <https://ref.engineersaustralia.org.au/def/ea-jargon> ;
        skos:broader eaj:code-of-ethics ;
        skos:definition """Promote Sustainability means:
        4.1 Engage responsibly with the community and other stakeholders. 
            a. be sensitive to public concerns 
            b. inform employers or clients of the likely consequences of proposed activities on the community and the environment, 
            c. promote the involvement of all stakeholders and the community in decisions and processes that may impact upon them and the environment ; 
        4.2 Practise engineering to foster the health, safety and wellbeing of the community and the environment. 
            a. incorporate social, cultural, health, safety, environmental and economic considerations into the engineering task ;
        4.3 Balance the needs of the present with the needs of future generations. 
            a. in identifying sustainable outcomes consider all options in terms of their economic, environmental and social consequences, 
            b. aim to deliver outcomes that do not compromise the ability of future life to enjoy the same or better environment, health, wellbeing and safety as currently enjoyed."""@en ;
        skos:altLabel "Sustainability"@en ;
        skos:prefLabel "Promote Sustainability"@en .

eaj:competence a skos:Concept ;
    dcterms:source "https://www.ieagreements.org/assets/Uploads/Documents/IEA-Extended-Glossary.pdf"^^xsd:anyURI ;
    rdfs:isDefinedBy <https://ref.engineersaustralia.org.au/def/ea-jargon> ;
    skos:related <https://ref.engineersaustralia.org.au/def/ea-engineering-competency> ;
    skos:inScheme <https://ref.engineersaustralia.org.au/def/ea-jargon> ;
    skos:topConceptOf <https://ref.engineersaustralia.org.au/def/ea-jargon>;
    skos:definition """The state of having the attributes necessary to perform the activities within the profession or occupation to the standards expected in independent employment or practice."""@en ;
    skos:prefLabel "Competence"@en .

eaj:competency-standard a skos:Concept ;
    dcterms:source "https://www.ieagreements.org/assets/Uploads/Documents/IEA-Extended-Glossary.pdf"^^xsd:anyURI ;
    rdfs:isDefinedBy <https://ref.engineersaustralia.org.au/def/ea-jargon> ;
    rdfs:seeAlso <https://ref.engineersaustralia.org.au/def/ea-engineering-competency> ;
    skos:inScheme <https://ref.engineersaustralia.org.au/def/ea-jargon> ;
    skos:topConceptOf <https://ref.engineersaustralia.org.au/def/ea-jargon>;
    skos:definition """A statement of competence required for a defined purpose."""@en ;
    skos:scopeNote """At Engineers Australia, competency standard typically refers to the Australian Engineering Competency Standards"""@en ;
    skos:prefLabel "Competency Standard"@en .

    eaj:prof-standard a skos:Concept ;
        dcterms:source "https://www.engineersaustralia.org.au/sites/default/files/2023-08/professional-standards-framework-v1-2023.pdf"^^xsd:anyURI ;
        rdfs:isDefinedBy <https://ref.engineersaustralia.org.au/def/ea-jargon> ;
        rdfs:seeAlso <https://ref.engineersaustralia.org.au/def/ea-engineering-competency> ;
        skos:inScheme <https://ref.engineersaustralia.org.au/def/ea-jargon> ;
        skos:broader eaj:competency-standard ;
        skos:definition """A professional standard is the integrated system of policies, processes and resources that guide and support a specific occupational group to practice ethically and competently and to contribute high value to their profession. It applies throughout their careers from pre-qualification (student) through to advanced practice and executive management and leadership. """@en ;
        skos:scopeNote """At Engineers Australia, competency standards and professional standards typically refer to the Australian Engineering Competency Standards"""@en ;
        skos:prefLabel "Professional Standards"@en .

        eaj:aecs a skos:Concept ;
            dcterms:source "https://linked.data.gov.au/org/engineersaustralia"^^xsd:anyURI ;
            rdfs:isDefinedBy <https://ref.engineersaustralia.org.au/def/ea-engineering-competency> ;
            rdfs:seeAlso <https://ref.engineersaustralia.org.au/def/ea-engineering-competency> ;
            skos:inScheme <https://ref.engineersaustralia.org.au/def/ea-jargon> ;
            skos:broader eaj:competency-standard;
            skos:definition """Commencing in 1992, Engineers Australia has progressively developed and used the Australian Engineering Competency Standards. These standards are regularly reviewed to ensure that they reflect government, employer and community expectations of members when they engage their services. There were revisions in 1998 and 2003. The Australian Engineering Competency Standards are in three distinct Stages, which correlate with the progression of a person's engineering career. These progress from Stage 1 members eligible for graduate level, Stage 2 Chartered Engineers, and Stage 3 Engineering Executives (EngExec)."""@en ;
            skos:notation "AECS" ;
            skos:altLabel "Engineering Competency"@en ;
            skos:prefLabel "Australian Engineering Competency Standards"@en .

eaj:consequence a skos:Concept ;
    dcterms:source "https://www.iso.org/standard/65694.html"^^xsd:anyURI ;
	rdfs:isDefinedBy <https://linked.data.gov.au/def/event-consequence>;
    rdfs:seeAlso <https://linked.data.gov.au/def/event-consequence> ;
    skos:inScheme <https://ref.engineersaustralia.org.au/def/ea-jargon> ;
    skos:topConceptOf <https://ref.engineersaustralia.org.au/def/ea-jargon> ;
	skos:definition """Outcome of an event affecting objectives.
    Note 1: A consequence can be certain or uncertain and can have positive or negative direct or indirect effects on objectives.
    Note 2: Consequences can be expressed qualitatively or quantitatively.
    Note 3: Any consequence can escalate through cascading and cumulative effects."""@en;
    skos:prefLabel "Consequence"@en .

eaj:continuous-monitoring a skos:Concept ;
    dcterms:source "https://www.crowdstrike.com/cybersecurity-101/observability/continuous-monitoring/"^^xsd:anyURI ;
    rdfs:isDefinedBy <https://ref.engineersaustralia.org.au/def/ea-jargon> ;
    skos:inScheme <https://ref.engineersaustralia.org.au/def/ea-jargon> ;
    skos:topConceptOf <https://ref.engineersaustralia.org.au/def/ea-jargon> ;
    skos:definition """Continuous monitoring is an approach where an organization constantly monitors its IT systems and networks to detect security threats, performance issues, or non-compliance problems in an automated manner. The goal is to identify potential problems and threats in real time to address them quickly."""@en ;
    skos:notation "CM" ;
    skos:altLabel "Continuous Monitoring and Logging"@en ;
    skos:prefLabel "Continuous Monitoring"@en .

eaj:continuing-professional-development a skos:Concept ;
    dcterms:source "https://www.engineersaustralia.org.au/membership/cpd-requirements"^^xsd:anyURI ;
    dcterms:references <https://www.engineersaustralia.org.au/membership/cpd-requirements>,
        <https://www.ieagreements.org/assets/Uploads/Documents/IEA-Extended-Glossary.pdf> ;
    rdfs:isDefinedBy <https://ref.engineersaustralia.org.au/def/ea-jargon> ;
    skos:inScheme <https://ref.engineersaustralia.org.au/def/ea-jargon> ;
    skos:topConceptOf <https://ref.engineersaustralia.org.au/def/ea-jargon> ;
    skos:definition """Continuing professional development or CPD, is imperative to ensuring the knowledge and technical skills of an engineer are optimised and up-to-date. CPD is the systematic, accountable maintenance, improvement and broadening of knowledge and skills, and the development of personal qualities necessary for the execution of professional and technical duties throughout an engineering practitioner's career.

    Continuing professional development is undertaken by engineering practitioners for the purposes of developing or maintaining the currency of the skills and knowledge necessary for ongoing competent engineering practice.
    
    Maintaining CPD requirements also ensures Engineers Australia Chartered or NER credentials stay valid.
    
    CPD is any sort of training or learning that helps to expand knowledge, maintain technical skills and progress the career of an engineer. Good CPD should facilitate:
    - maintainance of technical competence
    - retention and enhancement of workplace effectiveness
    - development of good leadership and mentoring skills
    - successful navigation of career challenges
    - better service to the community.
    
    For engineers wishing to retain their Chartered or Engineering Executive Status there is an obligation to achieve a minimum of 150 hours of structured CPD over a three-year period. Of the recommended 150 hours in three years: A proportion of CPD should relate to one's area of practice (a minimum of 50 hours in the three-year period is recommended. There are some limits on the number of hours you can claim for certain types of CPD. Please refer to the Engineers Australia Website for more detailed CPD policy information and the latest guidelines."""@en ;
    skos:notation "CPD" ;
    skos:altLabel "Continuing Professional Development (CPD)"@en,
        "Continuous Professional Development (CPD)"@en,
        "Continuous Professional Development"@en ;
    skos:prefLabel "Continuing Professional Development"@en . 

    eaj:continuing-education a skos:Concept ;
        dcterms:source "https://linked.data.gov.au/org/engineersaustralia"^^xsd:anyURI ;
        rdfs:isDefinedBy <https://ref.engineersaustralia.org.au/def/ea-jargon> ;
        skos:inScheme <https://ref.engineersaustralia.org.au/def/ea-jargon> ;
        skos:broader eaj:continuing-professional-development ;
        skos:definition """All practising Chartered members are required to continue their professional development throughout their careers. This includes undertaking at least 150 hours of acceptable Continuing Education in the past three years, and recorded in a log or diary. Use of the term Continuing Education (CE) is rare. The term Continuing Professional Development (CPD) is widely used to refer to both experiential development and Continuing Education."""@en ;
        skos:notation "CE" ;
        skos:prefLabel "Continuing Education"@en . 

    eaj:cpd-requirements a skos:Concept ;
        dcterms:source "https://www.engineersaustralia.org.au/sites/default/files/resource-files/2020-02/EA%20General%20Regulations%205%20Dec%202019.pdf"^^xsd:anyURI ;
        rdfs:isDefinedBy <https://ref.engineersaustralia.org.au/def/ea-jargon> ;
        skos:inScheme <https://ref.engineersaustralia.org.au/def/ea-jargon> ;
        skos:broader eaj:continuing-professional-development ;
        skos:definition """The requirements of the CPD Policy and Procedure as they apply in relation to the member."""@en ;
        skos:prefLabel "CPD Requirements"@en . 

eaj:control a skos:Concept ;
    dcterms:source "https://www.iso.org/standard/65694.html"^^xsd:anyURI ;
	rdfs:isDefinedBy <https://ref.engineersaustralia.org.au/def/ea-jargon>;
	rdfs:seeAlso <https://linked.data.gov.au/def/control-effectiveness> ;
    skos:inScheme <https://ref.engineersaustralia.org.au/def/ea-jargon> ;
    skos:topConceptOf <https://ref.engineersaustralia.org.au/def/ea-jargon> ;
	skos:definition """A measure that maintains and/or modifies risk
    Note 1: Controls include, but are not limited to, any process, policy, device, practice, or other conditions and/or actions which maintain and/or modify risk.
    Note 2: Controls may not always exert the intended or assumed modifying effect.
    Controls are already in place and help to:
    - limit the frequency or likelihood of a risk event occurring (preventative controls), and/or 
    - limit the potential impacts or consequences associated with a risk event should it occur (detective post-event controls)."""@en;
    skos:prefLabel "Control"@en .

eaj:control-owner a skos:Concept ;
    dcterms:source "https://www.iso.org/standard/65694.html"^^xsd:anyURI ;
	rdfs:isDefinedBy <https://ref.engineersaustralia.org.au/def/ea-jargon>;
    skos:inScheme <https://ref.engineersaustralia.org.au/def/ea-jargon> ;
    skos:topConceptOf <https://ref.engineersaustralia.org.au/def/ea-jargon> ;
	skos:definition """The person assigned responsibility for designing and implementing a specific risk control."""@en;
    skos:prefLabel "Control Owner"@en .

eaj:country-education-profiles a skos:Concept ;
    dcterms:source "https://internationaleducation.gov.au/services-and-resources/services-for-organisations/Pages/Services-for-organisations.aspx"^^xsd:anyURI ;
    rdfs:isDefinedBy <https://ref.engineersaustralia.org.au/def/ea-jargon> ;
    skos:inScheme <https://ref.engineersaustralia.org.au/def/ea-jargon> ;
    skos:topConceptOf <https://ref.engineersaustralia.org.au/def/ea-jargon> ;
    skos:definition """The Country Education Profiles (CEPs) is an online qualifications recognition tool designed to help organisations understand overseas higher education and postsecondary technical and vocational educational qualifications. It can be used by universities and other education providers, professional bodies, employers, international organisations and governments to help understand the level of an overseas qualification."""@en ;
    skos:notation "CEP" ;
    skos:prefLabel "Country Education Profiles"@en . 

eaj:credentials a skos:Concept ;
    dcterms:source "https://dictionary.cambridge.org/dictionary/english/credential"^^xsd:anyURI ;
    dcterms:references <https://dictionary.cambridge.org/dictionary/english/credential>,
        <https://www.engineersaustralia.org.au/credentials> ;
    rdfs:isDefinedBy <https://ref.engineersaustralia.org.au/def/ea-jargon> ;
    rdfs:seeAlso <https://ref.engineersaustralia.org.au/def/ea-engineering-credentials> ;
    skos:inScheme <https://ref.engineersaustralia.org.au/def/ea-jargon> ;
    skos:topConceptOf <https://ref.engineersaustralia.org.au/def/ea-jargon> ;
    skos:definition """The abilities and experience that make someone suitable for a particular job or activity, or proof of someone's abilities and experience. Evidence of an individuals credentials is commonly recorded in the form of certification, documention, and formally administered lists and registers by authoritative organisations."""@en ;
    skos:scopeNote """At Engineers Australia, credentials refers specifically to the formally administered lists and registers of credentials describing the experience of professional Engineers such as The National Engineering Register, Chartered, and EngExec."""@en ;
    skos:prefLabel "Credentials"@en .

eaj:crm a skos:Concept ;
    dcterms:source "https://www.salesforce.com/au/crm/what-is-crm/"^^xsd:anyURI ;
    rdfs:isDefinedBy <https://ref.engineersaustralia.org.au/def/ea-jargon> ;
    skos:inScheme <https://ref.engineersaustralia.org.au/def/ea-jargon> ;
    skos:topConceptOf <https://ref.engineersaustralia.org.au/def/ea-jargon> ;
    skos:definition """Customer relationship management (CRM) is a technology for managing all the relationships and interactions with customers and potential customers for a company. The goal is to improve business relationships. A CRM system helps companies stay connected to customers, streamline processes, and improve profitability."""@en ;
    skos:notation "CRM" ;
    skos:altLabel "Customer Relationship Management (CRM)"@en,
        "CRM"@en ;
    skos:prefLabel "Customer Relationship Management"@en .

earp:customer a skos:Concept ;
    skos:inScheme <https://ref.engineersaustralia.org.au/def/ea-jargon> ;
    skos:topConceptOf <https://ref.engineersaustralia.org.au/def/ea-jargon> .

eaj:data a skos:Concept ;
    dcterms:source "https://www.diffen.com/difference/Data_vs_Information"^^xsd:anyURI ;
    rdfs:isDefinedBy <https://ref.engineersaustralia.org.au/def/ea-jargon> ;
    skos:inScheme <https://ref.engineersaustralia.org.au/def/ea-jargon> ;
    skos:topConceptOf <https://ref.engineersaustralia.org.au/def/ea-jargon> ;
    skos:definition """Data is raw, unorganized facts that need to be processed. Data can be something simple and seemingly random and useless until it is organized."""@en ;
    skos:prefLabel "Data"@en .

    eaj:ref-data a skos:Concept ;
        dcterms:source "https://datamc.com/understanding-master-transactional-reference-data/"^^xsd:anyURI ;
        rdfs:isDefinedBy <https://ref.engineersaustralia.org.au/def/ea-jargon> ;
        skos:inScheme <https://ref.engineersaustralia.org.au/def/ea-jargon> ;
        skos:broader eaj:data;
        skos:definition """Reference Data is a type of data that is used to categorize or classify other data elements. It is data that describes other data, i.e. metadata. It consists of a set of values or codes that are used to identify, describe, or define data elements in a particular domain or context. For example, a list of country codes that are used to identify the country of origin for a product, and grades of membership in an organisation."""@en ;
        skos:prefLabel "Reference Data"@en .

    eaj:transactional-data a skos:Concept ;
        dcterms:source "https://datamc.com/understanding-master-transactional-reference-data/"^^xsd:anyURI ;
        rdfs:isDefinedBy <https://ref.engineersaustralia.org.au/def/ea-jargon> ;
        skos:inScheme <https://ref.engineersaustralia.org.au/def/ea-jargon> ;
        skos:broader eaj:data ;
        skos:definition """Transactional Data is a type of data that records specific events or transactions that occur within an organization. It refers to the data that is generated as part of day-to-day business operations, such as sales, purchases, invoices, and payments."""@en ;
        skos:prefLabel "Transactional Data"@en .

    eaj:master-data a skos:Concept ;
        dcterms:source "https://datamc.com/understanding-master-transactional-reference-data/"^^xsd:anyURI ;
        rdfs:isDefinedBy <https://ref.engineersaustralia.org.au/def/ea-jargon> ;
        skos:inScheme <https://ref.engineersaustralia.org.au/def/ea-jargon> ;
        skos:broader eaj:data ;
        skos:definition """Master Data refers to a set of core non-transactional data elements that are shared across multiple applications or business processes within an organization. It provides a consistent and unified view of key business entities such as Agents including organisations and individuals, products, services, locations, and associated attributes such as contact details and addresses. Master data management (MDM) focuses on creating and maintaining accurate, consistent, and reliable master data across different systems and applications. Master data is the data describing non-transactional entities, while MDM manages which instance of entity data is considered the master version."""@en ;
        skos:prefLabel "Master Data"@en .

eaj:data-dictionary a skos:Concept ;
    dcterms:source "https://dl.acm.org/doi/book/10.5555/541721"^^xsd:anyURI ;
    rdfs:isDefinedBy <https://ref.engineersaustralia.org.au/def/ea-jargon> ;
    skos:inScheme <https://ref.engineersaustralia.org.au/def/ea-jargon> ;
    skos:topConceptOf <https://ref.engineersaustralia.org.au/def/ea-jargon> ;
    skos:definition """A centralized repository of information about data such as meaning, relationships to other data, origin, usage, and format. 
    
    It provides a comprehensive index of data elements (Tables), their definitions, relationships, and constraints including logic rules and data types. It serves as a reference guide for developers, analysts, and business users to ensure consistent interpretation and usage of data across different applications and systems. In practice data definitions commonly describe and define the tables in a database, the columns in each table, their relationships and linkages, and the rules pertaining to the data such as valid data types and accepted values. Data dictionaries may also describe data flows and exchanges between systems and separate databases."""@en ;
    skos:prefLabel "Data Dictionary"@en .

eaj:defensibly-destroyed a skos:Concept ;
    dcterms:source "https://www.naa.gov.au/information-management/disposing-information/information-disposal/compliant-destruction-australian-government-information"^^xsd:anyURI ;
    rdfs:isDefinedBy <https://ref.engineersaustralia.org.au/def/ea-jargon> ;
    skos:inScheme <https://ref.engineersaustralia.org.au/def/ea-jargon> ;
    skos:topConceptOf <https://ref.engineersaustralia.org.au/def/ea-jargon> ;
    skos:definition """Defensibly Destroyed refers to the ability of an organisation to demonstrate that destruction of a record was planned, authorised, and compliant.
    
    Destruction is the irreversible removal of records from information systems and stores. Destruction may only be carried out where: 
    - the destruction method is secure and effective, and 
    - the destruction method is appropriate to the format of the records being destroyed, and 
    - details of the records destroyed are captured for future reference. 
    Records are considered to be approved for destruction when they: 
    - have fulfilled any relevant retention time criteria set in the Record and Disposal Schedule, and
    - are not subject to a Legal Hold, and
    - have been reviewed by the relevant business stakeholders (such as SMEs, technology service owners, or key consumers of the records), and 
    - have been approved for destruction by the Record Owners or their delegate."""@en ;
    skos:prefLabel "Defensibly Destroyed"@en .

eaj:digital-transformation a skos:Concept ;
    dcterms:source "https://www.ibm.com/topics/digital-transformation"^^xsd:anyURI ;
    rdfs:isDefinedBy <https://ref.engineersaustralia.org.au/def/ea-jargon> ;
    skos:inScheme <https://ref.engineersaustralia.org.au/def/ea-jargon> ;
    skos:topConceptOf <https://ref.engineersaustralia.org.au/def/ea-jargon> ;
    skos:definition """Digital transformation is a strategic initiative that incorporates digital technology across all areas of an organization. It evaluates and modernizes an organization's processes, products, operations and technology stack to enable continual, rapid, customer-driven innovation. Note that both digital experience and digital transformation are commonly abbreviated to DX."""@en ;
    skos:notation "DX" ;
    skos:prefLabel "Digital Transformation"@en .

eaj:digital-experience a skos:Concept ;
    dcterms:source "https://www.ibm.com/topics/digital-experience"^^xsd:anyURI ;
    rdfs:isDefinedBy <https://ref.engineersaustralia.org.au/def/ea-jargon> ;
    skos:inScheme <https://ref.engineersaustralia.org.au/def/ea-jargon> ;
    skos:topConceptOf <https://ref.engineersaustralia.org.au/def/ea-jargon> ;
    skos:definition """Digital experience refers to an interaction between a user and an organization that is made possible because of digital technologies. Note that both digital experience and digital transformation are commonly abbreviated to DX."""@en ;
    skos:notation "DX" ;
    skos:prefLabel "Digital Experience"@en .

eaj:documents a skos:Concept ;
    dcterms:source "https://linked.data.gov.au/org/engineersaustralia"^^xsd:anyURI ;
    rdfs:isDefinedBy <https://ref.engineersaustralia.org.au/def/ea-documents> ;
    skos:related <https://ref.engineersaustralia.org.au/def/ea-documents> ;
    skos:inScheme <https://ref.engineersaustralia.org.au/def/ea-jargon> ;
    skos:topConceptOf <https://ref.engineersaustralia.org.au/def/ea-jargon> ;
    skos:definition """Documents and other files that record information about a person, organisation, or process. Commonly used as for assessments, analyses, or for retention of evidence for processes and decisions. Documents may be physical or digital.
    For example Curriculum Vitae, Academic Transcripts, Competency Demonstration Reports, etc."""@en ;
    skos:altLabel "Documentation"@en,
        "EA Documents"@en,
        "Engineers Australia Documents"@en ;
	skos:prefLabel "Documents"@en .

eaj:div-rules a skos:Concept ;
    dcterms:source "https://linked.data.gov.au/org/engineersaustralia"^^xsd:anyURI ;
    rdfs:isDefinedBy <https://ref.engineersaustralia.org.au/def/ea-jargon> ;
    skos:inScheme <https://ref.engineersaustralia.org.au/def/ea-jargon> ;
    skos:topConceptOf <https://ref.engineersaustralia.org.au/def/ea-jargon> ;
    skos:definition """The local rules and regulations that govern the operation of each Engineers Australia Division."""@en ;
    skos:prefLabel "Division Rules"@en .

 eaj:disciplinary-and-appeals a skos:Concept ;
    dcterms:source "https://linked.data.gov.au/org/engineersaustralia"^^xsd:anyURI ;
    rdfs:isDefinedBy <https://ref.engineersaustralia.org.au/def/ea-jargon> ;
    skos:inScheme <https://ref.engineersaustralia.org.au/def/ea-jargon> ;
    skos:topConceptOf <https://ref.engineersaustralia.org.au/def/ea-jargon> ;
    skos:definition """Disciplinary and associated Appeal procedures govern how complaints against EA members are assessed and resolved. These procedures are managed by the Associate Director Ethics and Discipline at National Office."""@en ;
    skos:prefLabel "Disciplinary and Appeals Procedures"@en .

eaj:database a skos:Concept ;
    dcterms:source "https://www.oracle.com/au/database/what-is-database/"^^xsd:anyURI ;
    rdfs:isDefinedBy <https://ref.engineersaustralia.org.au/def/ea-jargon> ;
    skos:inScheme <https://ref.engineersaustralia.org.au/def/ea-jargon> ;
    skos:topConceptOf <https://ref.engineersaustralia.org.au/def/ea-jargon> ;
    skos:definition """A database is an organized collection of structured information, or data, typically stored electronically in a computer system. A database is usually controlled by a database management system (DBMS)."""@en ;
    skos:notation "DBMS" ;
    skos:prefLabel "Database"@en .

    eaj:relational-database a skos:Concept ;
        dcterms:source "https://www.mongodb.com/compare/relational-vs-non-relational-databases"^^xsd:anyURI ;
        rdfs:isDefinedBy <https://ref.engineersaustralia.org.au/def/ea-jargon> ;
        skos:inScheme <https://ref.engineersaustralia.org.au/def/ea-jargon> ;
        skos:broader eaj:database ;
        skos:definition """A relational database, or relational database management system (RDMS), stores information in tables. Often, these tables have shared information between them, causing a relationship to form between tables. This is where a relational database gets its name from.

        A table uses columns to define the information being stored and rows for the actual data. Each table will have a column that must have unique values-known as the primary key. This column can then be used in other tables, if relationships are to be defined between them. When one table's primary key is used in another table, this column in the second table is known as the foreign key."""@en ;
        skos:notation "RDMS" ;
        skos:prefLabel "Relational Database"@en .

    eaj:non-relational-database a skos:Concept ;
        dcterms:source "https://www.mongodb.com/compare/relational-vs-non-relational-databases"^^xsd:anyURI ;
        rdfs:isDefinedBy <https://ref.engineersaustralia.org.au/def/ea-jargon> ;
        skos:inScheme <https://ref.engineersaustralia.org.au/def/ea-jargon> ;
        skos:broader eaj:database ;
        skos:definition """A non-relational database, sometimes called NoSQL (Not Only SQL), is any kind of database that doesn't use the tables, fields, and columns structured data concept from relational databases. Non-relational databases have been designed with the cloud in mind, making them great at horizontal scaling.

        There are a few different groups of database types that store the data in different ways:
        Document Databases - store data in documents, which are usually JSON-like structures that support a variety of data types. 
        Key-Value Databases - This is the most basic type of database, where information is stored in two parts: key and value.
        Graph Databases - Graph databases are the most specialized of the non-relational database types. They use a structure of elements called nodes that store data, and edges between them contain attributes about the relationship. Relationships are defined in the edges, which makes searches related to these relationships naturally fast. Plus, they are flexible because new nodes and edges can be added easily. They also don't have to have a defined schema like a traditional relational database.
        Wide-column databases - Wide-column databases, similar to relational databases, store data in tables, columns, and rows. However, the names and formatting of the columns don't have to match in each row. The columns can even be stored across multiple servers. They are considered two-dimensional key-value stores because they use multi-dimensional mapping to reference data by row and column."""@en ;
        skos:notation "NoSQL" ;
        skos:prefLabel "Non-Relational Database"@en .

eaj:data-catalogue a skos:Concept ;
    dcterms:source "https://www.oracle.com/sg/big-data/data-catalog/what-is-a-data-catalog"^^xsd:anyURI ;
    rdfs:isDefinedBy <https://ref.engineersaustralia.org.au/def/ea-jargon> ;
    skos:inScheme <https://ref.engineersaustralia.org.au/def/ea-jargon> ;
    skos:topConceptOf <https://ref.engineersaustralia.org.au/def/ea-jargon> ;
    skos:definition """A data catalogue is an organized inventory of data assets in an organization. It uses metadata to help organizations manage their data. It also helps data professionals find, access, collect, organize, and enrich metadata to support data discovery and governance.
    
    Data catalogues describe the content of datasets, the location of datasets as uri locations or as direction to file storage assets, the types of data contained, associated files, security classification, usage rights, responsible agents, and dates of creation, modification, and applicable conditions for reuse or distribution. The purpose of a data catalogue is to make data and information assets findable and accessible. Data catalogues may also record relationships between datasets such as shared resouces, provenance and derivations, and source-of-truth hierarchy."""@en ;
    skos:altLabel "Data Catalog"@en ;
    skos:prefLabel "Data Catalogue"@en .

eaj:data-classification a skos:Concept ;
    dcterms:source "https://linked.data.gov.au/def/information-security-classification"^^xsd:anyURI ;
    rdfs:isDefinedBy <https://ref.engineersaustralia.org.au/def/ea-jargon> ;
    skos:inScheme <https://ref.engineersaustralia.org.au/def/ea-jargon> ;
    skos:topConceptOf <https://ref.engineersaustralia.org.au/def/ea-jargon> ;
    skos:definition """A categorisation of information and data assets that reflects the potential level of damage done to an organisation from unauthorised disclosure, or compromise of confidentiality. Sensitivity levels are based primarily on the legal framework of the Australian Government Office of the Australian Information Commissioner for personal and sensitive information. However, non-personal data and information, such as financial records, are also subject to this classification within the context of the potential level of damage from unauthorised disclosure."""@en ;
    skos:altLabel "Information Security Classification"@en ;
    skos:prefLabel "Data Classification"@en .

eaj:data-lifecycle a skos:Concept ;
    dcterms:source "https://www.ibm.com/au-en/topics/data-lifecycle-management"^^xsd:anyURI ;
    rdfs:isDefinedBy <https://ref.engineersaustralia.org.au/def/ea-jargon> ;
    skos:inScheme <https://ref.engineersaustralia.org.au/def/ea-jargon> ;
    skos:topConceptOf <https://ref.engineersaustralia.org.au/def/ea-jargon> ;
    skos:definition """A data lifecycle consists of a series of phases over the course its useful life. Each phase is governed by a set of policies that maximizes the data's value during each stage of the lifecycle. DLM becomes increasingly important as the volume of data that is incorporated into business workstreams grows.
    The stages of the data lifecycle are:
    1. Data Creation
    2. Data Storage
    3. Data Sharing and Usage
    4. Data Archival
    5. Data Deletion"""@en ;
    skos:altLabel "Data Lifecycle Management"@en ;
    skos:prefLabel "Data Lifecycle"@en .

    eaj:data-creation a skos:Concept ;
        dcterms:source "https://www.ibm.com/au-en/topics/data-lifecycle-management"^^xsd:anyURI ;
        rdfs:isDefinedBy <https://ref.engineersaustralia.org.au/def/ea-jargon> ;
        skos:inScheme <https://ref.engineersaustralia.org.au/def/ea-jargon> ;
        skos:broader eaj:data-lifecycle;
        dcterms:isPartOf eaj:data-lifecycle ;
        skos:definition """A new data lifecycle starts with data collection, but the sources of data are abundant. They can vary from web and mobile applications, internet of things (IoT) devices, forms, surveys, and more. While data can be generated in a variety of ways, the collection of all available data isn't necessary for the success of your business. The incorporation of new data should be always be evaluated based on its quality and relevancy to your business."""@en ;
        skos:prefLabel "Data Creation"@en .

    eaj:data-storage a skos:Concept ;
        dcterms:source "https://www.ibm.com/au-en/topics/data-lifecycle-management"^^xsd:anyURI ;
        rdfs:isDefinedBy <https://ref.engineersaustralia.org.au/def/ea-jargon> ;
        skos:inScheme <https://ref.engineersaustralia.org.au/def/ea-jargon> ;
        skos:broader eaj:data-lifecycle ;
        dcterms:isPartOf eaj:data-lifecycle ;
        skos:definition """During this phase, data becomes available to business users. DLM enables organizations to define who can use the data and the purpose for which it can be used. Once the data is made available it can be leveraged for a range of analyses-from basic exploratory data analysis and data visualizations to more advanced data mining and machine learning techniques. All of these methods play a role in business decision-making and communication to various stakeholders.

        Additionally, data usage isn't necessarily restricted to internal use only. For example, external service providers could use the data for purposes such as marketing analytics and advertising. Internal uses include day-to-day business processes and workflows, such as dashboards and presentations."""@en ;
        skos:prefLabel "Data Storage"@en .

    eaj:data-sharing a skos:Concept ;
        dcterms:source "https://www.ibm.com/au-en/topics/data-lifecycle-management"^^xsd:anyURI ;
        rdfs:isDefinedBy <https://ref.engineersaustralia.org.au/def/ea-jargon> ;
        skos:inScheme <https://ref.engineersaustralia.org.au/def/ea-jargon> ;
        skos:broader eaj:data-lifecycle ;
        dcterms:isPartOf eaj:data-lifecycle ;
        skos:definition """During this phase, data becomes available to business users. DLM enables organizations to define who can use the data and the purpose for which it can be used. Once the data is made available it can be leveraged for a range of analyses-from basic exploratory data analysis and data visualizations to more advanced data mining and machine learning techniques. All of these methods play a role in business decision-making and communication to various stakeholders.

        Additionally, data usage isn't necessarily restricted to internal use only. For example, external service providers could use the data for purposes such as marketing analytics and advertising. Internal uses include day-to-day business processes and workflows, such as dashboards and presentations."""@en ;
        skos:prefLabel "Data Sharing and Usage"@en .

    eaj:data-archival a skos:Concept ;
        dcterms:source "https://www.ibm.com/au-en/topics/data-lifecycle-management"^^xsd:anyURI ;
        rdfs:isDefinedBy <https://ref.engineersaustralia.org.au/def/ea-jargon> ;
        skos:inScheme <https://ref.engineersaustralia.org.au/def/ea-jargon> ;
        skos:broader eaj:data-lifecycle ;
        dcterms:isPartOf eaj:data-lifecycle ;
        skos:definition """After a certain amount of time, data is no longer useful for everyday operations. However, it is important to maintain copies of the organization's data that is not frequently accessed for potential litigation and investigation needs. Then, if required, archived data can be restored to an active production environment.

        An organization's DLM strategy should clearly define when, where, and for how long data should be archived. In this stage, data undergoes an archival process that ensures redundancy."""@en ;
        skos:prefLabel "Data Archival"@en .

    eaj:data-deletion a skos:Concept ;
        dcterms:source "https://www.ibm.com/au-en/topics/data-lifecycle-management"^^xsd:anyURI ;
        rdfs:isDefinedBy <https://ref.engineersaustralia.org.au/def/ea-jargon> ;
        skos:inScheme <https://ref.engineersaustralia.org.au/def/ea-jargon> ;
        skos:broader eaj:data-lifecycle ;
        dcterms:isPartOf eaj:data-lifecycle ;
        skos:definition """In this final stage of the lifecycle, data is purged from the records and destroyed securely. Businesses will delete data that they no longer need to create more storage space for active data. During this phase, data is removed from archives when it exceeds the required retention period or no longer serves a meaningful purpose to the organization."""@en ;
        skos:prefLabel "Data Deletion"@en .

eaj:data-model a skos:Concept ;
    dcterms:source "https://sciencelogic.com/glossary/data-modeling"^^xsd:anyURI ;
    rdfs:isDefinedBy <https://ref.engineersaustralia.org.au/def/ea-jargon> ;
    skos:inScheme <https://ref.engineersaustralia.org.au/def/ea-jargon> ;
    skos:topConceptOf <https://ref.engineersaustralia.org.au/def/ea-jargon> ;
    skos:definition """An abstract model that organizes elements of data and standardizes how they relate to one another and to the properties of real-world entities. A Data Model is a model of the real-world as represented by data. By extension, a Data Model is a representation of data structures and relationships between them. It is used to define and organize data in a structured way that can be understood by both humans and machines. A data model can be implemented in various forms such as a diagram, schema, or code, and it provides a framework for designing and implementing a database or data warehouse. Data models typically define entities, attributes, relationships, and constraints.

    Data models can be Conceptual, Logical, or Physical and are commonly represented as an Entity Relationship Diagram (ERD) or a Data Diagram. Typically, primary operational data models should be highly normalised and optimised for storage and retrieval of data with minimal duplication and no storage of derived data. This contrasts with semantic layers and database views that deliberately denormalise data to present human readable information and topical representations of the underlying entities. Data Models are typically implemented at the database or data warehouse level, while Semantic Layers are implemented in the business intelligence or analytics layer.
    
    By contrast, systems or solutions architectures describe how information flows between the components of a system.
    
    By contrast, Analytical Models are used to interrogate data to result in an assessment of a dataset to make descriptive, diagnostic, predictive or prescriptive conclusions."""@en ;
    skos:prefLabel "Data Model"@en .

    eaj:canonical-data-model a skos:Concept ;
        dcterms:source "https://www.bmc.com/blogs/canonical-data-model/"^^xsd:anyURI ;
        rdfs:isDefinedBy <https://ref.engineersaustralia.org.au/def/ea-jargon> ;
        skos:inScheme <https://ref.engineersaustralia.org.au/def/ea-jargon> ;
        skos:broader eaj:data-model ;
        skos:definition """Canonical Data Models are a type of applied data model that aims to present data entities and relationships in the simplest possible form to integrate processes across various systems and databases. A CDM is also known as a common data model because that serves as a common translator between various formats and systems, with the aim to provide a common language for data management. Canonical Data Models are typically highly normalised representations of real world entities and relationships.

        Commonly, the data exchanged across various systems rely on different languages, syntax, and protocols. The purpose of a CDM is to enable an enterprise to create and distribute a common definition of its entire data unit. CDMs act as a universal translator.
        
        Canonical Data Models and Operational Data Models are most commonly relational models, whereas Analytical Data Models are dimensional models."""@en ;
        skos:altLabel "Common Data Model"@en,
            "Enterprise Data Model"@en ;
        skos:prefLabel "Canonical Data Model"@en .

    eaj:ontological-data-model a skos:Concept ;
        dcterms:source "https://www.ontotext.com/knowledgehub/fundamentals/what-are-ontologies/"^^xsd:anyURI ;
        rdfs:isDefinedBy <https://ref.engineersaustralia.org.au/def/ea-jargon> ;
        skos:inScheme <https://ref.engineersaustralia.org.au/def/ea-jargon> ;
        skos:broader eaj:data-model ;
        skos:definition """A meta-model or ontology is a formal description of knowledge as a set of concepts within a domain and the relationships that hold between them. A meta-model describes how data is used to model the real world in a system-independent framework. By extension, a meta-model translates from real world objects to data entities and is a model of other data models.

        Where a canonical data model will define the data entities within a domain shared across systems, a meta-model defines why those data entities exist in the data model, what class of object those entities belong to, and therefore how they will be represented by the data. For example, a canonical model may describe customers, employees, contractors, volunteers in seperate tables, whereas the metamodel defines these as subclasses of Relationships between EA and its various contacts, and by extension defines a common core of attributes expected for all subclasses of agent-to-agent relationships.

        Meta-models describes what elements and classes of objects constitute a domain, their attributes, and their relationships to each other. Meta Models provide the framework to create other models by describing criteria for the defintion of classes of concepts in a system-independent manner. Meta-models may also decribe data restrictions, rules and axioms. 
        
        A meta model can be applied to a set of individual facts to create a Knowledge Graph expressed as subject-predicate-object triples.
        
        Since ontologies define the terms used to describe and represent an area of knowledge, they are used in many applications to capture relationships and boost knowledge management, such as vocabulary management, metadata management, master data management. The latter of which may be achieved by informing the development of a canonical model that describes and enables Master Data Management that efficiently captures master data entities, attributes, and relationships."""@en ;
        skos:altLabel "Ontological Data Model"@en,
            "Ontology"@en ;
        skos:prefLabel "Meta Model"@en .

    eaj:operational-data-model a skos:Concept ;
        dcterms:source "https://linked.data.gov.au/org/engineersaustralia"^^xsd:anyURI ;
        rdfs:isDefinedBy <https://ref.engineersaustralia.org.au/def/ea-jargon> ;
        skos:inScheme <https://ref.engineersaustralia.org.au/def/ea-jargon> ;
        skos:broader eaj:data-model ;
        skos:definition """Operational Data Models are used in transactional systems and focuses on ensuring data integrity and avoiding data redundancy. These are for day-to-day business operations, e.g. SalesForce and the Oracle Corporate Database.
        
        Canonical Data Models and Operational Data Models are most commonly relational models, whereas Analytical Data Models are dimensional models."""@en ;
        skos:altLabel "Transactional Data Model"@en ;
        skos:prefLabel "Operational Data Model"@en .

    eaj:analytical-data-model a skos:Concept ;
        dcterms:source "https://www.datameer.com/blog/what-is-a-semantic-layer/"^^xsd:anyURI ;
        rdfs:isDefinedBy <https://ref.engineersaustralia.org.au/def/ea-jargon> ;
        skos:inScheme <https://ref.engineersaustralia.org.au/def/ea-jargon> ;
        skos:broader eaj:data-model ;
        skos:definition """An Analytical Data Model is a business representation of data and a type of post-hoc dimensional data model. They are designed for analysis, typically denormalised, and oriented to subject areas. Analytical Data Models are for Business Insight, e.g. DAP, BI, DbT. Analytical Data Models are not to be confused with Analytical Models which model data analysis, whereas an analytical data model is a model of data used for analysis. 
        
        Analytical Data Models enable end-users to quickly discover and access data using standard search terms - like a customer, recent purchase, and prospect. It also provides human-readable terms to data sources that otherwise would be impossible to discover (e.g., table slsqtq121 becomes Sales West 1st Quarter 2021). Semantic layers are typically denormalised representations of data with deliberate replication for ease of human consumption.
        
        A Semantic Layer is an abstraction layer between the physical data sources and the end-users. It is a virtual layer that translates technical data into business terms, making it easier for non-technical users to access and analyse data. The Semantic Layer serves as a bridge between the technical and business worlds, and it can provide a single, unified view of data across multiple sources. It also allows users to create custom reports and queries without requiring technical expertise. Strictly speaking analytical data models are typically implemented at the data warehouse level, while Semantic Layers are implemented in the business intelligence or analytics layer.
        
        Semantic layers and non-materialised views are typically the location where derived information is calculated or generated. This ensures more efficient storage, reduces inconsistencies, and ensures derived information is current and synchronised with raw data in the underlying data model.
        
        Canonical Data Models and Operational Data Models are most commonly relational models, whereas Analytical Data Models are typically dimensional models, aka Star Schema."""@en ;
        skos:altLabel "Semantic Layer"@en,
            "Analytical Data Model"@en,
            "Star Schema"@en ;
        skos:prefLabel "Dimensional Data Model"@en .

eaj:analytical-model a skos:Concept ;
    dcterms:source "https://www.gartner.com/en/information-technology/glossary/advanced-analytics"^^xsd:anyURI ;
    rdfs:isDefinedBy <https://ref.engineersaustralia.org.au/def/ea-jargon> ;
    skos:inScheme <https://ref.engineersaustralia.org.au/def/ea-jargon> ;
    skos:topConceptOf <https://ref.engineersaustralia.org.au/def/ea-jargon> ;
    skos:definition """Analytical modeling is a mathematical approach to business analysis that uses complex calculations that often involve numerous variables and factors.
    This can be further categorised into 4 variants:
    - Descriptive Analytics: What happened?
    - Diagnostic Analytics: Why did it happen?
    - Predictive Analytics: What will happen?
    - Prescriptive Analytics: How can we make it happen? How can we influence the outcome?"""@en ;
    skos:prefLabel "Analytical Model"@en .
    
    eaj:descriptive-model a skos:Concept ;
        dcterms:source "https://www.gartner.com/en/information-technology/glossary/descriptive-analytics"^^xsd:anyURI ;
        rdfs:isDefinedBy <https://ref.engineersaustralia.org.au/def/ea-jargon> ;
        skos:inScheme <https://ref.engineersaustralia.org.au/def/ea-jargon> ;
        skos:broader eaj:analytical-model ;
        skos:definition """Descriptive Analytics is the examination of data or content, usually manually performed, to answer the question "What happened?" (or What is happening?), characterized by traditional business intelligence (BI) and visualizations such as pie charts, bar charts, line graphs, tables, or generated narratives.
        
        (gartner.com)."""@en ;
        skos:altLabel "Descriptive Analytics"@en,
            "Descriptive Model"@en ;
        skos:prefLabel "Descriptive Analytical Model"@en .

    eaj:diagnostic-model a skos:Concept ;
        dcterms:source "https://www.gartner.com/en/information-technology/glossary/diagnostic-analytics"^^xsd:anyURI ;
        rdfs:isDefinedBy <https://ref.engineersaustralia.org.au/def/ea-jargon> ;
        skos:inScheme <https://ref.engineersaustralia.org.au/def/ea-jargon> ;
        skos:broader eaj:analytical-model ;
        skos:definition """Diagnostic analytics is a form of advanced analytics that examines data or content to answer the question, "Why did it happen?" It is characterized by techniques such as drill-down, data discovery, data mining and correlations.
        
        (gartner.com)."""@en ;
        skos:altLabel "Diagnostic Analytics"@en,
            "Diagnostic Model"@en ;
        skos:prefLabel "Diagnostic Analytical Model"@en .

    eaj:predictive-model a skos:Concept ;
        dcterms:source "https://www.gartner.com/en/information-technology/glossary/predictive-analytics"^^xsd:anyURI ;
        rdfs:isDefinedBy <https://ref.engineersaustralia.org.au/def/ea-jargon> ;
        skos:inScheme <https://ref.engineersaustralia.org.au/def/ea-jargon> ;
        skos:broader eaj:analytical-model ;
        skos:definition """Predictive analytics describes any approach to data mining with four attributes:
        1. An emphasis on prediction (rather than description, classification or clustering)
        2. Rapid analysis measured in hours or days (rather than the stereotypical months of traditional data mining)
        3. An emphasis on the business relevance of the resulting insights (no ivory tower analyses)
        4. (increasingly) An emphasis on ease of use, thus making the tools accessible to business users.
        
        (gartner.com)."""@en ;
        skos:altLabel "Predictive Analytics"@en,
            "Predictive Model"@en ;
        skos:prefLabel "Predictive Analytical Model"@en .

    eaj:prescriptive-model a skos:Concept ;
        dcterms:source "https://www.gartner.com/en/information-technology/glossary/prescriptive-analytics"^^xsd:anyURI ;
        rdfs:isDefinedBy <https://ref.engineersaustralia.org.au/def/ea-jargon> ;
        skos:inScheme <https://ref.engineersaustralia.org.au/def/ea-jargon> ;
        skos:broader eaj:analytical-model ;
        skos:definition """Prescriptive Analytics is a form of advanced analytics which examines data or content to answer the question "What should be done?" or "What can we do to make X happen?", and is characterized by techniques such as graph analysis, simulation, complex event processing, neural networks, recommendation engines, heuristics, and machine learning.
        
        (gartner.com)."""@en ;
        skos:altLabel "Prescriptive Analytics"@en,
            "Prescriptive Model"@en ;
        skos:prefLabel "Prescriptive Analytical Model"@en .

eaj:data-profiling a skos:Concept ;
    dcterms:source "https://www.talend.com/resources/what-is-data-profiling/"^^xsd:anyURI ;
    rdfs:isDefinedBy <https://ref.engineersaustralia.org.au/def/ea-jargon> ;
    skos:inScheme <https://ref.engineersaustralia.org.au/def/ea-jargon> ;
    skos:topConceptOf <https://ref.engineersaustralia.org.au/def/ea-jargon> ;
    skos:definition """Data profiling is the process of examining, analyzing, and creating useful summaries of data. The process yields a high-level overview which aids in the discovery of data quality issues, risks, and overall trends. Data profiling produces critical insights into data that companies can then leverage to their advantage.
    
    More specifically, data profiling sifts through data to determine its legitimacy and quality. Analytical algorithms detect dataset characteristics such as mean, minimum, maximum, percentile, and frequency to examine data in minute detail. It then performs analyses to uncover metadata, including frequency distributions, key relationships, foreign key candidates, and functional dependencies. Finally, it uses all of this information to expose how those factors align with your business's standards and goals. Data profiling, involves the statistical analysis and assessment of data values within a data set for consistency, uniqueness and logic. The data profiling process cannot typically identify inaccurate data; it can only identify business rules violations and anomalies. The insight gained by data profiling can be used to determine how difficult it will be to use existing data for other purposes."""@en ;
    skos:prefLabel "Data Profiling"@en .

eaj:data-multiple-storage a skos:Concept ;
    dcterms:source "https://linked.data.gov.au/org/engineersaustralia"^^xsd:anyURI ;
    rdfs:isDefinedBy <https://ref.engineersaustralia.org.au/def/ea-jargon> ;
    skos:inScheme <https://ref.engineersaustralia.org.au/def/ea-jargon> ;
    skos:topConceptOf <https://ref.engineersaustralia.org.au/def/ea-jargon> ;
    skos:definition """Data that is multiplies across tables, systems, or platforms. This may be deliberate, accidental, or incidental."""@en ;
    skos:prefLabel "Data Storage Multiplication"@en .

    eaj:data-duplication a skos:Concept ;
        dcterms:source "https://linked.data.gov.au/org/engineersaustralia"^^xsd:anyURI ;
        rdfs:isDefinedBy <https://ref.engineersaustralia.org.au/def/ea-jargon> ;
        skos:inScheme <https://ref.engineersaustralia.org.au/def/ea-jargon> ;
        skos:broader eaj:data-multiple-storage ;
        skos:definition """The creation of multiple distinct and unconnected data records pertaining to the same instance of an entity (e.g. the same individual, organisation, opportunity, invoice, etc.), either within a single system or across multiple systems. In this context, duplication is almost always an unintended consequence of a combination of business and technical processes, and is something to be avoided. Data duplication is a data integrity problem which can have significant negative consequences for business operations."""@en ;
        skos:prefLabel "Data Duplication"@en .

    eaj:data-replication a skos:Concept ;
        dcterms:source "https://linked.data.gov.au/org/engineersaustralia"^^xsd:anyURI ;
        rdfs:isDefinedBy <https://ref.engineersaustralia.org.au/def/ea-jargon> ;
        skos:inScheme <https://ref.engineersaustralia.org.au/def/ea-jargon> ;
        skos:broader eaj:data-multiple-storage ;
        skos:definition """The act of creating an identical copy of an existing piece of data in a different location. Data replication is a deliberate and necessary feature of most non-trivial systems architectures. It is necessary for backups and disaster recovery, and can be used to facilitate more efficient access to data by multiple systems without requiring real-time cross-systems access (which can come with technical, bandwidth, and security issues)."""@en ;
        skos:prefLabel "Data Replication"@en .

    eaj:data-synchronisation a skos:Concept ;
        dcterms:source "https://linked.data.gov.au/org/engineersaustralia"^^xsd:anyURI ;
        rdfs:isDefinedBy <https://ref.engineersaustralia.org.au/def/ea-jargon> ;
        skos:inScheme <https://ref.engineersaustralia.org.au/def/ea-jargon> ;
        skos:broader eaj:data-multiple-storage ;
        skos:definition """The process of comparing and matching data for the purpose of selecting records for replication, or to identify and resolve instances of duplication or other data quality issues. It can be done as part of a replication process or independently. Data management best practice suggests synchronising enterprise data across relevant enterprise systems. This ensures a degree of consistency for internal stakeholders (staff) and external (customers), which can both increase operational efficiency and improve the customer experience. Data synchronization can be achieved using data replication, but data replication does not necessarily involve data synchronization."""@en ;
        skos:prefLabel "Data Synchronisation"@en .

eaj:data-store a skos:Concept ;
    dcterms:source "https://aws.amazon.com/what-is/data-store/"^^xsd:anyURI ;
    rdfs:isDefinedBy <https://ref.engineersaustralia.org.au/def/ea-jargon> ;
    skos:inScheme <https://ref.engineersaustralia.org.au/def/ea-jargon> ;
    skos:topConceptOf <https://ref.engineersaustralia.org.au/def/ea-jargon> ;
    skos:definition """A data store is a digital repository that stores and safeguards the information in computer systems. A data store can be network-connected storage, distributed cloud storage, a physical hard drive, or virtual storage. It can store both structured data like information tables and unstructured data like emails, images, and videos. Organizations use data stores to retain, share, and manage information across business units. Data Stores are where databases, data warehouses, data catalogues, and file storage are physically stored and managed.
    
    Examples of storage include Direct-attached storage (DAS) consisting of storage devices that connect physically to a computer, Network-attached storage (NAS) that make data continuously available for applications and users to collaborate on effectively over a network, and Cloud storage that is distributed storage infrastructure hosted and managed by cloud providers. It is more scalable, flexible, and remotely accessible compared to on-premises storage.
    
    Cloud data stores include products from major providers such as Azure Cloud Storage, AWS Cloud Storage and Google Cloud."""@en ;
    skos:prefLabel "Data Store"@en .

eaj:data-warehouse a skos:Concept ;
    dcterms:source "https://cloud.google.com/learn/what-is-a-data-warehouse"^^xsd:anyURI ;
    rdfs:isDefinedBy <https://ref.engineersaustralia.org.au/def/ea-jargon> ;
    skos:inScheme <https://ref.engineersaustralia.org.au/def/ea-jargon> ;
    skos:topConceptOf <https://ref.engineersaustralia.org.au/def/ea-jargon> ;
    skos:definition """A data warehouse is an enterprise system used for the analysis and reporting of structured and semi-structured data from multiple sources, such as point-of-sale transactions, marketing automation, customer relationship management, and more. A data warehouse is suited for ad hoc analysis as well custom reporting. A data warehouse can store both current and historical data in one place and is designed to give a long-range view of data over time, making it a primary component of business intelligence.
    
    Data Warehouses can create snapshots of historical databases and other datastores, synchornise with live databases and integrate other semi-structured data for anaylsis in a single platform, whilst creating a separation with the underlying raw data and therefore eliminating risk of accidental alteration."""@en ;
    skos:prefLabel "Data Warehouse"@en .

eaj:duty-separation a skos:Concept ;
    dcterms:source "https://www.counterfraud.gov.au/fraud-countermeasures/segregation-duties"^^xsd:anyURI ;
    rdfs:isDefinedBy <https://ref.engineersaustralia.org.au/def/ea-jargon> ;
    skos:inScheme <https://ref.engineersaustralia.org.au/def/ea-jargon> ;
    skos:topConceptOf <https://ref.engineersaustralia.org.au/def/ea-jargon> ;
    skos:definition """Separate duties by allocating tasks and associated privileges for a business process to multiple staff. This is very important in areas such as payroll, finance, procurement, contract management and human resources. Systems help to enforce the strong separation of duties. This is also known as segregation of duties. The distribution of roles and responsibilitiesto multiple staff ensures redundancy and process continuity in case of unplanned staff absence or departure."""@en ;
    skos:altLabel "Segregation of Duties"@en,
        "Duty Segregation"@en,
        "Duty Separation"@en,
        "Separate Duties"@en ;
    skos:prefLabel "Separation of Duties"@en .

eaj:digital-governance-groups a skos:Concept ;
    dcterms:source "https://linked.data.gov.au/org/engineersaustralia"^^xsd:anyURI ;
    rdfs:isDefinedBy <https://ref.engineersaustralia.org.au/def/ea-jargon> ;
    skos:inScheme <https://ref.engineersaustralia.org.au/def/ea-jargon> ;
    skos:topConceptOf <https://ref.engineersaustralia.org.au/def/ea-jargon> ;
    skos:definition """The groups and forums that drive digital change. These forums assess changes for alignment with strategic direction, architectural design adherence, and suitability for deployment."""@en ;
    skos:prefLabel "Digital Governance Groups"@en .

    eaj:digital-steering-committee a skos:Concept ;
        dcterms:source "https://linked.data.gov.au/org/engineersaustralia"^^xsd:anyURI ;
        rdfs:isDefinedBy <https://ref.engineersaustralia.org.au/def/ea-jargon> ;
        skos:inScheme <https://ref.engineersaustralia.org.au/def/ea-jargon> ;
        skos:topConceptOf <https://ref.engineersaustralia.org.au/def/ea-jargon> ;
        skos:definition """The groups that assesses the technological environment at a strategic level. Responsible for assessing large sclae change and setting strategic digital objectives."""@en ;
        skos:notation "DSC" ;
        skos:prefLabel "Digital Steering Committee"@en .

    eaj:design-review-board a skos:Concept ;
        dcterms:source "https://linked.data.gov.au/org/engineersaustralia"^^xsd:anyURI ;
        rdfs:isDefinedBy <https://ref.engineersaustralia.org.au/def/ea-jargon> ;
        skos:inScheme <https://ref.engineersaustralia.org.au/def/ea-jargon> ;
        skos:topConceptOf <https://ref.engineersaustralia.org.au/def/ea-jargon> ;
        skos:definition """The forum that assesses proposed digital changes. This includes new technology and enhancements to existing systems. This forum checks for alignment to architectural principles, adherence to privacy and security requirements, integration with analytics, infrastructure compatibility, testing requirements, etc."""@en ;
        skos:notation "DRB" ;
        skos:prefLabel "Design Review Board"@en .

    eaj:change-advisory-board a skos:Concept ;
        dcterms:source "https://linked.data.gov.au/org/engineersaustralia"^^xsd:anyURI ;
        rdfs:isDefinedBy <https://ref.engineersaustralia.org.au/def/ea-jargon> ;
        skos:inScheme <https://ref.engineersaustralia.org.au/def/ea-jargon> ;
        skos:topConceptOf <https://ref.engineersaustralia.org.au/def/ea-jargon> ;
        skos:definition """The group that  assesses proposals for changes for technical detail on implementation and deployment within the digital environment. This board schedules changes, assigns responsible persons to deploy changes, and manages release, testing, and rollback."""@en ;
        skos:prefLabel "Change Advisory Board"@en .

eaj:ea-assessment a skos:Concept ;
    dcterms:source "https://linked.data.gov.au/org/engineersaustralia"^^xsd:anyURI ;
    rdfs:isDefinedBy <https://ref.engineersaustralia.org.au/def/ea-jargon> ;
    skos:inScheme <https://ref.engineersaustralia.org.au/def/ea-jargon> ;
    skos:topConceptOf <https://ref.engineersaustralia.org.au/def/ea-jargon> ;
    skos:definition """An assessment by Engineers Australia to determine the Competence stage of the Engineer or Occupational Category. There are assessment processes at every level of membership or credentials. They can be more or less intensive (and/or expensive) depending on the level, the qualification(s) of the candidate, the pathway etc.
    The assessments involve human judgement and may follow one of two pathways to recognition: Accredited Engineering Qualifcations or a Competency Demonstration.
    Assessments at a high level sometimes grant a combination of credentials.
    
    For Example: 
    - A successful NER applicant who holds an accredited qualification will be granted Stage 1 competency.
    - A successful EngExec applicant who holds an accredited qualification will be granted Stage 1, Membership, and Stage 2 as well as Chartered in Leadership and Management."""@en ;
    skos:altLabel "Assessment"@en,
        "Pathways to Recognition"@en ;
    skos:prefLabel "Engineers Australia Assessment"@en .

    eaj:competency-assessment a skos:Concept ;
        dcterms:source "https://linked.data.gov.au/org/engineersaustralia"^^xsd:anyURI ;
        dcterms:references <https://www.ieagreements.org/assets/Uploads/Documents/IEA-Extended-Glossary.pdf> ;
        rdfs:isDefinedBy <https://ref.engineersaustralia.org.au/def/ea-jargon> ;
        skos:inScheme <https://ref.engineersaustralia.org.au/def/ea-jargon> ;
        skos:broader eaj:ea-assessment ;
        skos:definition """Competency Assessment is a summative assessment of an individual's competency against a prescribed standard based on evidence from the individual's work, reports by qualified observers, and other tests that may include a professional review.

        At Engineers Australia, competency is the ability to perform tasks within an occupation to the standard expected in employment. All membership applications for Engineers Australia are now competency based. However, this Competency-Based Assessment is used specifically to refer to assessments of eligibility where the applicant is required to submit a report to be evaluated by a National Assessor or College Membership Reviewer followed by an interview by an expert panel. In some cases the interview is at the discretion of the Assessor or College Membership Reviewer."""@en ;
        skos:notation "CBA" ;
        skos:altLabel "Competency Based Assessment"@en,
            "Competency-Based Assessment"@en ;
        skos:prefLabel "Competency Assessment"@en .

    eaj:cpd-assessment a skos:Concept ;
        dcterms:source "https://www.engineersaustralia.org.au/sites/default/files/resource-files/2020-02/EA%20General%20Regulations%205%20Dec%202019.pdf"^^xsd:anyURI ;
        rdfs:isDefinedBy <https://ref.engineersaustralia.org.au/def/ea-jargon> ;
        skos:inScheme <https://ref.engineersaustralia.org.au/def/ea-jargon> ;
        skos:broader eaj:ea-assessment ;
        skos:definition """For a member, CPD Assessment is an assessment of the member's compliance with the CPD requirements, made following a CPD audit."""@en ;
        skos:prefLabel "CPD Assessment"@en .

    eaj:s1-competency-assessment a skos:Concept ;
        dcterms:source "https://linked.data.gov.au/org/engineersaustralia"^^xsd:anyURI ;
        rdfs:isDefinedBy <https://ref.engineersaustralia.org.au/def/ea-jargon> ;
        skos:inScheme <https://ref.engineersaustralia.org.au/def/ea-jargon> ;
        skos:broader eaj:competency-assessment ;
        skos:definition """A Stage 1 Competency Assessment is undertaken for Australian residents with unaccredited Australian engineering qualifications and non-residents who have unaccredited overseas qualifications, where there is an intention or possible intention to join Engineers Australia.
        
        Applicants for recognition as Professional Engineers, Engineering Technologists or Engineering Associates are normally expected to have completed an Australian BE, BTech or Advanced Diploma or a qualification of equivalent standing. 
        
        However, some applicants do not have an acceptable undergraduate qualification but do have one that provides a suitable foundation of study together with one or more post-graduate qualifications. Where the post-graduate course forms a coherent extension of the basic qualification, Engineers Australia may judge that the aggregated academic achievements as an acceptable equivalent. In such cases, the applicant is regarded as having qualified upon completion of the last course taken into account."""@en ;
        skos:altLabel "Aggregation"@en,
            "Entry to Practice Assessment"@en ;
        skos:prefLabel "Stage 1 Competency Assessment"@en .

    eaj:s2-competency-assessment a skos:Concept ;
        dcterms:source "https://www.engineersaustralia.org.au/sites/default/files/2018-03/competency_standards_june.pdf"^^xsd:anyURI ;
        rdfs:isDefinedBy <https://ref.engineersaustralia.org.au/def/ea-jargon> ;
        skos:inScheme <https://ref.engineersaustralia.org.au/def/ea-jargon> ;
        skos:broader eaj:competency-assessment ;
        skos:definition """The Stage 2 Competency Standards are the profession's expression of the knowledge and skill base, engineering application abilities, and professional skills, values and attitudes that must be demonstrated in order to practise independently or unsupervised.

        The Stage 2 competency standards are used as the basis of assessment for Chartered membership of Engineers Australia (CPEng) and registration on the National Engineering Register (NER). Chartered membership is exclusive to Engineers Australia. It is a professional credential recognised by government, business and the general public worldwide. The achievement of CPEng brings with it a career-long obligation to maintain competence in a chosen practice area.
        
        The Stage 2 competency standards are generic in the sense that they apply to all disciplines of engineering in four units:
            - personal commitment
            - obligation to community
            - value in the workplace
            - technical proficiency
        Each unit contains elements of competence and indicators of attainment. The elements of competence are the capabilities necessary to the unit of competence and the indicators of attainment serve as a guide to the engineering work likely to be considered as demonstrating attainment of that competence."""@en ;
        skos:altLabel "Chartered Assessment"@en,
            "Assessment for Chartered Status"@en,
            "Independent Practice Assessment"@en ;
        skos:prefLabel "Stage 2 Competency Assessment"@en .

    eaj:s3-competency-assessment a skos:Concept ;
        dcterms:source "https://www.engineersaustralia.org.au/credentials/engexec"^^xsd:anyURI ;
        rdfs:isDefinedBy <https://ref.engineersaustralia.org.au/def/ea-jargon> ;
        skos:inScheme <https://ref.engineersaustralia.org.au/def/ea-jargon> ;
        skos:broader eaj:competency-assessment ;
        skos:definition """The Engineering Executive, or EngExec is a credential that recognises pre-eminent individuals in executive positions who have shown exceptional leadership and talent. After an outstanding career which has culminated in a senior leadership position, the receipt of EngExec is the next step.

        The EngExec credential isn't restricted to engineering professionals and can include senior business leaders who work in the engineering sector but aren't engineers.
            
        Attaining the level of EngExec also presents an opportunity to play a significant role in shaping the future of the Australian engineering profession.
            
        The exclusive nature of the credential means that the opportunity to apply for it is only offered to a select group of individuals on an invitation-only basis.
            
        Eligibility criteria requires applicants have 15 or more years of industry experience and be in a senior leadership and management role. Applicants need to be able to demonstrate the required leadership and management competencies for EngExec and complete a self-assessment if invited to apply. A professional interview with an Engineers Australia assessor is the final step to obtaining an EngExec credential.
            
        The competenices required include:
            - Leadership
            - Strategic direction and entrepreneurship
            - Planning
            - Change and improvement
            - Customer Focus."""@en ;
        skos:altLabel "Engineering Executive Assessment"@en,
            "EngExec Assessment"@en ;
        skos:prefLabel "Stage 3 Competency Assessment"@en .

    eaj:continuous-collaborative-assessment a skos:Concept ;
        dcterms:source "https://linked.data.gov.au/org/engineersaustralia"^^xsd:anyURI ;
        rdfs:isDefinedBy <https://ref.engineersaustralia.org.au/def/ea-jargon> ;
        rdfs:seeAlso <https://linked.data.gov.au/def/iea-occupational-categories/> ;
        skos:inScheme <https://ref.engineersaustralia.org.au/def/ea-jargon> ;
        skos:broader eaj:ea-assessment ;
        skos:definition """This is the process for progressive assessment of an engineer who is undergoing formation in an Engineers Australia approved Professional Development Program. The Program involves the lodging with Engineers Australia of a formal employer agreement, providing for appointment of a mentor, and the submission of regular reports by the Graduate during formation. The final report, leading to the Professional Interview for MIEAust CPEng, is accepted in lieu of the normal Engineering Practice Report (EPR). Formation under this program may be achieved in the minimum 3 years whereas those whose formation is less formal usually need at least 4 years. As these programs are under development, it is possible the final name for them be slightly different."""@en ;
        skos:notation "CCA" ;
        skos:prefLabel "Continuous Collaborative Assessment"@en .

    eaj:articulation a skos:Concept ;
        dcterms:source "https://linked.data.gov.au/org/engineersaustralia"^^xsd:anyURI ;
        rdfs:isDefinedBy <https://ref.engineersaustralia.org.au/def/ea-jargon> ;
        skos:inScheme <https://ref.engineersaustralia.org.au/def/ea-jargon> ;
        skos:broader eaj:ea-assessment ;
        skos:definition """Articulation is the process by which a person is able to attain a desired occupational category or to progress to a higher occupational category by demonstrating engineering competencies. Usually this is achieved by additional academic study but changes in occupational categories may also be achieved in part by relevant work experience, Continuous Professional Development (CPD) activities or a combination of both. The normal articulation pathways are from Engineering Associate to Engineering Technologist and from Engineering Technologist to Professional Engineer.
        
        The National Articulation Committee assists members of Engineers Australia to articulate from one category in the engineering workforce to another. The Committee also advocates for educational institutions to offer programs suitable for articulation and works provide members with achievable and clearly defined pathways to enable them to demonstrate the relevant competencies. The Committee may also assist members who wish to articulate directly from Engineering Associate to Professional Engineer and Affiliates who wish to move into a recognised occupational category."""@en ;
        skos:prefLabel "Articulation"@en .

    eaj:assessment-qualifications a skos:Concept ;
        dcterms:source "https://linked.data.gov.au/org/engineersaustralia"^^xsd:anyURI ;
        rdfs:isDefinedBy <https://ref.engineersaustralia.org.au/def/ea-jargon> ;
        rdfs:seeAlso <https://linked.data.gov.au/def/iea-occupational-categories/> ;
        skos:inScheme <https://ref.engineersaustralia.org.au/def/ea-jargon> ;
        skos:broader eaj:ea-assessment ;
        skos:definition """A formal Engineers Australia assessment to determine the relevant occupational category for an individual."""@en ;
        skos:notation "A/Q" ;
        skos:prefLabel "Assessment of Qualifications"@en .

    eaj:follow-on-activity a skos:Concept ;
        dcterms:source "https://linked.data.gov.au/org/engineersaustralia"^^xsd:anyURI ;
        rdfs:isDefinedBy <https://ref.engineersaustralia.org.au/def/ea-jargon> ;
        skos:inScheme <https://ref.engineersaustralia.org.au/def/ea-jargon> ;
        skos:broader eaj:ea-assessment ;
        skos:definition """A Follow-on Activity details an engineering assignment that a Person must complete as a result of not satisfying the Interview Panel that they are Stage 2 Competent at their Professional Interview."""@en ;
        skos:notation "FoA" ;
        skos:altLabel "Follow On Activity"@en,
            "Follow-On Activity Requirement"@en,
            "Follow On Activity Requirement"@en ;
        skos:prefLabel "Follow-On Activity"@en .

    eaj:migration-skills-assessment a skos:Concept ;
        dcterms:source "https://linked.data.gov.au/org/engineersaustralia"^^xsd:anyURI ;
        rdfs:isDefinedBy <https://ref.engineersaustralia.org.au/def/ea-jargon> ;
        skos:inScheme <https://ref.engineersaustralia.org.au/def/ea-jargon> ;
        skos:broader eaj:ea-assessment ;
        skos:definition """The Migration Skills Assessment (MSA) Unit of the Education and Assessment Directorate at National Office, undertakes assessments of the qualifications of overseas engineers.
        
        Overseas engineers who intend to apply for permanent residence in Australia under the Skilled Migration Program must have their qualifications and skills assessed by Engineers Australia before they lodge their migration application. Engineers Australia assesses overseas qualifications under a contract to AEI-NOOSR, a branch of the Commonwealth Department of Education, Science and Training. If an applicant appeals against an assessment outcome the case is reviewed by an honorary Committee of Review. The Migration Skills Assessment Unit does not assess persons who are already Australian Permanent Residents or Citizens. These persons must apply for an assessment using the Stage 1 Competency Assessment process."""@en ;
        skos:notation "MSA" ;
        skos:altLabel "Overseas Qualifications Assessment"@en,
            "OSQA"@en,
            "Foreign Qualifications Assessment"@en,
            "FQA"@en ;
        skos:prefLabel "Migration Skills Assessment"@en .

    eaj:mutual-recognition-agreement a skos:Concept ;
        dcterms:source "https://linked.data.gov.au/org/engineersaustralia"^^xsd:anyURI ;
        rdfs:isDefinedBy <https://ref.engineersaustralia.org.au/def/ea-jargon> ;
        skos:inScheme <https://ref.engineersaustralia.org.au/def/ea-jargon> ;
        skos:broader eaj:ea-assessment ;
        skos:definition """Engineers Australia has established agreements with institutions and organisations around the world, which accord their members an equivalent level of membership when applying to join Engineers Australia. Proof of membership of the mutually recognised organisation is required on application."""@en ;
        skos:notation "MRA" ;
        skos:altLabel "Recognition Agreement"@en,
            "International Recognition"@en ;
        skos:prefLabel "Mutual Recognition Agreement"@en .

    eaj:pre-application-skills-assessment a skos:Concept ;
        dcterms:source "https://linked.data.gov.au/org/engineersaustralia"^^xsd:anyURI ;
        rdfs:isDefinedBy <https://ref.engineersaustralia.org.au/def/ea-jargon> ;
        skos:inScheme <https://ref.engineersaustralia.org.au/def/ea-jargon> ;
        skos:broader eaj:ea-assessment ;
        skos:definition """The process of assessing a person's qualifications and skills by a designated assessing authority such as Engineers Australia. This process occurs before that person makes an application for permanent residence."""@en ;
        skos:notation "PASA" ;
        skos:prefLabel "Pre-Application Skills Assessment"@en .

    eaj:professional-interview a skos:Concept ;
        dcterms:source "https://linked.data.gov.au/org/engineersaustralia"^^xsd:anyURI ;
        rdfs:isDefinedBy <https://ref.engineersaustralia.org.au/def/ea-jargon> ;
        skos:inScheme <https://ref.engineersaustralia.org.au/def/ea-jargon> ;
        skos:broader eaj:ea-assessment ;
        skos:definition """A Professional Interview is a record of a Person's formal Stage 2 interview with EA Assessor(s) and optional Panel Member(s). The Professional Interview (PI) is the final stage of a candidate's application for Chartered Status and is essentially a peer review of the competencies the candidate has claimed in their Engineering Practice Report (EPR). The PI of a candidate for Chartered Membership (CPEng, CEngT or CEngO is carried out by an Assessment Panel normally consisting of two Interviewers and an Accredited National Assessor. An Interviewer is an experienced practitioner in either the candidate's discipline or industry sector. The Interviewer plays an important role within Engineers Australia of contributing towards a decision as to whether a candidate is assessed as having reached the professional standard they are expected to demonstrate at a PI. The PI is normally held in a Division Office and usually lasts 60 minutes. It includes a 30 minute session during which the two Interviewers ask in-depth questions concerning the candidate's discipline and industry, primarily based on the written and oral presentations."""@en ;
        skos:notation "PI"@en ;
        skos:prefLabel "Professional Interview"@en .

    eaj:s2-application a skos:Concept ;
        dcterms:source "https://linked.data.gov.au/org/engineersaustralia"^^xsd:anyURI ;
        rdfs:isDefinedBy <https://ref.engineersaustralia.org.au/def/ea-jargon> ;
        skos:inScheme <https://ref.engineersaustralia.org.au/def/ea-jargon> ;
        skos:broader eaj:ea-assessment ;
        dcterms:hasPart eaj:s2-competency-assessment,
            eaj:professional-interview,
            eaj:follow-on-activity ;
        skos:definition """A Stage 2 Application is comprised of the: 
            - Competency Requirements
            - Associated Submission(s)
            - Professional Interview
            - Follow-On Activities (if required)."""@en ;
        skos:prefLabel "Stage 2 Application"@en .

eaj:ea-award a skos:Concept ;
    dcterms:source "https://www.engineersaustralia.org.au/about-us/excellence-awards-program"^^xsd:anyURI ;
    rdfs:isDefinedBy <https://ref.engineersaustralia.org.au/def/ea-awards> ;
    skos:related <https://ref.engineersaustralia.org.au/def/ea-awards> ;
    skos:inScheme <https://ref.engineersaustralia.org.au/def/ea-jargon> ;
    skos:definition """An EA Award is an Engineers Australia managed award for service or achievement to the organisation of Engineers Australia or to the engineering profession."""@en ;
    skos:altLabel "EA Award"@en ;
    skos:prefLabel "Engineers Australia Award"@en .

eaj:ea-by-laws a skos:Concept ;
    dcterms:source "https://www.engineersaustralia.org.au/sites/default/files/2023-05/2023-royal-charter-by-laws.pdf"^^xsd:anyURI ;
    rdfs:isDefinedBy <https://ref.engineersaustralia.org.au/def/ea-jargon> ;
    skos:inScheme <https://ref.engineersaustralia.org.au/def/ea-jargon> ;
    skos:topConceptOf <https://ref.engineersaustralia.org.au/def/ea-jargon> ;
    skos:definition """The By-Laws of Engineers Australia are a set of provisions that form the legal 'constitution' and regulation for Engineers Australia operations in conjunction with the Royal Charter"""@en ;
    skos:altLabel "EA By-Laws"@en ;
    skos:prefLabel "Engineers Australia By-Laws"@en .

eaj:ea-event a skos:Concept ;
    dcterms:source "https://linked.data.gov.au/org/engineersaustralia"^^xsd:anyURI ;
    rdfs:isDefinedBy <https://ref.engineersaustralia.org.au/def/ea-awards> ;
    skos:related <https://ref.engineersaustralia.org.au/def/ea-awards> ;
    skos:inScheme <https://ref.engineersaustralia.org.au/def/ea-jargon> ;
    skos:topConceptOf <https://ref.engineersaustralia.org.au/def/ea-jargon> ;
    skos:definition """An EA Event is an organised event that provides information and networking opportunities to the EA membership base. Events typically focus on a theme or single topic such as an Engineering discipline such as civil engineering, a current topic of engineering focus such as renewable energy, a specific skillset such as root cause analysis, a socially focused initative such as gender diversity and equality, professional networking, or membership and career development."""@en ;
    skos:altLabel "EA Event"@en ;
    skos:prefLabel "Engineers Australia Event"@en .

eaj:ea-membership-regulations a skos:Concept ;
    dcterms:source "https://www.engineersaustralia.org.au/membership"^^xsd:anyURI ;
    rdfs:isDefinedBy <https://ref.engineersaustralia.org.au/def/ea-jargon> ;
    skos:inScheme <https://ref.engineersaustralia.org.au/def/ea-jargon> ;
    skos:topConceptOf <https://ref.engineersaustralia.org.au/def/ea-jargon> ;
    skos:definition """The formal regulations approved by the Engineers Australia Council that determine the rules and regulations of membership."""@en ;
    skos:altLabel "EA Membership Regulations"@en ;
    skos:prefLabel "Engineers Australia Membership Regulations"@en .

eaj:ea-activity-roles a skos:Concept ;
    dcterms:source "https://linked.data.gov.au/org/engineersaustralia"^^xsd:anyURI ;
    rdfs:isDefinedBy <https://ref.engineersaustralia.org.au/def/ea-activity-roles> ;
    skos:related <https://ref.engineersaustralia.org.au/def/ea-activity-roles> ;
    skos:inScheme <https://ref.engineersaustralia.org.au/def/ea-jargon> ;
    skos:topConceptOf <https://ref.engineersaustralia.org.au/def/ea-jargon> ;
    skos:definition """The roles an organisation, group, or individual can perform when performing an activity in an interaction with Engineers Australia."""@en ;
    skos:prefLabel "Engineers Australia Roles"@en .

eaj:ea-party-roles a skos:Concept ;
    dcterms:source "https://linked.data.gov.au/org/engineersaustralia"^^xsd:anyURI ;
    rdfs:isDefinedBy <https://ref.engineersaustralia.org.au/def/ea-party-roles> ;
    skos:related <https://ref.engineersaustralia.org.au/def/ea-party-roles> ;
    skos:inScheme <https://ref.engineersaustralia.org.au/def/ea-jargon> ;
    skos:topConceptOf <https://ref.engineersaustralia.org.au/def/ea-jargon> ;
    skos:definition """The relationships between organisations, groups, and individuals within the scope and interest of Engineers Australia."""@en ;
    skos:prefLabel "Engineers Australia Relationships"@en .

eaj:ea-royal-charter a skos:Concept ;
    dcterms:source "https://www.engineersaustralia.org.au/sites/default/files/2023-05/2023-royal-charter-by-laws.pdf"^^xsd:anyURI ;
    rdfs:isDefinedBy <https://ref.engineersaustralia.org.au/def/ea-jargon> ;
    skos:inScheme <https://ref.engineersaustralia.org.au/def/ea-jargon> ;
    skos:topConceptOf <https://ref.engineersaustralia.org.au/def/ea-jargon> ;
    skos:definition """Engineers Australia has operated under a Royal Charter since 1938. It also operates under a set of by-laws to ensure appropriate regulation and fair processes for governing boards and members alike."""@en ;
    skos:altLabel "EA Royal Charter"@en ;
    skos:prefLabel "Engineers Australia Royal Charter"@en .

eaj:event a skos:Concept ;
    dcterms:source "https://www.iso.org/standard/65694.html"^^xsd:anyURI ;
	rdfs:isDefinedBy <https://ref.engineersaustralia.org.au/def/ea-jargon>;
    skos:inScheme <https://ref.engineersaustralia.org.au/def/ea-jargon> ;
    skos:topConceptOf <https://ref.engineersaustralia.org.au/def/ea-jargon> ;
	skos:definition """An occurrence or change of a particular set of circumstances"""@en;
    skos:altLabel "Event (Risk)"@en ;
    skos:prefLabel "Event"@en .

eaj:ewc a skos:Concept ;
    dcterms:source "https://www.engineersaustralia.org.au/employers"^^xsd:anyURI ;
    rdfs:isDefinedBy <https://ref.engineersaustralia.org.au/def/ea-membership-agreements> ;
    skos:inScheme <https://ref.engineersaustralia.org.au/def/ea-jargon> ;
    skos:topConceptOf <https://ref.engineersaustralia.org.au/def/ea-jargon> ;
    skos:definition """EWC is an agreemenent between Engineers Autralia and an organisation for engineering staff to become Chartered or to apply for NER or state registration. Engineers Australia assists with:
    - understand the capabilities in the engineering workforce
    - scope requirements and propose a partnership model
    - create and activate EA memberships
    - guide employees through assessment requirements
    - conduct pre-assessments
    - conduct interview assessments
    - advise applicants of assessment outcomes
    - formalise credentials.
    The Engineers Australia workforce credentialing program also enables a workforce-wide view of the skills and competencies in an organisation's talent pool. This invaluable information helps to fill knowledge gaps and maintain a fully skilled workforce."""@en ;
    skos:notation "EWC" ;
    skos:prefLabel """Engineering Workforce Credentialing"""@en.

eaj:product-feature a skos:Concept ;
    dcterms:source "https://www.harness.io/harness-devops-academy/mastering-software-features-tips-measurement"^^xsd:anyURI ;
	rdfs:isDefinedBy <https://ref.engineersaustralia.org.au/def/ea-jargon>;
    skos:inScheme <https://ref.engineersaustralia.org.au/def/ea-jargon> ;
    skos:topConceptOf <https://ref.engineersaustralia.org.au/def/ea-jargon> ;
	skos:definition """A feature in software development is a specific functionality or capability introduced to satisfy user needs or enhance the products value. Every piece of software is comprised of multiple features, each designed to solve problems, streamline processes, or deliver unique benefits to its users."""@en;
    skos:altLabel "Feature"@en ;
    skos:prefLabel "Product Feature"@en .

eaj:ict-change a skos:Concept ;
    dcterms:source "https://linked.data.gov.au/org/engineersaustralia"^^xsd:anyURI ;
    rdfs:isDefinedBy <https://ref.engineersaustralia.org.au/def/ict-change> ;
    skos:inScheme <https://ref.engineersaustralia.org.au/def/ea-jargon> ;
    skos:topConceptOf <https://ref.engineersaustralia.org.au/def/ea-jargon> ;
    skos:definition """The addition, modification or removal of anything that could have an effect on IT services. The scope should include changes to all architectures, processes, tools, metrics and documentation, as well as changes to IT services and other configuration items."""@en ;
    skos:prefLabel """ICT Change"""@en .

eaj:ict-change-freeze a skos:Concept ;
    dcterms:source "https://linked.data.gov.au/org/engineersaustralia"^^xsd:anyURI ;
    rdfs:isDefinedBy <https://ref.engineersaustralia.org.au/def/ea-jargon> ;
    skos:inScheme <https://ref.engineersaustralia.org.au/def/ea-jargon> ;
    skos:topConceptOf <https://ref.engineersaustralia.org.au/def/ea-jargon> ;
    skos:scopeNote """A change freeze maybe imposed during business-critical periods, which can include any of the following in the context of Engineers Australia:
    - Renewals Period - For all the systems that support Yearly Membership renewal
    - End of Financial year processing - For Finance and Planning Systems
    - During the Performance periods (mid cycle and end of year) - For Human Resources Systems"""@en ;
    skos:definition """At certain critical times of the year, it may be necessary to impose a change freeze period. During these times, only changes deemed essential for business continuity of services will be considered. This is to ensure that the stability and integrity of the system is not compromised during these critical periods.
    
    Change freezes occur during holiday periods when the support teams are not as well resourced, but if the need for an emergency change should arise, then some scope is available."""@en ;
    skos:altLabel "Change Freeze"@en ;
    skos:prefLabel """ICT Change Freeze"""@en .

eaj:ict-change-priority a skos:Concept ;
    dcterms:source "https://linked.data.gov.au/org/engineersaustralia"^^xsd:anyURI ;
    rdfs:isDefinedBy <https://ref.engineersaustralia.org.au/def/ea-jargon> ;
    skos:inScheme <https://ref.engineersaustralia.org.au/def/ea-jargon> ;
    skos:topConceptOf <https://ref.engineersaustralia.org.au/def/ea-jargon> ;
    skos:definition """Priority reflects the relationship between the urgency of the change and the impact to business processes. This will have implications on the scheduling and overall prioritisation of changes."""@en ;
    skos:prefLabel """ICT Change Priority"""@en .

eaj:ict-event a skos:Concept ;
    dcterms:source "https://linked.data.gov.au/org/engineersaustralia"^^xsd:anyURI ;
    rdfs:isDefinedBy <https://ref.engineersaustralia.org.au/def/ea-jargon> ;
    skos:inScheme <https://ref.engineersaustralia.org.au/def/ea-jargon> ;
    skos:topConceptOf <https://ref.engineersaustralia.org.au/def/ea-jargon> ;
    skos:definition """An event that requires the intervention and involvement of the ICT Team."""@en ;
    skos:prefLabel """ICT Service Event"""@en .

    itev:ict-incident a skos:Concept ;
        skos:inScheme <https://ref.engineersaustralia.org.au/def/ea-jargon> ;
        skos:broader eaj:ict-event .

    itev:ict-request a skos:Concept ;
        skos:inScheme <https://ref.engineersaustralia.org.au/def/ea-jargon> ;
        skos:broader eaj:ict-event .

    itev:ict-enhancement a skos:Concept ;
        skos:inScheme <https://ref.engineersaustralia.org.au/def/ea-jargon> ;
        skos:broader eaj:ict-event .

    itev:ict-maintenance a skos:Concept ;
        skos:inScheme <https://ref.engineersaustralia.org.au/def/ea-jargon> ;
        skos:broader eaj:ict-event .

eaj:ict-problem a skos:Concept ;
    dcterms:source "https://wiki.en.it-processmaps.com/index.php/ITIL_Glossary/"^^xsd:anyURI ;
    rdfs:isDefinedBy <https://ref.engineersaustralia.org.au/def/ea-jargon> ;
    skos:inScheme <https://ref.engineersaustralia.org.au/def/ea-jargon> ;
    skos:topConceptOf <https://ref.engineersaustralia.org.au/def/ea-jargon> ;
    skos:definition """A cause of one or more incidents. The cause is not usually known at the time a problem record is created, and the problem management process is responsible for further investigation."""@en ;
    skos:prefLabel """ICT Problem"""@en .

eaj:ict-rfc a skos:Concept ;
    dcterms:source "https://wiki.en.it-processmaps.com/index.php/ITIL_Glossary/"^^xsd:anyURI ;
    rdfs:isDefinedBy <https://ref.engineersaustralia.org.au/def/ea-jargon> ;
    skos:inScheme <https://ref.engineersaustralia.org.au/def/ea-jargon> ;
    skos:topConceptOf <https://ref.engineersaustralia.org.au/def/ea-jargon> ;
    skos:definition """A template to be used when formally requesting a Change. An RFC includes details of the proposed Change."""@en ;
    skos:scopeNote """At EA, an RFC and is undertaken by creating a new change in RemedyForce (Change Module)."""@en ;
    skos:notation "RFC" ;
    skos:altLabel "Request for Change (RFC)"@en ;
    skos:prefLabel """Request for Change"""@en .

eaj:identity-management a skos:Concept ;
    dcterms:source "https://www.vmware.com/topics/glossary/content/identity-management.html"^^xsd:anyURI ;
    rdfs:seeAlso eaj:identity-management-app ;
    rdfs:isDefinedBy <https://ref.engineersaustralia.org.au/def/ea-jargon> ;
    skos:inScheme <https://ref.engineersaustralia.org.au/def/ea-jargon> ;
    skos:topConceptOf <https://ref.engineersaustralia.org.au/def/ea-jargon> ;
    skos:definition """Identity Management ensures that authorized people, and only authorized people, have access to the technology resources they need to perform their job functions. This includes management of enterprise sign-on and permissions management to components with a system."""@en ;
    skos:notation "IAM" ;
    skos:altLabel "Identity and Access Management"@en ;
    skos:prefLabel "Identity Management"@en .

    eaj:identity-validation a skos:Concept ;
        dcterms:source "https://www.experian.co.uk/blogs/latest-thinking/fraud-prevention/what-is-the-difference-between-validation-verification-and-authentication/"^^xsd:anyURI ;
        rdfs:isDefinedBy <https://ref.engineersaustralia.org.au/def/ea-jargon> ;
        skos:inScheme <https://ref.engineersaustralia.org.au/def/ea-jargon> ;
        skos:broader eaj:identity-management, eaj:validation ;
        skos:definition """Identity validation is the first level of identity confirmation in which an individual's personal information, such as their name, address, phone number and email address, are checked to validate that they exist in the real world."""@en ;
        skos:prefLabel "Identity Validation"@en .

    eaj:identity-verification a skos:Concept ;
        dcterms:source "https://www.experian.co.uk/blogs/latest-thinking/fraud-prevention/what-is-the-difference-between-validation-verification-and-authentication/"^^xsd:anyURI ;
        rdfs:isDefinedBy <https://ref.engineersaustralia.org.au/def/ea-jargon> ;
        skos:inScheme <https://ref.engineersaustralia.org.au/def/ea-jargon> ;
        skos:broader eaj:identity-management, eaj:verification ;
        skos:definition """Identity verification is the second level of identity confirmation after validation in which an individual is linked directly to identity data, and verified as genuine through additional checks."""@en ;
        skos:prefLabel "Identity Verification"@en .

    eaj:identity-authentication a skos:Concept ;
        dcterms:source "https://www.experian.co.uk/blogs/latest-thinking/fraud-prevention/what-is-the-difference-between-validation-verification-and-authentication/"^^xsd:anyURI ;
        rdfs:isDefinedBy <https://ref.engineersaustralia.org.au/def/ea-jargon> ;
        skos:inScheme <https://ref.engineersaustralia.org.au/def/ea-jargon> ;
        skos:broader eaj:identity-management ;
        skos:definition """Authentication is the process of checking user identity against information that only the user should have, or know. To check they are who they say they are."""@en ;
        skos:altLabel "Identity Authentication"@en ;
        skos:prefLabel "Authentication"@en .

    eaj:identity-authorisation a skos:Concept ;
        dcterms:source "https://www.experian.co.uk/blogs/latest-thinking/fraud-prevention/what-is-the-difference-between-validation-verification-and-authentication/"^^xsd:anyURI ;
        rdfs:isDefinedBy <https://ref.engineersaustralia.org.au/def/ea-jargon> ;
        skos:inScheme <https://ref.engineersaustralia.org.au/def/ea-jargon> ;
        skos:broader eaj:identity-management ;
        skos:definition """Authorisation is the process of granting a user access to resources (systems, platforms, or data) based on their identity, roles, and permissions."""@en ;
        skos:altLabel "Identity Authorisation"@en,
            "Identity Authorization"@en,
            "Authorization"@en ;
        skos:prefLabel "Authorisation"@en .

eaj:identity-management-app a skos:Concept ;
    dcterms:source "https://www.vmware.com/topics/glossary/content/identity-management.html"^^xsd:anyURI ;
    rdfs:seeAlso eaj:identity-management ;
    rdfs:isDefinedBy <https://ref.engineersaustralia.org.au/def/ea-jargon> ;
    skos:inScheme <https://ref.engineersaustralia.org.au/def/ea-jargon> ;
    skos:topConceptOf <https://ref.engineersaustralia.org.au/def/ea-jargon> ;
    skos:definition """An identity management system prevents unauthorized access to systems and resources, helps prevent exfiltration of enterprise or protected data, and raises alerts and alarms when access attempts are made by unauthorized personnel or programs, whether from inside or outside the enterprise perimeter."""@en ;
    skos:altLabel "Identity and Access Management Application"@en, 
        "Identity Management System"@en,
        "Identity Management Tool"@en;
    skos:prefLabel "Identity Management Application"@en .

eaj:information a skos:Concept ;
    dcterms:source "https://www.diffen.com/difference/Data_vs_Information"^^xsd:anyURI ;
    rdfs:isDefinedBy <https://ref.engineersaustralia.org.au/def/ea-jargon> ;
    skos:inScheme <https://ref.engineersaustralia.org.au/def/ea-jargon> ;
    skos:topConceptOf <https://ref.engineersaustralia.org.au/def/ea-jargon> ;
    skos:definition """When data is processed, organized, structured or presented in a given context so as to make it useful, it is called information.
    
    In practice, information management deals primarily with unstructured and semi-structured data and includes information, records, and document management in an organisation, whereas data management typically deals with the structured data stored in databases and other tabular formats."""@en ;
    skos:prefLabel "Information"@en .

eaj:issue a skos:Concept ;
    dcterms:source "https://wiki.en.it-processmaps.com/index.php/ITIL_Glossary/_ITIL_Terms_P#Problem"^^xsd:anyURI ;
	rdfs:isDefinedBy <https://ref.engineersaustralia.org.au/def/ea-jargon>;
    skos:inScheme <https://ref.engineersaustralia.org.au/def/ea-jargon> ;
    skos:topConceptOf <https://ref.engineersaustralia.org.au/def/ea-jargon> ;
	skos:definition """A cause of one or more Incidents. The cause is not usually known at the time a Problem Record is created."""@en;
    skos:altLabel "Problem"@en ;
    skos:prefLabel "Issue"@en .

eaj:knowledgebase a skos:Concept ;
    dcterms:source "https://www.atlassian.com/itsm/knowledge-management/what-is-a-knowledge-base/"^^xsd:anyURI ;
    rdfs:isDefinedBy <https://ref.engineersaustralia.org.au/def/ea-jargon> ;
    skos:inScheme <https://ref.engineersaustralia.org.au/def/ea-jargon> ;
    skos:topConceptOf <https://ref.engineersaustralia.org.au/def/ea-jargon> ;
    skos:definition """A knowledge base is a self-serve online library of information about a product, service, department, or topic. The data in your knowledge base can come from anywhere. Typically, contributors who are well versed in the relevant subjects add to and expand the knowledge base."""@en ;
    skos:notation "KB" ;
    skos:prefLabel "Knowledgebase"@en .

eaj:least-privilege a skos:Concept ;
    dcterms:source "https://www.okta.com/identity-101/minimum-access-policy/"^^xsd:anyURI ;
    rdfs:isDefinedBy <https://ref.engineersaustralia.org.au/def/ea-jargon> ;
    skos:inScheme <https://ref.engineersaustralia.org.au/def/ea-jargon> ;
    skos:topConceptOf <https://ref.engineersaustralia.org.au/def/ea-jargon> ;
    skos:definition """A minimum access policy restricts a user to only the least amount of access to privileged resources and permissions that are needed to perform an authorized activity or activities, such as those necessary for employees to do their jobs. This is a cybersecurity practice that can help to protect critical assets and sensitive data. This is also known as the Principle of Least Privilege.
    
    The minimum access policy allows a process or a user account to have only the privileges that are necessary to perform their intended function. Typically, this will mean setting the least amount of access as the default and only opening up permissions and privileges to essential resources and actions. User accounts should run and launch applications with the minimum number of privileges possible."""@en ;
    skos:altLabel "Minimium Access Policy"@en,
        "Minimum Access"@en,
        "Principle of Least Privilege" ;
    skos:prefLabel "Least Privilege"@en .

eaj:likelihood a skos:Concept ;
    dcterms:source "https://www.iso.org/standard/65694.html"^^xsd:anyURI ;
	rdfs:isDefinedBy <https://linked.data.gov.au/def/event-probability> ;
	rdfs:seeAlso <https://linked.data.gov.au/def/event-probability>;
    skos:inScheme <https://ref.engineersaustralia.org.au/def/ea-jargon> ;
    skos:topConceptOf <https://ref.engineersaustralia.org.au/def/ea-jargon> ;
	skos:definition """Chance of something happening"""@en;
    skos:altLabel "Event Likelihood"@en ;
    skos:prefLabel "Likelihood"@en .

eaj:master-data-management a skos:Concept ;
    dcterms:source "https://linked.data.gov.au/org/engineersaustralia"^^xsd:anyURI ;
    rdfs:isDefinedBy <https://ref.engineersaustralia.org.au/def/ea-jargon> ;
    skos:related eaj:master-data ;
    skos:inScheme <https://ref.engineersaustralia.org.au/def/ea-jargon> ;
    skos:topConceptOf <https://ref.engineersaustralia.org.au/def/ea-jargon> ;
    skos:definition """Master data management (MDM) focuses on creating and maintaining accurate, consistent, and reliable master data across different systems and applications. It is a technology-enabled discipline that ensures the uniformity, accuracy, stewardship, semantic consistency and accountability of the enterprise's official shared master data assets. Where Master Data refers to a set of core non-transactional data elements that are shared across multiple applications or business processes within an organization, Master Data Management controls which instance of master data is considered the mastered version and source-of-truth to be referred to or (where essential) replicated from and synchronised with."""@en ;
    skos:notation "MDM" ;
    skos:prefLabel "Master Data Management"@en .

eaj:membership-change a skos:Concept ;
    dcterms:source "https://linked.data.gov.au/org/engineersaustralia"^^xsd:anyURI ;
    rdfs:isDefinedBy <https://ref.engineersaustralia.org.au/def/ea-member-changes> ;
    skos:related <https://ref.engineersaustralia.org.au/def/ea-member-changes> ;
    skos:inScheme <https://ref.engineersaustralia.org.au/def/ea-jargon> ;
    skos:topConceptOf <https://ref.engineersaustralia.org.au/def/ea-jargon> ;
    skos:definition """The changes possible to membership status between non-members, active members, and past members intersecting with paid vs unpaid memberships withspecial considerations for students and honorary fellows. Membership churn risk also augmented with specific classes based on payment status in the context of member retention and erasure."""@en ;
    skos:prefLabel "Engineers Australia Membership Changes"@en .

eaj:membership-grade a skos:Concept ;
    dcterms:source "https://www.engineersaustralia.org.au/membership/member"^^xsd:anyURI ;
    rdfs:isDefinedBy <https://ref.engineersaustralia.org.au/def/ea-membership-grade> ;
    skos:related <https://ref.engineersaustralia.org.au/def/ea-membership-grade> ;
    skos:inScheme <https://ref.engineersaustralia.org.au/def/ea-jargon> ;
    skos:topConceptOf <https://ref.engineersaustralia.org.au/def/ea-jargon> ;
    skos:definition """The grade of membership of Engineers Australia. Grade reflects the experience and skill level of a member and corresponds to a specific level of EA Membership.
    The grades are:
        - Student
        - Graduate
        - Member
        - Fellow
        - Affiliate
        - Companion
        - Honorary Fellow."""@en ;
    skos:prefLabel "Engineers Australia Membership Grade"@en .

eaj:mfa a skos:Concept ;
    dcterms:source "https://www.cyber.gov.au/protect-yourself/securing-your-accounts/multi-factor-authentication"^^xsd:anyURI ;
    rdfs:isDefinedBy <https://linked.data.gov.au/def/australian-qualifications-framework> ;
    skos:inScheme <https://ref.engineersaustralia.org.au/def/ea-jargon> ;
    skos:topConceptOf <https://ref.engineersaustralia.org.au/def/ea-jargon> ;
    skos:definition """Multi-factor authentication (MFA) is a security measure that requires two or more proofs of identity to grant you access. Multi-factor authentication typically requires a combination of something the user knows (PIN, secret question), something you have (card, token) or something you are (fingerprint or other biometric)."""@en ;
    skos:notation "MFA" ;
    skos:altLabel "MFA"@en ;
    skos:prefLabel "Multi-factor authentication"@en .

eaj:monitoring a skos:Concept ;
    dcterms:source "https://www.iso.org/standard/65694.html"^^xsd:anyURI ;
	rdfs:isDefinedBy <https://ref.engineersaustralia.org.au/def/ea-jargon>;
    skos:inScheme <https://ref.engineersaustralia.org.au/def/ea-jargon> ;
    skos:topConceptOf <https://ref.engineersaustralia.org.au/def/ea-jargon> ;
	skos:definition """Continual checking, supervising, critically observing or determining the status in order to identify change from the performance level required or expected."""@en;
    skos:prefLabel "Monitoring"@en .

eaj:ner a skos:Concept ;
    dcterms:source "https://www.engineersaustralia.org.au/credentials/registration/national-engineering-register"^^xsd:anyURI ;
    rdfs:seeAlso <https://ref.engineersaustralia.org.au/def/areasofpractice/areas-of-practice-ner> ;
	rdfs:isDefinedBy <https://ref.engineersaustralia.org.au/def/ea-jargon>;
    skos:inScheme <https://ref.engineersaustralia.org.au/def/ea-jargon> ;
    skos:topConceptOf <https://ref.engineersaustralia.org.au/def/ea-jargon> ;
	skos:definition """Engineers Australia introduced the National Engineering Register (NER) in 2015. This comprehensive directory is a way to recognise engineers who meet the high standards of skill, qualification and professionalism expected in the industry.
    
    It provides a national framework of registration for professional engineers, engineering technologists and engineering associates across the private and public sectors.
    
    As a publicly-searchable database, the NER gives individuals and businesses access to a qualified pool of engineers, endorsed by Australia's engineering peak body."""@en;
    skos:notation "NER" ;
    skos:prefLabel "National Engineering Register"@en .

eaj:occupational-categories a skos:Concept ;
    dcterms:source "https://linked.data.gov.au/org/engineersaustralia"^^xsd:anyURI ;
    rdfs:isDefinedBy <https://linked.data.gov.au/def/iea-occupational-categories> ;
    skos:related <https://linked.data.gov.au/def/iea-occupational-categories> ;
    skos:inScheme <https://ref.engineersaustralia.org.au/def/ea-jargon> ;
    skos:topConceptOf <https://ref.engineersaustralia.org.au/def/ea-jargon> ;
    skos:definition """A category reflecting the level and type of engineering qualification held by a member of the engineering profession, as per the International Engineering Alliance Educational Accords. This include Engineering Associate, Engineering Technologist, and Professional Engineer."""@en ;
    skos:altLabel "International Engineering Accords Membership"@en,
        "Occupational Categories"@en ;
    skos:prefLabel "International Engineering Alliance Occupational Categories"@en .

    eaj:mra-occupational-categories a skos:Concept ;
        dcterms:source "https://linked.data.gov.au/org/engineersaustralia"^^xsd:anyURI ;
        rdfs:isDefinedBy <https://ref.engineersaustralia.org.au/def/ea-jargon> ;
        skos:related <https://linked.data.gov.au/def/iea-occupational-categories> ;
        skos:inScheme <https://ref.engineersaustralia.org.au/def/ea-jargon> ;
        skos:broader eaj:occupational-categories ;
        skos:definition """An MRA Occupational category is a translation between a specific MRA Occupational Category and the equivalent Engineers Australia Occupational Category."""@en ;
        skos:prefLabel "MRA Occupational Categories"@en .

eaj:offering a skos:Concept ;
    dcterms:source "https://opentext.wsu.edu/marketing/chapter/8-1-what-composes-an-offering/"^^xsd:anyURI ;
    rdfs:isDefinedBy <https://ref.engineersaustralia.org.au/def/ea-jargon> ;
    skos:inScheme <https://ref.engineersaustralia.org.au/def/ea-jargon> ;
    skos:topConceptOf <https://ref.engineersaustralia.org.au/def/ea-jargon> ;
    skos:definition """Offerings are products and services designed to deliver value to customers. Either to fulfill their needs, satisfy their wants, or both. Offerings are anything that delivers value to known stakeholders, users, or customers. This may be a service, a physical product, or an abstract product such as a qualification or title."""@en ;
    skos:scopeNote """Offerings are equivalent to the Scrum and Agile term Product."""@en ;
    skos:prefLabel "Offering"@en .

    eaj:product a skos:Concept ;
        dcterms:source "https://chisellabs.com/glossary/what-is-a-product-offering/"^^xsd:anyURI ;
        rdfs:isDefinedBy <https://ref.engineersaustralia.org.au/def/ea-jargon> ;
        skos:inScheme <https://ref.engineersaustralia.org.au/def/ea-jargon> ;
        skos:definition """A product offering refers to an item that you sell to customers, such as a tangible physical product or software, or it may refer to an intangible title, status, or registration such authorised recognition as a qualified professional."""@en ;
        skos:scopeNote """In Scrum and Agile terminology a Product encompasses both Products and Services and is therefore conceptually equivalent to the general concept of an Offering."""@en ;
        skos:prefLabel "Product"@en ;
        skos:broader eaj:offering .

        eaj:product-physical a skos:Concept ;
            dcterms:source "https://linked.data.gov.au/org/engineersaustralia"^^xsd:anyURI ;
            rdfs:isDefinedBy <https://ref.engineersaustralia.org.au/def/ea-jargon> ;
            skos:inScheme <https://ref.engineersaustralia.org.au/def/ea-jargon> ;
            skos:broader eaj:product ;
            skos:definition """A tangible output that provides value through its access and/or use. Example: Create Magazine."""@en ;
            skos:prefLabel "Physical Product"@en .

        eaj:product-intangible a skos:Concept ;
            dcterms:source "https://linked.data.gov.au/org/engineersaustralia"^^xsd:anyURI ;
            rdfs:isDefinedBy <https://ref.engineersaustralia.org.au/def/ea-jargon> ;
            skos:inScheme <https://ref.engineersaustralia.org.au/def/ea-jargon> ;
            skos:broader eaj:product ;
            skos:definition """An intangible output that provides value through its ownership or association. Example: Memberships, Titles, Status, Registration, Usage Rights."""@en ;
            skos:prefLabel "Intangible Product"@en .

            eaj:product-digital a skos:Concept ;
                dcterms:source "https://linked.data.gov.au/org/engineersaustralia"^^xsd:anyURI ;
                rdfs:isDefinedBy <https://ref.engineersaustralia.org.au/def/ea-jargon> ;
                skos:inScheme <https://ref.engineersaustralia.org.au/def/ea-jargon> ;
                skos:broader eaj:product-intangible ;
                skos:definition """A software output that provides value through its access and/or use. Typically made available through one or more underlying technologies, other digital products or data products. Example: EEA Online Dashboard; EEA Online Course (e.g., Systems Thinking in Engineering)."""@en ;
                skos:prefLabel "Digital Product"@en .

            eaj:product-data a skos:Concept ;
                dcterms:source "https://linked.data.gov.au/org/engineersaustralia"^^xsd:anyURI ;
                rdfs:isDefinedBy <https://ref.engineersaustralia.org.au/def/ea-jargon> ;
                skos:inScheme <https://ref.engineersaustralia.org.au/def/ea-jargon> ;
                skos:broader eaj:product-intangible ;
                skos:definition """A self-contained output that answers a business question; may be directly consumed or bundled in relevant digital products or services; are typically made available through one or more underlying technologies. Example: EA People Pulse Survey Summary (Results)."""@en ;
                skos:scopeNote """At EA, consumers of Data Products are primarily internal to the organisation."""@en ;
                skos:prefLabel "Data Product"@en .

    eaj:service a skos:Concept ;
        dcterms:source "https://chisellabs.com/glossary/what-is-a-product-offering/"^^xsd:anyURI ;
        rdfs:isDefinedBy <https://ref.engineersaustralia.org.au/def/ea-jargon> ;
        skos:inScheme <https://ref.engineersaustralia.org.au/def/ea-jargon> ;
        skos:broader eaj:offering ;
        skos:definition """A service offering involves providing intangible services or expertise to customers, such as consulting, maintenance, or professional services. Services are processes and activities undertaken on behalf of a customer."""@en ;
        skos:prefLabel "Service"@en .

        eaj:service-high-touch a skos:Concept ;
            dcterms:source "https://linked.data.gov.au/org/engineersaustralia"^^xsd:anyURI ;
            rdfs:isDefinedBy <https://ref.engineersaustralia.org.au/def/ea-jargon> ;
            skos:inScheme <https://ref.engineersaustralia.org.au/def/ea-jargon> ;
            skos:broader eaj:service ;
            skos:definition """Provides value to consumers through assisted access (e.g., via Business Processes) to resources and information. May bundle relevant physical products, digital products, data products and/or other services. Example: EngInsure Claim Lodgement; Engineer Registration; Chartered Assessment."""@en ;
            skos:prefLabel "High-Touch Service"@en .

        eaj:service-low-touch a skos:Concept ;
            dcterms:source "https://linked.data.gov.au/org/engineersaustralia"^^xsd:anyURI ;
            rdfs:isDefinedBy <https://ref.engineersaustralia.org.au/def/ea-jargon> ;
            skos:inScheme <https://ref.engineersaustralia.org.au/def/ea-jargon> ;
            skos:broader eaj:service ;
            skos:definition """Like a High-Touch Service, except that a consumer may access resources and information without assistance (e.g., via a given Role or Business Process); usually via a digital channel (e.g., portal/web page/app). Example: Meeting Room Booking via Outlook 365."""@en ;
            skos:altLabel "Self-Service"@en ;
            skos:prefLabel "Low-Touch Service"@en .

eaj:pcas a skos:Concept ;
    dcterms:source "https://linked.data.gov.au/org/engineersaustralia"^^xsd:anyURI ;
    rdfs:isDefinedBy <https://ref.engineersaustralia.org.au/def/ea-jargon> ;
    skos:inScheme <https://ref.engineersaustralia.org.au/def/ea-jargon> ;
    skos:topConceptOf <https://ref.engineersaustralia.org.au/def/ea-jargon> ;
    skos:definition """A scheme managed by the Engineers Australia for professional engineers (you must be on the NPER Register to be an Accredited Certifier) who want to be accredited as Private Certifiers under the Environmental Planning and Assessment ACT (NSW) 1979 (the EPA Act). Please contact the Registration & Practice Team for more information about the scheme. This scheme was transferred to the NSW State Government Building Professionals Board on 1 March 2007."""@en ;
    skos:notation "PCAS" ;
    skos:prefLabel "Private Certifier Accreditation Scheme"@en .

eaj:personal-information a skos:Concept ;
    dcterms:source "https://www.oaic.gov.au/privacy/privacy-guidance-for-organisations-and-government-agencies/handling-personal-information/what-is-personal-information"^^xsd:anyURI ;
    rdfs:isDefinedBy <https://ref.engineersaustralia.org.au/def/ea-jargon> ;
    skos:inScheme <https://ref.engineersaustralia.org.au/def/ea-jargon> ;
    skos:topConceptOf <https://ref.engineersaustralia.org.au/def/ea-jargon> ;
    skos:definition """Information or an opinion about an identified individual, or an individual who is reasonably identifiable:
    whether the information or opinion is true or not; and
    whether the information or opinion is recorded in a material form or not."""@en ;
    skos:prefLabel "Personal Information"@en .

eaj:personally-identifiable-information a skos:Concept ;
    dcterms:source "https://www.oaic.gov.au/privacy/privacy-guidance-for-organisations-and-government-agencies/handling-personal-information/what-is-personal-information"^^xsd:anyURI ;
    rdfs:isDefinedBy <https://ref.engineersaustralia.org.au/def/ea-jargon> ;
    skos:related <https://linked.data.gov.au/def/identifying-information> ;
    skos:inScheme <https://ref.engineersaustralia.org.au/def/ea-jargon> ;
    skos:topConceptOf <https://ref.engineersaustralia.org.au/def/ea-jargon> ;
    skos:definition """Personally identifiable information (PII) refers to details that can be used to confirm who you are or how to find you. Where personal information includes all details about a person who can be identified, PII is the specific information that can be used to make an identity connection.
    
    Personally identifiable information is any piece of information or data that can help to confirm who an individual is or how to find them. It may be identifying information on its own (direct identification) or in context with other information (indirect identification)."""@en ;
    skos:notation "PII" ;
    skos:prefLabel "Personally Identifiable Information"@en .

eaj:persistent-identifier a skos:Concept ;
    dcterms:source "https://github.com/geological-survey-of-queensland/persistent-identifiers/"^^xsd:anyURI ;
    rdfs:isDefinedBy <https://ref.engineersaustralia.org.au/def/ea-jargon> ;
    skos:inScheme <https://ref.engineersaustralia.org.au/def/ea-jargon> ;
    skos:topConceptOf <https://ref.engineersaustralia.org.au/def/ea-jargon> ;
    skos:definition """An identifier (ID) is any label used to uniquely name a thing (person, place, event), whether online or offline. URLs are an example of an identifier, as are serial numbers or personal names. A persistent identifier (PID) is an identifier that is guaranteed to be managed and kept up to date to reliably point to an individual or unique digital or physical entity."""@en ;
    skos:notation "PID" ;
    skos:altLabel "Global Unique Identifier"@en ;
    skos:prefLabel "Persistent Identifier"@en .

eaj:post-nominals a skos:Concept ;
    dcterms:source "https://linked.data.gov.au/org/engineersaustralia"^^xsd:anyURI ;
    dcterms:references <https://en.wikipedia.org/wiki/List_of_post-nominal_letters_(Australia)>,
        <https://www.stylemanual.gov.au/grammar-punctuation-and-conventions/titles-honours-forms-address/awards-and-honours>,
        <https://www.pmc.gov.au/honours-and-symbols/australian-honours-system/post-nominals> ;
    rdfs:isDefinedBy <https://ref.engineersaustralia.org.au/def/ea-jargon> ;
    skos:inScheme <https://ref.engineersaustralia.org.au/def/ea-jargon> ;
    skos:topConceptOf <https://ref.engineersaustralia.org.au/def/ea-jargon> ;
    skos:definition """Letters and notations placed following a person's last name to indicate education qualifications, title of office, decoration or honour. Postnominals include abbreviations of an award or awarding institution. 
    
    Post nominals follow an order of preference as per the following simplified heirarchy:
    - post-nominals for honours and awards
    - state appointments of King's Counsel (KC) or Senior Counsel (SC) or Justice of the Peace (JP)
    - university degrees and diplomas
    - membership of professional associations
    - membership of parliament
    - military post nominals."""@en ;
    skos:prefLabel "Post Nominals"@en .

    eaj:post-nominals-commonwealth-honours-awards a skos:Concept ;
        dcterms:source "https://www.pmc.gov.au/honours-and-symbols/australian-honours-system/post-nominals"^^xsd:anyURI ;
        rdfs:isDefinedBy <https://ref.engineersaustralia.org.au/def/ea-jargon> ;
        skos:inScheme <https://ref.engineersaustralia.org.au/def/ea-jargon> ;
        skos:broader eaj:post-nominals ;
        skos:definition """Post Nominals for honours and awards include those conferred by the Australian Commonwealth. These include current National and former Imperial honours. Examples include the Victoria Cross (VC), Member of the Order of Australia (AM) and the Conspicuous Service Medal (CSM)."""@en ;
        skos:prefLabel "Post Nominals - Commonwealth Honours and Awards"@en .

    eaj:post-nominals-state-appointments a skos:Concept ;
        dcterms:source "https://www.stylemanual.gov.au/grammar-punctuation-and-conventions/titles-honours-forms-address/awards-and-honours"^^xsd:anyURI ;
        rdfs:isDefinedBy <https://ref.engineersaustralia.org.au/def/ea-jargon> ;
        skos:inScheme <https://ref.engineersaustralia.org.au/def/ea-jargon> ;
        skos:broader eaj:post-nominals ;
        skos:definition """Post Nominals for appointments conferred by the Australian States and Territories. These include King's Counsel (KC)/Queens Counsel (QC), Senior Counsel (SC), and Justice of the Peace (JP)."""@en ;
        skos:altLabel "Official Appointments"@en,
            "Official Appointment Post Nominals"@en ;
        skos:prefLabel "Post Nominals - State and Territory Appointments"@en .

    eaj:post-nominals-qualifications a skos:Concept ;
        dcterms:source "https://www.stylemanual.gov.au/grammar-punctuation-and-conventions/titles-honours-forms-address/awards-and-honours"^^xsd:anyURI ;
        rdfs:isDefinedBy <https://ref.engineersaustralia.org.au/def/ea-jargon> ;
        rdfs:seeAlso <https://linked.data.gov.au/def/australian-qualifications-framework/> ;
        skos:inScheme <https://ref.engineersaustralia.org.au/def/ea-jargon> ;
        skos:broader eaj:post-nominals ;
        skos:definition """Academic Qualifications confer Post Nominals according to the Australian Qualifications Framework ordered from lowest-to-highest, then in chronological order within those groups."""@en ;
        skos:prefLabel "Post Nominals - Academic Qualifications"@en .

    eaj:post-nominals-memberships a skos:Concept ;
        dcterms:source "https://www.stylemanual.gov.au/grammar-punctuation-and-conventions/titles-honours-forms-address/awards-and-honours"^^xsd:anyURI ;
        rdfs:isDefinedBy <https://ref.engineersaustralia.org.au/def/ea-jargon> ;
        skos:inScheme <https://ref.engineersaustralia.org.au/def/ea-jargon> ;
        skos:broader eaj:post-nominals ;
        skos:definition """Professional and Academic bodies may confer post-nominals to their members and fellows. When displaying post-nominals fellowships appear before memberships."""@en ;
        skos:altLabel "Post Nominals - Memberships and Fellowships"@en ;
        skos:prefLabel "Post Nominals - Memberships"@en . 

        eaj:post-nominals-ea a skos:Concept ;
            dcterms:source "https://www.engineersaustralia.org.au/membership/member"^^xsd:anyURI ;
            rdfs:isDefinedBy <https://ref.engineersaustralia.org.au/def/ea-jargon> ;
            skos:inScheme <https://ref.engineersaustralia.org.au/def/ea-jargon> ;
            skos:broader eaj:post-nominals-memberships ;
            skos:definition """An Engineers Australia Post Nominal is a specific type of Post Nominal that EA can offer to its Members. Each member may only have one membership post-nominal at any one time."""@en ;
            skos:editorialNote "Post nominals are granted based on member attributes such as grade and occupational categories. They are derived constructs dependent on a member satisfying specified conditions. They are therefore not an independent attribute or primary data content."@en ;
            skos:prefLabel "Engineers Australia Post Nominals"@en .
            
            eaj:AffilIEAust a skos:Concept ;
                dcterms:source "https://linked.data.gov.au/org/engineersaustralia"^^xsd:anyURI ;
                rdfs:isDefinedBy <https://ref.engineersaustralia.org.au/def/ea-membership-grade> ;
                skos:related <https://ref.engineersaustralia.org.au/def/ea-membership-grade/affiliate> ;
                skos:inScheme <https://ref.engineersaustralia.org.au/def/ea-jargon> ;
                skos:broader eaj:post-nominals-ea ;
                skos:definition """A member of Engineers Australia who is not part of the engineering profession and is therefore ineligible to be a Fellow, Member, Graduate or Student, but who has an interest in the engineering profession. Similar to Member grade for a non-engineer."""@en ;
                skos:notation "AffilIEAust" ;
                skos:altLabel "AffilIEAust"@en ;
                skos:prefLabel "Affiliate of the Institute of Engineers Australia"@en .

            eaj:AFIEAust a skos:Concept ;
                dcterms:source "https://linked.data.gov.au/org/engineersaustralia"^^xsd:anyURI ;
                rdfs:isDefinedBy <https://ref.engineersaustralia.org.au/def/ea-jargon> ;
                skos:related <https://linked.data.gov.au/def/iea-occupational-categories/assoc-engineer> ;
                skos:related <https://ref.engineersaustralia.org.au/def/ea-membership-grade/fellow> ;
                skos:inScheme <https://ref.engineersaustralia.org.au/def/ea-jargon> ;
                skos:broader eaj:post-nominals-ea ;
                skos:definition """A member of Engineers Australia and very experienced engineer who has made a significant contribution to the profession, who holds a 2 Years Australian Advanced Diploma or Associated Degree in Engineering."""@en ;
                skos:notation "AFIEAust" ;
                skos:altLabel "AFIEAust"@en ;
                skos:prefLabel "Engineering Associate Fellow of the Institute of Engineers Australia"@en .

            eaj:AMIEAust a skos:Concept ;
                dcterms:source "https://linked.data.gov.au/org/engineersaustralia"^^xsd:anyURI ;
                rdfs:isDefinedBy <https://ref.engineersaustralia.org.au/def/ea-jargon> ;
                skos:related <https://linked.data.gov.au/def/iea-occupational-categories/assoc-engineer> ;
                skos:related <https://ref.engineersaustralia.org.au/def/ea-membership-grade/member> ;
                skos:inScheme <https://ref.engineersaustralia.org.au/def/ea-jargon> ;
                skos:broader eaj:post-nominals-ea ;
                skos:definition """A member of the Institute of Engineers Australia who has surpassed graduate membership but has not reached the level of experience of a Fellow, who holds a 2 Years Australian Advanced Diploma or Associated Degree in Engineering."""@en ;
                skos:notation "AMIEAust" ;
                skos:altLabel "AMIEAust"@en ;
                skos:prefLabel "Engineering Associate Member of the Institute of Engineers Australia"@en .

            eaj:GradAIEAust a skos:Concept ;
                dcterms:source "https://linked.data.gov.au/org/engineersaustralia"^^xsd:anyURI ;
                rdfs:isDefinedBy <https://ref.engineersaustralia.org.au/def/ea-jargon> ;
                skos:related <https://linked.data.gov.au/def/iea-occupational-categories/assoc-engineer> ;
                skos:related <https://ref.engineersaustralia.org.au/def/ea-membership-grade/graduate> ;
                skos:inScheme <https://ref.engineersaustralia.org.au/def/ea-jargon> ;
                skos:broader eaj:post-nominals-ea ;
                skos:definition """A member of the Institute of Engineers Australia prior to transitioning full professional membership. An Engineer with less than 3 years of relevant work experience according the the rules of membership who holds a 2 Years Australian Advanced Diploma or Associated Degree in Engineering."""@en ;
                skos:notation "GradAIEAust" ;
                skos:altLabel "GradAIEAust"@en ;
                skos:prefLabel "Engineering Associate Graduate of the Institute of Engineers Australia"@en .

            eaj:CEngA a skos:Concept ;
                dcterms:source "https://linked.data.gov.au/org/engineersaustralia"^^xsd:anyURI ;
                rdfs:isDefinedBy <https://ref.engineersaustralia.org.au/def/ea-jargon> ;
                skos:related <https://ref.engineersaustralia.org.au/def/ea-engineering-credentials/chartered> ;
                skos:related <https://linked.data.gov.au/def/iea-occupational-categories/assoc-engineer> ;
                skos:inScheme <https://ref.engineersaustralia.org.au/def/ea-jargon> ;
                skos:broader eaj:post-nominals-ea ;
                skos:definition """A person who holds a 2 Years Australian Advanced Diploma or Associated Degree in Engineering and has received Chartered status through an Engineers Australia assessment."""@en ;
                skos:notation "CEngA" ;
                skos:prefLabel "Chartered Engineering Associate"@en .

                eaj:CEngARet a skos:Concept ;
                    dcterms:source "https://linked.data.gov.au/org/engineersaustralia"^^xsd:anyURI ;
                    rdfs:isDefinedBy <https://ref.engineersaustralia.org.au/def/ea-jargon> ;
                    skos:related <https://ref.engineersaustralia.org.au/def/ea-engineering-credentials/chartered-ret> ;
                    skos:related <https://linked.data.gov.au/def/iea-occupational-categories/assoc-engineer> ;
                    skos:inScheme <https://ref.engineersaustralia.org.au/def/ea-jargon> ;
                    skos:broader eaj:CEngA ;
                    skos:definition """A person who has retired from the engineering profession having held a 2 Years Australian Advanced Diploma or Associated Degree in Engineering and having received Chartered status through an Engineers Australia assessment."""@en ;
                    skos:notation "CEngA(Ret)" ;
                    skos:prefLabel "Chartered Engineering Associate - Retired"@en .

            eaj:CEngT a skos:Concept ;
                dcterms:source "https://linked.data.gov.au/org/engineersaustralia"^^xsd:anyURI ;
                rdfs:isDefinedBy <https://ref.engineersaustralia.org.au/def/ea-jargon> ;
                skos:related <https://ref.engineersaustralia.org.au/def/ea-engineering-credentials/chartered> ;
                skos:related <https://linked.data.gov.au/def/iea-occupational-categories/tech-engineer> ;
                skos:inScheme <https://ref.engineersaustralia.org.au/def/ea-jargon> ;
                skos:broader eaj:post-nominals-ea ;
                skos:definition """A person who holds a 3 Years accredited Bachelor of Engineering Technology (BTech) and has received Chartered status through an Engineers Australia assessment."""@en ;
                skos:notation "CEngT" ;
                skos:prefLabel "Chartered Engineering Technologist"@en .

                eaj:CEngTRet a skos:Concept ;
                    dcterms:source "https://linked.data.gov.au/org/engineersaustralia"^^xsd:anyURI ;
                    rdfs:isDefinedBy <https://ref.engineersaustralia.org.au/def/ea-jargon> ;
                    skos:related <https://ref.engineersaustralia.org.au/def/ea-engineering-credentials/chartered-ret> ;
                    skos:related <https://linked.data.gov.au/def/iea-occupational-categories/tech-engineer> ;
                    skos:inScheme <https://ref.engineersaustralia.org.au/def/ea-jargon> ;
                    skos:broader eaj:CEngT ;
                    skos:definition """A person who has retired from the engineering profession having held a 3 Years accredited Bachelor of Engineering Technology (BTech) and having received Chartered status through an Engineers Australia assessment."""@en ;
                    skos:notation "CEngT(Ret)" ;
                    skos:prefLabel "Chartered Engineering Technologist - Retired"@en .

            eaj:CPEng a skos:Concept ;
                dcterms:source "https://linked.data.gov.au/org/engineersaustralia"^^xsd:anyURI ;
                rdfs:isDefinedBy <https://ref.engineersaustralia.org.au/def/ea-jargon> ;
                skos:related <https://ref.engineersaustralia.org.au/def/ea-engineering-credentials/chartered> ;
                skos:related <https://linked.data.gov.au/def/iea-occupational-categories/pro-engineer> ;
                skos:inScheme <https://ref.engineersaustralia.org.au/def/ea-jargon> ;
                skos:broader eaj:post-nominals-ea ;
                skos:definition """A person who holds a 4 Years accredited Bachelor of Engineering (BEng) and has received Chartered status through an Engineers Australia assessment."""@en ;
                skos:notation "CPEng" ;
                skos:prefLabel "Chartered Professional Engineer"@en .

                eaj:CPEngRet a skos:Concept ;
                    dcterms:source "https://linked.data.gov.au/org/engineersaustralia"^^xsd:anyURI ;
                    rdfs:isDefinedBy <https://ref.engineersaustralia.org.au/def/ea-jargon> ;
                    skos:related <https://ref.engineersaustralia.org.au/def/ea-engineering-credentials/chartered-ret> ;
                    skos:related <https://linked.data.gov.au/def/iea-occupational-categories/pro-engineer> ;
                    skos:inScheme <https://ref.engineersaustralia.org.au/def/ea-jargon> ;
                    skos:broader eaj:CPEng ;
                    skos:definition """A person who has retired from the engineering profession having held a 4 Years accredited Bachelor of Engineering (BEng) and having received Chartered status through an Engineers Australia assessment."""@en ;
                    skos:notation "CPEng(Ret)" ;
                    skos:prefLabel "Chartered Professional Engineer - Retired"@en .

            eaj:CompIEAust a skos:Concept ;
                dcterms:source "https://linked.data.gov.au/org/engineersaustralia"^^xsd:anyURI ;
                rdfs:isDefinedBy <https://ref.engineersaustralia.org.au/def/ea-membership-grade> ;
                skos:related <https://ref.engineersaustralia.org.au/def/ea-membership-grade/companion> ;
                skos:inScheme <https://ref.engineersaustralia.org.au/def/ea-jargon> ;
                skos:broader eaj:post-nominals-ea ;
                skos:definition """A member of Engineers Australia who is not part of the engineering profession and is therefore ineligible to be a Fellow, Member, Graduate or Student, but who has an interest in the engineering profession and has made a significant contribution. Similar to Fellow grade for a non-engineer."""@en ;
                skos:notation "CompIEAust" ;
                skos:prefLabel "Companion of the Institute of Engineers Australia"@en .

            eaj:FIEAust a skos:Concept ;
                dcterms:source "https://linked.data.gov.au/org/engineersaustralia"^^xsd:anyURI ;
                rdfs:isDefinedBy <https://ref.engineersaustralia.org.au/def/ea-jargon> ;
                skos:related <https://ref.engineersaustralia.org.au/def/ea-membership-grade/fellow> ;
                skos:related <https://linked.data.gov.au/def/iea-occupational-categories/pro-engineer> ;
                skos:inScheme <https://ref.engineersaustralia.org.au/def/ea-jargon> ;
                skos:broader eaj:post-nominals-ea ;
                skos:definition """A member of Engineers Australia and very experienced engineer who has made a significant contribution to the profession, and who holds a 4 Years accredited Bachelor of Engineering (BEng)."""@en ;
                skos:notation "FIEAust" ;
                skos:prefLabel "Professional Engineer Fellow of the Institute of Engineers Australia"@en .

            eaj:GradIEAust a skos:Concept ;
                dcterms:source "https://linked.data.gov.au/org/engineersaustralia"^^xsd:anyURI ;
                rdfs:isDefinedBy <https://ref.engineersaustralia.org.au/def/ea-membership-grade> ;
                skos:related <https://ref.engineersaustralia.org.au/def/ea-membership-grade/graduate> ;
                skos:inScheme <https://ref.engineersaustralia.org.au/def/ea-jargon> ;
                skos:broader eaj:post-nominals-ea ;
                skos:definition """A member of the Institute of Engineers Australia prior to transitioning full professional membership. An Engineer with less than 3 years of relevant work experience according the the rules of membership but who holds a 4 Years accredited Bachelor of Engineering (BEng)."""@en ;
                skos:notation "GradIEAust" ;
                skos:prefLabel "Professional Engineer Graduate of the Institute of Engineers Australia"@en .

            eaj:MIEAust a skos:Concept ;
                dcterms:source "https://linked.data.gov.au/org/engineersaustralia"^^xsd:anyURI ;
                rdfs:isDefinedBy <https://ref.engineersaustralia.org.au/def/ea-jargon> ;
                skos:related <https://ref.engineersaustralia.org.au/def/ea-membership-grade/member> ;
                skos:related <https://linked.data.gov.au/def/iea-occupational-categories/pro-engineer> ;
                skos:inScheme <https://ref.engineersaustralia.org.au/def/ea-jargon> ;
                skos:broader eaj:post-nominals-ea ;
                skos:definition """A member of the Institute of Engineers Australia who has surpassed graduate membership but has not reached the level of experience of a Fellow, and who holds a 4 Years accredited Bachelor of Engineering (BEng)."""@en ;
                skos:notation "MIEAust" ;
                skos:prefLabel "Professional Engineer Member of the Institute of Engineers Australia"@en .

            eaj:StudIEAust a skos:Concept ;
                dcterms:source "https://linked.data.gov.au/org/engineersaustralia"^^xsd:anyURI ;
                rdfs:isDefinedBy <https://ref.engineersaustralia.org.au/def/ea-membership-grade> ;
                skos:related <https://ref.engineersaustralia.org.au/def/ea-membership-grade/student> ;
                skos:inScheme <https://ref.engineersaustralia.org.au/def/ea-jargon> ;
                skos:broader eaj:post-nominals-ea ;
                skos:definition """A member of the Institute of Engineers Australia who is is a student in an engineering curriculum. Students are assumed to follow the professional engineer pathway and categorisation, however will typically not meet the qualification criteria for a true Professional Engineer."""@en ;
                skos:notation "StudIEAust" ;
                skos:prefLabel "Professional Engineer Student of the Institute of Engineers Australia"@en .

            eaj:TFIEAust a skos:Concept ;
                dcterms:source "https://linked.data.gov.au/org/engineersaustralia"^^xsd:anyURI ;
                rdfs:isDefinedBy <https://ref.engineersaustralia.org.au/def/ea-jargon> ;
                skos:related <https://ref.engineersaustralia.org.au/def/ea-membership-grade/fellow> ;
                skos:related <https://linked.data.gov.au/def/iea-occupational-categories/tech-engineer> ;
                skos:inScheme <https://ref.engineersaustralia.org.au/def/ea-jargon> ;
                skos:broader eaj:post-nominals-ea ;
                skos:definition """A member of Engineers Australia and very experienced engineer who has made a significant contribution to the profession, and who holds a 3 Years accredited Bachelor of Engineering Technology (BTech)."""@en ;
                skos:notation "TFIEAust" ;
                skos:prefLabel "Engineering Technologist Fellow of the Institute of Engineers Australia"@en .

            eaj:TMIEAust a skos:Concept ;
                dcterms:source "https://linked.data.gov.au/org/engineersaustralia"^^xsd:anyURI ;
                rdfs:isDefinedBy <https://ref.engineersaustralia.org.au/def/ea-jargon> ;
                skos:related <https://ref.engineersaustralia.org.au/def/ea-membership-grade/member> ;
                skos:related <https://linked.data.gov.au/def/iea-occupational-categories/tech-engineer> ;
                skos:inScheme <https://ref.engineersaustralia.org.au/def/ea-jargon> ;
                skos:broader eaj:post-nominals-ea ;
                skos:definition """A member of the Institute of Engineers Australia who has surpassed graduate membership but has not reached the level of experience of a Fellow, and who holds a 3 Years accredited Bachelor of Engineering Technology (BTech)."""@en ;
                skos:notation "TMIEAust" ;
                skos:prefLabel "Engineering Technologist Member of the Institute of Engineers Australia"@en .

            eaj:GradTIEAust a skos:Concept ;
                dcterms:source "https://linked.data.gov.au/org/engineersaustralia"^^xsd:anyURI ;
                rdfs:isDefinedBy <https://ref.engineersaustralia.org.au/def/ea-jargon> ;
                skos:related <https://ref.engineersaustralia.org.au/def/ea-membership-grade/graduate> ;
                skos:related <https://linked.data.gov.au/def/iea-occupational-categories/tech-engineer> ;
                skos:inScheme <https://ref.engineersaustralia.org.au/def/ea-jargon> ;
                skos:broader eaj:post-nominals-ea ;
                skos:definition """A member of the Institute of Engineers Australia prior to transitioning full professional membership. An Engineer with less than 3 years of relevant work experience according the the rules of membership, but who holds a 3 Years accredited Bachelor of Engineering Technology (BTech)."""@en ;
                skos:notation "GradTIEAust" ;
                skos:prefLabel "Engineering Technologist Graduate of the Institute of Engineers Australia"@en .

            eaj:HonFIEAust a skos:Concept ;
                dcterms:source "https://linked.data.gov.au/org/engineersaustralia"^^xsd:anyURI ;
                rdfs:isDefinedBy <https://ref.engineersaustralia.org.au/def/ea-membership-grade> ;
                skos:related <https://ref.engineersaustralia.org.au/def/ea-membership-grade/hon-fellow> ;
                skos:inScheme <https://ref.engineersaustralia.org.au/def/ea-jargon> ;
                skos:broader eaj:post-nominals-ea ;
                skos:definition """An honorary title for a member of Engineers Australia for outstanding achievement and contribution to the profession."""@en ;
                skos:notation "HonFIEAust" ;
                skos:prefLabel "Honorary Fellow of Engineers Australia"@en .

            eaj:GradOIEAust a skos:Concept ;
                dcterms:source "https://linked.data.gov.au/org/engineersaustralia"^^xsd:anyURI ;
                rdfs:isDefinedBy <https://ref.engineersaustralia.org.au/def/ea-membership-grade> ;
                skos:related <https://ref.engineersaustralia.org.au/def/ea-membership-grade/graduate> ;
                skos:inScheme <https://ref.engineersaustralia.org.au/def/ea-jargon> ;
                skos:broader eaj:post-nominals-ea ;
                skos:definition """A legacy designation that is no longer in current usage for a member of the Institute of Engineers Australia prior to transitioning full professional membership. Superseded by Graduate membership."""@en ;
                skos:notation "GradOIEAust" ;
                skos:prefLabel "Graduate Officer of Engineers Australia"@en .

            eaj:OFIEAust a skos:Concept ;
                dcterms:source "https://linked.data.gov.au/org/engineersaustralia"^^xsd:anyURI ;
                rdfs:isDefinedBy <https://ref.engineersaustralia.org.au/def/ea-membership-grade> ;
                skos:related <https://ref.engineersaustralia.org.au/def/ea-membership-grade/fellow> ;
                skos:inScheme <https://ref.engineersaustralia.org.au/def/ea-jargon> ;
                skos:broader eaj:post-nominals-ea ;
                skos:definition """A legacy designation that is no longer in current usage for a member of Engineers Australia and very experienced engineer who has made a significant contribution to the profession. Superseded by Fellow membership."""@en ;
                skos:notation "OFIEAust" ;
                skos:prefLabel "Officer Fellow of Engineers Australia"@en .

            eaj:OMIEAust a skos:Concept ;
                dcterms:source "https://linked.data.gov.au/org/engineersaustralia"^^xsd:anyURI ;
                rdfs:isDefinedBy <https://ref.engineersaustralia.org.au/def/ea-membership-grade> ;
                skos:related <https://ref.engineersaustralia.org.au/def/ea-membership-grade/member> ;
                skos:inScheme <https://ref.engineersaustralia.org.au/def/ea-jargon> ;
                skos:broader eaj:post-nominals-ea ;
                skos:definition """A legacy designation that is no longer in current usage for a member of the Institute of Engineers Australia who has surpassed graduate membership but has not reached the level of experience of a Fellow. Superseded by Member membership."""@en ;
                skos:notation "OMIEAust" ;
                skos:prefLabel "Officer Member of Engineers Australia"@en .

            eaj:SMIEAust a skos:Concept ;
                dcterms:source "https://linked.data.gov.au/org/engineersaustralia"^^xsd:anyURI ;
                rdfs:isDefinedBy <https://ref.engineersaustralia.org.au/def/ea-membership-grade> ;
                skos:related <https://ref.engineersaustralia.org.au/def/ea-membership-grade/member> ;
                skos:inScheme <https://ref.engineersaustralia.org.au/def/ea-jargon> ;
                skos:broader eaj:post-nominals-ea ;
                skos:definition """A legacy designation that is no longer in current usage for a member of the Institute of Engineers Australia who has professional experience exceeding that of a standard member. No new applications for this grade of membership have been accepted since August 1999."""@en ;
                skos:notation "SMIEAust" ;
                skos:prefLabel "Senior Member of Engineers Australia"@en .

    eaj:post-nominals-parliamentary a skos:Concept ;
        dcterms:source "https://www.stylemanual.gov.au/grammar-punctuation-and-conventions/titles-honours-forms-address/awards-and-honours"^^xsd:anyURI ;
        rdfs:isDefinedBy <https://ref.engineersaustralia.org.au/def/ea-jargon> ;
        skos:inScheme <https://ref.engineersaustralia.org.au/def/ea-jargon> ;
        skos:broader eaj:post-nominals ;
        skos:definition """Post Nominals indicating a member of parliament or another governing body. These include:
            - Member of the Australian House of Representatives	MP
            - Member of Parliament (Qld)	MP
            - Member of the Legislative Assembly (NSW)	MP
            - Member of the Legislative Assembly (Vic, WA, ACT)	MLA
            - Member of the Legislative Council (NSW, SA, Tas, Vic, WA)	MLC
            - Member of the House of Assembly (SA)	MHA
            - Member of the House of Assembly (Tas)	MP"""@en ;
        skos:prefLabel "Post Nominals - Parliamentary"@en .

    eaj:post-nominals-military a skos:Concept ;
        dcterms:source "https://www.stylemanual.gov.au/grammar-punctuation-and-conventions/titles-honours-forms-address/australian-defence-force"^^xsd:anyURI ;
        rdfs:isDefinedBy <https://ref.engineersaustralia.org.au/def/ea-jargon> ;
        skos:inScheme <https://ref.engineersaustralia.org.au/def/ea-jargon> ;
        skos:broader eaj:post-nominals ;
        skos:definition """Post Nominals indicating a member of the Australian Defence Force. Note that the full text rank occurs before the individuals name, e.g. Air Vice-Marshal Catherine Roberts AM CSC"""@en ;
        skos:prefLabel "Post Nominals - Military"@en .

eaj:professional-conduct-committee a skos:Concept ;
    dcterms:source "https://www.engineersaustralia.org.au/news-and-media/2024/05/join-engineers-australias-professional-conduct-committee"^^xsd:anyURI ;
    rdfs:isDefinedBy <https://ref.engineersaustralia.org.au/def/ea-jargon> ;
    skos:inScheme <https://ref.engineersaustralia.org.au/def/ea-jargon> ;
    skos:topConceptOf <https://ref.engineersaustralia.org.au/def/ea-jargon> ;
    skos:definition """The Professional Conduct Committee (PCC) is a committee formed under the General Regulations of Engineers Australia to consider and determine complaints against members of Engineers Australia and those on the National Engineering Register that they have engaged in unacceptable conduct. Unacceptable conduct is defined in Engineers Australia's General Regulations and includes breaches of the Engineers Australia Code of Ethics."""@en ;
    skos:notation "PCC" ;
    skos:altLabel "PCC"@en,
        "Professional Conduct Committee (PCC)"@en ;
    skos:prefLabel "Professional Conduct Committee"@en .

eaj:professional-development-program a skos:Concept ;
    dcterms:source "https://linked.data.gov.au/org/engineersaustralia"^^xsd:anyURI ;
    rdfs:isDefinedBy <https://ref.engineersaustralia.org.au/def/ea-jargon> ;
    skos:inScheme <https://ref.engineersaustralia.org.au/def/ea-jargon> ;
    skos:topConceptOf <https://ref.engineersaustralia.org.au/def/ea-jargon> ;
    skos:definition """The Professional Development Program (PDP) is a planned period of professional formation based in the workplace and structured around an identified job and career progression. It comprises the incremental acquisition and development of the competencies required to practise at the level of Chartered practitioner. This includes work-based training and assuming responsibility in appropriate roles.
    
    Participation in a PDP is open to engineering practitioners employed in all types and sizes of enterprise. Participating organisations include mining companies, utilities, consulting companies, aerospace, information technology, telecommunications, construction companies and public authorities."""@en ;
    skos:notation "PDP" ;
    skos:altLabel "PDP"@en,
        "GDP"@en,
        "Graduate Development Program"@en ;
    skos:prefLabel "Professional Development Program"@en .

    eaj:professional-development-program-online a skos:Concept ;
        dcterms:source "https://linked.data.gov.au/org/engineersaustralia"^^xsd:anyURI ;
        rdfs:isDefinedBy <https://ref.engineersaustralia.org.au/def/ea-jargon> ;
        skos:inScheme <https://ref.engineersaustralia.org.au/def/ea-jargon> ;
        skos:broader eaj:professional-development-program ;
        skos:definition """The Online offering of the Professional Development Program (PDP)."""@en ;
        skos:notation "PDO" ;
        skos:altLabel "PDO"@en,
            "ePDP"@en,
            "Online Professional Development Program"@en ;
        skos:prefLabel "Professional Development Program Online"@en .

eaj:prosci a skos:Concept ;
    dcterms:source "https://www.prosci.com/methodology-overview"^^xsd:anyURI ;
    rdfs:isDefinedBy <https://ref.engineersaustralia.org.au/def/ea-jargon> ;
    skos:inScheme <https://ref.engineersaustralia.org.au/def/ea-jargon> ;
    skos:topConceptOf <https://ref.engineersaustralia.org.au/def/ea-jargon> ;
    skos:definition """A structured, adaptable, repeatable approach to enable individuals to successfully move through changes in your organization
    
    Although the Prosci Methodology encompasses a variety of models, tools, assessments, processes and more, today it is comprised of three main components:
    - PCT Model: a simple but powerful framework for establishing and connecting the most important aspects of any successful change effort
    - ADKAR Model: a highly effective model for guiding individuals through the experiences-or elements-needed to make the change
    - Prosci 3-Phase Process: a structured, flexible framework for driving change at the organizational level."""@en ;
    skos:notation "PROSCI" ;
    skos:altLabel "Professional Science"@en ;
    skos:prefLabel "The Prosci Methodology"@en .

    eaj:adkar-model a skos:Concept ;
        dcterms:source "https://www.prosci.com/methodology-overview"^^xsd:anyURI ;
        rdfs:isDefinedBy <https://ref.engineersaustralia.org.au/def/ea-jargon> ;
        skos:inScheme <https://ref.engineersaustralia.org.au/def/ea-jargon> ;
        skos:broader eaj:prosci ;
        dcterms:isPartOf eaj:prosci ;
        skos:definition """Describes the five building blocks or 'elements' an individual needs to achieve for a change to be successful. Impacted individual is at the center of the Prosci Methodology. Individual success leads to organizational success.
        
        The Prosci ADKAR Model is one of the two foundational models of the Prosci Methodology. The word ADKAR is an acronym for the five outcomes an individual needs to achieve for a change to be successful: Awareness, Desire, Knowledge, Ability and Reinforcement. It is based on the understanding that organizational change can only happen when individuals change."""@en ;
        skos:notation "ADKAR" ;
        skos:prefLabel "ADKAR Model"@en .

    eaj:pct-model a skos:Concept ;
        dcterms:source "https://www.prosci.com/methodology/pct-model"^^xsd:anyURI ;
        rdfs:isDefinedBy <https://ref.engineersaustralia.org.au/def/ea-jargon> ;
        skos:inScheme <https://ref.engineersaustralia.org.au/def/ea-jargon> ;
        skos:broader eaj:prosci ;
        dcterms:isPartOf eaj:prosci ;
        skos:definition """A framework that shows the four critical aspects of any successful change effort and how they are interrelated, namely:
        Success - with shared deinfition and understanding
        Leadership/Sponsorship - with direction and accountability,
        Project Management - addressing the technical side of change through design and delivery, and
        Change Management - addressing the people side of change to enable, adopt, and use the solution."""@en ;
        skos:notation "PCT" ;
        skos:altLabel "PCT Model"@en ;
        skos:prefLabel "Prosci Change Triangle Model"@en ;.

    eaj:prosci-3-phase a skos:Concept ;
        dcterms:source "https://www.prosci.com/methodology-overview"^^xsd:anyURI ;
        rdfs:isDefinedBy <https://ref.engineersaustralia.org.au/def/ea-jargon> ;
        skos:inScheme <https://ref.engineersaustralia.org.au/def/ea-jargon> ;
        skos:broader eaj:prosci ;
        dcterms:isPartOf eaj:prosci ;
        skos:definition """A 3-phase approach to project management and change management consisting of:
        Phase 1 - Prepare Approach: Position the change for success by developing a customized and scaled change management strategy with the necessary sponsorship and commitment.
        Phase 2 - Manage Change: Achieve adoption and usage of the change by creating, implementing and adapting plan(s) that will move individuals and the organization through ADKAR transitions.
        Phase 3 - Sustain Outcomes: To realize the value of the change by ensuring the change is adopted and the organization is committed and prepared to sustain the change."""@en ;
        skos:prefLabel "Prosci 3-Phase Process"@en .

eaj:qualifications a skos:Concept ;
    dcterms:source "https://www.engineersaustralia.org.au/sites/default/files/2023-05/2023-royal-charter-by-laws.pdf"^^xsd:anyURI ;
    rdfs:isDefinedBy <https://ref.engineersaustralia.org.au/def/ea-jargon> ;
    skos:inScheme <https://ref.engineersaustralia.org.au/def/ea-jargon> ;
    skos:topConceptOf <https://ref.engineersaustralia.org.au/def/ea-jargon> ;
    skos:definition """Qualifications refer to all matters relevant to suitability for membership, including educational qualifications, training and work experience."""@en ;
    skos:prefLabel "Qualifications"@en .

    eaj:formal-qualifications a skos:Concept ;
    dcterms:source "https://www.ieagreements.org/assets/Uploads/Documents/IEA-Extended-Glossary.pdf"^^xsd:anyURI ;
    rdfs:isDefinedBy <https://ref.engineersaustralia.org.au/def/ea-jargon> ;
    skos:inScheme <https://ref.engineersaustralia.org.au/def/ea-jargon> ;
    skos:broader eaj:qualifications ;
    skos:definition """The formal recognition of a specified learning achievement, usually awarded on successful completion of a programme."""@en ;
    skos:altLabel "Academic Qualifications"@en,
        "Educational Qualifications"@en ;
    skos:prefLabel "Formal Qualifications"@en .

        eaj:study-aqf a skos:Concept ;
            dcterms:source "https://www.aqf.edu.au/"^^xsd:anyURI ;
            rdfs:isDefinedBy <https://linked.data.gov.au/def/australian-qualifications-framework> ;
            skos:related <https://linked.data.gov.au/def/australian-qualifications-framework> ;
            skos:inScheme <https://ref.engineersaustralia.org.au/def/ea-jargon> ;
            skos:broader eaj:formal-qualifications ;
            skos:definition """Australian Qualifications Framework Issued by the National Staff Development Committee Standards and Curriculum Council of ANTA, the AQF provides a comprehensive, nationally consistent yet flexible Framework for all qualifications in post-compulsory education in Australia. The Framework was introduced Australia wide on 1 January 1995."""@en ;
            skos:notation "AQF" ;
            skos:hiddenLabel "AQF Level"@en ;
            skos:prefLabel "Australian Qualifications Framework"@en .

eaj:quality-assurance a skos:Concept ;
    dcterms:source "https://www.iso.org/obp/ui/fr/#iso:std:iso:9000:ed-4:v1:en"^^xsd:anyURI ;
    rdfs:isDefinedBy <https://ref.engineersaustralia.org.au/def/ea-jargon> ;
    skos:inScheme <https://ref.engineersaustralia.org.au/def/ea-jargon> ;
    skos:topConceptOf <https://ref.engineersaustralia.org.au/def/ea-jargon> ;
    skos:definition """QA is a subset of quality management that consists of all the planned and systematic activities implemented within the quality system that can be demonstrated to provide confidence that a product or service will fulfil requirements for quality. (The confidence provided by quality assurance is two-fold: Internally to management and externally to customers, government agencies, regulators, certifiers, and third parties)."""@en ;
    skos:notation "QA" ;
    skos:prefLabel "Quality Assurance"@en .

eaj:quality-control a skos:Concept ;
    dcterms:source "https://www.iso.org/obp/ui/fr/#iso:std:iso:9000:ed-4:v1:en"^^xsd:anyURI ;
    rdfs:isDefinedBy <https://ref.engineersaustralia.org.au/def/ea-jargon> ;
    skos:inScheme <https://ref.engineersaustralia.org.au/def/ea-jargon> ;
    skos:topConceptOf <https://ref.engineersaustralia.org.au/def/ea-jargon> ;
    skos:definition """QC is a part of quality management focused on fulfilling quality requirements. While quality assurance relates to how a process is performed or how a product or service is made, quality control is more the inspection aspect of quality management. An alternate definition is "the operational techniques and activities used to fulfil requirements for quality."""@en ;
    skos:notation "QC" ;
    skos:prefLabel "Quality Control"@en .

eaj:raci a skos:Concept ;
    dcterms:source "https://en.wikipedia.org/wiki/Responsibility_assignment_matrix"^^xsd:anyURI ;
    rdfs:isDefinedBy <https://ref.engineersaustralia.org.au/def/ea-jargon> ;
    skos:inScheme <https://ref.engineersaustralia.org.au/def/ea-jargon> ;
    skos:topConceptOf <https://ref.engineersaustralia.org.au/def/ea-jargon> ;
    skos:definition """RACI is an acronym derived from the four key responsibilities most typically used in project management and task delivery: Responsible, Accountable, Consulted, Informed. It is used for clarifying and defining roles and responsibilities in cross-functional or departmental projects and processes."""@en ;
    skos:notation "RACI" ;
    skos:altLabel "RAM Matrix"@en,
        "Responsibility Assignment Matrix"@en,
        "Linear Responsibility Chart"@en ;
    skos:prefLabel "RACI Matrix"@en .

    eaj:raci-responsible a skos:Concept ;
        dcterms:source "https://pmicie.org/files/22/PM-Toolkit/85/racirweb31.pdf"^^xsd:anyURI ;
        rdfs:isDefinedBy <https://ref.engineersaustralia.org.au/def/ea-jargon>;
        skos:inScheme <https://ref.engineersaustralia.org.au/def/ea-jargon> ;
        skos:broader eaj:raci ;
        skos:definition """The responsible individual(s) who actually complete the task. The 'Doer' is responsible for action/implementation. Responsibility can be shared. The degree of responsibility is determined by the Accountable individual."""@en;
        skos:altLabel "Responsibility"@en,
            "The Doer"@en ; 
        skos:prefLabel "Responsible"@en .

    eaj:raci-accountable a skos:Concept ;
        dcterms:source "https://pmicie.org/files/22/PM-Toolkit/85/racirweb31.pdf"^^xsd:anyURI ;
        rdfs:isDefinedBy <https://ref.engineersaustralia.org.au/def/ea-jargon>;
        skos:inScheme <https://ref.engineersaustralia.org.au/def/ea-jargon> ;
        skos:broader eaj:raci ;
        skos:definition """The accountable person is the individual who is ultimately answerable for the activity or decision. This includes yes-or-no authority and veto power. Only one Accountable individual can be assigned to an action."""@en;
        skos:altLabel "Accountability"@en,
            "The Buck Stops Here"@en ; 
        skos:prefLabel "Accountable"@en .

    eaj:raci-consulted a skos:Concept ;
        dcterms:source "https://pmicie.org/files/22/PM-Toolkit/85/racirweb31.pdf"^^xsd:anyURI ;
        rdfs:isDefinedBy <https://ref.engineersaustralia.org.au/def/ea-jargon>;
        skos:inScheme <https://ref.engineersaustralia.org.au/def/ea-jargon> ;
        skos:broader eaj:raci ;
        skos:definition """Consulted individual are typically subject matter experts that are to be consulted prior to a final decision or action. This is a predetermined need for two-way communication. Input from the designated position is required."""@en;
        skos:altLabel "Consult"@en,
            "Consultation"@en,
            "In the Loop"@en ; 
        skos:prefLabel "Consulted"@en .

    eaj:raci-informed a skos:Concept ;
        dcterms:source "https://pmicie.org/files/22/PM-Toolkit/85/racirweb31.pdf"^^xsd:anyURI ;
        rdfs:isDefinedBy <https://ref.engineersaustralia.org.au/def/ea-jargon>;
        skos:inScheme <https://ref.engineersaustralia.org.au/def/ea-jargon> ;
        skos:broader eaj:raci ;
        skos:definition """Individuals who need to be informed after a decision or action is taken. They may be required to take action as a result of the outcome. It is a one-way communication."""@en;
        skos:altLabel "Inform"@en,
            "Keep in the Picture"@en ; 
        skos:prefLabel "Informed"@en .

eaj:recognition-of-prior-learning a skos:Concept ;
    dcterms:source "https://www.asqa.gov.au/guidance-resources/resources-providers/faqs/recognition-prior-learning-rpl"^^xsd:anyURI ;
    rdfs:isDefinedBy <https://ref.engineersaustralia.org.au/def/ea-jargon> ;
    skos:inScheme <https://ref.engineersaustralia.org.au/def/ea-jargon> ;
    skos:topConceptOf <https://ref.engineersaustralia.org.au/def/ea-jargon> ;
    skos:definition """Recognition of Prior Learning (RPL) means an assessment process that assesses the competency/s of an individual that may have been acquired through formal, non-formal and informal learning to determine the extent to which that individual meets the requirements specified in the training package or Vocational Education and Training (VET) accredited courses.
        - formal learning refers to learning that takes place through a structured program of instruction and is linked to the attainment of an AQF qualification or statement of attainment (for example, a certificate, diploma or university degree);
        - non-formal learning refers to learning that takes place through a structured program of instruction, but does not lead to the attainment of an AQF qualification or statement of attainment (for example, in-house professional development programs conducted by a business); and
        - informal learning refers to learning that results through experience of work-related, social, family, hobby or leisure activities (for example the acquisition of interpersonal skills developed through several years as a sales representative)."""@en ;
    skos:notation "RPL" ;
    skos:prefLabel "Recognition of Prior Learning"@en .

eaj:records a skos:Concept ;
    dcterms:source "https://www.iso.org/obp/ui/#iso:std:iso:15489:-1:dis:ed-2:v1:en"^^xsd:anyURI ;
    rdfs:isDefinedBy <https://ref.engineersaustralia.org.au/def/ea-jargon> ;
    skos:related <https://ref.engineersaustralia.org.au/def/ea-documents> ;
    skos:inScheme <https://ref.engineersaustralia.org.au/def/ea-jargon> ;
    skos:topConceptOf <https://ref.engineersaustralia.org.au/def/ea-jargon> ;
    skos:definition """As stated by ISO 15489 -1:2016, a record is 'information created, received and maintained as evidence and information by an organization or person, in pursuance of legal obligations or in the transaction of business'."""@en ;
	skos:prefLabel "Records"@en .

eaj:ref-data-management-system a skos:Concept ;
    dcterms:source "https://linked.data.gov.au/org/engineersaustralia"^^xsd:anyURI ;
    rdfs:isDefinedBy <https://ref.engineersaustralia.org.au/def/ea-jargon> ;
    skos:inScheme <https://ref.engineersaustralia.org.au/def/ea-jargon> ;
    skos:topConceptOf <https://ref.engineersaustralia.org.au/def/ea-jargon> ;
    skos:definition """Reference data management systems are the applications, governance processes, and tools that manage the terminology and categorisation metadata used to classify data and entities and establish taxonomic hierarchies across systems and business lines.
    
    Reference data management can be performed in multiple ways such as reference tables in a relational database, business glossaries, knowledge graph vocabularies for storage of terminology, and a range of business and version control processes to trace and maintain continuity and consistency."""@en ;
    skos:prefLabel "Reference Data Management System"@en .

eaj:doc-management-system a skos:Concept ;
    dcterms:source "https://www.iso.org/obp/ui/en/#!iso:std:76865:en"^^xsd:anyURI ;
    rdfs:isDefinedBy <https://ref.engineersaustralia.org.au/def/ea-jargon> ;
    skos:inScheme <https://ref.engineersaustralia.org.au/def/ea-jargon> ;
    skos:topConceptOf <https://ref.engineersaustralia.org.au/def/ea-jargon> ;
    skos:definition """A DMS is a computerised (usually) system used to store, share, track, and manage files and documents. It provides users with a single source of truth to access the latest version of documents."""@en ;
    skos:notation "DMS" ;
    skos:altLabel "Record Management System"@en ;
    skos:prefLabel "Document Management System"@en .

eaj:learning-management-system a skos:Concept ;
    dcterms:source "https://www.techtarget.com/searchcio/definition/learning-management-system"^^xsd:anyURI ;
    rdfs:isDefinedBy <https://ref.engineersaustralia.org.au/def/ea-jargon> ;
    skos:inScheme <https://ref.engineersaustralia.org.au/def/ea-jargon> ;
    skos:topConceptOf <https://ref.engineersaustralia.org.au/def/ea-jargon> ;
    skos:definition """A learning management system is a software application or web-based technology used to plan, implement and assess a specific learning process. It's used for e-learning practices and, in its most common form, consists of two elements: a server that performs the base functionality and a user interface (UI) that is operated by instructors, students and administrators."""@en ;
    skos:notation "LMS" ;
    skos:prefLabel "Learning Management System"@en .

eaj:review a skos:Concept ;
    dcterms:source "https://www.britannica.com/dictionary/review"^^xsd:anyURI ;
	rdfs:isDefinedBy <https://ref.engineersaustralia.org.au/def/ea-jargon>;
    skos:inScheme <https://ref.engineersaustralia.org.au/def/ea-jargon> ;
    skos:topConceptOf <https://ref.engineersaustralia.org.au/def/ea-jargon> ;
	skos:definition """An act of carefully looking at or examining the quality or condition of something or someone : examination or inspection."""@en;
    skos:prefLabel "Review"@en .

    eaj:cpd-assessment-review a skos:Concept ;
        dcterms:source "https://www.engineersaustralia.org.au/sites/default/files/resource-files/2020-02/EA%20General%20Regulations%205%20Dec%202019.pdf"^^xsd:anyURI ;
        rdfs:isDefinedBy <https://ref.engineersaustralia.org.au/def/ea-jargon>;
        skos:inScheme <https://ref.engineersaustralia.org.au/def/ea-jargon> ;
        skos:topConceptOf <https://ref.engineersaustralia.org.au/def/ea-jargon> ;
        skos:definition """A review of a CPD Assessment."""@en;
        skos:prefLabel "CPD Assessment Review"@en .

eaj:risk a skos:Concept ;
    dcterms:source "https://www.iso.org/standard/65694.html"^^xsd:anyURI ;
	rdfs:isDefinedBy <https://ref.engineersaustralia.org.au/def/ea-jargon>;
    skos:inScheme <https://ref.engineersaustralia.org.au/def/ea-jargon> ;
    skos:topConceptOf <https://ref.engineersaustralia.org.au/def/ea-jargon> ;
	skos:definition """The effect of uncertainty on objectives."""@en;
    skos:prefLabel "Risk"@en .

    eaj:inherent-risk a skos:Concept ;
        dcterms:source "https://www.iso.org/standard/65694.html"^^xsd:anyURI ;
        rdfs:isDefinedBy <https://ref.engineersaustralia.org.au/def/ea-jargon>;
        skos:inScheme <https://ref.engineersaustralia.org.au/def/ea-jargon> ;
        skos:broader eaj:risk ;
        skos:definition """A risk arising from an incident, event, or circumstance without any controls in place. The Level of Risk that is present at the time of the risk assessment. This is assessed by considering the risk treatments and controls that are currently in place."""@en;
        skos:prefLabel "Inherent Risk"@en .

    eaj:current-level-of-risk a skos:Concept ;
        dcterms:source "https://www.iso.org/standard/65694.html"^^xsd:anyURI ;
        rdfs:isDefinedBy <https://ref.engineersaustralia.org.au/def/ea-jargon>;
        skos:inScheme <https://ref.engineersaustralia.org.au/def/ea-jargon> ;
        skos:broader eaj:risk ;
        skos:definition """A risk arising from an incident, event, or circumstance that has existing controls in place. The existing level of risk, taking into account the current control environment. Expressed in terms of the combination of consequence and likelihood."""@en;
        skos:prefLabel "Current Level of Risk"@en .

    eaj:target-risk a skos:Concept ;
        dcterms:source "https://www.iso.org/standard/65694.html"^^xsd:anyURI ;
        rdfs:isDefinedBy <https://ref.engineersaustralia.org.au/def/ea-jargon>;
        skos:inScheme <https://ref.engineersaustralia.org.au/def/ea-jargon> ;
        skos:broader eaj:risk ;
        skos:definition """The risk rating that an organisation aspires to, taking into account the stated risk appetite."""@en;
        skos:prefLabel "Target Risk"@en .

    eaj:residual-risk a skos:Concept ;
        dcterms:source "https://www.iso.org/standard/65694.html"^^xsd:anyURI ;
        rdfs:isDefinedBy <https://ref.engineersaustralia.org.au/def/ea-jargon>;
        skos:inScheme <https://ref.engineersaustralia.org.au/def/ea-jargon> ;
        skos:broader eaj:risk ;
        skos:definition """A risk that is anticipated once additional controls are put in place and are working effecitvely. Risk remaining after risk treatment. Can also be referred to as Retained risk."""@en;
        skos:prefLabel "Residual Risk"@en .

eaj:risk-analysis a skos:Concept ;
    dcterms:source "https://www.iso.org/standard/65694.html"^^xsd:anyURI ;
	rdfs:isDefinedBy <https://ref.engineersaustralia.org.au/def/ea-jargon>;
    skos:inScheme <https://ref.engineersaustralia.org.au/def/ea-jargon> ;
    skos:topConceptOf <https://ref.engineersaustralia.org.au/def/ea-jargon> ;
	skos:definition """Process to comprehend the nature of risk and to determine the level of risk."""@en;
    skos:prefLabel "Risk Analysis"@en .

eaj:risk-appetite a skos:Concept ;
    dcterms:source "https://www.iso.org/standard/65694.html"^^xsd:anyURI ;
	rdfs:isDefinedBy <https://ref.engineersaustralia.org.au/def/ea-jargon>;
    skos:inScheme <https://ref.engineersaustralia.org.au/def/ea-jargon> ;
    skos:topConceptOf <https://ref.engineersaustralia.org.au/def/ea-jargon> ;
	skos:definition """The total risk that the organization can bear in a given risk profile, usually expressed in aggregate."""@en;
    skos:prefLabel "Risk Appetite"@en .

eaj:risk-criteria a skos:Concept ;
    dcterms:source "https://www.iso.org/standard/65694.html"^^xsd:anyURI ;
	rdfs:isDefinedBy <https://ref.engineersaustralia.org.au/def/ea-jargon>;
    skos:inScheme <https://ref.engineersaustralia.org.au/def/ea-jargon> ;
    skos:topConceptOf <https://ref.engineersaustralia.org.au/def/ea-jargon> ;
	skos:definition """Terms of reference against which the significance of a risk is evaluated."""@en;
    skos:prefLabel "Risk Criteria"@en .

eaj:risk-owner a skos:Concept ;
    dcterms:source "https://www.iso.org/standard/65694.html"^^xsd:anyURI ;
	rdfs:isDefinedBy <https://ref.engineersaustralia.org.au/def/ea-jargon>;
    skos:inScheme <https://ref.engineersaustralia.org.au/def/ea-jargon> ;
    skos:topConceptOf <https://ref.engineersaustralia.org.au/def/ea-jargon> ;
	skos:definition """A person or entity with the accountability and authority to manage a Risk. The Risk Owner is responsible to plan, design and implement risk actions and provide status updates to risk sponsor as requested. Risk Owner to ensure risk register is kept updated for the assigned risks."""@en;
    skos:prefLabel "Risk Owner"@en .

eaj:risk-profile a skos:Concept ;
    dcterms:source "https://www.iso.org/standard/65694.html"^^xsd:anyURI ;
	rdfs:isDefinedBy <https://ref.engineersaustralia.org.au/def/ea-jargon>;
    skos:inScheme <https://ref.engineersaustralia.org.au/def/ea-jargon> ;
    skos:topConceptOf <https://ref.engineersaustralia.org.au/def/ea-jargon> ;
	skos:definition """The risk profile reflects the relationship between the impact of a change and the likelihood of failure."""@en;
    skos:prefLabel "Risk Profile"@en .

eaj:risk-source a skos:Concept ;
    dcterms:source "https://www.iso.org/standard/65694.html"^^xsd:anyURI ;
	rdfs:isDefinedBy <https://ref.engineersaustralia.org.au/def/ea-jargon>;
    skos:inScheme <https://ref.engineersaustralia.org.au/def/ea-jargon> ;
    skos:topConceptOf <https://ref.engineersaustralia.org.au/def/ea-jargon> ;
	skos:definition """Element which alone or in combination has the potential to give risk to the Risk."""@en;
    skos:prefLabel "Risk Source"@en .

eaj:risk-sponsor a skos:Concept ;
    dcterms:source "https://www.iso.org/standard/65694.html"^^xsd:anyURI ;
	rdfs:isDefinedBy <https://ref.engineersaustralia.org.au/def/ea-jargon>;
    skos:inScheme <https://ref.engineersaustralia.org.au/def/ea-jargon> ;
    skos:topConceptOf <https://ref.engineersaustralia.org.au/def/ea-jargon> ;
	skos:definition """A person or entity with the accountability for the risk profile. The sponsor would set the risk appetite and will ensure it fits within the risk appetite for the organisation. The Risk Sponsor would seek direct updates from the Risk Owner on the risk closure actions, risk mitigation actions and agreement on the risk closure date."""@en;
    skos:prefLabel "Risk Sponsor"@en .

eaj:risk-exposure a skos:Concept ;
    dcterms:source "https://www.iso.org/standard/65694.html"^^xsd:anyURI ;
	rdfs:isDefinedBy <https://ref.engineersaustralia.org.au/def/ea-jargon>;
    skos:inScheme <https://ref.engineersaustralia.org.au/def/ea-jargon> ;
    skos:topConceptOf <https://ref.engineersaustralia.org.au/def/ea-jargon> ;
	skos:definition """The combination(s) of likelihood (or frequency) of a risk occurring and the consequence were it to occur."""@en;
    skos:prefLabel "Risk Exposure"@en .

eaj:risk-tolerance a skos:Concept ;
    dcterms:source "https://www.iso.org/standard/65694.html"^^xsd:anyURI ;
	rdfs:isDefinedBy <https://ref.engineersaustralia.org.au/def/ea-jargon>;
    skos:inScheme <https://ref.engineersaustralia.org.au/def/ea-jargon> ;
    skos:topConceptOf <https://ref.engineersaustralia.org.au/def/ea-jargon> ;
	skos:definition """Risk tolerance is the level of risk that an organization can accept per individual risk. Risk tolerance is related to the acceptance of the outcomes of a risk should they occur"""@en;
    skos:prefLabel "Risk Tolerance"@en .

eaj:risk-treatment a skos:Concept ;
    dcterms:source "https://www.iso.org/standard/65694.html"^^xsd:anyURI ;
	rdfs:isDefinedBy <https://ref.engineersaustralia.org.au/def/ea-jargon>;
    skos:inScheme <https://ref.engineersaustralia.org.au/def/ea-jargon> ;
    skos:topConceptOf <https://ref.engineersaustralia.org.au/def/ea-jargon> ;
	skos:definition """Process to modify risk. An action or set of actions that are put in place to help modify a risk"""@en;
    skos:prefLabel "Risk Treatment"@en .

eaj:risk-maturity a skos:Concept ;
    dcterms:source "https://www.iso.org/standard/65694.html"^^xsd:anyURI ;
	rdfs:isDefinedBy <https://ref.engineersaustralia.org.au/def/ea-jargon>;
    skos:inScheme <https://ref.engineersaustralia.org.au/def/ea-jargon> ;
    skos:topConceptOf <https://ref.engineersaustralia.org.au/def/ea-jargon> ;
	skos:definition """The risk capability and the level of sophistication the organization operates at in terms of its risk processes and procedures"""@en;
    skos:prefLabel "Risk Maturity"@en .

eaj:risk-evaluation a skos:Concept ;
    dcterms:source "https://www.iso.org/standard/65694.html"^^xsd:anyURI ;
	rdfs:isDefinedBy <https://ref.engineersaustralia.org.au/def/ea-jargon>;
    skos:inScheme <https://ref.engineersaustralia.org.au/def/ea-jargon> ;
    skos:topConceptOf <https://ref.engineersaustralia.org.au/def/ea-jargon> ;
	skos:definition """Process of comparing the results of the risk analysis with the risk criteria to determine whether the risk and/or its magnitude is acceptable or tolerable."""@en;
    skos:prefLabel "Risk Evaluation"@en .

eaj:risk-assessment a skos:Concept ;
    dcterms:source "https://www.iso.org/standard/65694.html"^^xsd:anyURI ;
	rdfs:isDefinedBy <https://ref.engineersaustralia.org.au/def/ea-jargon>;
    skos:inScheme <https://ref.engineersaustralia.org.au/def/ea-jargon> ;
    skos:topConceptOf <https://ref.engineersaustralia.org.au/def/ea-jargon> ;
	skos:definition """The overall process of risk identification, risk analysis and risk evaluation."""@en;
    skos:prefLabel "Risk Assessment"@en .

eaj:shared-risks a skos:Concept ;
    dcterms:source "https://www.iso.org/standard/65694.html"^^xsd:anyURI ;
	rdfs:isDefinedBy <https://ref.engineersaustralia.org.au/def/ea-jargon>;
    skos:inScheme <https://ref.engineersaustralia.org.au/def/ea-jargon> ;
    skos:topConceptOf <https://ref.engineersaustralia.org.au/def/ea-jargon> ;
	skos:definition """Risks shared by two or more agencies that require coordinated management by more than one agency."""@en;
    skos:prefLabel "Shared risks"@en .

eaj:source-of-truth a skos:Concept ;
    dcterms:source "https://en.wikipedia.org/wiki/Single_source_of_truth"^^xsd:anyURI ;
    rdfs:isDefinedBy <https://ref.engineersaustralia.org.au/def/ea-jargon> ;
    skos:inScheme <https://ref.engineersaustralia.org.au/def/ea-jargon> ;
    skos:topConceptOf <https://ref.engineersaustralia.org.au/def/ea-jargon> ;
    skos:definition """A source of truth is the practice of structuring data models and information architectures such that each data element has a mastered version in single location. A source of truth for a data element is the data holding that is considered a true representation of that element. Mastered data is related to Master Data, however reference data and transactional data can also be mastered with a 'true' source of truth location.
    
    When copying or updating Mastered Data, single source of truth can be achieved through several methods:
    - Never copying the master version of data. Only storing references in downstream systems so that all create-read-update-delete commands occur at the source of truth.
    - Master versions are replicated in dependent systems as read-only versions. Opearations that create-update-delete mastered data only occur in the source of truth.
    - Master versions are replicated in dependent systems and create-update-delete operations on those copies are reconciled and synchronised with the master copy, such as through a merge function that is either periodic or triggered by an event in the dependent client system."""@en ;
    skos:altLabel "Single Source of Truth"@en,
        "Single Point of Truth"@en ;
    skos:prefLabel "Source of Truth"@en .

eaj:sponsorship a skos:Concept ;
    dcterms:source "https://linked.data.gov.au/org/engineersaustralia"^^xsd:anyURI ;
    rdfs:isDefinedBy <https://ref.engineersaustralia.org.au/def/ea-jargon> ;
    skos:related <https://ref.engineersaustralia.org.au/def/ea-sponsorship>,
        earl:sponsor ;
    skos:inScheme <https://ref.engineersaustralia.org.au/def/ea-jargon> ;
    skos:topConceptOf <https://ref.engineersaustralia.org.au/def/ea-jargon> ;
    skos:definition """A Sponsorship is a pledge of money, services, or products offered to Engineers Australia by an External Entity to help fund an award, event, or campaign that is being managed by Engineers Australia."""@en ;
    skos:prefLabel "Sponsorship"@en .

eaj:sso a skos:Concept ;
    dcterms:source "https://www.okta.com/au/blog/2021/02/single-sign-on-sso/"^^xsd:anyURI ;
    rdfs:isDefinedBy <https://ref.engineersaustralia.org.au/def/ea-jargon> ;
    skos:inScheme <https://ref.engineersaustralia.org.au/def/ea-jargon> ;
    skos:topConceptOf <https://ref.engineersaustralia.org.au/def/ea-jargon> ;
    skos:definition """Single sign-on (SSO) is a user authentication tool that enables users to securely access multiple applications and services using just one set of credentials. There are various SSO protocols including Security Access Markup Language (SAML), Open Authorisation (OAuth), OpenID Connect (OIDC), Kerberos."""@en ;
    skos:notation "SSO" ;
    skos:prefLabel "Single Sign-On"@en .

eaj:stakeholder a skos:Concept ;
    dcterms:source "https://www.iso.org/standard/65694.html"^^xsd:anyURI ;
	rdfs:isDefinedBy <https://ref.engineersaustralia.org.au/def/ea-jargon>;
    skos:inScheme <https://ref.engineersaustralia.org.au/def/ea-jargon> ;
    skos:topConceptOf <https://ref.engineersaustralia.org.au/def/ea-jargon> ;
	skos:definition """Person or organisation that can affect, be affected by, or perceive themselves to be affected by a decision or activity. [As defined in the ISO 31000:2018]"""@en;
    skos:prefLabel "Stakeholder"@en .

eaj:strategic-context a skos:Concept ;
    dcterms:source "https://www.iso.org/standard/65694.html"^^xsd:anyURI ;
	rdfs:isDefinedBy <https://ref.engineersaustralia.org.au/def/ea-jargon>;
    skos:inScheme <https://ref.engineersaustralia.org.au/def/ea-jargon> ;
    skos:topConceptOf <https://ref.engineersaustralia.org.au/def/ea-jargon> ;
	skos:definition """The environment in which an agency seeks to achieve its objectives. This encompasses both the internal and external environments."""@en;
    skos:prefLabel "Strategic Context"@en .

    eaj:internal-context a skos:Concept ;
        dcterms:source "https://www.iso.org/standard/65694.html"^^xsd:anyURI ;
        rdfs:isDefinedBy <https://ref.engineersaustralia.org.au/def/ea-jargon>;
        skos:inScheme <https://ref.engineersaustralia.org.au/def/ea-jargon> ;
        skos:broader eaj:strategic-context ;
        skos:definition """The internal environment in which an agency seeks to achieve its objectives. Can include governance, roles and accountabilities, policies, objectives, strategic priorities, information systems, culture etc."""@en;
        skos:prefLabel "Internal Context"@en .

    eaj:external-context a skos:Concept ;
        dcterms:source "https://www.iso.org/standard/65694.html"^^xsd:anyURI ;
        rdfs:isDefinedBy <https://ref.engineersaustralia.org.au/def/ea-jargon>;
        skos:inScheme <https://ref.engineersaustralia.org.au/def/ea-jargon> ;
        skos:broader eaj:strategic-context ;
        skos:definition """The external environment in which an agency seeks to achieve its objectives. Can include the cultural, social, political, legal, regulatory, financial, technological, economic, natural and competitive environment, whether international, national, regional or local."""@en;
        skos:prefLabel "External Context"@en .

eaj:study-bridging a skos:Concept ;
    dcterms:source "https://linked.data.gov.au/org/engineersaustralia"^^xsd:anyURI ;
    rdfs:isDefinedBy <https://linked.data.gov.au/def/australian-qualifications-framework> ;
    skos:inScheme <https://ref.engineersaustralia.org.au/def/ea-jargon> ;
    skos:topConceptOf <https://ref.engineersaustralia.org.au/def/ea-jargon> ;
    skos:definition """A course designed to enable Articulation. Bridging courses do not usually, of themselves, provide a formal academic qualification. Some formal academic courses are recognised for articulation purposes but these are not normally referred to as Bridging Courses. The National Office for Overseas Skills Recognition (NOOSR) has arranged with some Australian Universities to provide special Bridging Courses for those with overseas qualifications, which cannot be fully recognised in Australia. These courses do not result in a formal testamur but Engineers Australia accepts a certificate of successful completion as evidence of Stage 1 eligibility."""@en ;
    skos:prefLabel "Bridging Course"@en .

eaj:system-architecture a skos:Concept ;
    dcterms:source "https://en.wikipedia.org/wiki/Systems_architecture"^^xsd:anyURI ;
    rdfs:isDefinedBy <https://ref.engineersaustralia.org.au/def/ea-jargon> ;
    skos:inScheme <https://ref.engineersaustralia.org.au/def/ea-jargon> ;
    skos:topConceptOf <https://ref.engineersaustralia.org.au/def/ea-jargon> ;
    skos:definition """A description of a solution and a representation of the data flows, relationships, and interactions between the components of a complete system. In a hardware architecture this will include the structures and behaviours that define what data moves and any rules and transformations applied. Commonly illustrated using a Data Flow Diagram (DFD).
    
    By contrast, a data model describes how real-world entities are described by data including entity or object classes, their attributes and relationships."""@en ;
    skos:altLabel "Systems Architecture"@en,
        "Data Architecture"@en,
        "Solution Architecture"@en,
        "System Model"@en ;
    skos:prefLabel "System Architecture"@en .

docs:skilled-visa a skos:Concept ;
    rdfs:isDefinedBy <https://ref.engineersaustralia.org.au/def/ea-documents> ;
    skos:inScheme <https://ref.engineersaustralia.org.au/def/ea-jargon> ;
    skos:topConceptOf <https://ref.engineersaustralia.org.au/def/ea-jargon> .

docs:policy a skos:Concept ;
    rdfs:isDefinedBy <https://ref.engineersaustralia.org.au/def/ea-documents> ;
    skos:inScheme <https://ref.engineersaustralia.org.au/def/ea-jargon> ;
    skos:topConceptOf <https://ref.engineersaustralia.org.au/def/ea-jargon> .

docs:procedure a skos:Concept ;
    rdfs:isDefinedBy <https://ref.engineersaustralia.org.au/def/ea-documents> ;
    skos:inScheme <https://ref.engineersaustralia.org.au/def/ea-jargon> ;
    skos:topConceptOf <https://ref.engineersaustralia.org.au/def/ea-jargon> .

eaj:threats-opportunities a skos:Concept ;
    dcterms:source "https://www.iso.org/standard/65694.html"^^xsd:anyURI ;
    rdfs:isDefinedBy <https://ref.engineersaustralia.org.au/def/ea-jargon>;
    skos:inScheme <https://ref.engineersaustralia.org.au/def/ea-jargon> ;
    skos:topConceptOf <https://ref.engineersaustralia.org.au/def/ea-jargon> ;
    skos:definition """Issues that haven't materialised into risks, but warrant being actively monitored. A threat is a potential cause of an incident that may result in harm to a system or organization. An opportunity is a potential cause of an incident that may result in a benefit to a system or organization."""@en;
    skos:prefLabel "Threats and Opportunities"@en .

eaj:trades-recognition-australia a skos:Concept ;
    dcterms:source "https://www.tradesrecognitionaustralia.gov.au/"^^xsd:anyURI ;
    rdfs:isDefinedBy <https://ref.engineersaustralia.org.au/def/ea-jargon> ;
    skos:inScheme <https://ref.engineersaustralia.org.au/def/ea-jargon> ;
    skos:topConceptOf <https://ref.engineersaustralia.org.au/def/ea-jargon> ;
    skos:definition """Trades Recognition Australia (TRA) is a skills assessment service for people with trade skills gained overseas or in Australia that require a skills assessment for the purpose of migration."""@en ;
    skos:notation "TRA" ;
    skos:prefLabel "Trades Recognition Australia"@en .

eaj:unsolicited-customer-data a skos:Concept ;
    dcterms:source "https://www.oaic.gov.au/privacy/australian-privacy-principles/australian-privacy-principles-guidelines/chapter-4-app-4-dealing-with-unsolicited-personal-information"^^xsd:anyURI ;
    rdfs:isDefinedBy <https://ref.engineersaustralia.org.au/def/ea-jargon> ;
    skos:inScheme <https://ref.engineersaustralia.org.au/def/ea-jargon> ;
    skos:topConceptOf <https://ref.engineersaustralia.org.au/def/ea-jargon> ;
    skos:definition """Unsolicited personal information is personal information received by the organisation where no active steps have been taken to collect the information."""@en ;
    skos:altLabel "Unsolicited Customer Information"@en,
        "Unsolicited Customer Data"@en,
        "Unsolicited Personal Information"@en ;
    skos:prefLabel "Unsolicited Personal Data"@en .

eaj:user-story a skos:Concept ;
    dcterms:source "https://www.atlassian.com/agile/project-management/user-stories"^^xsd:anyURI ;
    rdfs:isDefinedBy <https://ref.engineersaustralia.org.au/def/ea-jargon> ;
    skos:inScheme <https://ref.engineersaustralia.org.au/def/ea-jargon> ;
    skos:topConceptOf <https://ref.engineersaustralia.org.au/def/ea-jargon> ;
    skos:definition """A user story is an informal, general explanation of a software feature written from the perspective of the end user. Its purpose is to articulate how a software feature will provide value to the customer. User stories are typically represented in the format: As a (actor) I need to (action) so that (result)."""@en ;
    skos:altLabel "User Stories"@en ;
    skos:prefLabel "User Story"@en .

eaj:validation a skos:Concept ;
    dcterms:source "https://www.iso.org/obp/ui/fr/#iso:std:iso:9000:ed-4:v1:en"^^xsd:anyURI ;
    rdfs:isDefinedBy <https://ref.engineersaustralia.org.au/def/ea-jargon> ;
    skos:inScheme <https://ref.engineersaustralia.org.au/def/ea-jargon> ;
    skos:topConceptOf <https://ref.engineersaustralia.org.au/def/ea-jargon> ;
    skos:definition """Confirmation, through the provision of objective evidence, that the requirements for a specific intended use or application have been fulfilled.
    Note 1 to entry: The objective evidence needed for a validation is the result of a test or other form of determination, such as performing alternative calculations or reviewing documents.
    Note 2 to entry: The word 'validated' is used to designate the corresponding status.
    Note 3 to entry: The use conditions for validation can be real or simulated."""@en ;
    skos:prefLabel "Validation"@en .

eaj:verification a skos:Concept ;
    dcterms:source "https://www.iso.org/obp/ui/fr/#iso:std:iso:9000:ed-4:v1:en"^^xsd:anyURI ;
    rdfs:isDefinedBy <https://ref.engineersaustralia.org.au/def/ea-jargon> ;
    skos:inScheme <https://ref.engineersaustralia.org.au/def/ea-jargon> ;
    skos:topConceptOf <https://ref.engineersaustralia.org.au/def/ea-jargon> ;
    skos:definition """Confirmation, through the provision of objective evidence, that specified requirements have been fulfilled.
    Note 1 to entry: The objective evidence needed for a verification can be the result of an inspection or of other forms of determination, such as performing alternative calculations or reviewing documents.
    Note 2 to entry: The activities carried out for verification are sometimes called a qualification process.
    Note 3 to entry: The word 'verified' is used to designate the corresponding status."""@en ;
    skos:prefLabel "Verification"@en .

prty:board a skos:Concept ;
    rdfs:seeAlso <https://ref.engineersaustralia.org.au/def/ea-regulated-bodies/ea-board> ;
    rdfs:isDefinedBy <https://ref.engineersaustralia.org.au/def/ea-party> ;
    skos:inScheme <https://ref.engineersaustralia.org.au/def/ea-jargon> ;
    skos:topConceptOf <https://ref.engineersaustralia.org.au/def/ea-jargon> .

prty:committee a skos:Concept ;
    skos:inScheme <https://ref.engineersaustralia.org.au/def/ea-jargon> ;
    skos:topConceptOf <https://ref.engineersaustralia.org.au/def/ea-jargon> .

prty:project-control-board a skos:Concept ;
    skos:inScheme <https://ref.engineersaustralia.org.au/def/ea-jargon> ;
    skos:topConceptOf <https://ref.engineersaustralia.org.au/def/ea-jargon> .

prty:technical-society a skos:Concept ;
    skos:inScheme <https://ref.engineersaustralia.org.au/def/ea-jargon> ;
    skos:topConceptOf <https://ref.engineersaustralia.org.au/def/ea-jargon>  .

#Collections

eaj:data-theory-terms a skos:Collection ;
    dcterms:source "https://linked.data.gov.au/org/engineersaustralia"^^xsd:anyURI ;
	skos:prefLabel "Glossary - Data and Digital Concepts and Theory"@en ;
	skos:definition """The terminology used to describe and distinguish data and its associated processes."""@en ;
    skos:member
        eaj:analytical-model,
            eaj:descriptive-model,
            eaj:diagnostic-model,
            eaj:predictive-model,
            eaj:prescriptive-model,
        eaj:data,
            eaj:ref-data,
            eaj:transactional-data,
            eaj:master-data,
            eaj:data-dictionary,
        eaj:identity-management,
        eaj:information,
        eaj:data-catalogue,
        eaj:data-model,
            eaj:ontological-data-model,
            eaj:canonical-data-model,
            eaj:operational-data-model,
            eaj:analytical-data-model,
        eaj:data-profiling,
        eaj:data-lifecycle,
        eaj:digital-transformation,
        eaj:digital-experience,
        eaj:least-privilege,
        eaj:master-data-management,
        eaj:mfa,
        eaj:sso,
        eaj:system-architecture,
        eaj:persistent-identifier.

eaj:platform-terms a skos:Collection ;
    dcterms:source "https://linked.data.gov.au/org/engineersaustralia"^^xsd:anyURI ;
	skos:prefLabel "Glossary - ICT Systems, Platforms, and Processes"@en ;
	skos:definition """Types of Processes, Systems, Software, Tools, Portals, and Products used by Engineers Australia to interact with data and users."""@en ;
    skos:member
        eaj:active-directory,
        eaj:bi-platform,
        eaj:content-management-system,
        eaj:crm,
        eaj:database,
            eaj:relational-database,
            eaj:non-relational-database,
        eaj:data-catalogue,
        eaj:data-dictionary,
        eaj:data-warehouse,
        eaj:data-store,
        eaj:doc-management-system,
        eaj:ict-change,
        eaj:ict-change-freeze,
        eaj:ict-change-priority,
        eaj:ict-event,
        eaj:ict-problem,
        eaj:ict-rfc,
        itev:ict-incident,
        itev:ict-request,
        itev:ict-enhancement,
        itev:ict-maintenance,
        eaj:identity-management-app,
        eaj:learning-management-system,
        eaj:knowledgebase,
        eaj:ref-data-management-system,
        eaj:duty-separation,
        eaj:sso .

eaj:policy-terms a skos:Collection ;
    dcterms:source "https://linked.data.gov.au/org/engineersaustralia"^^xsd:anyURI ;
	skos:prefLabel "Glossary - Policy and Procedure"@en ;
	skos:definition """Documents that outline objectives and ways of working. Distinct from operational documents that record instances of information."""@en ;
    skos:member
        eaj:aus-privacy-act,
        eaj:aus-privacy-principles,
        eaj:code-of-ethics,
        eaj:ea-membership-regulations,
        eaj:div-rules,
        eaj:disciplinary-and-appeals .

eaj:professional-standards-terms a skos:Collection ;
    dcterms:source "https://linked.data.gov.au/org/engineersaustralia"^^xsd:anyURI ;
    prov:qualifiedAttribution
        [
            dcat:hadRole earl:data-steward ;
            prov:agent [
                    a prov:Agent ;
                    rdfs:label "Engineers Australia: Professional Standards"
                ],
                eatm:prof-stds ;
        ] ;
	skos:prefLabel "Glossary - Professional Standards"@en ;
	skos:definition """Terminology used by the Professional Standards team of Engineers Australia to interact with users, partner organisations, and representative bodies such as the International Engineering Alliance."""@en ;
    skos:member
        prty:committee,
        docs:policy,
        docs:procedure,
        eaj:accreditation,
        eaj:aecs,
        eaj:areas-of-practice,
        eaj:audit,
        eaj:awareness,
        eaj:benchmarking,
        eaj:change-management,
        eaj:chartered,
        eaj:code-of-ethics,
        eaj:competence,
        eaj:competency-assessment,
        eaj:competency-standard,
        eaj:consequence,
        eaj:continuing-professional-development,
        eaj:control,
        eaj:cpd-assessment,
        eaj:cpd-assessment-review,
        eaj:cpd-audit,
        eaj:cpd-requirements,
        eaj:credentials,
        eaj:current-level-of-risk,
        eaj:demonstrate-integrity,
        eaj:doc-management-system,
        eaj:ea-assessment,
        eaj:engineering-accords,
        eaj:event,
        eaj:exercise-leadership,
        eaj:formal-qualifications,
        eaj:inherent-risk,
        eaj:likelihood,
        eaj:practise-competently,
        eaj:prof-standard,
        eaj:promote-sustainability,
        eaj:qualifications,
        eaj:quality-assurance,
        eaj:quality-control,
        eaj:residual-risk,
        eaj:risk,
        eaj:risk-analysis,
        eaj:risk-assessment,
        eaj:risk-appetite,
        eaj:risk-criteria,
        eaj:risk-owner,
        eaj:risk-source,
        eaj:risk-sponsor,
        eaj:risk-tolerance,
        eaj:risk-treatment,
        eaj:validation,
        eaj:verification,
        earp:applicant ,
        ieaoc:assoc-engineer,
        ieaoc:pro-engineer,
        ieaoc:tech-engineer .

eaj:program-mgmt-terms a skos:Collection ;
    dcterms:source "https://linked.data.gov.au/org/engineersaustralia"^^xsd:anyURI ;
	skos:prefLabel "Glossary - Program Management"@en ;
	skos:definition """Terminology used in program management, particularly those involved in techology implementation or software development."""@en ;
    skos:member
        earl:actor,
        eaj:product-feature,
        eaj:user-story .

eaj:risk-terms a skos:Collection ;
    dcterms:source "https://linked.data.gov.au/org/engineersaustralia"^^xsd:anyURI ;
    prov:qualifiedAttribution
        [
            dcat:hadRole earl:data-steward ;
            prov:agent [
                    a prov:Agent ;
                    rdfs:label "Engineers Australia: Risk and Compliance Manager"
                ],
                eatm:prof-stds ;
        ] ;
	skos:prefLabel "Glossary - Risk Concepts"@en ;
	skos:definition """Standard definitions within the Australian risk standard AS ISO 31000:2018 and ISO Guide 73:2009."""@en ;
    skos:member
        eaj:consequence,
        eaj:control,
        eaj:event,
        eaj:likelihood,
        eaj:risk,
        eaj:inherent-risk,
        eaj:current-level-of-risk,
        eaj:residual-risk,
        eaj:risk-analysis,
        eaj:risk-appetite,
        eaj:risk-criteria,
        eaj:risk-owner,
        eaj:risk-profile,
        eaj:risk-source,
        eaj:risk-sponsor,
        eaj:risk-exposure,
        eaj:risk-tolerance,
        eaj:risk-treatment,
        eaj:risk-maturity,
        eaj:risk-evaluation,
        eaj:risk-assessment,
        eaj:strategic-context,
        eaj:internal-context,
        eaj:external-context,
        eaj:monitoring,
        eaj:shared-risks,
        eaj:stakeholder .