@prefix dcterms: <http://purl.org/dc/terms/> .
@prefix eagrd: <https://ref.engineersaustralia.org.au/def/ea-membership-grade/> .
@prefix cs: <https://ref.engineersaustralia.org.au/def/ea-membership-grade> .
@prefix owl: <http://www.w3.org/2002/07/owl#> .
@prefix rdfs: <http://www.w3.org/2000/01/rdf-schema#> .
@prefix sdo: <http://schema.org/> .
@prefix skos: <http://www.w3.org/2004/02/skos/core#> .
@prefix xsd: <http://www.w3.org/2001/XMLSchema#> .

<https://ref.engineersaustralia.org.au/def/ea-membership-grade> a owl:Ontology,
        skos:ConceptScheme ;
    dcterms:accessRights <https://linked.data.gov.au/def/data-access-rights/open> ;
    dcterms:created "2022-11-08"^^xsd:date ;
    dcterms:creator <https://linked.data.gov.au/org/engineersaustralia> ;
    dcterms:modified "2023-05-09"^^xsd:date ;
    dcterms:publisher <https://linked.data.gov.au/org/engineersaustralia> ;
    dcterms:source "https://linked.data.gov.au/org/engineersaustralia"^^xsd:anyURI ;
    skos:definition "The grade of membership of Engineers Australia. Grade reflects the experience and skill level of a member and corresponds to a specific level of EA Membership. The members of Engineers Australia are those persons whose names are entered in the register of members."@en ;
    skos:hasTopConcept
        eagrd:fellow,
        eagrd:member,
        eagrd:graduate,
        eagrd:student,
        eagrd:hon-fellow,
        eagrd:companion,
        eagrd:affiliate,
        eagrd:40-year ;
    skos:altLabel "Full Member"@en ;
    skos:prefLabel "Engineers Australia Membership Grade"@en .

<https://linked.data.gov.au/org/engineersaustralia> a sdo:Organization ;
    sdo:name "Engineers Australia" ;
    sdo:url "https://www.engineersaustralia.org.au"^^xsd:anyURI .
    
eagrd:affiliate a skos:Concept ;
    dcterms:source "https://linked.data.gov.au/org/engineersaustralia"^^xsd:anyURI ;
    rdfs:isDefinedBy cs: ;
    skos:inScheme cs: ;
    skos:topConceptOf cs: ;
    skos:definition """A member of Engineers Australia who is not part of the engineering profession and is therefore ineligible to be a Fellow, Member, Graduate or Student, but who has an interest in the engineering profession. Similar to Member grade for a non-engineer."""@en ;
    skos:notation "Affil" ;
    skos:prefLabel "Affiliate"@en .

eagrd:companion a skos:Concept ;
    dcterms:source "https://linked.data.gov.au/org/engineersaustralia"^^xsd:anyURI ;
    rdfs:isDefinedBy cs: ;
    skos:inScheme cs: ;
    skos:topConceptOf cs: ;
    skos:definition """A member of Engineers Australia who is not part of the engineering profession and is therefore ineligible to be a Fellow, Member, Graduate or Student, but who has an interest in the engineering profession and has made a significant contribution. Similar to Fellow grade for a non-engineer."""@en ;
    skos:notation "Comp" ;
    skos:prefLabel "Companion"@en .

eagrd:fellow a skos:Concept ;
    dcterms:source "https://linked.data.gov.au/org/engineersaustralia"^^xsd:anyURI ;
    rdfs:isDefinedBy cs: ;
    skos:inScheme cs: ;
    skos:topConceptOf cs: ;
    skos:definition """A member of Engineers Australia and very experienced engineer who has made a significant contribution to the profession. To apply for membership at the grade of Fellow, an applicant must:
    - Have held a sustained major responsibility in the design or execution of important engineering work; or
    - Have high education qualifications, held a prominent position in the profession and made a major contribution to the science or practice of engineering; or
    - Have had suitable engineering education/training, extensive responsibility in the design/execution of important engineering work and achieved exceptional eminence in the profession.
    - In all but exceptional circumstances, an applicant for Fellow will be a Chartered Member or have been Chartered with Engineers Australia Previously known as an Officer Fellow."""@en ;
    skos:hiddenLabel "Officer Fellow"@en ;
    skos:notation "F" ;
    skos:prefLabel "Fellow"@en .

eagrd:graduate a skos:Concept ;
    dcterms:source "https://linked.data.gov.au/org/engineersaustralia"^^xsd:anyURI ;
    rdfs:isDefinedBy cs: ;
    skos:inScheme cs: ;
    skos:topConceptOf cs: ;
    skos:definition """Graduate membership is available to graduated engineers who studied an accredited or recognised course in Engineering and are no more than four years out of university. Previously known as a Graduate Officer."""@en ;
    skos:hiddenLabel "Graduate Officer"@en ;
    skos:notation "Grad" ;
    skos:prefLabel "Graduate"@en .

eagrd:year-0-graduate a skos:Concept ;
    dcterms:source "https://linked.data.gov.au/org/engineersaustralia"^^xsd:anyURI ;
    rdfs:isDefinedBy cs: ;
    skos:inScheme cs: ;
    skos:broader eagrd:graduate ;
    skos:definition """Year-0 Graduate membership is available to graduated engineers who studied an accredited or recognised course in Engineering and are no more than four years out of university, and who have been granted a graduate membership through the Engineering Education Australia (EEA) Graduate Program upgrade. """@en ;
    skos:altLabel "Year 0 Graduate"@en ;
    skos:notation "Grad" ;
    skos:prefLabel "Graduate - Year 0"@en .

eagrd:hon-fellow a skos:Concept ;
    dcterms:source "https://linked.data.gov.au/org/engineersaustralia"^^xsd:anyURI ;
    rdfs:isDefinedBy cs: ;
    skos:inScheme cs: ;
    skos:topConceptOf cs: ;
    skos:definition """An honorary title for a member of Engineers Australia for outstanding achievement and contribution to the profession."""@en ;
    skos:notation "HonF" ;
    skos:prefLabel "Honorary Fellow"@en .

eagrd:member a skos:Concept ;
    dcterms:source "https://linked.data.gov.au/org/engineersaustralia"^^xsd:anyURI ;
    rdfs:isDefinedBy cs: ;
    skos:inScheme cs: ;
    skos:topConceptOf cs: ;
    skos:definition """The grade of Member is open to those who hold an Engineers Australia accredited or recognised Australian tertiary qualification in engineering, and have gained at least 3 years of postgraduate experience in the engineering industry. Previously known as an Officer Member."""@en ;
    skos:hiddenLabel "Officer Member"@en ;
    skos:notation "M" ;
    skos:prefLabel "Member"@en .

eagrd:student a skos:Concept ;
    dcterms:source "https://linked.data.gov.au/org/engineersaustralia"^^xsd:anyURI ;
    rdfs:isDefinedBy cs: ;
    skos:inScheme cs: ;
    skos:topConceptOf cs: ;
    skos:definition """Student membership is available to undergraduate students studying an accredited or recognised Australian course in Engineering."""@en ;
    skos:notation "Stud" ;
    skos:prefLabel "Student"@en .

eagrd:40-year a skos:Concept ;
    dcterms:source "https://linked.data.gov.au/org/engineersaustralia"^^xsd:anyURI ;
    owl:deprecated true ;
    rdfs:isDefinedBy cs: ;
    skos:inScheme cs: ;
    skos:topConceptOf cs: ;
    skos:definition """A legacy member grade for Engineers Australia members who qualified for a complimentary membership after 40-years continuous membership."""@en ;
    skos:notation "40Y" ;
    skos:prefLabel "40-Year Free Member"@en .

eagrd:paid a skos:Collection ;
    skos:prefLabel "Paid Membership"@en ;
	skos:definition """Membership grades that require payment to maintain and access Engineers Australia services and products."""@en ;
    skos:member
        eagrd:affiliate,
        eagrd:companion,
        eagrd:fellow,
        eagrd:graduate,
        eagrd:member .

eagrd:unpaid a skos:Collection ;
    skos:prefLabel "Unpaid Membership"@en ;
    skos:altLabel "Free Membership"@en ;
	skos:definition """Membership grades that are provided free of charge for members to access Engineers Australia services and products.."""@en ;
    skos:member
        eagrd:student,
        eagrd:year-0-graduate,
        eagrd:hon-fellow,
        eagrd:40-year .
