@prefix dcterms: <http://purl.org/dc/terms/> .
@prefix eagrd: <https://linked.data.gov.au/def/ea-membership-grade/> .
@prefix owl: <http://www.w3.org/2002/07/owl#> .
@prefix rdfs: <http://www.w3.org/2000/01/rdf-schema#> .
@prefix sdo: <http://schema.org/> .
@prefix skos: <http://www.w3.org/2004/02/skos/core#> .
@prefix xsd: <http://www.w3.org/2001/XMLSchema#> .

<https://linked.data.gov.au/def/ea-membership-grade> a owl:Ontology,
        skos:ConceptScheme ;
    dcterms:accessRights <https://linked.data.gov.au/def/data-access-rights/open> ;
    dcterms:created "2022-11-08"^^xsd:date ;
    dcterms:creator <https://linked.data.gov.au/org/engineersaustralia> ;
    dcterms:modified "2023-05-09"^^xsd:date ;
    dcterms:publisher <https://linked.data.gov.au/org/engineersaustralia> ;
    dcterms:source "https://linked.data.gov.au/org/engineersaustralia"^^xsd:anyURI ;
    skos:definition "The grade of membership of Engineers Australia. Grade reflects the experience and skill level of a member and corresponds to a specific level of EA Membership."@en ;
    skos:altLabel "Full Member"@en ;
    skos:prefLabel "Engineers Australia Membership Grade"@en .

<https://linked.data.gov.au/org/engineersaustralia> a sdo:Organization ;
    sdo:name "Engineers Australia" ;
    sdo:url "https://www.engineersaustralia.org.au"^^xsd:anyURI .
    
eagrd:affiliate a skos:Concept ;
    dcterms:source "https://linked.data.gov.au/org/engineersaustralia"^^xsd:anyURI ;
    rdfs:isDefinedBy <https://linked.data.gov.au/def/ea-membership-grade> ;
    skos:definition """A member of Engineers Australia who is not part of the engineering profession and is therefore ineligible to be a Fellow, Member, Graduate or Student, but who has an interest in the engineering profession. Similar to Member grade for a non-engineer."""@en ;
    skos:inScheme <https://linked.data.gov.au/def/ea-membership-grade> ;
    skos:notation "Affil" ;
    skos:prefLabel "Affiliate"@en ;
    skos:topConceptOf <https://linked.data.gov.au/def/ea-membership-grade> .

eagrd:companion a skos:Concept ;
    dcterms:source "https://linked.data.gov.au/org/engineersaustralia"^^xsd:anyURI ;
    rdfs:isDefinedBy <https://linked.data.gov.au/def/ea-membership-grade> ;
    skos:definition """A member of Engineers Australia who is not part of the engineering profession and is therefore ineligible to be a Fellow, Member, Graduate or Student, but who has an interest in the engineering profession and has made a significant contribution. Similar to Fellow grade for a non-engineer."""@en ;
    skos:inScheme <https://linked.data.gov.au/def/ea-membership-grade> ;
    skos:notation "Comp" ;
    skos:prefLabel "Companion"@en ;
    skos:topConceptOf <https://linked.data.gov.au/def/ea-membership-grade> .

eagrd:fellow a skos:Concept ;
    dcterms:source "https://linked.data.gov.au/org/engineersaustralia"^^xsd:anyURI ;
    rdfs:isDefinedBy <https://linked.data.gov.au/def/ea-membership-grade> ;
    skos:definition """A member of Engineers Australia and very experienced engineer who has made a significant contribution to the profession. To apply for membership at the grade of Fellow, an applicant must:
    - Have held a sustained major responsibility in the design or execution of important engineering work; or
    - Have high education qualifications, held a prominent position in the profession and made a major contribution to the science or practice of engineering; or
    - Have had suitable engineering education/training, extensive responsibility in the design/execution of important engineering work and achieved exceptional eminence in the profession.
    - In all but exceptional circumstances, an applicant for Fellow will be a Chartered Member or have been Chartered with Engineers Australia Previously known as an Officer Fellow."""@en ;
    skos:hiddenLabel "Officer Fellow"@en ;
    skos:inScheme <https://linked.data.gov.au/def/ea-membership-grade> ;
    skos:notation "F" ;
    skos:prefLabel "Fellow"@en ;
    skos:topConceptOf <https://linked.data.gov.au/def/ea-membership-grade> .

eagrd:graduate a skos:Concept ;
    dcterms:source "https://linked.data.gov.au/org/engineersaustralia"^^xsd:anyURI ;
    rdfs:isDefinedBy <https://linked.data.gov.au/def/ea-membership-grade> ;
    skos:definition """Graduate membership is available to graduated engineers who an accredited or recognised course in Engineering and are no more than four years out of university.  Previously known as a Graduate Officer."""@en ;
    skos:hiddenLabel "Graduate Officer"@en ;
    skos:inScheme <https://linked.data.gov.au/def/ea-membership-grade> ;
    skos:notation "Grad" ;
    skos:prefLabel "Graduate"@en ;
    skos:topConceptOf <https://linked.data.gov.au/def/ea-membership-grade> .

eagrd:hon-fellow a skos:Concept ;
    dcterms:source "https://linked.data.gov.au/org/engineersaustralia"^^xsd:anyURI ;
    rdfs:isDefinedBy <https://linked.data.gov.au/def/ea-membership-grade> ;
    skos:definition """An honorary title for a member of Engineers Australia for outstanding achievement and contribution to the profession."""@en ;
    skos:inScheme <https://linked.data.gov.au/def/ea-membership-grade> ;
    skos:notation "HonF" ;
    skos:prefLabel "Honorary Fellow"@en ;
    skos:topConceptOf <https://linked.data.gov.au/def/ea-membership-grade> .

eagrd:member a skos:Concept ;
    dcterms:source "https://linked.data.gov.au/org/engineersaustralia"^^xsd:anyURI ;
    rdfs:isDefinedBy <https://linked.data.gov.au/def/ea-membership-grade> ;
    skos:definition """The grade of Member is open to those who hold an Engineers Australia accredited or recognised Australian tertiary qualification in engineering, and have gained at least 3 years of postgraduate experience in the engineering industry. Previously known as an Officer Member."""@en ;
    skos:hiddenLabel "Officer Member"@en ;
    skos:inScheme <https://linked.data.gov.au/def/ea-membership-grade> ;
    skos:notation "M" ;
    skos:prefLabel "Member"@en ;
    skos:topConceptOf <https://linked.data.gov.au/def/ea-membership-grade> .

eagrd:student a skos:Concept ;
    dcterms:source "https://linked.data.gov.au/org/engineersaustralia"^^xsd:anyURI ;
    rdfs:isDefinedBy <https://linked.data.gov.au/def/ea-membership-grade> ;
    skos:definition """Student membership is available to undergraduate students studying an accredited or recognised Australian course in Engineering."""@en ;
    skos:inScheme <https://linked.data.gov.au/def/ea-membership-grade> ;
    skos:notation "Stud" ;
    skos:prefLabel "Student"@en ;
    skos:topConceptOf <https://linked.data.gov.au/def/ea-membership-grade> .

eagrd:40-year a skos:Concept ;
    dcterms:source "https://linked.data.gov.au/org/engineersaustralia"^^xsd:anyURI ;
    rdfs:isDefinedBy <https://linked.data.gov.au/def/ea-membership-grade> ;
    skos:definition """A legacy member grade for Engineers Australia members who qualified for a complimentary membership after 40-years continuous membership."""@en ;
    skos:inScheme <https://linked.data.gov.au/def/ea-membership-grade> ;
    skos:notation "40Y" ;
    skos:prefLabel "40-Year Free Member"@en ;
    skos:topConceptOf <https://linked.data.gov.au/def/ea-membership-grade> .

eagrd:paid a skos:Collection ;
    skos:prefLabel "Paid Membership"@en ;
	skos:definition """Membership grades that require payment to maintain and access Engineers Australia services and products."""@en ;
    skos:member
        eagrd:affiliate,
        eagrd:companion,
        eagrd:fellow,
        eagrd:graduate,
        eagrd:member .

eagrd:unpaid a skos:Collection ;
    skos:prefLabel "Unpaid Membership"@en ;
    skos:altLabel "Free Membership"@en ;
	skos:definition """Membership grades that are provided free of charge for members to access Engineers Australia services and products.."""@en ;
    skos:member
        eagrd:student,
        eagrd:hon-fellow,
        eagrd:40-year .
