@prefix eamc: <https://linked.data.gov.au/def/ea-member-changes/> .
@prefix dc: <http://purl.org/dc/elements/1.1/> .
@prefix dcterms: <http://purl.org/dc/terms/> .
@prefix owl: <http://www.w3.org/2002/07/owl#> .
@prefix rdf: <http://www.w3.org/1999/02/22-rdf-syntax-ns#> .
@prefix rdfs: <http://www.w3.org/2000/01/rdf-schema#> .
@prefix sdo: <http://schema.org/> .
@prefix skos: <http://www.w3.org/2004/02/skos/core#> .
@prefix xml: <http://www.w3.org/XML/1998/namespace> .
@prefix xsd: <http://www.w3.org/2001/XMLSchema#> .

<https://linked.data.gov.au/def/ea-member-changes> a owl:Ontology ,
        skos:ConceptScheme ;
    dcterms:created "2023-03-07"^^xsd:date ;
    dcterms:creator <https://linked.data.gov.au/org/engineersaustralia>;
    dcterms:publisher <https://linked.data.gov.au/org/engineersaustralia>;
    dcterms:modified "2023-03-07"^^xsd:date ;
    dcterms:contributor <https://orcid.org/0000-0003-2309-7004> ;
    dcterms:source "https://www.engineersaustralia.org.au"^^xsd:anyURI ;
    dcterms:accessRights <https://linked.data.gov.au/def/data-access-rights/open> ;
    skos:definition """The changes to membership that a may occur within the framework of Engineers Australia membership. Changes are defined by status and grade and payment status. The terminating assignable concepts are nested in a dual hierarchy of status and payment groupings of membership grades. The status classification qualifies membership flux, i.e. the gains, losses, retention, and at-risk members. The payment classification qualifies impacts to revenue that result from changes to membership."""@en ;
    skos:prefLabel "Engineers Australia Membership Changes"@en .

<https://linked.data.gov.au/org/engineersaustralia>
    a sdo:Organization ;
    sdo:name "Engineers Australia" ;
    sdo:url "https://www.engineersaustralia.org.au"^^xsd:anyURI .

<https://orcid.org/0000-0003-2309-7004> a owl:NamedIndividual,
    sdo:Person ;
    sdo:affiliation [ a sdo:Organization ;
        sdo:name "Engineers Australia" ;
        sdo:url "https://www.engineersaustralia.org.au"^^xsd:anyURI ] ;
    sdo:name "Vance Kelly" ;
    sdo:identifier <https://orcid.org/0000-0003-2309-7004> .

eamc:current-member a skos:Concept ;
    dcterms:source "https://linked.data.gov.au/org/engineersaustralia"^^xsd:anyURI ;
    rdfs:isDefinedBy <https://linked.data.gov.au/def/ea-member-changes> ;
    skos:definition """An individual who has a current and active membership with Engineers Australia."""@en ;
    skos:inScheme <https://linked.data.gov.au/def/ea-member-changes> ;
    skos:prefLabel "Current Member"@en ;
    skos:topConceptOf <https://linked.data.gov.au/def/ea-member-changes> .

    eamc:revenue-gain a skos:Concept ;
        dcterms:source "https://linked.data.gov.au/org/engineersaustralia"^^xsd:anyURI ;
        rdfs:isDefinedBy <https://linked.data.gov.au/def/ea-member-changes> ;
        skos:definition """An individual who has a current and active paid membership with Engineers Australia and in the previous year provided no payment due to never having been a member, inactive membership, or free membership. A member change that increases member revenue relative to the prevous financial year."""@en ;
        skos:inScheme <https://linked.data.gov.au/def/ea-member-changes> ;
        skos:prefLabel "Revenue Gain"@en ;
        skos:broader eamc:current-member .

    eamc:revenue-potential a skos:Concept ;
        dcterms:source "https://linked.data.gov.au/org/engineersaustralia"^^xsd:anyURI ;
        rdfs:isDefinedBy <https://linked.data.gov.au/def/ea-member-changes> ;
        skos:definition """An individual who has a current and active free membership with Engineers Australia and in the previous year also provided no payment due to never having been a member, inactive membership, or free membership. A member change that may become a future source of revenue."""@en ;
        skos:inScheme <https://linked.data.gov.au/def/ea-member-changes> ;
        skos:prefLabel "Revenue Potential"@en ;
        skos:broader eamc:current-member .

    eamc:revenue-exemption a skos:Concept ;
        dcterms:source "https://linked.data.gov.au/org/engineersaustralia"^^xsd:anyURI ;
        rdfs:isDefinedBy <https://linked.data.gov.au/def/ea-member-changes> ;
        skos:definition """An individual who has a current and active free and complimentary membership with Engineers Australia that is exempt from fees regardless of prevous membership or lack thereof. Complimentary membership and fee exemption is conferred upon Honorary Fellows."""@en ;
        skos:inScheme <https://linked.data.gov.au/def/ea-member-changes> ;
        skos:prefLabel "Revenue Exemption"@en ;
        skos:broader eamc:current-member .    

    eamc:acquisition a skos:Concept ;
        dcterms:source "https://linked.data.gov.au/org/engineersaustralia"^^xsd:anyURI ;
        rdfs:isDefinedBy <https://linked.data.gov.au/def/ea-member-changes> ;
        skos:definition """An individual who has a current and active membership with Engineers Australia but did not have active membership during the previous financial year. A member who has been added to active membership since last financial year."""@en ;
        skos:inScheme <https://linked.data.gov.au/def/ea-member-changes> ;
        skos:altLabel "Addition"@en ;
        skos:prefLabel "Aquisition"@en ;
        skos:broader eamc:current-member .

        eamc:admission a skos:Concept ;
            dcterms:source "https://linked.data.gov.au/org/engineersaustralia"^^xsd:anyURI ;
            rdfs:isDefinedBy <https://linked.data.gov.au/def/ea-member-changes> ;
            skos:definition """An individual who has a current and active membership with Engineers Australia but did not have active membership during the previous financial year or at any other preceding time. An individual who has joined EA membership since last financial year."""@en ;
            skos:inScheme <https://linked.data.gov.au/def/ea-member-changes> ;
            skos:prefLabel "Admission"@en ;
            skos:broader eamc:acquisition .

            eamc:free-admission a skos:Concept ;
                dcterms:source "https://linked.data.gov.au/org/engineersaustralia"^^xsd:anyURI ;
                rdfs:isDefinedBy <https://linked.data.gov.au/def/ea-member-changes> ;
                skos:definition """An individual who has a current and active free membership with Engineers Australia but did not have active membership during the previous financial year or at any other preceding time. An individual who has joined EA membership as a free member since last financial year."""@en ;
                skos:inScheme <https://linked.data.gov.au/def/ea-member-changes> ;
                skos:prefLabel "Free Admission"@en ;
                skos:broader eamc:admission .

                eamc:new-student a skos:Concept ;
                    dcterms:source "https://linked.data.gov.au/org/engineersaustralia"^^xsd:anyURI ;
                    rdfs:isDefinedBy <https://linked.data.gov.au/def/ea-member-changes> ;
                    skos:definition """An individual who has a current and active free and feeless Student grade membership with Engineers Australia but did not have active membership during the previous financial year or at any other preceding time. An individual who has joined EA membership as a free Student member since last financial year."""@en ;
                    skos:inScheme <https://linked.data.gov.au/def/ea-member-changes> ;
                    skos:prefLabel "New Student"@en ;
                    skos:broader eamc:free-admission, eamc:revenue-potential .

                eamc:new-hon-fellowship a skos:Concept ;
                    dcterms:source "https://linked.data.gov.au/org/engineersaustralia"^^xsd:anyURI ;
                    rdfs:isDefinedBy <https://linked.data.gov.au/def/ea-member-changes> ;
                    skos:definition """An individual who has a current and active free and complimentary Honorary Fellow grade membership with Engineers Australia but did not have active membership during the previous financial year or at any other preceding time. An individual who has joined EA membership as an Honorary Fellow since last financial year."""@en ;
                    skos:inScheme <https://linked.data.gov.au/def/ea-member-changes> ;
                    skos:prefLabel "New Honorary Fellowship"@en ;
                    skos:broader eamc:free-admission, eamc:revenue-exemption .

            eamc:new-member a skos:Concept ;
                dcterms:source "https://linked.data.gov.au/org/engineersaustralia"^^xsd:anyURI ;
                rdfs:isDefinedBy <https://linked.data.gov.au/def/ea-member-changes> ;
                skos:definition """An individual who has a current and active paid membership with Engineers Australia but did not have active membership during the previous financial year or at any other preceding time. An individual who has joined EA membership as a paid member since last financial year."""@en ;
                skos:inScheme <https://linked.data.gov.au/def/ea-member-changes> ;
                skos:prefLabel "New Member"@en ;
                skos:broader eamc:admission, eamc:revenue-gain .

        eamc:return a skos:Concept ;
            dcterms:source "https://linked.data.gov.au/org/engineersaustralia"^^xsd:anyURI ;
            rdfs:isDefinedBy <https://linked.data.gov.au/def/ea-member-changes> ;
            skos:definition """An individual who has a current and active membership with Engineers Australia but did not have active membership during the previous financial year. However, has held membership with Engineers Australia prior to the previous financial year. An individual who has re-joined EA membership after not having active membership in the last financial year."""@en ;
            skos:inScheme <https://linked.data.gov.au/def/ea-member-changes> ;
            skos:prefLabel "Return"@en ;
            skos:broader eamc:acquisition .

            eamc:paid-return a skos:Concept ;
                dcterms:source "https://linked.data.gov.au/org/engineersaustralia"^^xsd:anyURI ;
                rdfs:isDefinedBy <https://linked.data.gov.au/def/ea-member-changes> ;
                skos:definition """An individual who has a current and active paid membership with Engineers Australia but did not have active membership during the previous financial year. However, has held membership with Engineers Australia prior to the previous financial year. An individual who has re-joined EA membership as a paid member after not having active membership in the last financial year."""@en ;
                skos:inScheme <https://linked.data.gov.au/def/ea-member-changes> ;
                skos:prefLabel "Paid Return"@en ;
                skos:broader eamc:return .

                eamc:member-readmission a skos:Concept ;
                    dcterms:source "https://linked.data.gov.au/org/engineersaustralia"^^xsd:anyURI ;
                    rdfs:isDefinedBy <https://linked.data.gov.au/def/ea-member-changes> ;
                    skos:definition """An individual who has a current and active paid membership with Engineers Australia but did not have active membership during the previous financial year. However, has held membership with Engineers Australia prior to the previous financial year. An individual who had paid membership and has re-joined EA membership as a paid member after not having active membership in the last financial year."""@en ;
                    skos:inScheme <https://linked.data.gov.au/def/ea-member-changes> ;
                    skos:altLabel "Member Return"@en ;
                    skos:prefLabel "Member Readmission"@en ;
                    skos:broader eamc:paid-return, eamc:revenue-gain .

                eamc:ex-student-to-member a skos:Concept ;
                    dcterms:source "https://linked.data.gov.au/org/engineersaustralia"^^xsd:anyURI ;
                    rdfs:isDefinedBy <https://linked.data.gov.au/def/ea-member-changes> ;
                    skos:definition """An individual who has a current and active paid membership with Engineers Australia but did not have active membership during the previous financial year. However, has held membership with Engineers Australia prior to the previous financial year. An individual who had free Student grade membership that ended and has re-joined EA membership as a paid member after not having active membership in the last financial year."""@en ;
                    skos:inScheme <https://linked.data.gov.au/def/ea-member-changes> ;
                    skos:hiddenLabel "Ghost of Student Past"@en ;
                    skos:prefLabel "Ex-Student to Member"@en ;
                    skos:broader eamc:paid-return, eamc:revenue-gain . 

            eamc:student-readmission a skos:Concept ;
                dcterms:source "https://linked.data.gov.au/org/engineersaustralia"^^xsd:anyURI ;
                rdfs:isDefinedBy <https://linked.data.gov.au/def/ea-member-changes> ;
                skos:definition """An individual who has a current and active free Student membership with Engineers Australia but did not have active membership during the previous financial year. However, has held membership with Engineers Australia prior to the previous financial year. An individual who has re-joined EA membership as a Student member after not having active membership in the last financial year."""@en ;
                skos:inScheme <https://linked.data.gov.au/def/ea-member-changes> ;
                skos:altLabel "Unpaid Return"@en ;
                skos:prefLabel "Student Readmission"@en ;
                skos:broader eamc:return, eamc:revenue-potential .

    eamc:continuation a skos:Concept ;
        dcterms:source "https://linked.data.gov.au/org/engineersaustralia"^^xsd:anyURI ;
        rdfs:isDefinedBy <https://linked.data.gov.au/def/ea-member-changes> ;
        skos:definition """An individual who has a current and active membership with Engineers Australia carried over from the previous financial year."""@en ;
        skos:inScheme <https://linked.data.gov.au/def/ea-member-changes> ;
        skos:prefLabel "Continuation"@en ;
        skos:broader eamc:current-member .

        eamc:student-upgrade a skos:Concept ;
            dcterms:source "https://linked.data.gov.au/org/engineersaustralia"^^xsd:anyURI ;
            rdfs:isDefinedBy <https://linked.data.gov.au/def/ea-member-changes> ;
            skos:definition """An individual who has a current and active paid membership with Engineers Australia carried over from a free Student grade membership in the previous financial year."""@en ;
            skos:inScheme <https://linked.data.gov.au/def/ea-member-changes> ;
            skos:prefLabel "Student Upgrade"@en ;
            skos:broader eamc:continuation .

            eamc:promotion a skos:Concept ;
                dcterms:source "https://linked.data.gov.au/org/engineersaustralia"^^xsd:anyURI ;
                rdfs:isDefinedBy <https://linked.data.gov.au/def/ea-member-changes> ;
                skos:definition """An individual who has a current and active paid membership at non-Graduate grade with Engineers Australia carried over from a free Student grade membership in the previous financial year."""@en ;
                skos:inScheme <https://linked.data.gov.au/def/ea-member-changes> ;
                skos:prefLabel "Promotion"@en ;
                skos:broader eamc:student-upgrade, eamc:revenue-gain .

            eamc:graduation a skos:Concept ;
                dcterms:source "https://linked.data.gov.au/org/engineersaustralia"^^xsd:anyURI ;
                rdfs:isDefinedBy <https://linked.data.gov.au/def/ea-member-changes> ;
                skos:definition """An individual who has a current and active paid membership at Graduate grade with Engineers Australia carried over from a free Student grade membership in the previous financial year."""@en ;
                skos:inScheme <https://linked.data.gov.au/def/ea-member-changes> ;
                skos:prefLabel "Graduation"@en ;
                skos:broader eamc:student-upgrade, eamc:revenue-gain .

        eamc:retention a skos:Concept ;
            dcterms:source "https://linked.data.gov.au/org/engineersaustralia"^^xsd:anyURI ;
            rdfs:isDefinedBy <https://linked.data.gov.au/def/ea-member-changes> ;
            skos:definition """An individual who has a current and active paid membership with Engineers Australia carried over from likewise paid membership in the previous financial year."""@en ;
            skos:inScheme <https://linked.data.gov.au/def/ea-member-changes> ;
            skos:altLabel "Revenue Retention"@en,
                "Member Retention"@en ;
            skos:prefLabel "Retention"@en ;
            skos:broader eamc:continuation .

            eamc:renewal a skos:Concept ;
                dcterms:source "https://linked.data.gov.au/org/engineersaustralia"^^xsd:anyURI ;
                rdfs:isDefinedBy <https://linked.data.gov.au/def/ea-member-changes> ;
                skos:definition """An individual who has a current and active paid membership with Engineers Australia carried over from likewise paid membership in the previous financial year who made payment prior to the renewal fee due date."""@en ;
                skos:inScheme <https://linked.data.gov.au/def/ea-member-changes> ;
                skos:prefLabel "Renewal"@en ;
                skos:broader eamc:retention .

            eamc:reactivation a skos:Concept ;
                dcterms:source "https://linked.data.gov.au/org/engineersaustralia"^^xsd:anyURI ;
                rdfs:isDefinedBy <https://linked.data.gov.au/def/ea-member-changes> ;
                skos:definition """An individual who has a current and active paid membership with Engineers Australia carried over from likewise paid membership in the previous financial year but who failed to make payment prior to the renewal fee due date, and therefore transitioned to Lapsed membership status during the processing and erasure period."""@en ;
                skos:inScheme <https://linked.data.gov.au/def/ea-member-changes> ;
                skos:prefLabel "Reactivation"@en ;
                skos:broader eamc:retention .

        eamc:hon-fellowship a skos:Concept ;
            dcterms:source "https://linked.data.gov.au/org/engineersaustralia"^^xsd:anyURI ;
            rdfs:isDefinedBy <https://linked.data.gov.au/def/ea-member-changes> ;
            skos:definition """An individual who has a current and active free and complimentary Honorary Fellow grade membership with Engineers Australia carried over from a paid membership in the previous financial year. An individual who had paid EA membership and was been awarded Honorary Fellowship in the last financial year."""@en ;
            skos:inScheme <https://linked.data.gov.au/def/ea-member-changes> ;
            skos:prefLabel "Honorary Fellowship"@en ;
            skos:broader eamc:continuation, eamc:revenue-exemption .

        eamc:student-continuation a skos:Concept ;
            dcterms:source "https://linked.data.gov.au/org/engineersaustralia"^^xsd:anyURI ;
            rdfs:isDefinedBy <https://linked.data.gov.au/def/ea-member-changes> ;
            skos:definition """An individual who has a current and active free Student grade membership with Engineers Australia carried over from the previous financial year. A student membership that has not been cancelled or passed the maximum student membership duration."""@en ;
            skos:inScheme <https://linked.data.gov.au/def/ea-member-changes> ;
            skos:prefLabel "Student Continuation"@en ;
            skos:broader eamc:continuation, eamc:revenue-potential .

eamc:at-risk-member a skos:Concept ;
    dcterms:source "https://linked.data.gov.au/org/engineersaustralia"^^xsd:anyURI ;
    rdfs:isDefinedBy <https://linked.data.gov.au/def/ea-member-changes> ;
    skos:definition """An individual who had an active membership with Engineers Australia during the past financial year, but has not made sufficient payment by the due date to continue membership. A member at risk of erasure."""@en ;
    skos:inScheme <https://linked.data.gov.au/def/ea-member-changes> ;
    skos:prefLabel "At-Risk Member"@en ;
    skos:topConceptOf <https://linked.data.gov.au/def/ea-member-changes> .

    eamc:lapse a skos:Concept ;
        dcterms:source "https://linked.data.gov.au/org/engineersaustralia"^^xsd:anyURI ;
        rdfs:isDefinedBy <https://linked.data.gov.au/def/ea-member-changes> ;
        skos:definition """An individual who had an active membership with Engineers Australia during the past financial year, but has not made any renewal payment by the due date to continue membership. A member at risk of erasure."""@en ;
        skos:inScheme <https://linked.data.gov.au/def/ea-member-changes> ;
        skos:prefLabel "Lapse"@en ;
        skos:broader at-risk-member .    

    eamc:part-payment a skos:Concept ;
        dcterms:source "https://linked.data.gov.au/org/engineersaustralia"^^xsd:anyURI ;
        rdfs:isDefinedBy <https://linked.data.gov.au/def/ea-member-changes> ;
        skos:definition """An individual who had an active membership with Engineers Australia during the past financial year, and who has made incomplete payment of  renewal fees by the due date to continue membership. A member at risk of erasure."""@en ;
        skos:inScheme <https://linked.data.gov.au/def/ea-member-changes> ;
        skos:prefLabel "Lapse"@en ;
        skos:broader at-risk-member .    

eamc:lost-member a skos:Concept ;
    dcterms:source "https://linked.data.gov.au/org/engineersaustralia"^^xsd:anyURI ;
    rdfs:isDefinedBy <https://linked.data.gov.au/def/ea-member-changes> ;
    skos:definition """An individual who held membership with Engineers Australia in the past financial year but whose membership is now inactive."""@en ;
    skos:inScheme <https://linked.data.gov.au/def/ea-member-changes> ;
    skos:prefLabel "Lost Member"@en ;
    skos:topConceptOf <https://linked.data.gov.au/def/ea-member-changes> .

    eamc:termination a skos:Concept ;
        dcterms:source "https://linked.data.gov.au/org/engineersaustralia"^^xsd:anyURI ;
        rdfs:isDefinedBy <https://linked.data.gov.au/def/ea-member-changes> ;
        skos:definition """An individual who held a paid membership with Engineers Australia in the past financial year but whose membership is now inactive."""@en ;
        skos:inScheme <https://linked.data.gov.au/def/ea-member-changes> ;
        skos:altLabel "Revenue Loss"@en,
            "Member Loss"@en ;
        skos:prefLabel "Termination"@en ;
        skos:broader eamc:lost-member .

        eamc:erasure a skos:Concept ;
            dcterms:source "https://linked.data.gov.au/org/engineersaustralia"^^xsd:anyURI ;
            rdfs:isDefinedBy <https://linked.data.gov.au/def/ea-member-changes> ;
            skos:definition """An individual who held a paid membership with Engineers Australia in the past financial year but whose membership is now inactive after failure to make payment by the end of the processing and erasure period. A passive non-payment of fees and subsequent termination of membership."""@en ;
            skos:inScheme <https://linked.data.gov.au/def/ea-member-changes> ;
            skos:prefLabel "Erasure"@en ;
            skos:broader eamc:termination .

        eamc:cancellation a skos:Concept ;
            dcterms:source "https://linked.data.gov.au/org/engineersaustralia"^^xsd:anyURI ;
            rdfs:isDefinedBy <https://linked.data.gov.au/def/ea-member-changes> ;
            skos:definition """An individual who held a paid membership with Engineers Australia in the past financial year but whose membership is now inactive after informing Engineers Australia of intent to not renew membership. An active cancellation or deliberate non-payment of fees and subsequent termination of membership."""@en ;
            skos:inScheme <https://linked.data.gov.au/def/ea-member-changes> ;
            skos:prefLabel "Cancellation"@en ;
            skos:broader eamc:termination .

    eamc:student-cancellation a skos:Concept ;
        dcterms:source "https://linked.data.gov.au/org/engineersaustralia"^^xsd:anyURI ;
        rdfs:isDefinedBy <https://linked.data.gov.au/def/ea-member-changes> ;
        skos:definition """An individual who held a free Student grade membership with Engineers Australia in the past financial year but whose membership is now inactive due to active cancellation or exceeding the maximum student membership duration. Note: Maximum student membership duration may be extended at the discretion of Engineers Australia for extenuating or unusual circumstances."""@en ;
        skos:inScheme <https://linked.data.gov.au/def/ea-member-changes> ;
        skos:altLabel "Revenue Lost Potential"@en ;
        skos:prefLabel "Student Cancellation"@en ;
        skos:broader eamc:lost-member .

#COLLECTIONS

eamc:single-change-process a skos:Collection ;
    skos:prefLabel "Selectable Processes"@en ;
    skos:altLabel "Single-Change Processes"@en ;
	skos:definition """The current concepts without narrower concepts that are used to describe specific membership state changes."""@en ;
    skos:member
        eamc:new-member,
        eamc:new-student,
        eamc:new-hon-fellowship,
        eamc:member-readmission,
        eamc:ex-student-to-member,
        eamc:student-readmission,
        eamc:promotion,
        eamc:graduation,
        eamc:renewal,
        eamc:reactivation,
        eamc:hon-fellowship,
        eamc:student-continuation,
        eamc:lapse,
        eamc:part-payment,
        eamc:erasure,
        eamc:cancellation,
        eamc:student-cancellation .