@prefix eamc: <https://ref.engineersaustralia.org.au/def/ea-member-changes/> .
@prefix eamccs: <https://ref.engineersaustralia.org.au/def/ea-member-changes> .
@prefix dc: <http://purl.org/dc/elements/1.1/> .
@prefix dcterms: <http://purl.org/dc/terms/> .
@prefix owl: <http://www.w3.org/2002/07/owl#> .
@prefix rdf: <http://www.w3.org/1999/02/22-rdf-syntax-ns#> .
@prefix rdfs: <http://www.w3.org/2000/01/rdf-schema#> .
@prefix sdo: <http://schema.org/> .
@prefix skos: <http://www.w3.org/2004/02/skos/core#> .
@prefix xml: <http://www.w3.org/XML/1998/namespace> .
@prefix xsd: <http://www.w3.org/2001/XMLSchema#> .

<https://ref.engineersaustralia.org.au/def/ea-member-changes> a owl:Ontology ,
        skos:ConceptScheme ;
    dcterms:created "2023-03-07"^^xsd:date ;
    dcterms:creator <https://linked.data.gov.au/org/engineersaustralia>;
    dcterms:publisher <https://linked.data.gov.au/org/engineersaustralia>;
    dcterms:modified "2023-05-15"^^xsd:date ;
    dcterms:contributor <https://orcid.org/0000-0003-2309-7004> ;
    dcterms:source "https://www.engineersaustralia.org.au"^^xsd:anyURI ;
    dcterms:accessRights <https://linked.data.gov.au/def/data-access-rights/restricted> ;
    skos:hasTopConcept
        eamc:current-member,
        eamc:non-current-member ;
    skos:definition """The changes to membership that a may occur within the framework of Engineers Australia membership. Changes are defined by status and grade and payment status. The terminating assignable concepts are nested in a dual hierarchy of status and payment groupings of membership grades. The status classification qualifies membership flux, i.e. the gains, losses, retention, and at-risk members. The payment classification qualifies impacts to revenue that result from changes to membership.
    
    Processes are defined as the difference in membership attributes between two points in time. A reference period date that is typically the end of the last financial year, past quarter, or past month compared with an effective date of the analysis."""@en ;
    skos:prefLabel "Engineers Australia Membership Changes"@en .

<https://linked.data.gov.au/org/engineersaustralia>
    a sdo:Organization ;
    sdo:name "Engineers Australia" ;
    sdo:url "https://www.engineersaustralia.org.au"^^xsd:anyURI .

<https://orcid.org/0000-0003-2309-7004> a owl:NamedIndividual,
    sdo:Person ;
    sdo:affiliation [ a sdo:Organization ;
        sdo:name "Engineers Australia" ;
        sdo:url "https://www.engineersaustralia.org.au"^^xsd:anyURI ] ;
    sdo:name "Vance Kelly" ;
    sdo:identifier <https://orcid.org/0000-0003-2309-7004> .

#MEMBERSHIP FLUX - changes as categorised by their effect to the organisation's membership base

eamc:non-current-member a skos:Concept ;
    dcterms:source "https://linked.data.gov.au/org/engineersaustralia"^^xsd:anyURI ;
    rdfs:isDefinedBy eamccs: ;
    skos:definition """An individual whose membership with Engineers Australia is inactive."""@en ;
    skos:inScheme eamccs: ;
    skos:prefLabel "Non-Current Member"@en ;
    skos:topConceptOf eamccs: .

eamc:past-member a skos:Concept ;
    dcterms:source "https://linked.data.gov.au/org/engineersaustralia"^^xsd:anyURI ;
    rdfs:isDefinedBy eamccs: ;
    skos:definition """An individual whose membership is inactive, did not hold membership with Engineers Australia in the reference period, but who has previously been a member of EA."""@en ;
    skos:inScheme eamccs: ;
    skos:prefLabel "Past Member"@en ;
    skos:broader eamc:non-current-member .

eamc:lost-member a skos:Concept ;
    dcterms:source "https://linked.data.gov.au/org/engineersaustralia"^^xsd:anyURI ;
    rdfs:isDefinedBy eamccs: ;
    skos:definition """An individual whose membership is inactive but who held membership with Engineers Australia in the reference period."""@en ;
    skos:inScheme eamccs: ;
    skos:prefLabel "Lost Member"@en ;
    skos:broader eamc:non-current-member .

eamc:termination a skos:Concept ;
    dcterms:source "https://linked.data.gov.au/org/engineersaustralia"^^xsd:anyURI ;
    rdfs:isDefinedBy eamccs: ;
    skos:definition """An individual whose membership is inactive but who held a paid membership type with Engineers Australia in the reference period."""@en ;
    skos:inScheme eamccs: ;
    skos:prefLabel "Termination"@en ;
    skos:broader eamc:lost-member .

eamc:cancellation a skos:Concept ;
    dcterms:source "https://linked.data.gov.au/org/engineersaustralia"^^xsd:anyURI ;
    rdfs:isDefinedBy eamccs: ;
    skos:definition """An individual whose membership is inactive after resigning from the organisation or informing Engineers Australia of intent to not renew membership, but who held a paid membership type with Engineers Australia in the reference period.

    An active cancellation or deliberate non-payment of fees and subsequent termination of membership."""@en ;
    skos:inScheme eamccs: ;
    skos:prefLabel "Cancellation"@en ;
    skos:broader eamc:termination .

eamc:erasure a skos:Concept ;
    dcterms:source "https://linked.data.gov.au/org/engineersaustralia"^^xsd:anyURI ;
    rdfs:isDefinedBy eamccs: ;
    skos:definition """An individual whose membership is inactive after failure to make payment by the end of the processing and erasure period, but who held a paid membership type with Engineers Australia in the reference period.

    A passive non-payment of fees and subsequent termination of membership. Erasure occurs subsequent to a Lapsed status."""@en ;
    skos:inScheme eamccs: ;
    skos:prefLabel "Erasure"@en ;
    skos:broader eamc:termination .

eamc:student-erasure a skos:Concept ;
    dcterms:source "https://linked.data.gov.au/org/engineersaustralia"^^xsd:anyURI ;
    rdfs:isDefinedBy eamccs: ;
    skos:definition """An individual whose membership is inactive but who held a Student membership type with Engineers Australia in the reference period.

    Note: Student erasure is most commonly due to the maximum duration for student membership being exceeding. This duration may be extended at the discretion of Engineers Australia under extenuating or unusual circumstances."""@en ;
    skos:inScheme eamccs: ;
    skos:prefLabel "Student Erasure"@en ;
    skos:broader eamc:lost-member .

eamc:current-member a skos:Concept ;
    dcterms:source "https://linked.data.gov.au/org/engineersaustralia"^^xsd:anyURI ;
    rdfs:isDefinedBy eamccs: ;
    skos:definition """An individual whose membership with Engineers Australia is current and active."""@en ;
    skos:inScheme eamccs: ;
    skos:prefLabel "Current Member"@en ;
    skos:topConceptOf eamccs: .

eamc:carry-over a skos:Concept ;
    dcterms:source "https://linked.data.gov.au/org/engineersaustralia"^^xsd:anyURI ;
    rdfs:isDefinedBy eamccs: ;
    skos:definition """An individual whose membership with Engineers Australia is current and active, carried over from the reference period.

    A member who has been carried over as active membership from the reference period."""@en ;
    skos:inScheme eamccs: ;
    skos:prefLabel "Carry-Over"@en ;
    skos:broader eamc:current-member .

eamc:at-risk a skos:Concept ;
    dcterms:source "https://linked.data.gov.au/org/engineersaustralia"^^xsd:anyURI ;
    rdfs:isDefinedBy eamccs: ;
    skos:definition """An individual whose membership with Engineers Australia is current and active, carried over from the reference period, but who has not no owing membership fees prior to the due date to continue membership.

    A member at risk of erasure upon conclusion of the erasure period."""@en ;
    skos:inScheme eamccs: ;
    skos:prefLabel "At-Risk"@en ;
    skos:broader eamc:carry-over .

eamc:retention a skos:Concept ;
    dcterms:source "https://linked.data.gov.au/org/engineersaustralia"^^xsd:anyURI ;
    rdfs:isDefinedBy eamccs: ;
    skos:definition """An individual whose membership with Engineers Australia is current and active, carried over from the reference period, and who has no owing membership fees."""@en ;
    skos:inScheme eamccs: ;
    skos:prefLabel "Retention"@en ;
    skos:broader eamc:carry-over .

eamc:retention-from-unpaid a skos:Concept ;
    dcterms:source "https://linked.data.gov.au/org/engineersaustralia"^^xsd:anyURI ;
    rdfs:isDefinedBy eamccs: ;
    skos:definition """An individual whose membership with Engineers Australia is current and active, carried over from an Unpaid membership type in the reference period, and who has no owing membership fees."""@en ;
    skos:inScheme eamccs: ;
    skos:prefLabel "Retention from Unpaid"@en ;
    skos:broader eamc:retention .

eamc:unpaid-continuation a skos:Concept ;
    dcterms:source "https://linked.data.gov.au/org/engineersaustralia"^^xsd:anyURI ;
    rdfs:isDefinedBy eamccs: ;
    skos:definition """An individual whose membership with Engineers Australia is current and active, carried over from an Unpaid membership type in the reference period, and who has no owing membership fees due to a current Free-or-Complimentary membership."""@en ;
    skos:inScheme eamccs: ;
    skos:prefLabel "Unpaid Continuation"@en ;
    skos:broader eamc:retention-from-unpaid .

eamc:honorary-fellowship-continuation a skos:Concept ;
    dcterms:source "https://linked.data.gov.au/org/engineersaustralia"^^xsd:anyURI ;
    rdfs:isDefinedBy eamccs: ;
    skos:definition """An individual whose membership with Engineers Australia is current and active, carried over from an Unpaid membership type in the reference period, and who has no owing membership fees due to a current complimentary Honorary Fellow membership."""@en ;
    skos:inScheme eamccs: ;
    skos:prefLabel "Honorary Fellowship Continuation"@en ;
    skos:broader eamc:unpaid-continuation .

eamc:student-continuation a skos:Concept ;
    dcterms:source "https://linked.data.gov.au/org/engineersaustralia"^^xsd:anyURI ;
    rdfs:isDefinedBy eamccs: ;
    skos:definition """An individual whose membership with Engineers Australia is current and active, carried over from an Unpaid membership type in the reference period, and who has no owing membership fees due to a current free Student membership."""@en ;
    skos:inScheme eamccs: ;
    skos:prefLabel "Student Continuation"@en ;
    skos:broader eamc:unpaid-continuation .

eamc:student-upgrade a skos:Concept ;
    dcterms:source "https://linked.data.gov.au/org/engineersaustralia"^^xsd:anyURI ;
    rdfs:isDefinedBy eamccs: ;
    skos:definition """An individual whose membership with Engineers Australia is current and active, carried over from an Unpaid membership type in the reference period, and who has no owing membership for an upgraded Paid membership type."""@en ;
    skos:inScheme eamccs: ;
    skos:prefLabel "Student Upgrade"@en ;
    skos:broader eamc:retention-from-unpaid .

eamc:graduate-intake a skos:Concept ;
    dcterms:source "https://linked.data.gov.au/org/engineersaustralia"^^xsd:anyURI ;
    rdfs:isDefinedBy eamccs: ;
    skos:definition """An individual whose membership with Engineers Australia is current and active, carried over from an Unpaid membership type in the reference period, and who has no owing membership fees for an upgraded Paid Graduate membership type."""@en ;
    skos:inScheme eamccs: ;
    skos:prefLabel "Graduate Intake"@en ;
    skos:broader eamc:student-upgrade .

eamc:graduate-program-upgrade a skos:Concept ;
    dcterms:source "https://linked.data.gov.au/org/engineersaustralia"^^xsd:anyURI ;
    rdfs:isDefinedBy eamccs: ;
    skos:definition """An individual whose membership with Engineers Australia is current and active, carried over from an Unpaid membership type in the reference period, and who has no owing membership fees for an upgraded Paid Graduate membership type due to a 1 year fee dispensation upon completion of the EEA Graduate Program."""@en ;
    skos:inScheme eamccs: ;
    skos:prefLabel "Graduate Program Upgrade"@en ;
    skos:broader eamc:graduate-intake .

eamc:graduation a skos:Concept ;
    dcterms:source "https://linked.data.gov.au/org/engineersaustralia"^^xsd:anyURI ;
    rdfs:isDefinedBy eamccs: ;
    skos:definition """An individual whose membership with Engineers Australia is current and active, carried over from an Unpaid membership type in the reference period, and who has no owing membership fees for an upgraded Paid Graduate membership type due to full payment of membership fees."""@en ;
    skos:inScheme eamccs: ;
    skos:prefLabel "Graduation"@en ;
    skos:broader eamc:graduate-intake .

eamc:promotion a skos:Concept ;
    dcterms:source "https://linked.data.gov.au/org/engineersaustralia"^^xsd:anyURI ;
    rdfs:isDefinedBy eamccs: ;
    skos:definition """An individual whose membership with Engineers Australia is current and active, carried over from an Unpaid membership type in the reference period, and who has no owing membership fees for an upgraded Paid non-Graduate membership type."""@en ;
    skos:inScheme eamccs: ;
    skos:prefLabel "Promotion"@en ;
    skos:broader eamc:student-upgrade .

eamc:retention-from-paid a skos:Concept ;
    dcterms:source "https://linked.data.gov.au/org/engineersaustralia"^^xsd:anyURI ;
    rdfs:isDefinedBy eamccs: ;
    skos:definition """An individual whose membership with Engineers Australia is current and active, carried over from a Paid membership type in the reference period, and who has no owing membership fees."""@en ;
    skos:inScheme eamccs: ;
    skos:prefLabel "Retention from Paid"@en ;
    skos:broader eamc:retention .

eamc:paid-continuation a skos:Concept ;
    dcterms:source "https://linked.data.gov.au/org/engineersaustralia"^^xsd:anyURI ;
    rdfs:isDefinedBy eamccs: ;
    skos:definition """An individual whose membership with Engineers Australia is current and active, carried over from a Paid membership type in the reference period, and who has no owing membership fees due to full payment of membership fees."""@en ;
    skos:inScheme eamccs: ;
    skos:prefLabel "Paid Continuation"@en ;
    skos:broader eamc:retention-from-paid .

eamc:graduate-year-0-to-1 a skos:Concept ;
    dcterms:source "https://linked.data.gov.au/org/engineersaustralia"^^xsd:anyURI ;
    rdfs:isDefinedBy eamccs: ;
    skos:definition """An individual whose membership with Engineers Australia is current and active, carried over from a Paid membership type in the reference period, and who has no owing membership fees due to full payment of membership fees for the first time after a Year-0 Graduate dispensation."""@en ;
    skos:inScheme eamccs: ;
    skos:prefLabel "Graduate Year 0-to-1"@en ;
    skos:broader eamc:paid-continuation .

eamc:fee-rollover a skos:Concept ;
    dcterms:source "https://linked.data.gov.au/org/engineersaustralia"^^xsd:anyURI ;
    rdfs:isDefinedBy eamccs: ;
    skos:definition """An individual whose membership with Engineers Australia is current and active, carried over from a Paid membership type in the reference period, and who has no owing membership fees due to full payment of membership fees as a continuing fee-payer."""@en ;
    skos:inScheme eamccs: ;
    skos:prefLabel "Fee Rollover"@en ;
    skos:broader eamc:paid-continuation .

eamc:renewal a skos:Concept ;
    dcterms:source "https://linked.data.gov.au/org/engineersaustralia"^^xsd:anyURI ;
    rdfs:isDefinedBy eamccs: ;
    skos:definition """An individual whose membership with Engineers Australia is current and active, carried over from a Paid membership type in the reference period, and who has no owing membership fees due to full payment of membership fees as a continuing fee-payer prior to the renewal date."""@en ;
    skos:inScheme eamccs: ;
    skos:prefLabel "Renewal"@en ;
    skos:broader eamc:fee-rollover .

eamc:late-renewal a skos:Concept ;
    dcterms:source "https://linked.data.gov.au/org/engineersaustralia"^^xsd:anyURI ;
    rdfs:isDefinedBy eamccs: ;
    skos:definition """An individual whose membership with Engineers Australia is current and active, carried over from a Paid membership type in the reference period, and who has no owing membership fees due to full payment of membership fees as a continuing fee-payer after the renewal date but before the erasure date."""@en ;
    skos:inScheme eamccs: ;
    skos:prefLabel "Late Renewal"@en ;
    skos:broader eamc:fee-rollover .

eamc:reactivation a skos:Concept ;
    dcterms:source "https://linked.data.gov.au/org/engineersaustralia"^^xsd:anyURI ;
    rdfs:isDefinedBy eamccs: ;
    skos:definition """An individual whose membership with Engineers Australia is current and active, carried over from a Paid membership type in the reference period, and who has no owing membership fees due to full payment of membership fees as a continuing fee-payer after the erasure date but before the time period has elapsed that triggers the requirement for reassessment and readmission."""@en ;
    skos:inScheme eamccs: ;
    skos:prefLabel "Reactivation"@en ;
    skos:broader eamc:fee-rollover .

eamc:honorary-fellowship a skos:Concept ;
    dcterms:source "https://linked.data.gov.au/org/engineersaustralia"^^xsd:anyURI ;
    rdfs:isDefinedBy eamccs: ;
    skos:definition """An individual whose membership with Engineers Australia is current and active, carried over from a Paid membership type in the reference period, and who has no owing membership fees due to being granted a complimentary Honorary Fellow membership."""@en ;
    skos:inScheme eamccs: ;
    skos:prefLabel "Honorary Fellowship"@en ;
    skos:broader eamc:retention-from-paid .

eamc:member-gain a skos:Concept ;
    dcterms:source "https://linked.data.gov.au/org/engineersaustralia"^^xsd:anyURI ;
    rdfs:isDefinedBy eamccs: ;
    skos:definition """An individual whose membership with Engineers Australia is current and active, but did not have active membership during the reference period.

    A member who has been added to active membership from the reference period."""@en ;
    skos:inScheme eamccs: ;
    skos:prefLabel "Member Gain"@en ;
    skos:broader eamc:current-member .

eamc:new-admission a skos:Concept ;
    dcterms:source "https://linked.data.gov.au/org/engineersaustralia"^^xsd:anyURI ;
    rdfs:isDefinedBy eamccs: ;
    skos:definition """An individual whose membership with Engineers Australia is current and active, but did not have active membership during the reference period or at any other preceding time.

    An individual who has joined EA membership since the reference period."""@en ;
    skos:inScheme eamccs: ;
    skos:prefLabel "New Admission"@en ;
    skos:broader eamc:member-gain .

eamc:free-admission a skos:Concept ;
    dcterms:source "https://linked.data.gov.au/org/engineersaustralia"^^xsd:anyURI ;
    rdfs:isDefinedBy eamccs: ;
    skos:definition """An individual whose Free-or-Complimentary membership with Engineers Australia is current and active, but did not have active membership during the reference period or at any other preceding time.

    An individual who has joined EA membership as a free member since the reference period."""@en ;
    skos:inScheme eamccs: ;
    skos:prefLabel "Free Admission"@en ;
    skos:broader eamc:new-admission .

eamc:new-honorary-fellowship a skos:Concept ;
    dcterms:source "https://linked.data.gov.au/org/engineersaustralia"^^xsd:anyURI ;
    rdfs:isDefinedBy eamccs: ;
    skos:definition """An individual whose Complimentary Honorary Fellow membership with Engineers Australia is current and active, but did not have active membership during the reference period or at any other preceding time.

    An individual who has joined EA membership throughthe award of an Honorary Fellowhip since the reference period."""@en ;
    skos:inScheme eamccs: ;
    skos:prefLabel "New Honorary Fellowship"@en ;
    skos:broader eamc:free-admission .

eamc:new-student a skos:Concept ;
    dcterms:source "https://linked.data.gov.au/org/engineersaustralia"^^xsd:anyURI ;
    rdfs:isDefinedBy eamccs: ;
    skos:definition """An individual whose Free Student membership with Engineers Australia is current and active, but did not have active membership during the reference period or at any other preceding time.

    An individual who has joined EA membership as a free and feeless Student member sincethe reference period."""@en ;
    skos:inScheme eamccs: ;
    skos:prefLabel "New Student"@en ;
    skos:broader eamc:free-admission .

eamc:new-member a skos:Concept ;
    dcterms:source "https://linked.data.gov.au/org/engineersaustralia"^^xsd:anyURI ;
    rdfs:isDefinedBy eamccs: ;
    skos:definition """An individual whose Paid membership with Engineers Australia is current and active, but did not have active membership during the reference period or at any other preceding time.

    An individual who has joined EA membership as a paid member since reference period for the first time."""@en ;
    skos:inScheme eamccs: ;
    skos:prefLabel "New Member"@en ;
    skos:broader eamc:new-admission .

eamc:readmission a skos:Concept ;
    dcterms:source "https://linked.data.gov.au/org/engineersaustralia"^^xsd:anyURI ;
    rdfs:isDefinedBy eamccs: ;
    skos:definition """An individual whose membership with Engineers Australia is current and active, but did not have active membership during the reference period after holding a prior memberhsip.

    An individual who has re-joined EA membership after not having active membership during the reference period."""@en ;
    skos:inScheme eamccs: ;
    skos:prefLabel "Readmission"@en ;
    skos:broader eamc:member-gain .

eamc:student-readmission a skos:Concept ;
    dcterms:source "https://linked.data.gov.au/org/engineersaustralia"^^xsd:anyURI ;
    rdfs:isDefinedBy eamccs: ;
    skos:definition """An individual whose free Student membership with Engineers Australia is current and active, but did not have active membership during the reference period after holding a prior memberhsip.

    An individual who has re-joined EA Student membership after not having active membership during the reference period."""@en ;
    skos:inScheme eamccs: ;
    skos:prefLabel "Student Readmission"@en ;
    skos:broader eamc:readmission .

eamc:paid-readmission a skos:Concept ;
    dcterms:source "https://linked.data.gov.au/org/engineersaustralia"^^xsd:anyURI ;
    rdfs:isDefinedBy eamccs: ;
    skos:definition """An individual whose Paid membership with Engineers Australia is current and active, but did not have active membership during the reference period after holding a prior memberhsip.

    An individual who has re-joined EA Paid membership after not having active membership during the reference period."""@en ;
    skos:inScheme eamccs: ;
    skos:prefLabel "Paid Readmission"@en ;
    skos:broader eamc:readmission .

eamc:ex-student-to-member a skos:Concept ;
    dcterms:source "https://linked.data.gov.au/org/engineersaustralia"^^xsd:anyURI ;
    rdfs:isDefinedBy eamccs: ;
    skos:definition """An individual whose Paid membership with Engineers Australia is current and active, but did not have active membership during the reference period after holding a prior Student memberhsip.

    An individual who has re-joined EA Paid membership after not having active membership during the reference period, but having most recently been a student member."""@en ;
    skos:inScheme eamccs: ;
    skos:prefLabel "Ex-Student to Member"@en ;
    skos:broader eamc:paid-readmission .

eamc:member-readmission a skos:Concept ;
    dcterms:source "https://linked.data.gov.au/org/engineersaustralia"^^xsd:anyURI ;
    rdfs:isDefinedBy eamccs: ;
    skos:definition """An individual whose Paid membership with Engineers Australia is current and active, but did not have active membership during the reference period after holding a prior Paid memberhsip.

    An individual who has re-joined EA Paid membership after not having active membership during the reference period, and having most recently also been a Paid member."""@en ;
    skos:inScheme eamccs: ;
    skos:prefLabel "Member Readmission"@en ;
    skos:broader eamc:paid-readmission .

    
#COLLECTIONS

    eamc:revenue-acquisition a skos:Collection ;
        dcterms:source "https://linked.data.gov.au/org/engineersaustralia"^^xsd:anyURI ;
        skos:definition """An individual who has a current and active paid membership with Engineers Australia and in the reference period provided no payment due to never having been a member, an inactive membership, or a free membership. A member change that increases member revenue relative to the reference period."""@en ;
        skos:prefLabel "Revenue Acquisition"@en ;
        skos:member
            eamc:graduate-year-0-to-1,
            eamc:graduation,
            eamc:promotion,
            eamc:ex-student-to-member,
            eamc:member-readmission,
            eamc:new-member .

    eamc:revenue-retention a skos:Collection ;
        dcterms:source "https://linked.data.gov.au/org/engineersaustralia"^^xsd:anyURI ;
        skos:definition """An individual who has a current and active paid membership with Engineers Australia carried over from likewise paid membership in the reference period. An unchanged paid membership and maintained revenue."""@en ;
        skos:prefLabel "Member Change - Revenue Retention"@en ;
        skos:member
            eamc:renewal,
            eamc:late-renewal,
            eamc:reactivation .

    eamc:revenue-potential-gain a skos:Collection ;
        dcterms:source "https://linked.data.gov.au/org/engineersaustralia"^^xsd:anyURI ;
        skos:definition """An individual who has a current and active free membership with Engineers Australia and in the previous reference period also did not hold an active membership. A member change that adds potential for a future source of revenue."""@en ;
        skos:prefLabel "Member Change - Revenue Potential Gain"@en ;
        skos:member
            eamc:new-student,
            eamc:student-readmission .

    eamc:revenue-neutral a skos:Collection ;
        dcterms:source "https://linked.data.gov.au/org/engineersaustralia"^^xsd:anyURI ;
        skos:definition """An individual who has a current and active unpaid membership with Engineers Australia and in the reference period possessed a likewise free membership. A member change that has no impact on revenue or potential revenue relative to the reference period."""@en ;
        skos:prefLabel "Member Change - Revenue Neutral"@en ;
        skos:member
            eamc:honorary-fellowship-continuation,
            eamc:student-continuation,
            eamc:graduate-program-upgrade .

   eamc:revenue-exemption a skos:Collection ;
        dcterms:source "https://linked.data.gov.au/org/engineersaustralia"^^xsd:anyURI ;
        skos:definition """An individual who has a current and active free and complimentary membership with Engineers Australia as an that is exempt from fees and did not hold complimentary membership in the reference period. Complimentary membership and fee exemption is conferred upon Honorary Fellows. A member change that decreases member revenue relative to the reference period due to members being awarded complimentary membership"""@en ;
        skos:prefLabel "Member Change - Revenue Exemption"@en ;
        skos:member
            eamc:honorary-fellowship,
            eamc:new-honorary-fellowship .

    eamc:revenue-lost-potential a skos:Collection ;
        dcterms:source "https://linked.data.gov.au/org/engineersaustralia"^^xsd:anyURI ;
        skos:definition """An individual who held a free membership with Engineers Australia in the reference period but whose membership is now inactive. A member change that reduces leads and potential future revenue."""@en ;
        skos:prefLabel "Member Change - Revenue Potential Loss"@en ;
        skos:member
            eamc:student-erasure .

    eamc:revenue-at-risk a skos:Collection ;
        dcterms:source "https://linked.data.gov.au/org/engineersaustralia"^^xsd:anyURI ;
        skos:definition """An individual who had an active paid membership with Engineers Australia during the reference period, but has not made sufficient payment by the due date to continue membership. A member change that indicates a risk of revenue loss to the organisation if membership is not reactivated."""@en ;
        skos:altLabel "Revenue At-Risk"@en ;
        skos:prefLabel "Member Change - Revenue Risk"@en ;
        skos:member
            eamc:at-risk .

    eamc:revenue-loss a skos:Collection ;
        dcterms:source "https://linked.data.gov.au/org/engineersaustralia"^^xsd:anyURI ;
        skos:definition """An individual who held a paid membership with Engineers Australia in the reference period but whose membership is now inactive. A member change that decreases member revenue relative to the reference period due to membership reduction."""@en ;
        skos:prefLabel "Member Change - Revenue Loss"@en ;
        skos:member
            eamc:cancellation,
            eamc:erasure .

    eamc:revenue-historic a skos:Collection ;
        dcterms:source "https://linked.data.gov.au/org/engineersaustralia"^^xsd:anyURI ;
        skos:definition """An individual who held a paid membership with Engineers Australia prior-to-but-not-during the reference period and whose membership is now inactive. A state that does not affect revenue relative to the reference period but notes an individual who was once a member."""@en ;
        skos:prefLabel "Member Change - Revenue Historic"@en ;
        skos:member
            eamc:past-member .  

eamc:single-change-process a skos:Collection ;
    dcterms:source "https://linked.data.gov.au/org/engineersaustralia"^^xsd:anyURI ;
    skos:altLabel "Selectable Processes"@en ;
    skos:prefLabel "Member Change - Specific"@en ;
	skos:definition """The concepts without narrower concepts that are used to describe specific membership state changes."""@en ;
    skos:member
        eamc:past-member,
        eamc:cancellation,
        eamc:erasure,
        eamc:student-erasure,
        eamc:at-risk,
        eamc:honorary-fellowship-continuation,
        eamc:student-continuation,
        eamc:graduate-program-upgrade,
        eamc:graduation,
        eamc:promotion,
        eamc:graduate-year-0-to-1,
        eamc:renewal,
        eamc:late-renewal,
        eamc:reactivation,
        eamc:honorary-fellowship,
        eamc:new-honorary-fellowship,
        eamc:new-student,
        eamc:new-member,
        eamc:student-readmission,
        eamc:ex-student-to-member,
        eamc:member-readmission .
