PREFIX dcterms: <http://purl.org/dc/terms/>
PREFIX eams: <https://ref.engineersaustralia.org.au/def/ea-membership-status/>
PREFIX owl: <http://www.w3.org/2002/07/owl#>
PREFIX prov: <http://www.w3.org/ns/prov#>
PREFIX rdfs: <http://www.w3.org/2000/01/rdf-schema#>
PREFIX sdo: <http://schema.org/>
PREFIX skos: <http://www.w3.org/2004/02/skos/core#>
PREFIX xsd: <http://www.w3.org/2001/XMLSchema#>

<https://ref.engineersaustralia.org.au/def/ea-membership-status> a owl:Ontology,
        skos:ConceptScheme ;
    dcterms:accessRights <https://linked.data.gov.au/def/data-access-rights/restricted> ;
    dcterms:created "2024-01-17"^^xsd:date ;
    dcterms:creator <https://linked.data.gov.au/org/engineersaustralia> ;
    dcterms:modified "2024-01-17"^^xsd:date ;
    dcterms:publisher <https://linked.data.gov.au/org/engineersaustralia> ;
    dcterms:source "https://linked.data.gov.au/org/engineersaustralia"^^xsd:anyURI ;
    prov:qualifiedAttribution
    [
        dcat:hadRole earl:data-steward ;
        prov:agent [
                a prov:Agent ;
                rdfs:label "Engineers Australia: Customer Engagement and Assessments"
            ]
    ] ;
    skos:hasTopConcept
        eams:non-member,
        eams:active,
        eams:lapsed,
        eams:inactive ;
    skos:definition "The status of membership of an Engineers Australia member or prospective member."@en ;
    skos:prefLabel "Engineers Australia Membership Status"@en .
    
<https://linked.data.gov.au/org/engineersaustralia>
    a sdo:Organization ;
    sdo:name "Engineers Australia" ;
    sdo:url "https://www.engineersaustralia.org.au"^^xsd:anyURI .

<https://orcid.org/0000-0003-2309-7004> a owl:NamedIndividual,
    sdo:Person ;
    sdo:affiliation [ a sdo:Organization ;
        sdo:name "Engineers Australia" ;
        sdo:url "https://www.engineersaustralia.org.au"^^xsd:anyURI ] ;
    sdo:name "Vance Kelly" ;
    sdo:identifier <https://orcid.org/0000-0003-2309-7004> .

eams:non-member a skos:Concept ;
    dcterms:source "https://linked.data.gov.au/org/engineersaustralia"^^xsd:anyURI ;
    rdfs:isDefinedBy <https://ref.engineersaustralia.org.au/def/ea-membership-status> ;
    skos:inScheme <https://ref.engineersaustralia.org.au/def/ea-membership-status> ;
    skos:topConceptOf <https://ref.engineersaustralia.org.au/def/ea-membership-status> ;
    skos:definition """An individual who is not a current or former member of Engineers Australia.
    
    In application these individuals will have no membership events or member history."""@en ;
    skos:prefLabel "Non-Member"@en .

    eams:disallowed a skos:Concept ;
        dcterms:source "https://linked.data.gov.au/org/engineersaustralia"^^xsd:anyURI ;
        skos:inScheme <https://ref.engineersaustralia.org.au/def/ea-membership-status> ;
        rdfs:isDefinedBy <https://ref.engineersaustralia.org.au/def/ea-membership-status> ;
        skos:broader eams:non-member ;
        skos:definition """An individual who is not a current or former member of Engineers Australia and is disallowed from joining Engineers Australia membership."""@en ;
        skos:scopeNote """Applied to individuals who are not allowed to join EA, but is not indicative of the reason for prohibition. Access to sensitive documents may be required for further information."""@en ;
        skos:altLabel "Banned Applicant"@en,
            "Disallowed Applicant"@en,
            "Nuisance Applicant"@en,
            "Prohibited Applicant"@en ;
        skos:prefLabel "Disallowed"@en .

eams:active a skos:Concept ;
    dcterms:source "https://linked.data.gov.au/org/engineersaustralia"^^xsd:anyURI ;
    rdfs:isDefinedBy <https://ref.engineersaustralia.org.au/def/ea-membership-status> ;
    skos:inScheme <https://ref.engineersaustralia.org.au/def/ea-membership-status> ;
    skos:topConceptOf <https://ref.engineersaustralia.org.au/def/ea-membership-status> ;
    skos:broadMatch <https://ref.engineersaustralia.org.au/def/general-status/active> ;
    skos:definition """A member of Engineers Australia with a current membership with all fees and charges fully paid. These members have access to member benefits and are able to participate in Engineers Australia events, forums, and other services.

    In application the current date will be earlier than the membership renewal due date for these individuals."""@en ;
    skos:altLabel "Current"@en ;
    skos:prefLabel "Active"@en .

eams:restricted a skos:Concept ;
    dcterms:source "https://linked.data.gov.au/org/engineersaustralia"^^xsd:anyURI ;
    rdfs:isDefinedBy <https://ref.engineersaustralia.org.au/def/ea-membership-status> ;
    skos:inScheme <https://ref.engineersaustralia.org.au/def/ea-membership-status> ;
    skos:topConceptOf <https://ref.engineersaustralia.org.au/def/ea-membership-status> ;
    skos:definition """A member of Engineers Australia whose membership has expired due to non-payment before the due date, but whose membership has not yet been terminated as part of the subsequent erasure process. Lapsed or Restricted membership is only a valid status between the due date for renewal and the conclusion of the processing and erasure period when payment for membership has lapsed. Restrictions of services due to non payment of fees includes; ineligibility to be awarded Chartered and EngExec credentials, and may limited access to all members benefits e.g. mentoring program.
    
    In application the current date will be later than the membership renewal due date for these individuals but before the erasure date."""@en ;
    skos:altLabel "Lapsed"@en ;
    skos:prefLabel "Restricted"@en .

eams:inactive a skos:Concept ;
    dcterms:source "https://linked.data.gov.au/org/engineersaustralia"^^xsd:anyURI ;
    rdfs:isDefinedBy <https://ref.engineersaustralia.org.au/def/ea-membership-status> ;
    skos:inScheme <https://ref.engineersaustralia.org.au/def/ea-membership-status> ;
    skos:topConceptOf <https://ref.engineersaustralia.org.au/def/ea-membership-status> ;
    skos:broadMatch <https://ref.engineersaustralia.org.au/def/general-status/inactive> ;
    skos:definition """An individual who is not a current member of Engineers Australia but has held membership previously. These individuals do not have access to member benefits or the ability to participate in Engineers Australia events, forums, and other services.
    
    In application the current date will be later than both the membership renewal due date for these individuals and the erasure date."""@en ;
    skos:altLabel "Past"@en ;
    skos:prefLabel "Inactive"@en .

    eams:expelled-member a skos:Concept ;
        dcterms:source "https://www.engineersaustralia.org.au/sites/default/files/resource-files/2019-05/EA%20General%20Regulations%2002.05.19.pdf"^^xsd:anyURI ;
        skos:inScheme <https://ref.engineersaustralia.org.au/def/ea-membership-status> ;
        rdfs:isDefinedBy <https://ref.engineersaustralia.org.au/def/ea-membership-status> ;
        skos:broader eams:inactive ;
        skos:definition """An individual who is not a current member of Engineers Australia but has held membership previously, and is now permanently disallowed from re-joining Engineers Australia membership."""@en ;
        skos:scopeNote """Applied to former members who are not allowed to rejoin EA, but is not indicative of the reason for expulsion. Access to sensitive documents may be required for further information."""@en ;
        skos:altLabel "Banned Member"@en,
            "Prohibited Member"@en,
            "Cancelled"@en ;
        skos:prefLabel "Expelled"@en .

    eams:resigned a skos:Concept ;
        dcterms:source "https://linked.data.gov.au/org/engineersaustralia"^^xsd:anyURI ;
        skos:inScheme <https://ref.engineersaustralia.org.au/def/ea-membership-status> ;
        rdfs:isDefinedBy <https://ref.engineersaustralia.org.au/def/ea-membership-status> ;
        skos:broader eams:inactive ;
        skos:definition """An individual who is not a current member of Engineers Australia but has held membership previously, and who actively withdrew their membership from Engineers Australia through resignation."""@en ;
        skos:prefLabel "Resigned"@en .

    eams:suspended a skos:Concept ;
        dcterms:source "https://www.engineersaustralia.org.au/sites/default/files/resource-files/2019-05/EA%20General%20Regulations%2002.05.19.pdf"^^xsd:anyURI ;
        skos:inScheme <https://ref.engineersaustralia.org.au/def/ea-membership-status> ;
        rdfs:isDefinedBy <https://ref.engineersaustralia.org.au/def/ea-membership-status> ;
        skos:broader eams:inactive ;
        skos:definition """An individual who is not a current member of Engineers Australia but has held membership previously, and is now temporarily disallowed from re-joining Engineers Australia membership."""@en ;
        skos:scopeNote """Applied to former members who are not allowed to rejoin EA, but is not indicative of the reason for suspension of membership. Access to sensitive documents may be required for further information."""@en ;
        skos:prefLabel "Suspended"@en .

    eams:deceased a skos:Concept ;
        dcterms:source "https://linked.data.gov.au/org/engineersaustralia"^^xsd:anyURI ;
        skos:inScheme <https://ref.engineersaustralia.org.au/def/ea-membership-status> ;
        rdfs:isDefinedBy <https://ref.engineersaustralia.org.au/def/ea-membership-status> ;
        skos:broader eams:inactive ;
        skos:definition """A deceased individual who previously held membership with Engineers Australia."""@en ;
        skos:prefLabel "Deceased"@en .
