@prefix dcterms: <http://purl.org/dc/terms/> .
@prefix eagrd: <https://linked.data.gov.au/def/ea-membership-grade/> .
@prefix eams: <https://linked.data.gov.au/def/ea-membership-status/> .
@prefix owl: <http://www.w3.org/2002/07/owl#> .
@prefix rdfs: <http://www.w3.org/2000/01/rdf-schema#> .
@prefix sdo: <http://schema.org/> .
@prefix skos: <http://www.w3.org/2004/02/skos/core#> .
@prefix xsd: <http://www.w3.org/2001/XMLSchema#> .

<https://linked.data.gov.au/def/ea-membership-status> a owl:Ontology,
        skos:ConceptScheme ;
    dcterms:accessRights <https://linked.data.gov.au/def/data-access-rights/restricted> ;
    dcterms:created "2023-03-08"^^xsd:date ;
    dcterms:creator <https://linked.data.gov.au/org/engineersaustralia> ;
    dcterms:modified "2023-03-09"^^xsd:date ;
    dcterms:publisher <https://linked.data.gov.au/org/engineersaustralia> ;
    dcterms:source "https://linked.data.gov.au/org/engineersaustralia"^^xsd:anyURI ;
    skos:definition "The status of membership of an Engineers Australia member or prospective member."@en ;
    skos:prefLabel "Engineers Australia Membership Status"@en .
    
<https://linked.data.gov.au/org/engineersaustralia>
    a sdo:Organization ;
    sdo:name "Engineers Australia" ;
    sdo:url "https://www.engineersaustralia.org.au"^^xsd:anyURI .

<https://orcid.org/0000-0003-2309-7004> a owl:NamedIndividual,
    sdo:Person ;
    sdo:affiliation [ a sdo:Organization ;
        sdo:name "Engineers Australia" ;
        sdo:url "https://www.engineersaustralia.org.au"^^xsd:anyURI ] ;
    sdo:name "Vance Kelly" ;
    sdo:identifier <https://orcid.org/0000-0003-2309-7004> .

eams:non-member a skos:Concept ;
    dcterms:source "https://linked.data.gov.au/org/engineersaustralia"^^xsd:anyURI ;
    rdfs:isDefinedBy <https://linked.data.gov.au/def/ea-membership-status> ;
    skos:definition "An individual who is a prospective member of Engineers Australia and has not previously held membership with the organisation."@en ;
    skos:inScheme <https://linked.data.gov.au/def/ea-membership-status> ;
    skos:prefLabel "Non-Member"@en ;
    skos:topConceptOf <https://linked.data.gov.au/def/ea-membership-status> .

eams:active a skos:Concept ;
    dcterms:source "https://linked.data.gov.au/org/engineersaustralia"^^xsd:anyURI ;
    rdfs:isDefinedBy <https://linked.data.gov.au/def/ea-membership-status> ;
    skos:definition "A member of Engineers Australia with access to member benefits and able to participate in Engineers Australia events, forums, and other services."@en ;
    skos:inScheme <https://linked.data.gov.au/def/ea-membership-status> ;
    skos:prefLabel "Active"@en ;
    skos:topConceptOf <https://linked.data.gov.au/def/ea-membership-status> .

    eams:gratis a skos:Concept ;
        dcterms:source "https://linked.data.gov.au/org/engineersaustralia"^^xsd:anyURI ;
        rdfs:isDefinedBy <https://linked.data.gov.au/def/ea-membership-status> ;
        skos:definition "An active member of Engineers Australia exempt from payment. Typically a student membership."@en ;
        skos:related eagrd:student ;
        skos:inScheme <https://linked.data.gov.au/def/ea-membership-status> ;
            skos:altLabel "Gratis"@en,
                "Active Student"@en ;
        skos:prefLabel "Unpaid Active"@en ;
        skos:broader eams:active .

    eams:paid a skos:Concept ;
        dcterms:source "https://linked.data.gov.au/org/engineersaustralia"^^xsd:anyURI ;
        rdfs:isDefinedBy <https://linked.data.gov.au/def/ea-membership-status> ;
        skos:definition "An active non-student member of Engineers Australia with a paid membership. A membership that is a source of revenue."@en ;
        skos:inScheme <https://linked.data.gov.au/def/ea-membership-status> ;
        skos:altLabel "Fully Paid"@en;
        skos:prefLabel "Paid"@en ;
        skos:broader eams:active .

    eams:lapsed a skos:Concept ;
        dcterms:source "https://linked.data.gov.au/org/engineersaustralia"^^xsd:anyURI ;
        rdfs:isDefinedBy <https://linked.data.gov.au/def/ea-membership-status> ;
        skos:definition "An active non-student member of Engineers Australia whose paid membership has expired due to non-payment before the due date, but whose membership has not been terminated as part of the erasure process."@en ;
        skos:inScheme <https://linked.data.gov.au/def/ea-membership-status> ;
        skos:prefLabel "Lapsed"@en ;
        skos:broader eams:active .

eams:inactive a skos:Concept ;
    dcterms:source "https://linked.data.gov.au/org/engineersaustralia"^^xsd:anyURI ;
    rdfs:isDefinedBy <https://linked.data.gov.au/def/ea-membership-status> ;
    skos:definition "A previous member of Engineers Australia who has lost access to member benefits and the ability to participate in Engineers Australia events, forums, and other services. Typically due to membership cancellation or erasure."@en ;
    skos:inScheme <https://linked.data.gov.au/def/ea-membership-status> ;
    skos:prefLabel "Inactive"@en ;
    skos:topConceptOf <https://linked.data.gov.au/def/ea-membership-status> .

    eams:past-paid a skos:Concept ;
        dcterms:source "https://linked.data.gov.au/org/engineersaustralia"^^xsd:anyURI ;
        rdfs:isDefinedBy <https://linked.data.gov.au/def/ea-membership-status> ;
        skos:definition "A previous non-student member of Engineers Australia whose paid membership has expired due to active cancellation of membership or erasure following non-payment before the due date."@en ;
        skos:inScheme <https://linked.data.gov.au/def/ea-membership-status> ;
        skos:prefLabel "Past Paid"@en ;
        sskos:broader eams:inactive .

    eams:past-unpaid a skos:Concept ;
        dcterms:source "https://linked.data.gov.au/org/engineersaustralia"^^xsd:anyURI ;
        rdfs:isDefinedBy <https://linked.data.gov.au/def/ea-membership-status> ;
        skos:definition "A previous student member of Engineers Australia whose free membership has expired. Typically due to active cancellation of membership or cancellation due to surpassing the maximum duration for a student membership.
        
        The maximum duration of a student membership may be exceeded at the discretion of Engineers Australia to allow for interrupted and part time study."@en ;
        skos:inScheme <https://linked.data.gov.au/def/ea-membership-status> ;
        skos:prefLabel "Past Unpaid"@en ;
        skos:topConceptOf <https://linked.data.gov.au/def/ea-membership-status> .
