@prefix eats: <https://linked.data.gov.au/def/ea-tech-societies/> .
@prefix dc: <http://purl.org/dc/elements/1.1/> .
@prefix dcterms: <http://purl.org/dc/terms/> .
@prefix owl: <http://www.w3.org/2002/07/owl#> .
@prefix rdf: <http://www.w3.org/1999/02/22-rdf-syntax-ns#> .
@prefix rdfs: <http://www.w3.org/2000/01/rdf-schema#> .
@prefix sdo: <http://schema.org/> .
@prefix skos: <http://www.w3.org/2004/02/skos/core#> .
@prefix xml: <http://www.w3.org/XML/1998/namespace> .
@prefix xsd: <http://www.w3.org/2001/XMLSchema#> .

<https://linked.data.gov.au/def/ea-tech-societies> a owl:Ontology ,
        skos:ConceptScheme ;
    dcterms:created "2022-11-23"^^xsd:date ;
    dcterms:creator <https://linked.data.gov.au/org/engineersaustralia>;
    dcterms:publisher <https://linked.data.gov.au/org/engineersaustralia>;
    dcterms:modified "2022-11-23"^^xsd:date ;
    dcterms:contributor <https://orcid.org/0000-0003-2309-7004> ;
    dcterms:source "https://www.engineersaustralia.org.au/engineering-communities/technical-societies"^^xsd:anyURI ;
    dcterms:accessRights <https://linked.data.gov.au/def/data-access-rights/open> ;
    skos:definition """Engineers Australia has incorporated and unincorporated technical societies. Incorporated technical societies are governed by their own constitutions but choose to be aligned with Engineers Australia.

    Unincorporated technical societies are governed by a technical society committee that's under the direction of the Engineers Australia Board and is responsible to it.

    The Asset Management Council technical societies provide an important link between the wider profession and specific areas of technical practice.
    
    Joining a technical society allows you to network with other professionals in the same area of expertise, join discussion forums, read technical papers and watch presentations. By joining a technical society you'll also be able to participate in professional technical development opportunities. You don't need to be an Engineers Australia member to join a technical society. """@en ;
    skos:hasTopConcept
        eats:amc,       # Asset Management Council
        eats:aaee,      # Australasian Association for Engineering Education
        eats:aftes,     # Australian Fluid and Thermal Engineering Society (AFTES)
        eats:apts,      # Australian Particle Technology Society (APTS)
        eats:ats,       # Australian Tunnelling Society
        eats:acss,      # Australian Composite Structures Society
        eats:aces,      # Australian Cost Engineering Society
        eats:aees,      # Australian Earthquake Engineering Society
        eats:ags,       # Australian Geomechanics Society
        eats:ass,       # Australian Shotcrete Society
        eats:asbsh,     # Australian Society for Bulk Solids Handling
        eats:asde,      # Australian Society for Defence Engineering
        eats:ascp,      # Australian Society for Concrete Pavements
        eats:ecsa,      # Electromagnetic Compatibility Society of Australia
        eats:eesa,      # Electric Energy Society of Australia
        eats:iea,       # Industrial Engineers Australia
        eats:ipwea,     # Institute of Public Works Engineering Australasia
        eats:ma,        # Materials Australia
        eats:msts,      # Mine Subsidence Technological Society
        eats:memmes,    # Mining Electrical and Mining Mechanical Engineering Society
        eats:rtsa,      # Railway Technical Society of Australasia
        eats:rra,       # RedR Australia
        eats:res,       # Risk Engineering Society
        eats:ras,       # Royal Aeronautical Society
        eats:rina,      # Royal Institution of Naval Architects
        eats:sbse,      # Society for Building Services Engineers
        eats:sea,       # Society for Engineering in Agriculture
        eats:ses,       # Sustainable Engineering Society
        eats:sfs,       # Society of Fire Safety
        eats:sesa,      # Systems Engineering Society of Australia
        eats:tas ;      # Transport Australia Society

    skos:prefLabel "Engineers Australia Colleges"@en .

<https://linked.data.gov.au/org/engineersaustralia>
    a sdo:Organization ;
    sdo:name "Engineers Australia" ;
    sdo:url "https://www.engineersaustralia.org.au"^^xsd:anyURI .

<https://orcid.org/0000-0003-2309-7004> a owl:NamedIndividual,
        sdo:Person ;
    sdo:affiliation [ a sdo:Organization ;
            sdo:name "Engineers Australia" ;
            sdo:url "https://www.engineersaustralia.org.au"^^xsd:anyURI ] ;
    sdo:name "Vance Kelly" ;""
    sdo:identifier <https://orcid.org/0000-0003-2309-7004> .

eats:amc a skos:Concept ;
    rdfs:isDefinedBy <https://linked.data.gov.au/def/ea-tech-societies> ;
    dcterms:source "https://www.amcouncil.com.au/about-us/what-is-the-asset-management-council.html"^^xsd:anyURI ;
    rdfs:seeAlso <https://www.amcouncil.com.au/> ;
    skos:definition """The Asset Management Council is a membership-based, not-for-profit organization, a Technical Society of Engineers Australia, a founding member of the Global Forum on Maintenance and Asset Management (GFMAM) and a founding member of the World Partners in Asset Management (WPiAM).
    
    As an internationally recognized organisation at the forefront of asset management knowledge and development, we provide information and guidance on asset management across a multitude of industries and professional roles, both in Australia and overseas. The Asset Management Council professional services, technical knowledge, and organisational experience act as a platform for professional development and industry recognition, and its international affiliations link The Asset Management Council stakeholders to a community whose knowledge and experience is drawn from all levels of practice."""@en ;
    skos:prefLabel "Asset Management Council"@en ;
    skos:inScheme <https://linked.data.gov.au/def/ea-tech-societies> ;
    skos:topConceptOf <https://linked.data.gov.au/def/ea-tech-societies> .

eats:aaee a skos:Concept ;
    rdfs:isDefinedBy <https://linked.data.gov.au/def/ea-tech-societies> ;
    dcterms:source "https://aaee.net.au/about-aaee/"^^xsd:anyURI ;
    rdfs:seeAlso <https://aaee.net.au/> ;
    skos:definition """The Australasian Association for Engineering Education, AAEE (often spoken as A squared, E squared), is a professional association of academics, support staff, postgraduate students, librarians, professional engineers and employers who all have vested interest in fostering excellence and innovation in engineering education. A technical society of Engineers Australia, AAEE is governed by an elected executive committee that guides the direction of AAEE and undertake the day-to-day operations of the Association. The executive also includes representatives of the aligned bodies Engineers Australia, Engineering New Zealand and the Australian Council of Engineering Deans (ACED). AAEE has it's own journal, the Australasian Journal of Engineering Education, that presents work that is at the forefront of engineering education internationally."""@en ;
    skos:prefLabel "Australasian Association for Engineering Education"@en ;
    skos:inScheme <https://linked.data.gov.au/def/ea-tech-societies> ;
    skos:topConceptOf <https://linked.data.gov.au/def/ea-tech-societies> .
