PREFIX ieaoc: <https://linked.data.gov.au/def/iea-occupational-categories/>
PREFIX dcterms: <http://purl.org/dc/terms/>
PREFIX owl: <http://www.w3.org/2002/07/owl#>
PREFIX rdfs: <http://www.w3.org/2000/01/rdf-schema#>
PREFIX sdo: <http://schema.org/>
PREFIX skos: <http://www.w3.org/2004/02/skos/core#>
PREFIX xsd: <http://www.w3.org/2001/XMLSchema#>

<https://linked.data.gov.au/org/engineersaustralia> a sdo:Organization ;
    sdo:name "Engineers Australia" ;
    sdo:url "https://www.engineersaustralia.org.au"^^xsd:anyURI .

<https://linked.data.gov.au/def/iea-occupational-categories> a owl:Ontology,
        skos:ConceptScheme ;
    dcterms:accessRights <https://linked.data.gov.au/def/data-access-rights/open> ;
    dcterms:created "2022-11-09"^^xsd:date ;
    dcterms:creator <https://linked.data.gov.au/org/engineersaustralia> ;
    dcterms:modified "2024-03-15"^^xsd:date ;
    dcterms:publisher <https://linked.data.gov.au/org/engineersaustralia> ;
    dcterms:source "https://www.ieagreements.org/accords/acknowledgements-accords"^^xsd:anyURI ;
    skos:hasTopConcept
        ieaoc:assoc-engineer,
        ieaoc:pro-engineer,
        ieaoc:tech-engineer,
        ieaoc:engineering-manager ;
    skos:altLabel "International Engineering Accords Membership"@en,
        "Occupational Categories"@en ;
    skos:definition "A category reflecting the level and type of engineering qualification held by a member of the engineering profession, as per the International Engineering Alliance Educational Accords."@en ;
    skos:prefLabel "International Engineering Alliance Occupational Categories"@en .

ieaoc:assoc-engineer a skos:Concept ;
    dcterms:source "https://www.ieagreements.org/accords/dublin/"^^xsd:anyURI ;
    rdfs:isDefinedBy <https://linked.data.gov.au/def/iea-occupational-categories> ;
    skos:inScheme <https://linked.data.gov.au/def/iea-occupational-categories> ;
    skos:topConceptOf <https://linked.data.gov.au/def/iea-occupational-categories> ;
    skos:definition """Engineering associates hold a two-year advanced diploma or associate degree of engineering that's accredited or recognised by Engineers Australia. 
    
    Engineering associates can also hold a comparable overseas qualification or a degree that's accredited by a signatory to the Dublin Accord. The qualification needs to have a strong practical focus.
    
    As an engineering associate, you have the skills to:
    - focus on specific elements of the system,
    - work within codes and apply established practices and procedures."""@en ;
    skos:notation "A" ;
    skos:altLabel "Dublin Accords"@en ;
    skos:prefLabel "Engineering Associate"@en .

ieaoc:pro-engineer a skos:Concept ;
    dcterms:source "https://www.ieagreements.org/accords/washington/"^^xsd:anyURI ;
    rdfs:isDefinedBy <https://linked.data.gov.au/def/iea-occupational-categories> ;
    skos:inScheme <https://linked.data.gov.au/def/iea-occupational-categories> ;
    skos:topConceptOf <https://linked.data.gov.au/def/iea-occupational-categories> ;
    skos:definition """Professional engineers hold a four-year professional engineering degree that's accredited or recognised by Engineers Australia.
    
    Professional engineers can also hold comparable overseas qualifications or a degree that's accredited by a signatory to the Washington Accord.
    
    As a professional engineer, you have the skills to:
    - focus on overall systems,
    - develop and apply new engineering practices,
    - apply leadership and management skills,
    - pursue engineering opportunities in a holistic way, taking environmental, community and social issues into consideration,
    - solve diverse problems."""@en ;
    skos:notation "P" ;
    skos:altLabel "Washington Accords"@en ;
    skos:prefLabel "Professional Engineer"@en .

ieaoc:tech-engineer a skos:Concept ;
    dcterms:source "https://www.ieagreements.org/accords/sydney/"^^xsd:anyURI ;
    rdfs:isDefinedBy <https://linked.data.gov.au/def/iea-occupational-categories> ;
    skos:inScheme <https://linked.data.gov.au/def/iea-occupational-categories> ;
    skos:topConceptOf <https://linked.data.gov.au/def/iea-occupational-categories> ;
    skos:definition """Engineering technologists hold a three-year engineering technology degree that's accredited or recognised by Engineers Australia.
    
    Engineering technologists can also hold comparable overseas qualifications or a degree that's accredited by a signatory to the Sydney Accord.
    
    As an engineering technologist, you have the skills to:
    - focus on interactions with the system
    - modify and adapt established engineering practices
    - advance engineering technology."""@en ;
    skos:altLabel "Sydney Accords"@en ;
    skos:notation "T" ;
    skos:prefLabel "Engineering Technologist"@en .

ieaoc:engineering-manager a skos:Concept ;
    dcterms:source "https://www.engineersaustralia.org.au/publications/occupational-category-description-and-competencies-entry-practice-engineering-manager"^^xsd:anyURI ;
    rdfs:isDefinedBy <https://linked.data.gov.au/def/iea-occupational-categories> ;
    rdfs:seeAlso <https://linked.data.gov.au/def/anzsco/1> ;
    skos:inScheme <https://linked.data.gov.au/def/iea-occupational-categories> ;
    skos:topConceptOf <https://linked.data.gov.au/def/iea-occupational-categories> ;
    skos:definition """The role of engineering manager is a high-level executive position. It involves the formulation of engineering strategies, policies and plans and the direction, administration and review of engineering operations for an organisation. This category is not part of the International Engineering Accords.
    
    Overseas engineers whose qualifications don't fit one of the three IEA categories, can apply for a migrant skills assessment using the occupational category of Engineering manager. This occupation isn't an engineering occupation, it belongs to the Managers OSCA group listed by the Australian Bureau of Statistics.
    
    Engineering managers hold a Bachelor of Engineering degree or comparable qualification in a field related to engineering plus relevant experience. As an engineering manager, you have the skills to:
    - formulate, implement and monitor engineering strategies, policies and plans,
    - direct the administration and review of engineering operations for an organisation."""@en ;
    skos:notation "M" ;
    skos:prefLabel "Engineering Manager"@en .